@prefix : <http://www.ontologydesignpatterns.org/ont/odin/odin_inferred.owl#> .
@prefix owl: <http://www.w3.org/2002/07/owl#> .
@prefix rdf: <http://www.w3.org/1999/02/22-rdf-syntax-ns#> .
@prefix xml: <http://www.w3.org/XML/1998/namespace> .
@prefix xsd: <http://www.w3.org/2001/XMLSchema#> .
@prefix odin: <http://www.ontologydesignpatterns.org/ont/odin/odin.owl#> .
@prefix rdfs: <http://www.w3.org/2000/01/rdf-schema#> .
@prefix isnet: <http://www.ontologydesignpatterns.org/ont/is/isnet.owl#> .
@base <http://www.ontologydesignpatterns.org/ont/odin/odin_inferred.owl> .

<http://www.ontologydesignpatterns.org/ont/odin/odin_inferred.owl> rdf:type owl:Ontology ;
                                                                    rdfs:comment """ODIN is an ontological module realized for Ontology Design grounded in Image-schematic kNowledge. It reuses all the entities and properties from previous ODP .owl files (bootstrapped from ontologydesignpattern.org) which are annotated via \"rdfs:comment\". The text of this comment is passed through an automatic image schema detector and for each Ontology Design Pattern it is automatically extracted an Image Schema profile, namely the set of primitive mental building blocks which can be reused to cognitively ground the modelling pattern embodied cognition theory.

Designed by Stefano De Giorgis and Aldo Gangemi. """ ;
                                                                    owl:versionInfo "1.0 - Used only rdfs:comment, future works include cpannotationschema and labels." .

#################################################################
#    Object Properties
#################################################################

###  http://www.ontologydesignpatterns.org/ont/is/isnet.owl#activates
isnet:activates rdf:type owl:ObjectProperty .


###  http://www.ontologydesignpatterns.org/ont/is/isnet.owl#hasActivator
isnet:hasActivator rdf:type owl:ObjectProperty .


###  http://www.ontologydesignpatterns.org/ont/odin/odin.owl#describedIn
odin:describedIn rdf:type owl:ObjectProperty .


###  http://www.ontologydesignpatterns.org/ont/odin/odin.owl#hasODPComponent
odin:hasODPComponent rdf:type owl:ObjectProperty ;
                     rdfs:subPropertyOf owl:topObjectProperty ;
                     rdfs:domain odin:ODP ;
                     rdfs:range odin:ODPElement .


###  http://www.ontologydesignpatterns.org/ont/odin/odin.owl#odpType
odin:odpType rdf:type owl:ObjectProperty .


###  http://www.w3.org/2002/07/owl#topObjectProperty
owl:topObjectProperty rdf:type owl:ObjectProperty ;
                      owl:inverseOf owl:topObjectProperty ;
                      rdf:type owl:SymmetricProperty ,
                               owl:TransitiveProperty .


#################################################################
#    Classes
#################################################################

###  http://www.ontologydesignpatterns.org/ont/odin/odin.owl#ODP
odin:ODP rdf:type owl:Class .


###  http://www.ontologydesignpatterns.org/ont/odin/odin.owl#ODPElement
odin:ODPElement rdf:type owl:Class .


###  http://www.ontologydesignpatterns.org/ont/odin/odin.owl#ODPType
odin:ODPType rdf:type owl:Class .


###  http://www.ontologydesignpatterns.org/ont/odin/odin_inferred.owl#ODPDescription
:ODPDescription rdf:type owl:Class .


#################################################################
#    Individuals
#################################################################

###  http://dbpedia.org/ontology/City
<http://dbpedia.org/ontology/City> rdf:type owl:NamedIndividual ;
                                   odin:describedIn odin:City_Descr ;
                                   rdfs:comment "a relatively large and permanent settlement, particularly a large urban settlement" .


###  http://dbpedia.org/ontology/MeanOfTransportation
<http://dbpedia.org/ontology/MeanOfTransportation> rdf:type owl:NamedIndividual ;
                                                   odin:describedIn odin:MeanOfTransportation_Descr ;
                                                   rdfs:comment "Relation between Airline and Aircraft" ,
                                                                "Relazione tra Airline e Aircraft" .


###  http://dbpedia.org/ontology/River
<http://dbpedia.org/ontology/River> rdf:type owl:NamedIndividual ;
                                    odin:describedIn odin:River_Descr ;
                                    rdfs:comment "a large natural stream" .


###  http://dbpedia.org/ontology/Town
<http://dbpedia.org/ontology/Town> rdf:type owl:NamedIndividual ;
                                   odin:describedIn odin:Town_Descr ;
                                   rdfs:comment "a settlement ranging from a few hundred to several thousand (occasionally hundreds of thousands). The precise meaning varies between countries and is not always a matter of legal definition. Usually, a town is thought of as larger than a village but smaller than a city, though there are exceptions to this rule." .


###  http://delicias.dia.fi.upm.es/ontologies/ObjectWithStates.owl
<http://delicias.dia.fi.upm.es/ontologies/ObjectWithStates.owl> rdf:type owl:NamedIndividual ,
                                                                         odin:ODP ;
                                                                odin:describedIn odin:ObjectWithStates.owl_Descr ;
                                                                odin:hasODPComponent <http://delicias.dia.fi.upm.es/ontologies/ObjectWithStates.owl#Object> ,
                                                                                     <http://delicias.dia.fi.upm.es/ontologies/ObjectWithStates.owl#State> ,
                                                                                     <http://delicias.dia.fi.upm.es/ontologies/ObjectWithStates.owl#StateSet> ,
                                                                                     <http://delicias.dia.fi.upm.es/ontologies/ObjectWithStates.owl#hasState> ,
                                                                                     <http://delicias.dia.fi.upm.es/ontologies/ObjectWithStates.owl#isStateOf> ;
                                                                odin:odpType odin:Foundational ;
                                                                rdfs:comment "Ontology including the content ontology design pattern for modelling objects with states." .


###  http://delicias.dia.fi.upm.es/ontologies/PeriodicInterval.owl
<http://delicias.dia.fi.upm.es/ontologies/PeriodicInterval.owl> rdf:type owl:NamedIndividual ,
                                                                         odin:ODP ;
                                                                odin:describedIn odin:PeriodicInterval.owl_Descr ;
                                                                rdfs:comment "This ontology design pattern extends the OWL-Time ontology (http://www.w3.org/TR/owl-time) defining periodic intervals." .


###  http://delicias.dia.fi.upm.es/ontologies/ObjectWithStates.owl#Object
<http://delicias.dia.fi.upm.es/ontologies/ObjectWithStates.owl#Object> rdf:type owl:NamedIndividual ,
                                                                                odin:ODPElement ;
                                                                       odin:describedIn odin:Object_Descr ;
                                                                       rdfs:comment "Objects are entities that have different states and that in each state different restrictions on their properties apply." .


###  http://delicias.dia.fi.upm.es/ontologies/ObjectWithStates.owl#State
<http://delicias.dia.fi.upm.es/ontologies/ObjectWithStates.owl#State> rdf:type owl:NamedIndividual ,
                                                                               odin:ODPElement ;
                                                                      odin:describedIn odin:State_Descr ;
                                                                      odin:odpType odin:Foundational ;
                                                                      rdfs:comment "States are the different states that an object can have. States must belong to a single collection of non-duplicate elements (i.e., to a set)." .


###  http://delicias.dia.fi.upm.es/ontologies/ObjectWithStates.owl#StateSet
<http://delicias.dia.fi.upm.es/ontologies/ObjectWithStates.owl#StateSet> rdf:type owl:NamedIndividual ,
                                                                                  odin:ODPElement ;
                                                                         odin:describedIn odin:StateSet_Descr ;
                                                                         rdfs:comment "State sets are sets of states (i.e., collections of non-duplicate states)." .


###  http://delicias.dia.fi.upm.es/ontologies/ObjectWithStates.owl#hasState
<http://delicias.dia.fi.upm.es/ontologies/ObjectWithStates.owl#hasState> rdf:type owl:NamedIndividual ,
                                                                                  odin:ODPElement ;
                                                                         odin:describedIn odin:hasState_Descr ;
                                                                         odin:odpType odin:Foundational ;
                                                                         rdfs:comment "Defines the state of an object." .


###  http://delicias.dia.fi.upm.es/ontologies/ObjectWithStates.owl#isStateOf
<http://delicias.dia.fi.upm.es/ontologies/ObjectWithStates.owl#isStateOf> rdf:type owl:NamedIndividual ,
                                                                                   odin:ODPElement ;
                                                                          odin:describedIn odin:isStateOf_Descr ;
                                                                          odin:odpType odin:Foundational ;
                                                                          rdfs:comment "Defines the object that has an state" .


###  http://delicias.dia.fi.upm.es/ontologies/SimpleOrAggregated.owl#AggregatedObject
<http://delicias.dia.fi.upm.es/ontologies/SimpleOrAggregated.owl#AggregatedObject> rdf:type owl:NamedIndividual ,
                                                                                            odin:ODPElement ;
                                                                                   odin:describedIn odin:AggregatedObject_Descr ;
                                                                                   rdfs:comment "An object that is an aggregation of two or more objects." ,
                                                                                                "Un objeto resultante de la agregación de dos o más objetos." .


###  http://delicias.dia.fi.upm.es/ontologies/SimpleOrAggregated.owl#Object
<http://delicias.dia.fi.upm.es/ontologies/SimpleOrAggregated.owl#Object> rdf:type owl:NamedIndividual ,
                                                                                  odin:ODPElement ;
                                                                         odin:describedIn odin:Object_Descr ;
                                                                         odin:odpType odin:Foundational ;
                                                                         rdfs:comment "Any physical, social, or mental object, or a substance." ,
                                                                                      "Cualquier objeto físico, social o mental o sustancia." .


###  http://delicias.dia.fi.upm.es/ontologies/SimpleOrAggregated.owl#SimpleObject
<http://delicias.dia.fi.upm.es/ontologies/SimpleOrAggregated.owl#SimpleObject> rdf:type owl:NamedIndividual ,
                                                                                        odin:ODPElement ;
                                                                               odin:describedIn odin:SimpleObject_Descr ;
                                                                               odin:odpType odin:Foundational ;
                                                                               rdfs:comment "A simple object, that is, an object that has no aggregated objects." ,
                                                                                            "Un objeto simple, es decir, un objeto que no tiene objetos agregados." .


###  http://descartes-core.org/ontologies/activities/1.0/ActivityPattern
<http://descartes-core.org/ontologies/activities/1.0/ActivityPattern> rdf:type owl:NamedIndividual ,
                                                                               odin:ODP ;
                                                                      odin:describedIn odin:ActivityPattern_Descr ;
                                                                      odin:odpType odin:Foundational ;
                                                                      rdfs:comment "While this pattern so far focuses on human activities, the agents that are involved in this pattern may also be other autonomous agents, such as animals." .


###  http://ecareathome-ontology.mpi.aass.oru.se/patterns/SmartHome_Object.owl
<http://ecareathome-ontology.mpi.aass.oru.se/patterns/SmartHome_Object.owl> rdf:type owl:NamedIndividual ,
                                                                                     odin:ODP ;
                                                                            odin:describedIn odin:SmartHome_Object.owl_Descr ;
                                                                            rdfs:comment "This pattern relies on both the SSN ontology and DUL in order to represent an object in the context of Smart Home. Using this model we categorize the objects in to two groups of Smart Objects and NodeHolder based on the reason behind their existance in a smart home.      Due to usual difficulties to install sensors in a smart home environment it is common that some other objects (i.e. NodeHolder) are used to attache sensors on so as to observe the situation of other objects (i.e. SmartObject) specifically for the configuration planner. Using this pattern we are able to diffrentiate between these two types of objects.     This pattern also allows us to extend the definition of an object's properties in the context of smart home. The properties of a SmartObject which are the interest of the sensing process can be defined as either a subclass of the class http://purl.oclc.org/NET/ssnx/ssn#Property (e.g. the temperature of a stove) or as part of the smart object (e.g. the door of a friedge)" .


###  http://ecareathome-ontology.mpi.aass.oru.se/patterns/SmartHome_Network.owl#Network
<http://ecareathome-ontology.mpi.aass.oru.se/patterns/SmartHome_Network.owl#Network> rdf:type owl:NamedIndividual ,
                                                                                              odin:ODPElement ;
                                                                                     odin:describedIn odin:Network_Descr ;
                                                                                     rdfs:comment "A network which is a collection of Nodes" .


###  http://ecareathome-ontology.mpi.aass.oru.se/patterns/SmartHome_Place.owl#SmartHomeSection
<http://ecareathome-ontology.mpi.aass.oru.se/patterns/SmartHome_Place.owl#SmartHomeSection> rdf:type owl:NamedIndividual ,
                                                                                                     odin:ODPElement ;
                                                                                            odin:describedIn odin:SmartHomeSection_Descr ;
                                                                                            rdfs:comment "Sections belonging to a SmartHome" .


###  http://mklab.iti.gr/pericles/BornDigitalArchives_ODP#File
<http://mklab.iti.gr/pericles/BornDigitalArchives_ODP#File> rdf:type owl:NamedIndividual ,
                                                                     odin:ODPElement ;
                                                            odin:describedIn odin:File_Descr ;
                                                            rdfs:comment "An organized unit of documents grouped together either for current use by the creator or in the process of archival arrangement, because they relate to the same subject, activity, or transaction. A file is usually the basic unit within a record series." .


###  http://mklab.iti.gr/pericles/BornDigitalArchives_ODP#Fonds
<http://mklab.iti.gr/pericles/BornDigitalArchives_ODP#Fonds> rdf:type owl:NamedIndividual ,
                                                                      odin:ODPElement ;
                                                             odin:describedIn odin:Fonds_Descr ;
                                                             rdfs:comment "Fonds:  The whole of the records, regardless of form or medium, organically created and/or accumulated and used by a particular person, family, or corporate body in the course of that creator's activities and functions." ,
                                                                          "Sub-fonds:  A subdivision of a fonds containing a body of related records corresponding to administrative subdivisions in the originating agency or organization or, when that is not possible, to geographical, chronological, functional, or similar groupings of the material itself. When the creating body has a complex hierarchical structure, each sub-fonds has as many subordinate sub-fonds as are necessary to reflect the levels of the hierarchical structure of the primary subordinate administrative unit." .


###  http://mklab.iti.gr/pericles/BornDigitalArchives_ODP#Item
<http://mklab.iti.gr/pericles/BornDigitalArchives_ODP#Item> rdf:type owl:NamedIndividual ,
                                                                     odin:ODPElement ;
                                                            odin:describedIn odin:Item_Descr ;
                                                            rdfs:comment "The smallest intellectually indivisible archival unit, e.g., a letter, memorandum, report, photograph, sound recording." .


###  http://mklab.iti.gr/pericles/BornDigitalArchives_ODP#Series
<http://mklab.iti.gr/pericles/BornDigitalArchives_ODP#Series> rdf:type owl:NamedIndividual ,
                                                                       odin:ODPElement ;
                                                              odin:describedIn odin:Series_Descr ;
                                                              rdfs:comment "Documents arranged in accordance with a filing system or maintained as a unit because they result from the same accumulation or filing process, or the same activity; have a particular form; or because of some other relationship arising out of their creation, receipt, or use. A series is also known as a records series." .


###  http://mklab.iti.gr/pericles/BornDigitalArchives_ODP#hasCreator
<http://mklab.iti.gr/pericles/BornDigitalArchives_ODP#hasCreator> rdf:type owl:NamedIndividual ,
                                                                           odin:ODPElement ;
                                                                  odin:describedIn odin:hasCreator_Descr ;
                                                                  rdfs:comment "Indicates the creator of a unit." .


###  http://mklab.iti.gr/pericles/BornDigitalArchives_ODP#hasPart
<http://mklab.iti.gr/pericles/BornDigitalArchives_ODP#hasPart> rdf:type owl:NamedIndividual ,
                                                                        odin:ODPElement ;
                                                               odin:describedIn odin:hasPart_Descr ;
                                                               rdfs:comment "Indicates that a unit includes another unit." .


###  http://mklab.iti.gr/pericles/ComputerSystem_ODP#Computer
<http://mklab.iti.gr/pericles/ComputerSystem_ODP#Computer> rdf:type owl:NamedIndividual ,
                                                                    odin:ODPElement ;
                                                           odin:describedIn odin:Computer_Descr ;
                                                           rdfs:comment "This entity represents computers of any type, size, cost and application." .


###  http://mklab.iti.gr/pericles/ComputerSystem_ODP#Hardware
<http://mklab.iti.gr/pericles/ComputerSystem_ODP#Hardware> rdf:type owl:NamedIndividual ,
                                                                    odin:ODPElement ;
                                                           odin:describedIn odin:Hardware_Descr ;
                                                           rdfs:comment "A physical component or a collection of physical components used by (or within or aside) a computer." .


###  http://mklab.iti.gr/pericles/ComputerSystem_ODP#isCompatibleWith
<http://mklab.iti.gr/pericles/ComputerSystem_ODP#isCompatibleWith> rdf:type owl:NamedIndividual ,
                                                                            odin:ODPElement ;
                                                                   odin:describedIn odin:isCompatibleWith_Descr ;
                                                                   rdfs:comment "Represents the relationship of compatibility between two components." .


###  http://mklab.iti.gr/pericles/ComputerSystem_ODP#requiresHardware
<http://mklab.iti.gr/pericles/ComputerSystem_ODP#requiresHardware> rdf:type owl:NamedIndividual ,
                                                                            odin:ODPElement ;
                                                                   odin:describedIn odin:requiresHardware_Descr ;
                                                                   rdfs:comment "Indicates that an entity requires a certain piece of hardware to operate." .


###  http://mklab.iti.gr/pericles/ComputerSystem_ODP#requiresSoftware
<http://mklab.iti.gr/pericles/ComputerSystem_ODP#requiresSoftware> rdf:type owl:NamedIndividual ,
                                                                            odin:ODPElement ;
                                                                   odin:describedIn odin:requiresSoftware_Descr ;
                                                                   rdfs:comment "Indicates that an entity requires a certain piece of software to operate." .


###  http://mklab.iti.gr/pericles/ComputerSystem_ODP#usesDriver
<http://mklab.iti.gr/pericles/ComputerSystem_ODP#usesDriver> rdf:type owl:NamedIndividual ,
                                                                      odin:ODPElement ;
                                                             odin:describedIn odin:usesDriver_Descr ;
                                                             rdfs:comment "Indicates the usage of a specific driver." .


###  http://mklab.iti.gr/pericles/ComputerSystem_ODP#usesHardware
<http://mklab.iti.gr/pericles/ComputerSystem_ODP#usesHardware> rdf:type owl:NamedIndividual ,
                                                                        odin:ODPElement ;
                                                               odin:describedIn odin:usesHardware_Descr ;
                                                               rdfs:comment "Indicates the usage of a specific piece of hardware." .


###  http://mklab.iti.gr/pericles/ComputerSystem_ODP#usesOperatingSystem
<http://mklab.iti.gr/pericles/ComputerSystem_ODP#usesOperatingSystem> rdf:type owl:NamedIndividual ,
                                                                               odin:ODPElement ;
                                                                      odin:describedIn odin:usesOperatingSystem_Descr ;
                                                                      rdfs:comment "Indicates the usage of a certain Operating System." .


###  http://mklab.iti.gr/pericles/ComputerSystem_ODP#usesSoftware
<http://mklab.iti.gr/pericles/ComputerSystem_ODP#usesSoftware> rdf:type owl:NamedIndividual ,
                                                                        odin:ODPElement ;
                                                               odin:describedIn odin:usesSoftware_Descr ;
                                                               rdfs:comment "Indicates the usage of a specific piece of software." .


###  http://mklab.iti.gr/pericles/DigitalVideo_ODP#AnalogBroadcastStandard
<http://mklab.iti.gr/pericles/DigitalVideo_ODP#AnalogBroadcastStandard> rdf:type owl:NamedIndividual ,
                                                                                 odin:ODPElement ;
                                                                        odin:describedIn odin:AnalogBroadcastStandard_Descr ;
                                                                        rdfs:comment "E.g. NTSC, PAL, etc." ,
                                                                                     "The video color encoding system, if the video originates from analog television broadcasts." .


###  http://mklab.iti.gr/pericles/DigitalVideo_ODP#AspectRatio
<http://mklab.iti.gr/pericles/DigitalVideo_ODP#AspectRatio> rdf:type owl:NamedIndividual ,
                                                                     odin:ODPElement ;
                                                            odin:describedIn odin:AspectRatio_Descr ;
                                                            rdfs:comment "The aspect ratio of an image describes the proportional relationship between its width and its height. It is commonly expressed as two numbers separated by a colon, as in 16:9." .


###  http://mklab.iti.gr/pericles/DigitalVideo_ODP#AudioCodec
<http://mklab.iti.gr/pericles/DigitalVideo_ODP#AudioCodec> rdf:type owl:NamedIndividual ,
                                                                    odin:ODPElement ;
                                                           odin:describedIn odin:AudioCodec_Descr ;
                                                           rdfs:comment "An audio codec is a device or computer program capable of coding or decoding a digital data stream of audio." ,
                                                                        "E.g. MP3" .


###  http://mklab.iti.gr/pericles/DigitalVideo_ODP#AudioStream
<http://mklab.iti.gr/pericles/DigitalVideo_ODP#AudioStream> rdf:type owl:NamedIndividual ;
                                                            odin:describedIn odin:AudioStream_Descr ;
                                                            rdfs:comment "An audio stream is a stream where the carried data is audio content." .


###  http://mklab.iti.gr/pericles/DigitalVideo_ODP#BitRate
<http://mklab.iti.gr/pericles/DigitalVideo_ODP#BitRate> rdf:type owl:NamedIndividual ;
                                                        odin:describedIn odin:BitRate_Descr ;
                                                        rdfs:comment "E.g. 2 MBits/s" ,
                                                                     "The bitrate is the data rate for a video or audio file. Video and audio data rates are given in bits per second." .


###  http://mklab.iti.gr/pericles/DigitalVideo_ODP#ChromaFormat
<http://mklab.iti.gr/pericles/DigitalVideo_ODP#ChromaFormat> rdf:type owl:NamedIndividual ,
                                                                      odin:ODPElement ;
                                                             odin:describedIn odin:ChromaFormat_Descr ;
                                                             rdfs:comment "E.g. 4:2:0" ,
                                                                          "The chroma subsampling type. Chroma subsampling is the practice of encoding images by implementing less resolution for chroma information than for luma information, taking advantage of the human visual system's lower acuity for color differences than for luminance." .


###  http://mklab.iti.gr/pericles/DigitalVideo_ODP#Codec
<http://mklab.iti.gr/pericles/DigitalVideo_ODP#Codec> rdf:type owl:NamedIndividual ,
                                                               odin:ODPElement ;
                                                      odin:describedIn odin:Codec_Descr ;
                                                      rdfs:comment "A codec is a device or computer program capable of encoding or decoding a digital data stream or signal." .


###  http://mklab.iti.gr/pericles/DigitalVideo_ODP#CodingStandard
<http://mklab.iti.gr/pericles/DigitalVideo_ODP#CodingStandard> rdf:type owl:NamedIndividual ,
                                                                        odin:ODPElement ;
                                                               odin:describedIn odin:CodingStandard_Descr ;
                                                               rdfs:comment "Also known as coding format or compression format." ,
                                                                            "E.g. H.264/MPEG-4 AVC" .


###  http://mklab.iti.gr/pericles/DigitalVideo_ODP#ColourSpaceType
<http://mklab.iti.gr/pericles/DigitalVideo_ODP#ColourSpaceType> rdf:type owl:NamedIndividual ;
                                                                odin:describedIn odin:ColourSpaceType_Descr ;
                                                                rdfs:comment "A color space is a specific organization of colors. It allows for reproducible representations of color, in both analog and digital representations. A color space may be arbitrary, with particular colors assigned to a set of physical color swatches and corresponding assigned names or numbers." ,
                                                                             "E.g. YUV, RGB, etc." .


###  http://mklab.iti.gr/pericles/DigitalVideo_ODP#CompressionType
<http://mklab.iti.gr/pericles/DigitalVideo_ODP#CompressionType> rdf:type owl:NamedIndividual ,
                                                                         odin:ODPElement ;
                                                                odin:describedIn odin:CompressionType_Descr ;
                                                                rdfs:comment "E.g. lossy, lossless or uncompressed" ,
                                                                             "The type of video compression." .


###  http://mklab.iti.gr/pericles/DigitalVideo_ODP#Container
<http://mklab.iti.gr/pericles/DigitalVideo_ODP#Container> rdf:type owl:NamedIndividual ,
                                                                   odin:ODPElement ;
                                                          odin:describedIn odin:Container_Descr ;
                                                          rdfs:comment "A container or wrapper format is a metafile format whose specification describes how different elements of data and metadata coexist in a computer file." ,
                                                                       "E.g. Matroska (MKV), MP4, etc." .


###  http://mklab.iti.gr/pericles/DigitalVideo_ODP#Descriptor
<http://mklab.iti.gr/pericles/DigitalVideo_ODP#Descriptor> rdf:type owl:NamedIndividual ,
                                                                    odin:ODPElement ;
                                                           odin:describedIn odin:Descriptor_Descr ;
                                                           rdfs:comment "Descriptors are the various elements describing a digital video, a container, a stream or a codec." .


###  http://mklab.iti.gr/pericles/DigitalVideo_ODP#DigitalVideo
<http://mklab.iti.gr/pericles/DigitalVideo_ODP#DigitalVideo> rdf:type owl:NamedIndividual ,
                                                                      odin:ODPElement ;
                                                             odin:describedIn odin:DigitalVideo_Descr ;
                                                             rdfs:comment "A digital video file." .


###  http://mklab.iti.gr/pericles/DigitalVideo_ODP#EmbeddingType
<http://mklab.iti.gr/pericles/DigitalVideo_ODP#EmbeddingType> rdf:type owl:NamedIndividual ,
                                                                       odin:ODPElement ;
                                                              odin:describedIn odin:EmbeddingType_Descr ;
                                                              rdfs:comment "E.g. hard, prerendered, soft, etc." ,
                                                                           "The type of embedment used to attach a subtitle stream to a video." .


###  http://mklab.iti.gr/pericles/DigitalVideo_ODP#FrameRate
<http://mklab.iti.gr/pericles/DigitalVideo_ODP#FrameRate> rdf:type owl:NamedIndividual ;
                                                          odin:describedIn odin:FrameRate_Descr ;
                                                          rdfs:comment "E.g. 60 FPS" ,
                                                                       "Frame rate, also known as frame frequency, is the frequency (rate) at which an imaging device produces unique consecutive images called frames. The term applies equally well to film and video cameras, computer graphics, and motion capture systems. Frame rate is most often expressed in frames per second (FPS) and is also expressed in progressive scan monitors as hertz (Hz)." .


###  http://mklab.iti.gr/pericles/DigitalVideo_ODP#FrameSize
<http://mklab.iti.gr/pericles/DigitalVideo_ODP#FrameSize> rdf:type owl:NamedIndividual ,
                                                                   odin:ODPElement ;
                                                          odin:describedIn odin:FrameSize_Descr ;
                                                          rdfs:comment "E.g. 1920 x 1080" ,
                                                                       "The dimensions of a video's frame." .


###  http://mklab.iti.gr/pericles/DigitalVideo_ODP#PlaybackDuration
<http://mklab.iti.gr/pericles/DigitalVideo_ODP#PlaybackDuration> rdf:type owl:NamedIndividual ;
                                                                 odin:describedIn odin:PlaybackDuration_Descr ;
                                                                 rdfs:comment "E.g. 22 minutes" ,
                                                                              "The duration of a video, video stream or audio stream." .


###  http://mklab.iti.gr/pericles/DigitalVideo_ODP#RangeType
<http://mklab.iti.gr/pericles/DigitalVideo_ODP#RangeType> rdf:type owl:NamedIndividual ,
                                                                   odin:ODPElement ;
                                                          odin:describedIn odin:RangeType_Descr ;
                                                          rdfs:comment "E.g. broadcast range or full range" ,
                                                                       "The type of range a video is created for." .


###  http://mklab.iti.gr/pericles/DigitalVideo_ODP#SampleRate
<http://mklab.iti.gr/pericles/DigitalVideo_ODP#SampleRate> rdf:type owl:NamedIndividual ,
                                                                    odin:ODPElement ;
                                                           odin:describedIn odin:SampleRate_Descr ;
                                                           rdfs:comment "E.g. 74.25 MHz" ,
                                                                        "E.g. 96 kHz" ,
                                                                        "The audio sample rate is the number of samples of audio carried per second, measured in Hz or kHz (one kHz being 1 000 Hz). For example, 44 100 samples per second can be expressed as either 44 100 Hz, or 44.1 kHz." ,
                                                                        "The video sample rate of a digital video format determines how often the light intensity of each video line is sampled." .


###  http://mklab.iti.gr/pericles/DigitalVideo_ODP#ScanType
<http://mklab.iti.gr/pericles/DigitalVideo_ODP#ScanType> rdf:type owl:NamedIndividual ;
                                                         odin:describedIn odin:ScanType_Descr ;
                                                         rdfs:comment "Progressive or interlaced scan." .


###  http://mklab.iti.gr/pericles/DigitalVideo_ODP#SetOfStandards
<http://mklab.iti.gr/pericles/DigitalVideo_ODP#SetOfStandards> rdf:type owl:NamedIndividual ,
                                                                        odin:ODPElement ;
                                                               odin:describedIn odin:SetOfStandards_Descr ;
                                                               rdfs:comment "E.g. BT.601 or BT.709" ,
                                                                            "Sets of standards standardize the format of a video stream." .


###  http://mklab.iti.gr/pericles/DigitalVideo_ODP#Stream
<http://mklab.iti.gr/pericles/DigitalVideo_ODP#Stream> rdf:type owl:NamedIndividual ,
                                                                odin:ODPElement ;
                                                       odin:describedIn odin:Stream_Descr ;
                                                       rdfs:comment "A (data) stream is a sequence of digitally encoded coherent signals (packets of data or data packets) used to transmit or receive information that is in the process of being transmitted. The term stream is used here to define raw, uncompressed content (video or audio) prior to being encoded into a wrapper or after being decoded from a wrapper." .


###  http://mklab.iti.gr/pericles/DigitalVideo_ODP#SubtitleStream
<http://mklab.iti.gr/pericles/DigitalVideo_ODP#SubtitleStream> rdf:type owl:NamedIndividual ;
                                                               odin:describedIn odin:SubtitleStream_Descr ;
                                                               rdfs:comment "A subtitle stream is a stream where the carried data is subtitle content for a video." .


###  http://mklab.iti.gr/pericles/DigitalVideo_ODP#SubtitleTextFormat
<http://mklab.iti.gr/pericles/DigitalVideo_ODP#SubtitleTextFormat> rdf:type owl:NamedIndividual ,
                                                                            odin:ODPElement ;
                                                                   odin:describedIn odin:SubtitleTextFormat_Descr ;
                                                                   rdfs:comment "E.g. SubRip, SubViewer, etc." ,
                                                                                "The file format of subtitles." .


###  http://mklab.iti.gr/pericles/DigitalVideo_ODP#VideoCodec
<http://mklab.iti.gr/pericles/DigitalVideo_ODP#VideoCodec> rdf:type owl:NamedIndividual ,
                                                                    odin:ODPElement ;
                                                           odin:describedIn odin:VideoCodec_Descr ;
                                                           rdfs:comment "A video codec is an electronic circuit or software that compresses or decompresses digital video, thus converting raw (uncompressed) digital video to a compressed format or vice-versa." ,
                                                                        "E.g. QuickTime H.264 (Apple's implementation for H.264/MPEG-4 AVC coding format)" .


###  http://mklab.iti.gr/pericles/DigitalVideo_ODP#VideoCodecLevel
<http://mklab.iti.gr/pericles/DigitalVideo_ODP#VideoCodecLevel> rdf:type owl:NamedIndividual ,
                                                                         odin:ODPElement ;
                                                                odin:describedIn odin:VideoCodecLevel_Descr ;
                                                                rdfs:comment "A video codec level is a specified set of constraints that indicate a degree of required decoder performance for a profile." ,
                                                                             "E.g. 4" .


###  http://mklab.iti.gr/pericles/DigitalVideo_ODP#VideoCodecProfile
<http://mklab.iti.gr/pericles/DigitalVideo_ODP#VideoCodecProfile> rdf:type owl:NamedIndividual ,
                                                                           odin:ODPElement ;
                                                                  odin:describedIn odin:VideoCodecProfile_Descr ;
                                                                  rdfs:comment "E.g. baseline profile, extended profile, main profile, high profile, etc." ,
                                                                               "The video codec profile is a set of capabilities and constraints apllied in the encoder. It allows the decoder to recognize the requirements to decode a specific stream." .


###  http://mklab.iti.gr/pericles/DigitalVideo_ODP#VideoQualityMeasurement
<http://mklab.iti.gr/pericles/DigitalVideo_ODP#VideoQualityMeasurement> rdf:type owl:NamedIndividual ,
                                                                                 odin:ODPElement ;
                                                                        odin:describedIn odin:VideoQualityMeasurement_Descr ;
                                                                        rdfs:comment "Measurement carried out according to the video quality metric." .


###  http://mklab.iti.gr/pericles/DigitalVideo_ODP#VideoQualityMetric
<http://mklab.iti.gr/pericles/DigitalVideo_ODP#VideoQualityMetric> rdf:type owl:NamedIndividual ,
                                                                            odin:ODPElement ;
                                                                   odin:describedIn odin:VideoQualityMetric_Descr ;
                                                                   rdfs:comment "E.g. VQM" ,
                                                                                "Process or software used to measure the quality of a video." .


###  http://mklab.iti.gr/pericles/DigitalVideo_ODP#VideoStream
<http://mklab.iti.gr/pericles/DigitalVideo_ODP#VideoStream> rdf:type owl:NamedIndividual ,
                                                                     odin:ODPElement ;
                                                            odin:describedIn odin:VideoStream_Descr ;
                                                            rdfs:comment "A video stream is a stream where the carried data is video content." .


###  http://mklab.iti.gr/pericles/DigitalVideo_ODP#YUVSampleRange
<http://mklab.iti.gr/pericles/DigitalVideo_ODP#YUVSampleRange> rdf:type owl:NamedIndividual ,
                                                                        odin:ODPElement ;
                                                               odin:describedIn odin:YUVSampleRange_Descr ;
                                                               rdfs:comment "E.g. 16-235" .


###  http://mklab.iti.gr/pericles/DigitalVideo_ODP#hasAnalogBroadcastStandard
<http://mklab.iti.gr/pericles/DigitalVideo_ODP#hasAnalogBroadcastStandard> rdf:type owl:NamedIndividual ,
                                                                                    odin:ODPElement ;
                                                                           odin:describedIn odin:hasAnalogBroadcastStandard_Descr ;
                                                                           rdfs:comment "Associates a digital video with an analog broadcast standard." .


###  http://mklab.iti.gr/pericles/DigitalVideo_ODP#hasAspectRatio
<http://mklab.iti.gr/pericles/DigitalVideo_ODP#hasAspectRatio> rdf:type owl:NamedIndividual ,
                                                                        odin:ODPElement ;
                                                               odin:describedIn odin:hasAspectRatio_Descr ;
                                                               rdfs:comment "Associates a video stream with an aspect ratio." .


###  http://mklab.iti.gr/pericles/DigitalVideo_ODP#hasAudioStream
<http://mklab.iti.gr/pericles/DigitalVideo_ODP#hasAudioStream> rdf:type owl:NamedIndividual ,
                                                                        odin:ODPElement ;
                                                               odin:describedIn odin:hasAudioStream_Descr ;
                                                               rdfs:comment "Associates a digital video with an audio stream." .


###  http://mklab.iti.gr/pericles/DigitalVideo_ODP#hasBitRate
<http://mklab.iti.gr/pericles/DigitalVideo_ODP#hasBitRate> rdf:type owl:NamedIndividual ,
                                                                    odin:ODPElement ;
                                                           odin:describedIn odin:hasBitRate_Descr ;
                                                           rdfs:comment "Associates an audio or video stream with a bit rate." .


###  http://mklab.iti.gr/pericles/DigitalVideo_ODP#hasChromaFormat
<http://mklab.iti.gr/pericles/DigitalVideo_ODP#hasChromaFormat> rdf:type owl:NamedIndividual ,
                                                                         odin:ODPElement ;
                                                                odin:describedIn odin:hasChromaFormat_Descr ;
                                                                rdfs:comment "Associates a video stream with a chroma format." .


###  http://mklab.iti.gr/pericles/DigitalVideo_ODP#hasCodingStandard
<http://mklab.iti.gr/pericles/DigitalVideo_ODP#hasCodingStandard> rdf:type owl:NamedIndividual ,
                                                                           odin:ODPElement ;
                                                                  odin:describedIn odin:hasCodingStandard_Descr ;
                                                                  rdfs:comment "Associates a video or audio stream with a coding standard." .


###  http://mklab.iti.gr/pericles/DigitalVideo_ODP#hasColourSpaceType
<http://mklab.iti.gr/pericles/DigitalVideo_ODP#hasColourSpaceType> rdf:type owl:NamedIndividual ,
                                                                            odin:ODPElement ;
                                                                   odin:describedIn odin:hasColourSpaceType_Descr ;
                                                                   rdfs:comment "Associates a video stream with a colour space type." .


###  http://mklab.iti.gr/pericles/DigitalVideo_ODP#hasCompressionType
<http://mklab.iti.gr/pericles/DigitalVideo_ODP#hasCompressionType> rdf:type owl:NamedIndividual ;
                                                                   odin:describedIn odin:hasCompressionType_Descr ;
                                                                   rdfs:comment "Associates a video or audio codec with a compression type." .


###  http://mklab.iti.gr/pericles/DigitalVideo_ODP#hasEmbeddingType
<http://mklab.iti.gr/pericles/DigitalVideo_ODP#hasEmbeddingType> rdf:type owl:NamedIndividual ,
                                                                          odin:ODPElement ;
                                                                 odin:describedIn odin:hasEmbeddingType_Descr ;
                                                                 rdfs:comment "Associates a subtitle stream with an embedding type." .


###  http://mklab.iti.gr/pericles/DigitalVideo_ODP#hasFrameRate
<http://mklab.iti.gr/pericles/DigitalVideo_ODP#hasFrameRate> rdf:type owl:NamedIndividual ,
                                                                      odin:ODPElement ;
                                                             odin:describedIn odin:hasFrameRate_Descr ;
                                                             rdfs:comment "Associates a video stream with a frame rate." .


###  http://mklab.iti.gr/pericles/DigitalVideo_ODP#hasFrameSize
<http://mklab.iti.gr/pericles/DigitalVideo_ODP#hasFrameSize> rdf:type owl:NamedIndividual ,
                                                                      odin:ODPElement ;
                                                             odin:describedIn odin:hasFrameSize_Descr ;
                                                             rdfs:comment "Associates a video stream with a frame size." .


###  http://mklab.iti.gr/pericles/DigitalVideo_ODP#hasPlaybackDuration
<http://mklab.iti.gr/pericles/DigitalVideo_ODP#hasPlaybackDuration> rdf:type owl:NamedIndividual ,
                                                                             odin:ODPElement ;
                                                                    odin:describedIn odin:hasPlaybackDuration_Descr ;
                                                                    rdfs:comment "Associates a digital video, a video stream or an audio stream with a playback duration." .


###  http://mklab.iti.gr/pericles/DigitalVideo_ODP#hasRangeType
<http://mklab.iti.gr/pericles/DigitalVideo_ODP#hasRangeType> rdf:type owl:NamedIndividual ,
                                                                      odin:ODPElement ;
                                                             odin:describedIn odin:hasRangeType_Descr ;
                                                             rdfs:comment "Associates a video stream with a range type." .


###  http://mklab.iti.gr/pericles/DigitalVideo_ODP#hasSampleRate
<http://mklab.iti.gr/pericles/DigitalVideo_ODP#hasSampleRate> rdf:type owl:NamedIndividual ,
                                                                       odin:ODPElement ;
                                                              odin:describedIn odin:hasSampleRate_Descr ;
                                                              rdfs:comment "Associates a video stream or audio stream with a sample rate." .


###  http://mklab.iti.gr/pericles/DigitalVideo_ODP#hasScanType
<http://mklab.iti.gr/pericles/DigitalVideo_ODP#hasScanType> rdf:type owl:NamedIndividual ,
                                                                     odin:ODPElement ;
                                                            odin:describedIn odin:hasScanType_Descr ;
                                                            rdfs:comment "Associates a video stream with a scan type." .


###  http://mklab.iti.gr/pericles/DigitalVideo_ODP#hasSetOfStandards
<http://mklab.iti.gr/pericles/DigitalVideo_ODP#hasSetOfStandards> rdf:type owl:NamedIndividual ,
                                                                           odin:ODPElement ;
                                                                  odin:describedIn odin:hasSetOfStandards_Descr ;
                                                                  rdfs:comment "Associates a video stream with a set of standards." .


###  http://mklab.iti.gr/pericles/DigitalVideo_ODP#hasStream
<http://mklab.iti.gr/pericles/DigitalVideo_ODP#hasStream> rdf:type owl:NamedIndividual ,
                                                                   odin:ODPElement ;
                                                          odin:describedIn odin:hasStream_Descr ;
                                                          rdfs:comment "Associates a digital video with a stream." .


###  http://mklab.iti.gr/pericles/DigitalVideo_ODP#hasSubtitleStream
<http://mklab.iti.gr/pericles/DigitalVideo_ODP#hasSubtitleStream> rdf:type owl:NamedIndividual ,
                                                                           odin:ODPElement ;
                                                                  odin:describedIn odin:hasSubtitleStream_Descr ;
                                                                  rdfs:comment "Associates a digital video with an subtitle stream." .


###  http://mklab.iti.gr/pericles/DigitalVideo_ODP#hasSubtitleTextFormat
<http://mklab.iti.gr/pericles/DigitalVideo_ODP#hasSubtitleTextFormat> rdf:type owl:NamedIndividual ,
                                                                               odin:ODPElement ;
                                                                      odin:describedIn odin:hasSubtitleTextFormat_Descr ;
                                                                      rdfs:comment "Associates a subtitle stream with a subtitle text format." .


###  http://mklab.iti.gr/pericles/DigitalVideo_ODP#hasVideoCodecLevel
<http://mklab.iti.gr/pericles/DigitalVideo_ODP#hasVideoCodecLevel> rdf:type owl:NamedIndividual ,
                                                                            odin:ODPElement ;
                                                                   odin:describedIn odin:hasVideoCodecLevel_Descr ;
                                                                   rdfs:comment "Associates a video codec with a video codec level." .


###  http://mklab.iti.gr/pericles/DigitalVideo_ODP#hasVideoCodecProfile
<http://mklab.iti.gr/pericles/DigitalVideo_ODP#hasVideoCodecProfile> rdf:type owl:NamedIndividual ,
                                                                              odin:ODPElement ;
                                                                     odin:describedIn odin:hasVideoCodecProfile_Descr ;
                                                                     rdfs:comment "Associates a video codec with a video codec profile." .


###  http://mklab.iti.gr/pericles/DigitalVideo_ODP#hasVideoQualityMeasurement
<http://mklab.iti.gr/pericles/DigitalVideo_ODP#hasVideoQualityMeasurement> rdf:type owl:NamedIndividual ,
                                                                                    odin:ODPElement ;
                                                                           odin:describedIn odin:hasVideoQualityMeasurement_Descr ;
                                                                           rdfs:comment "Associates a video stream with a video quality measurement." .


###  http://mklab.iti.gr/pericles/DigitalVideo_ODP#hasVideoQualityMetric
<http://mklab.iti.gr/pericles/DigitalVideo_ODP#hasVideoQualityMetric> rdf:type owl:NamedIndividual ,
                                                                               odin:ODPElement ;
                                                                      odin:describedIn odin:hasVideoQualityMetric_Descr ;
                                                                      rdfs:comment "Associates a video stream with a video quality metric." .


###  http://mklab.iti.gr/pericles/DigitalVideo_ODP#hasVideoStream
<http://mklab.iti.gr/pericles/DigitalVideo_ODP#hasVideoStream> rdf:type owl:NamedIndividual ,
                                                                        odin:ODPElement ;
                                                               odin:describedIn odin:hasVideoStream_Descr ;
                                                               rdfs:comment "Associates a digital video with a video stream." .


###  http://mklab.iti.gr/pericles/DigitalVideo_ODP#hasYUVSampleRange
<http://mklab.iti.gr/pericles/DigitalVideo_ODP#hasYUVSampleRange> rdf:type owl:NamedIndividual ,
                                                                           odin:ODPElement ;
                                                                  odin:describedIn odin:hasYUVSampleRange_Descr ;
                                                                  rdfs:comment "Associates a video stream with a YUV sample range." .


###  http://mklab.iti.gr/pericles/DigitalVideo_ODP#processedBy
<http://mklab.iti.gr/pericles/DigitalVideo_ODP#processedBy> rdf:type owl:NamedIndividual ,
                                                                     odin:ODPElement ;
                                                            odin:describedIn odin:processedBy_Descr ;
                                                            rdfs:comment "Associates a stream with a codec." .


###  http://mklab.iti.gr/pericles/DigitalVideo_ODP#wrappedBy
<http://mklab.iti.gr/pericles/DigitalVideo_ODP#wrappedBy> rdf:type owl:NamedIndividual ,
                                                                   odin:ODPElement ;
                                                          odin:describedIn odin:wrappedBy_Descr ;
                                                          rdfs:comment "Associates a digital video file with a container type." .


###  http://mklab.iti.gr/pericles/Policy_ODP#AutomationStatus
<http://mklab.iti.gr/pericles/Policy_ODP#AutomationStatus> rdf:type owl:NamedIndividual ,
                                                                    odin:ODPElement ;
                                                           odin:describedIn odin:AutomationStatus_Descr ;
                                                           rdfs:comment "E.g. manual, automated with human intervention, automated with human validation, fully automated, etc." ,
                                                                        "The level of automation of a policy. Specifies if a policy implementation requires human intervention." .


###  http://mklab.iti.gr/pericles/Policy_ODP#Descriptor
<http://mklab.iti.gr/pericles/Policy_ODP#Descriptor> rdf:type owl:NamedIndividual ,
                                                              odin:ODPElement ;
                                                     odin:describedIn odin:Descriptor_Descr ;
                                                     rdfs:comment "The various elements describing a policy." .


###  http://mklab.iti.gr/pericles/Policy_ODP#ImplementationStatus
<http://mklab.iti.gr/pericles/Policy_ODP#ImplementationStatus> rdf:type owl:NamedIndividual ,
                                                                        odin:ODPElement ;
                                                               odin:describedIn odin:ImplementationStatus_Descr ;
                                                               rdfs:comment "E.g. implemented, partially implemented, unimplemented, not-implementable, etc." ,
                                                                            "The level of implementation of a policy" .


###  http://mklab.iti.gr/pericles/Policy_ODP#Language
<http://mklab.iti.gr/pericles/Policy_ODP#Language> rdf:type owl:NamedIndividual ,
                                                            odin:ODPElement ;
                                                   odin:describedIn odin:Language_Descr ;
                                                   rdfs:comment "E.g. natural language, ReAL, SPIN, etc." ,
                                                                "The language used for the policy definition" .


###  http://mklab.iti.gr/pericles/Policy_ODP#Policy
<http://mklab.iti.gr/pericles/Policy_ODP#Policy> rdf:type owl:NamedIndividual ,
                                                          odin:ODPElement ;
                                                 odin:describedIn odin:Policy_Descr ;
                                                 rdfs:comment "A deliberate system of principles to guide decisions and achieve rational outcomes. A policy is a statement of intent, and is implemented as a procedure or protocol." .


###  http://mklab.iti.gr/pericles/Policy_ODP#PolicyType
<http://mklab.iti.gr/pericles/Policy_ODP#PolicyType> rdf:type owl:NamedIndividual ,
                                                              odin:ODPElement ;
                                                     odin:describedIn odin:PolicyType_Descr ;
                                                     rdfs:comment "E.g. mandatory, legal requirement, aspirational, business driven, etc." ,
                                                                  "Not all policies are equal; mandatory ones must be implemented to satisfy law or other requirements, others are aspirational, and most are met with the best possible effort." ,
                                                                  "The type of policy." .


###  http://mklab.iti.gr/pericles/Policy_ODP#Process
<http://mklab.iti.gr/pericles/Policy_ODP#Process> rdf:type owl:NamedIndividual ,
                                                           odin:ODPElement ;
                                                  odin:describedIn odin:Process_Descr ;
                                                  rdfs:comment "A sequence of interdependent and linked procedures which, at every stage, consume one or more resources (time, energy, machines, money) to convert inputs (data, material, parts, etc.) into outputs." .


###  http://mklab.iti.gr/pericles/Policy_ODP#RequirementLevel
<http://mklab.iti.gr/pericles/Policy_ODP#RequirementLevel> rdf:type owl:NamedIndividual ,
                                                                    odin:ODPElement ;
                                                           odin:describedIn odin:RequirementLevel_Descr ;
                                                           rdfs:comment "E.g. must, must not, should, shoud not, may, etc." ,
                                                                        "The level of a policy's compliance" .


###  http://mklab.iti.gr/pericles/Policy_ODP#Statement
<http://mklab.iti.gr/pericles/Policy_ODP#Statement> rdf:type owl:NamedIndividual ,
                                                             odin:ODPElement ;
                                                    odin:describedIn odin:Statement_Descr ;
                                                    rdfs:comment "Detailed definition of the policy contents." .


###  http://mklab.iti.gr/pericles/Policy_ODP#Version
<http://mklab.iti.gr/pericles/Policy_ODP#Version> rdf:type owl:NamedIndividual ,
                                                           odin:ODPElement ;
                                                  odin:describedIn odin:Version_Descr ;
                                                  rdfs:comment "A policy's version" .


###  http://mklab.iti.gr/pericles/Policy_ODP#assignedTo
<http://mklab.iti.gr/pericles/Policy_ODP#assignedTo> rdf:type owl:NamedIndividual ,
                                                              odin:ODPElement ;
                                                     odin:describedIn odin:assignedTo_Descr ;
                                                     rdfs:comment "Associates a policy to the agent that is responsible for the application of the policy (person or role)." .


###  http://mklab.iti.gr/pericles/Policy_ODP#hasAutomationStatus
<http://mklab.iti.gr/pericles/Policy_ODP#hasAutomationStatus> rdf:type owl:NamedIndividual ,
                                                                       odin:ODPElement ;
                                                              odin:describedIn odin:hasAutomationStatus_Descr ;
                                                              rdfs:comment "Associates a policy with an automation level." .


###  http://mklab.iti.gr/pericles/Policy_ODP#hasImplementationStatus
<http://mklab.iti.gr/pericles/Policy_ODP#hasImplementationStatus> rdf:type owl:NamedIndividual ,
                                                                           odin:ODPElement ;
                                                                  odin:describedIn odin:hasImplementationStatus_Descr ;
                                                                  rdfs:comment "Associates a policy with an implementation level." .


###  http://mklab.iti.gr/pericles/Policy_ODP#hasLanguage
<http://mklab.iti.gr/pericles/Policy_ODP#hasLanguage> rdf:type owl:NamedIndividual ,
                                                               odin:ODPElement ;
                                                      odin:describedIn odin:hasLanguage_Descr ;
                                                      rdfs:comment "Associates a policy with the language used for the policy definition." .


###  http://mklab.iti.gr/pericles/Policy_ODP#hasPolicyType
<http://mklab.iti.gr/pericles/Policy_ODP#hasPolicyType> rdf:type owl:NamedIndividual ,
                                                                 odin:ODPElement ;
                                                        odin:describedIn odin:hasPolicyType_Descr ;
                                                        rdfs:comment "Associates a policy with a policy type." .


###  http://mklab.iti.gr/pericles/Policy_ODP#hasRequirementLevel
<http://mklab.iti.gr/pericles/Policy_ODP#hasRequirementLevel> rdf:type owl:NamedIndividual ,
                                                                       odin:ODPElement ;
                                                              odin:describedIn odin:hasRequirementLevel_Descr ;
                                                              rdfs:comment "Associates a policy with an requirement level." .


###  http://mklab.iti.gr/pericles/Policy_ODP#hasStatement
<http://mklab.iti.gr/pericles/Policy_ODP#hasStatement> rdf:type owl:NamedIndividual ,
                                                                odin:ODPElement ;
                                                       odin:describedIn odin:hasStatement_Descr ;
                                                       rdfs:comment "Associates a policy with a statement, which is a detailed definition of the policy contents." .


###  http://mklab.iti.gr/pericles/Policy_ODP#hasSubPolicy
<http://mklab.iti.gr/pericles/Policy_ODP#hasSubPolicy> rdf:type owl:NamedIndividual ,
                                                                odin:ODPElement ;
                                                       odin:describedIn odin:hasSubPolicy_Descr ;
                                                       rdfs:comment "Associates a policy to another policy that is contained in the initial." .


###  http://mklab.iti.gr/pericles/Policy_ODP#hasValidationProcess
<http://mklab.iti.gr/pericles/Policy_ODP#hasValidationProcess> rdf:type owl:NamedIndividual ,
                                                                        odin:ODPElement ;
                                                               odin:describedIn odin:hasValidationProcess_Descr ;
                                                               rdfs:comment "Associates a policy with a process that is used to validate the policy." .


###  http://mklab.iti.gr/pericles/Policy_ODP#hasVersion
<http://mklab.iti.gr/pericles/Policy_ODP#hasVersion> rdf:type owl:NamedIndividual ,
                                                              odin:ODPElement ;
                                                     odin:describedIn odin:hasVersion_Descr ;
                                                     rdfs:comment "Defines a policy's version." .


###  http://mklab.iti.gr/pericles/Policy_ODP#implementedBy
<http://mklab.iti.gr/pericles/Policy_ODP#implementedBy> rdf:type owl:NamedIndividual ,
                                                                 odin:ODPElement ;
                                                        odin:describedIn odin:implementedBy_Descr ;
                                                        rdfs:comment "Associates a policy with a process that is used to implement the policy." .


###  http://mklab.iti.gr/pericles/Policy_ODP#targetsEntity
<http://mklab.iti.gr/pericles/Policy_ODP#targetsEntity> rdf:type owl:NamedIndividual ,
                                                                 odin:ODPElement ;
                                                        odin:describedIn odin:targetsEntity_Descr ;
                                                        rdfs:comment "Associates a policy with an entity that is subject to the policy." .


###  http://mklab.iti.gr/pericles/Policy_ODP#targetsUsers
<http://mklab.iti.gr/pericles/Policy_ODP#targetsUsers> rdf:type owl:NamedIndividual ,
                                                                odin:ODPElement ;
                                                       odin:describedIn odin:targetsUsers_Descr ;
                                                       rdfs:comment "Associates a policy to the user community the policy has been designed for." .


###  http://ontologydesignpatterns.org/ekp/Airline.owl
<http://ontologydesignpatterns.org/ekp/Airline.owl> rdf:type owl:NamedIndividual ,
                                                             odin:ODP ;
                                                    odin:describedIn odin:Airline.owl_Descr ;
                                                    odin:hasODPComponent <http://ontologydesignpatterns.org/ekp/Airline.owl#hasAircraft> ;
                                                    rdfs:comment "Airline Encyclopedic Knowledge Pattern" .


###  http://ontologydesignpatterns.org/ekp/Airline.owl#hasAircraft
<http://ontologydesignpatterns.org/ekp/Airline.owl#hasAircraft> rdf:type owl:NamedIndividual ,
                                                                         odin:ODPElement ;
                                                                odin:describedIn odin:hasAircraft_Descr ;
                                                                rdfs:comment "Relation between Airline and Aircraft" ,
                                                                             "Relazione tra Airline e Aircraft" .


###  http://ontologydesignpatterns.org/ekp/owl/EthnicGroup.owl
<http://ontologydesignpatterns.org/ekp/owl/EthnicGroup.owl> rdf:type owl:NamedIndividual ,
                                                                     odin:ODP ;
                                                            odin:describedIn <http://www.ontologydesignpatterns.org/ont/odin/odin.owl#owl/EthnicGroup.owl_Descr> ;
                                                            odin:hasODPComponent <http://ontologydesignpatterns.org/ekp/owl/EthnicGroup.owl#linksToAdministrativeRegion> ,
                                                                                 <http://ontologydesignpatterns.org/ekp/owl/EthnicGroup.owl#linksToCity> ,
                                                                                 <http://ontologydesignpatterns.org/ekp/owl/EthnicGroup.owl#linksToContinent> ,
                                                                                 <http://ontologydesignpatterns.org/ekp/owl/EthnicGroup.owl#linksToCountry> ,
                                                                                 <http://ontologydesignpatterns.org/ekp/owl/EthnicGroup.owl#linksToEthnicGroup> ,
                                                                                 <http://ontologydesignpatterns.org/ekp/owl/EthnicGroup.owl#linksToIsland> ,
                                                                                 <http://ontologydesignpatterns.org/ekp/owl/EthnicGroup.owl#linksToLanguage> ,
                                                                                 <http://ontologydesignpatterns.org/ekp/owl/EthnicGroup.owl#linksToMilitaryConflict> ,
                                                                                 <http://ontologydesignpatterns.org/ekp/owl/EthnicGroup.owl#linksToMusicalArtist> ,
                                                                                 <http://ontologydesignpatterns.org/ekp/owl/EthnicGroup.owl#linksToOfficeHolder> ,
                                                                                 <http://ontologydesignpatterns.org/ekp/owl/EthnicGroup.owl#linksToPresident> ,
                                                                                 <http://ontologydesignpatterns.org/ekp/owl/EthnicGroup.owl#linksToRiver> ,
                                                                                 <http://ontologydesignpatterns.org/ekp/owl/EthnicGroup.owl#linksToTown> ,
                                                                                 <http://ontologydesignpatterns.org/ekp/owl/EthnicGroup.owl#linksToWriter> ;
                                                            rdfs:comment "An encyclopedic knowledge pattern (EKP) identifying the core knowledge that describes a EthnicGroup" .


###  http://ontologydesignpatterns.org/ekp/owl/EthnicGroup.owl#linksToAdministrativeRegion
<http://ontologydesignpatterns.org/ekp/owl/EthnicGroup.owl#linksToAdministrativeRegion> rdf:type owl:NamedIndividual ,
                                                                                                 odin:ODPElement ;
                                                                                        odin:describedIn odin:linksToAdministrativeRegion_Descr ;
                                                                                        rdfs:comment "Relation between Ethnic Group and Administrative Region" ,
                                                                                                     "Relazione tra Ethnic Group e Administrative Region" .


###  http://ontologydesignpatterns.org/ekp/owl/EthnicGroup.owl#linksToCity
<http://ontologydesignpatterns.org/ekp/owl/EthnicGroup.owl#linksToCity> rdf:type owl:NamedIndividual ,
                                                                                 odin:ODPElement ;
                                                                        odin:describedIn odin:linksToCity_Descr ;
                                                                        rdfs:comment "Relation between Ethnic Group and City" ,
                                                                                     "Relazione tra Ethnic Group e City" .


###  http://ontologydesignpatterns.org/ekp/owl/EthnicGroup.owl#linksToContinent
<http://ontologydesignpatterns.org/ekp/owl/EthnicGroup.owl#linksToContinent> rdf:type owl:NamedIndividual ,
                                                                                      odin:ODPElement ;
                                                                             odin:describedIn odin:linksToContinent_Descr ;
                                                                             rdfs:comment "Relation between Ethnic Group and Continent" ,
                                                                                          "Relazione tra Ethnic Group e Continent" .


###  http://ontologydesignpatterns.org/ekp/owl/EthnicGroup.owl#linksToCountry
<http://ontologydesignpatterns.org/ekp/owl/EthnicGroup.owl#linksToCountry> rdf:type owl:NamedIndividual ,
                                                                                    odin:ODPElement ;
                                                                           odin:describedIn odin:linksToCountry_Descr ;
                                                                           rdfs:comment "Relation between Ethnic Group and Country" ,
                                                                                        "Relazione tra Ethnic Group e Country" .


###  http://ontologydesignpatterns.org/ekp/owl/EthnicGroup.owl#linksToEthnicGroup
<http://ontologydesignpatterns.org/ekp/owl/EthnicGroup.owl#linksToEthnicGroup> rdf:type owl:NamedIndividual ,
                                                                                        odin:ODPElement ;
                                                                               odin:describedIn odin:linksToEthnicGroup_Descr ;
                                                                               rdfs:comment "Relation between Ethnic Group and Ethnic Group" ,
                                                                                            "Relazione tra Ethnic Group e Ethnic Group" .


###  http://ontologydesignpatterns.org/ekp/owl/EthnicGroup.owl#linksToIsland
<http://ontologydesignpatterns.org/ekp/owl/EthnicGroup.owl#linksToIsland> rdf:type owl:NamedIndividual ,
                                                                                   odin:ODPElement ;
                                                                          odin:describedIn odin:linksToIsland_Descr ;
                                                                          rdfs:comment "Relation between Ethnic Group and Island" ,
                                                                                       "Relazione tra Ethnic Group e Island" .


###  http://ontologydesignpatterns.org/ekp/owl/EthnicGroup.owl#linksToLanguage
<http://ontologydesignpatterns.org/ekp/owl/EthnicGroup.owl#linksToLanguage> rdf:type owl:NamedIndividual ,
                                                                                     odin:ODPElement ;
                                                                            odin:describedIn odin:linksToLanguage_Descr ;
                                                                            rdfs:comment "Relation between Ethnic Group and Language" .


###  http://ontologydesignpatterns.org/ekp/owl/EthnicGroup.owl#linksToMilitaryConflict
<http://ontologydesignpatterns.org/ekp/owl/EthnicGroup.owl#linksToMilitaryConflict> rdf:type owl:NamedIndividual ,
                                                                                             odin:ODPElement ;
                                                                                    odin:describedIn odin:linksToMilitaryConflict_Descr ;
                                                                                    rdfs:comment "Relation between Ethnic Group and Military Conflict" ,
                                                                                                 "Relazione tra Ethnic Group e Military Conflict" .


###  http://ontologydesignpatterns.org/ekp/owl/EthnicGroup.owl#linksToMusicalArtist
<http://ontologydesignpatterns.org/ekp/owl/EthnicGroup.owl#linksToMusicalArtist> rdf:type owl:NamedIndividual ,
                                                                                          odin:ODPElement ;
                                                                                 odin:describedIn odin:linksToMusicalArtist_Descr ;
                                                                                 rdfs:comment "Relation between Ethnic Group and Musical Artist" ,
                                                                                              "Relazione tra Ethnic Group e Musical Artist" .


###  http://ontologydesignpatterns.org/ekp/owl/EthnicGroup.owl#linksToOfficeHolder
<http://ontologydesignpatterns.org/ekp/owl/EthnicGroup.owl#linksToOfficeHolder> rdf:type owl:NamedIndividual ,
                                                                                         odin:ODPElement ;
                                                                                odin:describedIn odin:linksToOfficeHolder_Descr ;
                                                                                rdfs:comment "Relation between Ethnic Group and Office Holder" ,
                                                                                             "Relazione tra Ethnic Group e Office Holder" .


###  http://ontologydesignpatterns.org/ekp/owl/EthnicGroup.owl#linksToPresident
<http://ontologydesignpatterns.org/ekp/owl/EthnicGroup.owl#linksToPresident> rdf:type owl:NamedIndividual ,
                                                                                      odin:ODPElement ;
                                                                             odin:describedIn odin:linksToPresident_Descr ;
                                                                             rdfs:comment "Relation between Ethnic Group and President" ,
                                                                                          "Relazione tra Ethnic Group e President" .


###  http://ontologydesignpatterns.org/ekp/owl/EthnicGroup.owl#linksToRiver
<http://ontologydesignpatterns.org/ekp/owl/EthnicGroup.owl#linksToRiver> rdf:type owl:NamedIndividual ,
                                                                                  odin:ODPElement ;
                                                                         odin:describedIn odin:linksToRiver_Descr ;
                                                                         rdfs:comment "Relation between Ethnic Group and River" ,
                                                                                      "Relazione tra Ethnic Group e River" .


###  http://ontologydesignpatterns.org/ekp/owl/EthnicGroup.owl#linksToTown
<http://ontologydesignpatterns.org/ekp/owl/EthnicGroup.owl#linksToTown> rdf:type owl:NamedIndividual ,
                                                                                 odin:ODPElement ;
                                                                        odin:describedIn odin:linksToTown_Descr ;
                                                                        rdfs:comment "Relation between Ethnic Group and Town" ,
                                                                                     "Relazione tra Ethnic Group e Town" .


###  http://ontologydesignpatterns.org/ekp/owl/EthnicGroup.owl#linksToWriter
<http://ontologydesignpatterns.org/ekp/owl/EthnicGroup.owl#linksToWriter> rdf:type owl:NamedIndividual ,
                                                                                   odin:ODPElement ;
                                                                          odin:describedIn odin:linksToWriter_Descr ;
                                                                          rdfs:comment "Relation between Ethnic Group and Writer" ,
                                                                                       "Relazione tra Ethnic Group e Writer" .


###  http://purl.org/NET/rdfchess/ontology/encodedAsSAN
<http://purl.org/NET/rdfchess/ontology/encodedAsSAN> rdf:type owl:NamedIndividual ,
                                                              odin:ODPElement ;
                                                     odin:describedIn odin:encodedAsSAN_Descr ;
                                                     rdfs:comment "SAN = Standard Algebraic Notation" .


###  http://purl.org/NET/rdfchess/ontology/hasECOCode
<http://purl.org/NET/rdfchess/ontology/hasECOCode> rdf:type owl:NamedIndividual ,
                                                            odin:ODPElement ;
                                                   odin:describedIn odin:hasECOCode_Descr ;
                                                   rdfs:comment "ECO = Encyclopedia of Chess Opening" .


###  http://purl.org/NET/rdfchess/ontology/hasPGNFile
<http://purl.org/NET/rdfchess/ontology/hasPGNFile> rdf:type owl:NamedIndividual ,
                                                            odin:ODPElement ;
                                                   odin:describedIn odin:hasPGNFile_Descr ;
                                                   rdfs:comment "PGN = Portable Game Notation" .


###  http://purl.org/NET/rdfchess/ontology/hasSANRecord
<http://purl.org/NET/rdfchess/ontology/hasSANRecord> rdf:type owl:NamedIndividual ,
                                                              odin:ODPElement ;
                                                     odin:describedIn odin:hasSANRecord_Descr ;
                                                     rdfs:comment "SAN = Standard Algebraic Notation" .


###  http://semantic.cs.put.poznan.pl/ontologies/newsreportingevent.owl
<http://semantic.cs.put.poznan.pl/ontologies/newsreportingevent.owl> rdf:type owl:NamedIndividual ,
                                                                              odin:ODP ;
                                                                     odin:describedIn odin:newsreportingevent.owl_Descr ;
                                                                     odin:hasODPComponent <http://semantic.cs.put.poznan.pl/ontologies/newsreportingevent.owl#Media> ,
                                                                                          <http://semantic.cs.put.poznan.pl/ontologies/newsreportingevent.owl#NewsEventReporter> ,
                                                                                          <http://semantic.cs.put.poznan.pl/ontologies/newsreportingevent.owl#NewsPresentationContext> ,
                                                                                          <http://semantic.cs.put.poznan.pl/ontologies/newsreportingevent.owl#NewsProvider> ,
                                                                                          <http://semantic.cs.put.poznan.pl/ontologies/newsreportingevent.owl#NewsReportingEvent> ,
                                                                                          <http://semantic.cs.put.poznan.pl/ontologies/newsreportingevent.owl#PresentationContext> ,
                                                                                          <http://semantic.cs.put.poznan.pl/ontologies/newsreportingevent.owl#hasPresentationContext> ,
                                                                                          <http://semantic.cs.put.poznan.pl/ontologies/newsreportingevent.owl#owns> ,
                                                                                          <http://semantic.cs.put.poznan.pl/ontologies/newsreportingevent.owl#presentedAt> ;
                                                                     rdfs:comment "Pattern description is available at: http://ontologydesignpatterns.org/wiki/Submissions:NewsReportingEvent" ,
                                                                                  "This ontology is a formalisation of the News Reporting Event ontology design pattern." .


###  http://semantic.cs.put.poznan.pl/ontologies/reportingevent.owl
<http://semantic.cs.put.poznan.pl/ontologies/reportingevent.owl> rdf:type owl:NamedIndividual ,
                                                                          odin:ODP ;
                                                                 odin:describedIn odin:reportingevent.owl_Descr ;
                                                                 odin:hasODPComponent <http://semantic.cs.put.poznan.pl/ontologies/reportingevent.owl#ActualEvent> ,
                                                                                      <http://semantic.cs.put.poznan.pl/ontologies/reportingevent.owl#ActualEventViewContext> ,
                                                                                      <http://semantic.cs.put.poznan.pl/ontologies/reportingevent.owl#SourceActivity> ,
                                                                                      <http://semantic.cs.put.poznan.pl/ontologies/reportingevent.owl#SourceObject> ,
                                                                                      <http://semantic.cs.put.poznan.pl/ontologies/reportingevent.owl#hasContext> ,
                                                                                      <http://semantic.cs.put.poznan.pl/ontologies/reportingevent.owl#isBasedOn> ,
                                                                                      <http://semantic.cs.put.poznan.pl/ontologies/reportingevent.owl#isBasedOnSourceActivity> ,
                                                                                      <http://semantic.cs.put.poznan.pl/ontologies/reportingevent.owl#isBasedOnSourceObject> ,
                                                                                      <http://semantic.cs.put.poznan.pl/ontologies/reportingevent.owl#reports> ;
                                                                 rdfs:comment "Pattern description is available at: http://ontologydesignpatterns.org/wiki/Submissions:ReportingEvent" .


###  http://semantic.cs.put.poznan.pl/ontologies/newsreportingevent.owl#Media
<http://semantic.cs.put.poznan.pl/ontologies/newsreportingevent.owl#Media> rdf:type owl:NamedIndividual ,
                                                                                    odin:ODPElement ;
                                                                           odin:describedIn odin:Media_Descr ;
                                                                           rdfs:comment "An entity that allows a communication of news messages, for example a TV station, radio station, newspaper, website, etc." .


###  http://semantic.cs.put.poznan.pl/ontologies/newsreportingevent.owl#NewsEventReporter
<http://semantic.cs.put.poznan.pl/ontologies/newsreportingevent.owl#NewsEventReporter> rdf:type owl:NamedIndividual ,
                                                                                                odin:ODPElement ;
                                                                                       odin:describedIn odin:NewsEventReporter_Descr ;
                                                                                       rdfs:comment "An Actor (usually a Person) that is an author of a certain ActualEventView.  NewsEventReporter is not linked to an ActualEventView directly, it is connected to NewsReportingEvent, which is designed to document the act of reporting." .


###  http://semantic.cs.put.poznan.pl/ontologies/newsreportingevent.owl#NewsPresentationContext
<http://semantic.cs.put.poznan.pl/ontologies/newsreportingevent.owl#NewsPresentationContext> rdf:type owl:NamedIndividual ,
                                                                                                      odin:ODPElement ;
                                                                                             odin:describedIn odin:NewsPresentationContext_Descr ;
                                                                                             rdfs:comment "Class for denoting circumstances of an actual event presentation. For example if an event was presented at the end of website, then end of website is its NewsPresentationContext.  NewsPresentationContext is not directly attached to an ActualEventView, it is attached to NewsReportingEvent, which designates the act of an event reporting." .


###  http://semantic.cs.put.poznan.pl/ontologies/newsreportingevent.owl#NewsProvider
<http://semantic.cs.put.poznan.pl/ontologies/newsreportingevent.owl#NewsProvider> rdf:type owl:NamedIndividual ,
                                                                                           odin:ODPElement ;
                                                                                  odin:describedIn odin:NewsProvider_Descr ;
                                                                                  rdfs:comment "An entity, usually a company, that ows a certain Media. For example Fox Entertainment Group owns the Fox News Channel. Fox Entertainment Group is a NewsProvider." .


###  http://semantic.cs.put.poznan.pl/ontologies/newsreportingevent.owl#NewsReportingEvent
<http://semantic.cs.put.poznan.pl/ontologies/newsreportingevent.owl#NewsReportingEvent> rdf:type owl:NamedIndividual ,
                                                                                                 odin:ODPElement ;
                                                                                        odin:describedIn odin:NewsReportingEvent_Descr ;
                                                                                        rdfs:comment "This is a subclass of ReportingEvent, designed to represent an act of reporting a certain actual event during a news programme or via other news media." .


###  http://semantic.cs.put.poznan.pl/ontologies/newsreportingevent.owl#PresentationContext
<http://semantic.cs.put.poznan.pl/ontologies/newsreportingevent.owl#PresentationContext> rdf:type owl:NamedIndividual ,
                                                                                                  odin:ODPElement ;
                                                                                         odin:describedIn odin:PresentationContext_Descr ;
                                                                                         rdfs:comment "Class for denoting circumstances of an entity presentation. If a waiter presented a dish with an apologetic smile, then the apologetic smile is a PresentationContext." .


###  http://semantic.cs.put.poznan.pl/ontologies/newsreportingevent.owl#hasPresentationContext
<http://semantic.cs.put.poznan.pl/ontologies/newsreportingevent.owl#hasPresentationContext> rdf:type owl:NamedIndividual ,
                                                                                                     odin:ODPElement ;
                                                                                            odin:describedIn odin:hasPresentationContext_Descr ;
                                                                                            rdfs:comment "This property can be used to link NewsReportingEvent to a NewsPresentationContext." .


###  http://semantic.cs.put.poznan.pl/ontologies/newsreportingevent.owl#owns
<http://semantic.cs.put.poznan.pl/ontologies/newsreportingevent.owl#owns> rdf:type owl:NamedIndividual ,
                                                                                   odin:ODPElement ;
                                                                          odin:describedIn odin:owns_Descr ;
                                                                          rdfs:comment "This property can be used to link a certain NewsProvider with a Media that the NewsProvider ows, e.g. Fox News Channel is owned by Fox Entertainment Group, which also owns other Media (FXX Channel, etc.).  This is an universal property, it can be also used in different context (e.g. Ruslana owns a Persian cat)." .


###  http://semantic.cs.put.poznan.pl/ontologies/newsreportingevent.owl#presentedAt
<http://semantic.cs.put.poznan.pl/ontologies/newsreportingevent.owl#presentedAt> rdf:type owl:NamedIndividual ,
                                                                                          odin:ODPElement ;
                                                                                 odin:describedIn odin:presentedAt_Descr ;
                                                                                 rdfs:comment "This property can be used to link a NewsReportingEvent to a Media (TV station, radio station, newspaper, webpage) at which a certain ActualEventView was presented.   This is an universal property and can be used in different contexts." .


###  http://semantic.cs.put.poznan.pl/ontologies/reportingevent.owl#ActualEvent
<http://semantic.cs.put.poznan.pl/ontologies/reportingevent.owl#ActualEvent> rdf:type owl:NamedIndividual ,
                                                                                      odin:ODPElement ;
                                                                             odin:describedIn odin:ActualEvent_Descr ;
                                                                             rdfs:comment "The event that is claimed to be real by a particular EventReporter.   The EventReporter is also making different claims about the event: its time interval, participants, place, cause, effect, etc. These properties are not directly attached to the ActualEvent, because it would make these facts the universal truths. Instead they are attached to an ActualEventView, There is one ActualEventView per each event report, but different instances can link to the same ActualEvent using the isAbout property." .


###  http://semantic.cs.put.poznan.pl/ontologies/reportingevent.owl#ActualEventViewContext
<http://semantic.cs.put.poznan.pl/ontologies/reportingevent.owl#ActualEventViewContext> rdf:type owl:NamedIndividual ,
                                                                                                 odin:ODPElement ;
                                                                                        odin:describedIn odin:ActualEventViewContext_Descr ;
                                                                                        rdfs:comment "Any object that is associated with an ActualEventView using property hasContext: time, place, cause, effect, participant, etc.  For example, if an EventReporter claims that an ActualEvent took place at Rome, then tookPlaceAt would be a subproperty of hasContext (attached to the ActualEventView) and Rome would be an instance of ActualEventViewContext.   There is no restriction on complexity of ActualEventViewContext, it can be for example a TimeInterval or a TimeIndexedParticipation." .


###  http://semantic.cs.put.poznan.pl/ontologies/reportingevent.owl#SourceActivity
<http://semantic.cs.put.poznan.pl/ontologies/reportingevent.owl#SourceActivity> rdf:type owl:NamedIndividual ,
                                                                                         odin:ODPElement ;
                                                                                odin:describedIn odin:SourceActivity_Descr ;
                                                                                rdfs:comment "The activity that was a source of information for a particular event report. For example, if a reporter visited a place in which a particular ActualEvent took place, to later describe the event as an ActualEventView in the act of ReportingEvent, his visit is a SourceActivity." .


###  http://semantic.cs.put.poznan.pl/ontologies/reportingevent.owl#SourceObject
<http://semantic.cs.put.poznan.pl/ontologies/reportingevent.owl#SourceObject> rdf:type owl:NamedIndividual ,
                                                                                       odin:ODPElement ;
                                                                              odin:describedIn odin:SourceObject_Descr ;
                                                                              rdfs:comment "The object that was a source of information for a particular event report. For example, if a historian describes a particular event based on a historical book, the book is an instance of the class SourceObject." .


###  http://semantic.cs.put.poznan.pl/ontologies/reportingevent.owl#hasContext
<http://semantic.cs.put.poznan.pl/ontologies/reportingevent.owl#hasContext> rdf:type owl:NamedIndividual ,
                                                                                     odin:ODPElement ;
                                                                            odin:describedIn odin:hasContext_Descr ;
                                                                            rdfs:comment "This is a general property to be used when attributing ActualEventView with any information. We can use any ontology designed for events description (CIDOC, LODE, etc.) in order to denote information about an actual event in ActualEventView, but it is assumed that all of this ontology properties will inherit from hasContext property and all objects of relations will inherit from ActualEventViewContext." .


###  http://semantic.cs.put.poznan.pl/ontologies/reportingevent.owl#isBasedOn
<http://semantic.cs.put.poznan.pl/ontologies/reportingevent.owl#isBasedOn> rdf:type owl:NamedIndividual ,
                                                                                    odin:ODPElement ;
                                                                           odin:describedIn odin:isBasedOn_Descr ;
                                                                           rdfs:comment "This property can be used to link ReportingEvent and sources it used to gather the knowledge about an ActualEvent." .


###  http://semantic.cs.put.poznan.pl/ontologies/reportingevent.owl#isBasedOnSourceActivity
<http://semantic.cs.put.poznan.pl/ontologies/reportingevent.owl#isBasedOnSourceActivity> rdf:type owl:NamedIndividual ,
                                                                                                  odin:ODPElement ;
                                                                                         odin:describedIn odin:isBasedOnSourceActivity_Descr ;
                                                                                         rdfs:comment "We specialised property isBasedOn so that the specialisation can be mapped to PROV vocabulary. Property isBasedOnSourceActivity is a subproperty of prov:wasInformedBy, which links two instances of prov:Activity.  This property can be used to link ReportingEvent with the SourceActivity that was used as a source of information about an ActualEvent, for example a correspondent visit to the event place." .


###  http://semantic.cs.put.poznan.pl/ontologies/reportingevent.owl#isBasedOnSourceObject
<http://semantic.cs.put.poznan.pl/ontologies/reportingevent.owl#isBasedOnSourceObject> rdf:type owl:NamedIndividual ,
                                                                                                odin:ODPElement ;
                                                                                       odin:describedIn odin:isBasedOnSourceObject_Descr ;
                                                                                       rdfs:comment "We specialised property isBasedOn so that the specialisation can be mapped to PROV vocabulary. Property isBasedOnSourceActivity is a subproperty of prov:used, which links an instance of prov:Activity and an instance of prov:Entity.  This property can be used to link a ReportingEvent and a SourceObject that was used as a source of information about an ActualEvent, for example a historical book." .


###  http://semantic.cs.put.poznan.pl/ontologies/reportingevent.owl#reports
<http://semantic.cs.put.poznan.pl/ontologies/reportingevent.owl#reports> rdf:type owl:NamedIndividual ,
                                                                                  odin:ODPElement ;
                                                                         odin:describedIn odin:reports_Descr ;
                                                                         rdfs:comment "This property can be used to link a ReportingEvent to an ActualEventView." .


###  http://w3id.org/daselab/onto/event#DASE_RULE
<http://w3id.org/daselab/onto/event#DASE_RULE> rdf:type owl:NamedIndividual ,
                                                        odin:ODPElement ;
                                               odin:describedIn odin:DASE_RULE_Descr ;
                                               rdfs:comment "Attached to an axiom, this annotation property provides information on the original (SWRL) rule from which the axiom was obtained through translation." .


###  http://w3id.org/daselab/onto/event#Event
<http://w3id.org/daselab/onto/event#Event> rdf:type owl:NamedIndividual ,
                                                    odin:ODPElement ;
                                           odin:describedIn odin:Event_Descr ;
                                           odin:odpType odin:Foundational ;
                                           rdfs:comment "Represents any kind of events. An event possesses a spatiotemporal extent, provides at least one participant-role, which is performed by some entity (agents or otherwise), and may be a sub-event of another event. An event may also have additional descriptive information, which is consolidated through an information object." .


###  http://w3id.org/daselab/onto/event#InformationObject
<http://w3id.org/daselab/onto/event#InformationObject> rdf:type owl:NamedIndividual ,
                                                                odin:ODPElement ;
                                                       odin:describedIn odin:InformationObject_Descr ;
                                                       odin:odpType odin:Foundational ;
                                                       rdfs:comment "An entity that encapsulates all descriptive or non-defining information of the corresponding event, e.g., names, additional identifiers, textual descriptions, etc. Should normally be aligned to a separate Information Object pattern." .


###  http://w3id.org/daselab/onto/event#SpatioTemporalExtent
<http://w3id.org/daselab/onto/event#SpatioTemporalExtent> rdf:type owl:NamedIndividual ,
                                                                   odin:ODPElement ;
                                                          odin:describedIn odin:SpatioTemporalExtent_Descr ;
                                                          rdfs:comment "Hook to a complex notion representing a unified spatial and temporal extent. Intended to cover non-static or discontinuous spatiotemporal extent. Should be aligned to a separate Spatiotemporal Extent pattern." .


###  http://w3id.org/daselab/onto/event#freshProp1
<http://w3id.org/daselab/onto/event#freshProp1> rdf:type owl:NamedIndividual ,
                                                         odin:ODPElement ;
                                                odin:describedIn odin:freshProp1_Descr ;
                                                rdfs:comment "This property is artificially generated in order to express the following rule in OWL: :Event(?x) ^ :providesParticipantRole(?x,?p) ^ :subEventOf(?x,?y) -> :providesParticipantRole(?y,?p).   The rule is translated into two axioms:   1. :Event SubClassOf: :freshProp1 some Self   2. inverse (:subEventOf) o :freshProp1 o :providesParticipantRole SubPropertyOf: : :providesParticipantRole" .


###  http://w3id.org/daselab/onto/event#freshProp2
<http://w3id.org/daselab/onto/event#freshProp2> rdf:type owl:NamedIndividual ,
                                                         odin:ODPElement ;
                                                odin:describedIn odin:freshProp2_Descr ;
                                                rdfs:comment "This property is artificially generated in order to express the following rule in OWL: :Event(?x) ^ :hasSpatioTemporalExtent(?x,?w) ^ :subEventOf(?x,?y) ^ :Event(?y) ^ :hasSpatioTemporalExtent(?y,?z) -> :subSpatioTemporalExtentOf(?w,?z).  The rule is translated into two axioms:   1. :Event SubClassOf: :freshProp2 some Self   2. inverse (:hasSpatioTemporalExtent) o :freshProp2 o :subEventOf o :freshProp2 o :hasSpatioTemporalExtent SubPropertyOf: :subSpatioTemporalExtentOf" .


###  http://w3id.org/daselab/onto/event#hasInformationObject
<http://w3id.org/daselab/onto/event#hasInformationObject> rdf:type owl:NamedIndividual ,
                                                                   odin:ODPElement ;
                                                          odin:describedIn odin:hasInformationObject_Descr ;
                                                          odin:odpType odin:Foundational ;
                                                          rdfs:comment "Property relating Event to InformationObject in this pattern. The domain of this property is not restricted to Event since it is possible that non-event to have an information object. The range is always InformationObject since it makes no sense to have a property named hasInformationObject to point to anything other than information object." .


###  http://w3id.org/daselab/onto/event#hasSpatioTemporalExtent
<http://w3id.org/daselab/onto/event#hasSpatioTemporalExtent> rdf:type owl:NamedIndividual ,
                                                                      odin:ODPElement ;
                                                             odin:describedIn odin:hasSpatioTemporalExtent_Descr ;
                                                             rdfs:comment "Property relating Event to SpatioTemporalExtent in this pattern. The range is always SpatioTemporalExtent (globally) since it makes no sense to have a property named hasSpatioTemporalExtent to point to anything other than spatiotemporal extent. Tthe domain is not set to Event as non-Event may also have spatiotemporal extent." .


###  http://w3id.org/daselab/onto/event#providesParticipantRole
<http://w3id.org/daselab/onto/event#providesParticipantRole> rdf:type owl:NamedIndividual ,
                                                                      odin:ODPElement ;
                                                             odin:describedIn odin:providesParticipantRole_Descr ;
                                                             odin:odpType odin:Foundational ;
                                                             rdfs:comment "Property relating Event to ParticipantRole in this pattern. The range is always ParticipantRole since it makes no sense to have a property named as providesParticipantRole not to point to a participant role. The domain is not set to Event as non-Event may also provide a participant role." .


###  http://w3id.org/daselab/onto/event#subEventOf
<http://w3id.org/daselab/onto/event#subEventOf> rdf:type owl:NamedIndividual ,
                                                         odin:ODPElement ;
                                                odin:describedIn odin:subEventOf_Descr ;
                                                rdfs:comment "Property expressing partonomic relation between two events. Domain and range are always Event." .


###  http://w3id.org/daselab/onto/event#subSpatioTemporalExtentOf
<http://w3id.org/daselab/onto/event#subSpatioTemporalExtentOf> rdf:type owl:NamedIndividual ,
                                                                        odin:ODPElement ;
                                                               odin:describedIn odin:subSpatioTemporalExtentOf_Descr ;
                                                               odin:odpType odin:Foundational ;
                                                               rdfs:comment "Property indicating partonomic relation between two spatiotemporal extents. The Event pattern only assumes that this is given by the spatiotemporal extent pattern actually used. Thus, domain and range are not explicitly stated and this property is included in axioms resulted by OWL translation of the following rule: :Event(?x) ^ :hasSpatioTemporalExtent(?x,?w) ^ :subEventOf(?x,?y) ^ :Event(?y) ^ :hasSpatioTemporalExtent(?y,?z) -> :subSpatioTemporalExtentOf(?w,?z)" .


###  http://w3id.org/daselab/onto/spatiotemporalextent#SpatioTemporalExtent
<http://w3id.org/daselab/onto/spatiotemporalextent#SpatioTemporalExtent> rdf:type owl:NamedIndividual ,
                                                                                  odin:ODPElement ;
                                                                         odin:describedIn odin:SpatioTemporalExtent_Descr ;
                                                                         odin:odpType odin:Foundational ;
                                                                         rdfs:comment "The class that represents the notion of spatiotemporal extent. A spatiotemporal extent is realized as a collection of generalized trajectories that have no temporal overlap." .


###  http://w3id.org/daselab/onto/spatiotemporalextent#Trajectory
<http://w3id.org/daselab/onto/spatiotemporalextent#Trajectory> rdf:type owl:NamedIndividual ,
                                                                        odin:ODPElement ;
                                                               odin:describedIn odin:Trajectory_Descr ;
                                                               odin:odpType odin:Foundational ;
                                                               rdfs:comment "The hook to the Trajectory pattern, which acts as a component of the Spatiotemporal Extent pattern." .


###  http://w3id.org/daselab/onto/spatiotemporalextent#hasTrajectory
<http://w3id.org/daselab/onto/spatiotemporalextent#hasTrajectory> rdf:type owl:NamedIndividual ,
                                                                           odin:ODPElement ;
                                                                  odin:describedIn odin:hasTrajectory_Descr ;
                                                                  odin:odpType odin:Foundational ;
                                                                  rdfs:comment "Set to be equivalent to trj:hasTrajectory from the Trajectory pattern, this property relates anything (including SpatioTemporalExtent) to Trajectory." .


###  http://w3id.org/daselab/onto/trajectory#Attribute
<http://w3id.org/daselab/onto/trajectory#Attribute> rdf:type owl:NamedIndividual ,
                                                             odin:ODPElement ;
                                                    odin:describedIn odin:Attribute_Descr ;
                                                    rdfs:comment "Captures additional information that enriches some fix or segment." .


###  http://w3id.org/daselab/onto/trajectory#EndingFix
<http://w3id.org/daselab/onto/trajectory#EndingFix> rdf:type owl:NamedIndividual ,
                                                             odin:ODPElement ;
                                                    odin:describedIn odin:EndingFix_Descr ;
                                                    rdfs:comment "The last fix in a particular sequence of fixes." .


###  http://w3id.org/daselab/onto/trajectory#Fix
<http://w3id.org/daselab/onto/trajectory#Fix> rdf:type owl:NamedIndividual ,
                                                       odin:ODPElement ;
                                              odin:describedIn odin:Fix_Descr ;
                                              rdfs:comment "Describes a fix, which is an adorned spatiotemporal point. A sequence of fixes form the trajectory." .


###  http://w3id.org/daselab/onto/trajectory#MovingObject
<http://w3id.org/daselab/onto/trajectory#MovingObject> rdf:type owl:NamedIndividual ,
                                                                odin:ODPElement ;
                                                       odin:describedIn odin:MovingObject_Descr ;
                                                       odin:odpType odin:Foundational ;
                                                       rdfs:comment "This is the hook to an ontology/pattern that describes the moving object, if any, which moves along the trajectory." .


###  http://w3id.org/daselab/onto/trajectory#Place
<http://w3id.org/daselab/onto/trajectory#Place> rdf:type owl:NamedIndividual ,
                                                         odin:ODPElement ;
                                                odin:describedIn odin:Place_Descr ;
                                                odin:odpType odin:Foundational ;
                                                rdfs:comment "This is the hook to other pattern/ontology that describes the notion of place, which is more general than just a location/geo-coordinate." .


###  http://w3id.org/daselab/onto/trajectory#Segment
<http://w3id.org/daselab/onto/trajectory#Segment> rdf:type owl:NamedIndividual ,
                                                           odin:ODPElement ;
                                                  odin:describedIn odin:Segment_Descr ;
                                                  rdfs:comment "The Segment class captures the connection between two consecutive fixes. That is, a segment starts from a fix and ends at another fix. If the pattern is used to model the trajectory of some moving object, each segment is traversed by that moving object. Additional information about a segment can be attached as attributes." .


###  http://w3id.org/daselab/onto/trajectory#StartingFix
<http://w3id.org/daselab/onto/trajectory#StartingFix> rdf:type owl:NamedIndividual ,
                                                               odin:ODPElement ;
                                                      odin:describedIn odin:StartingFix_Descr ;
                                                      odin:odpType odin:Foundational ;
                                                      rdfs:comment "The first fix in a particular sequence of fixes." .


###  http://w3id.org/daselab/onto/trajectory#TimeEntity
<http://w3id.org/daselab/onto/trajectory#TimeEntity> rdf:type owl:NamedIndividual ,
                                                              odin:ODPElement ;
                                                     odin:describedIn odin:TimeEntity_Descr ;
                                                     odin:odpType odin:Foundational ;
                                                     rdfs:comment "The hook to class/pattern/ontology that models time, this class provides the temporal extent of the trajectory. One example of time model is the W3C Time Ontology." .


###  http://w3id.org/daselab/onto/trajectory#Trajectory
<http://w3id.org/daselab/onto/trajectory#Trajectory> rdf:type owl:NamedIndividual ,
                                                              odin:ODPElement ;
                                                     odin:describedIn odin:Trajectory_Descr ;
                                                     rdfs:comment "Represents the notion of trajectory, this is the main class that can be hooked with other patterns that use the Trajectory pattern. Trajectory in this model is understood as a sequence of fixes connected by segments. There is exactly one starting fix and exactly one ending fix. Each fix has a temporal extent and a place (which is more general than just a location)." .


###  http://w3id.org/daselab/onto/trajectory#atPlace
<http://w3id.org/daselab/onto/trajectory#atPlace> rdf:type owl:NamedIndividual ,
                                                           odin:ODPElement ;
                                                  odin:describedIn odin:atPlace_Descr ;
                                                  odin:odpType odin:Foundational ;
                                                  rdfs:comment "Connects anything (including fixes in this pattern) to Place." .


###  http://w3id.org/daselab/onto/trajectory#atTime
<http://w3id.org/daselab/onto/trajectory#atTime> rdf:type owl:NamedIndividual ,
                                                          odin:ODPElement ;
                                                 odin:describedIn odin:atTime_Descr ;
                                                 rdfs:comment "Connects anything (including fixes in this pattern) to TimeEntity" .


###  http://w3id.org/daselab/onto/trajectory#endsAt
<http://w3id.org/daselab/onto/trajectory#endsAt> rdf:type owl:NamedIndividual ,
                                                          odin:ODPElement ;
                                                 odin:describedIn odin:endsAt_Descr ;
                                                 rdfs:comment "Connects a segment to the fix it ends at." .


###  http://w3id.org/daselab/onto/trajectory#hasAttribute
<http://w3id.org/daselab/onto/trajectory#hasAttribute> rdf:type owl:NamedIndividual ,
                                                                odin:ODPElement ;
                                                       odin:describedIn odin:hasAttribute_Descr ;
                                                       odin:odpType odin:Foundational ;
                                                       rdfs:comment "Connects a fix or a segment to an additional information as represented by an instance of Attribute." .


###  http://w3id.org/daselab/onto/trajectory#hasFix
<http://w3id.org/daselab/onto/trajectory#hasFix> rdf:type owl:NamedIndividual ,
                                                          odin:ODPElement ;
                                                 odin:describedIn odin:hasFix_Descr ;
                                                 rdfs:comment "Relating the trajectory to each of its fixes." .


###  http://w3id.org/daselab/onto/trajectory#hasSegment
<http://w3id.org/daselab/onto/trajectory#hasSegment> rdf:type owl:NamedIndividual ,
                                                              odin:ODPElement ;
                                                     odin:describedIn odin:hasSegment_Descr ;
                                                     odin:odpType odin:Foundational ;
                                                     rdfs:comment "Relating the trajectory to each of its segments." .


###  http://w3id.org/daselab/onto/trajectory#hasTrajectory
<http://w3id.org/daselab/onto/trajectory#hasTrajectory> rdf:type owl:NamedIndividual ,
                                                                 odin:ODPElement ;
                                                        odin:describedIn odin:hasTrajectory_Descr ;
                                                        rdfs:comment "Anything that has a trajectory can use this property to connect it to the trajectory instance." .


###  http://w3id.org/daselab/onto/trajectory#nextFix
<http://w3id.org/daselab/onto/trajectory#nextFix> rdf:type owl:NamedIndividual ,
                                                           odin:ODPElement ;
                                                  odin:describedIn odin:nextFix_Descr ;
                                                  odin:odpType odin:Foundational ;
                                                  rdfs:comment "Relates one fix to the immediately following fix in the sequence." .


###  http://w3id.org/daselab/onto/trajectory#startsFrom
<http://w3id.org/daselab/onto/trajectory#startsFrom> rdf:type owl:NamedIndividual ,
                                                              odin:ODPElement ;
                                                     odin:describedIn odin:startsFrom_Descr ;
                                                     odin:odpType odin:Foundational ;
                                                     rdfs:comment "Connects a segment to the fix it starts from." .


###  http://w3id.org/daselab/onto/trajectory#traversedBy
<http://w3id.org/daselab/onto/trajectory#traversedBy> rdf:type owl:NamedIndividual ,
                                                               odin:ODPElement ;
                                                      odin:describedIn odin:traversedBy_Descr ;
                                                      rdfs:comment "Connect a segment to the moving object that traverses it." .


###  http://w3id.org/food/ontology/dir_Descr
<http://w3id.org/food/ontology/dir_Descr> rdf:type owl:NamedIndividual ;
                                          isnet:activates <http://www.ontologydesignpatterns.org/ont/is/isaac_vanilla.owl#CENTER_PERIPHERY> ,
                                                          <http://www.ontologydesignpatterns.org/ont/is/isaac_vanilla.owl#PART_WHOLE> ;
                                          isnet:hasActivator <https://w3id.org/framester/wn/wn30/instances/synset-context-noun-1> ,
                                                             <https://w3id.org/framester/wn/wn30/instances/synset-range-verb-1> .


###  http://www.descartes-core.org/patterns/owl/transportPattern#TransportEntity
<http://www.descartes-core.org/patterns/owl/transportPattern#TransportEntity> rdf:type owl:NamedIndividual ,
                                                                                       odin:ODPElement ;
                                                                              odin:describedIn odin:TransportEntity_Descr ;
                                                                              odin:odpType odin:Foundational ;
                                                                              rdfs:comment "The Transport Entity concept represents the identity of the circumscribed portion of energy or mass that is moved." .


###  http://www.descartes-core.org/patterns/owl/transportPattern#TransportEvent
<http://www.descartes-core.org/patterns/owl/transportPattern#TransportEvent> rdf:type owl:NamedIndividual ,
                                                                                      odin:ODPElement ;
                                                                             odin:describedIn odin:TransportEvent_Descr ;
                                                                             rdfs:comment "A Transport Event describes a specific transport phenomenon, as movement of some mass or energy (measurable entity) from one location to another, based on a common and persistent frame of reference." .


###  http://www.descartes-core.org/patterns/owl/transportPattern#TransportMechanim
<http://www.descartes-core.org/patterns/owl/transportPattern#TransportMechanim> rdf:type owl:NamedIndividual ,
                                                                                         odin:ODPElement ;
                                                                                odin:describedIn odin:TransportMechanim_Descr ;
                                                                                rdfs:comment "The transportMechanism concept captures the nature of the source that acts upon the transportEntity, and thus induces a transportEvent." .


###  http://www.descartes-core.org/patterns/owl/transportPattern#referenceFrame
<http://www.descartes-core.org/patterns/owl/transportPattern#referenceFrame> rdf:type owl:NamedIndividual ,
                                                                                      odin:ODPElement ;
                                                                             odin:describedIn odin:referenceFrame_Descr ;
                                                                             rdfs:comment "This property is significant in that it serves to restrict and disambiguate a myriad of inherent facets, often in juxtaposition, associated with the Earths complex phenomena. The reference frame is provided to restrict the input values for a given instantiation, inherently providing context to the local representation." .


###  http://www.irit.fr/recherches/MELODI/ontologies/AAE
<http://www.irit.fr/recherches/MELODI/ontologies/AAE> rdf:type owl:NamedIndividual ,
                                                               odin:ODP ;
                                                      odin:describedIn odin:AAE_Descr ;
                                                      odin:hasODPComponent <http://www.irit.fr/recherches/MELODI/ontologies/AAE#consumes> ;
                                                      rdfs:comment "This ontology samples the ontology hosted at http://www.irit.fr/recherches/MELODI/ontologies/SAN.owl. It describes with specific annotation the Actuation-Actuator-Effect ontology design pattern, which mirrors the Stimulus-Sensor-Observation ontology design pattern, found in the SSN ontology." .


###  http://www.irit.fr/recherches/MELODI/ontologies/AAE#consumes
<http://www.irit.fr/recherches/MELODI/ontologies/AAE#consumes> rdf:type owl:NamedIndividual ,
                                                                        odin:ODPElement ;
                                                               odin:describedIn odin:consumes_Descr ;
                                                               rdfs:comment "An Actuation involves an Actuator, and the Input this Actuator consumes." .


###  http://www.irit.fr/recherches/MELODI/ontologies/SAN.owl#ActuatingCapability
<http://www.irit.fr/recherches/MELODI/ontologies/SAN.owl#ActuatingCapability> rdf:type owl:NamedIndividual ;
                                                                              odin:describedIn odin:ActuatingCapability_Descr ;
                                                                              rdfs:comment "Represents actuation properties such as precision, latency, power consumption, and the environmental conditions in which these actuation can take place normally." .


###  http://www.irit.fr/recherches/MELODI/ontologies/SAN.owl#ActuatingDevice
<http://www.irit.fr/recherches/MELODI/ontologies/SAN.owl#ActuatingDevice> rdf:type owl:NamedIndividual ;
                                                                          odin:describedIn odin:ActuatingDevice_Descr ;
                                                                          rdfs:comment "A device that implements actuating" .


###  http://www.irit.fr/recherches/MELODI/ontologies/SAN.owl#ActuatingRange
<http://www.irit.fr/recherches/MELODI/ontologies/SAN.owl#ActuatingRange> rdf:type owl:NamedIndividual ;
                                                                         odin:describedIn odin:ActuatingRange_Descr ;
                                                                         rdfs:comment "Range of commands that the actuator can receive and transduce into the physical world without damage to itself or security issues to its surrounding environment." .


###  http://www.irit.fr/recherches/MELODI/ontologies/SAN.owl#ActuatingTime
<http://www.irit.fr/recherches/MELODI/ontologies/SAN.owl#ActuatingTime> rdf:type owl:NamedIndividual ;
                                                                        odin:describedIn odin:ActuatingTime_Descr ;
                                                                        rdfs:comment "Time between the moment when the actuator receives an actuation command and the actual actuation." .


###  http://www.irit.fr/recherches/MELODI/ontologies/SAN.owl#Actuator
<http://www.irit.fr/recherches/MELODI/ontologies/SAN.owl#Actuator> rdf:type owl:NamedIndividual ;
                                                                   odin:describedIn odin:Actuator_Descr ;
                                                                   rdfs:comment "An actuator is an entity which is able to act upon the physical world. Whether it is a light bulb or a servomotor, an actuator receives inputs represented by Actuations and produces an effect on the world." .


###  http://www.irit.fr/recherches/MELODI/ontologies/SAN.owl#ActuatorInput
<http://www.irit.fr/recherches/MELODI/ontologies/SAN.owl#ActuatorInput> rdf:type owl:NamedIndividual ;
                                                                        odin:describedIn odin:ActuatorInput_Descr ;
                                                                        rdfs:comment "An actuator input is a piece of information provided to an actuator describing its expected behaviour, and it is described by an Actuation Value" .


###  http://www.irit.fr/recherches/MELODI/ontologies/SAN.owl#ActuatorOutput
<http://www.irit.fr/recherches/MELODI/ontologies/SAN.owl#ActuatorOutput> rdf:type owl:NamedIndividual ;
                                                                         odin:describedIn odin:ActuatorOutput_Descr ;
                                                                         rdfs:comment "Behaviour of an actuator after it has been given an input. To stick to its definition, an actuator output must have an effect on the physical world." .


###  http://www.irit.fr/recherches/MELODI/ontologies/SAN.owl#Effect
<http://www.irit.fr/recherches/MELODI/ontologies/SAN.owl#Effect> rdf:type owl:NamedIndividual ;
                                                                 odin:describedIn odin:Effect_Descr ;
                                                                 rdfs:comment "Concept bound to the definition of an actuator as an agent havong an effect on the physical world. Therefore, an effect is any kind of physical modification induced by an actuator." .


###  http://www.irit.fr/recherches/MELODI/ontologies/SAN.owl#actsOn
<http://www.irit.fr/recherches/MELODI/ontologies/SAN.owl#actsOn> rdf:type owl:NamedIndividual ;
                                                                 odin:describedIn odin:actsOn_Descr ;
                                                                 rdfs:comment "Relationship between an entity that acts upon a quantity or another entity" .


###  http://www.irit.fr/recherches/MELODI/ontologies/SAN.owl#actuationResults
<http://www.irit.fr/recherches/MELODI/ontologies/SAN.owl#actuationResults> rdf:type owl:NamedIndividual ;
                                                                           odin:describedIn odin:actuationResults_Descr ;
                                                                           rdfs:comment "Relation between an actuation and an actuator input, its result. Implements the ODP Effect-Actuator-Observation" .


###  http://www.irit.fr/recherches/MELODI/ontologies/SAN.owl#controlledBy
<http://www.irit.fr/recherches/MELODI/ontologies/SAN.owl#controlledBy> rdf:type owl:NamedIndividual ;
                                                                       odin:describedIn odin:controlledBy_Descr ;
                                                                       rdfs:comment "Describes the relationship between a controller entity and a controlled situation" .


###  http://www.irit.fr/recherches/MELODI/ontologies/SAN.owl#hasActuatingCapability
<http://www.irit.fr/recherches/MELODI/ontologies/SAN.owl#hasActuatingCapability> rdf:type owl:NamedIndividual ;
                                                                                 odin:describedIn odin:hasActuatingCapability_Descr ;
                                                                                 rdfs:comment "Relation between an Actuator and an ActuatingCapability, describing the actuating properties of an actuator." .


###  http://www.irit.fr/recherches/MELODI/ontologies/SAN.owl#hasActuatingProperty
<http://www.irit.fr/recherches/MELODI/ontologies/SAN.owl#hasActuatingProperty> rdf:type owl:NamedIndividual ;
                                                                               odin:describedIn odin:hasActuatingProperty_Descr ;
                                                                               rdfs:comment "Relation from an actuation capability to an actuation property." .


###  http://www.irit.fr/recherches/MELODI/ontologies/SAN.owl#hasEffect
<http://www.irit.fr/recherches/MELODI/ontologies/SAN.owl#hasEffect> rdf:type owl:NamedIndividual ;
                                                                    odin:describedIn odin:hasEffect_Descr ;
                                                                    rdfs:comment "Relationship between an Actuator and the effect that it induces. The Effect will be linked to a physical property that the actuator impacts" .


###  http://www.irit.fr/recherches/MELODI/ontologies/SAN.owl#hasPowerConsumption
<http://www.irit.fr/recherches/MELODI/ontologies/SAN.owl#hasPowerConsumption> rdf:type owl:NamedIndividual ;
                                                                              odin:describedIn odin:hasPowerConsumption_Descr ;
                                                                              rdfs:comment "This relationship expresses the power consumption of an appliance over time depending on its state." .


###  http://www.irit.fr/recherches/MELODI/ontologies/SAN.owl#impacts
<http://www.irit.fr/recherches/MELODI/ontologies/SAN.owl#impacts> rdf:type owl:NamedIndividual ;
                                                                  odin:describedIn odin:impacts_Descr ;
                                                                  rdfs:comment "Relationship between an effect and the property it impacts. Used in the Effect-Actuator-Actuation design pattern to describe the link between an actuator and the physical property it acts upon." .


###  http://www.irit.fr/recherches/MELODI/ontologies/SAN.owl#impactsState
<http://www.irit.fr/recherches/MELODI/ontologies/SAN.owl#impactsState> rdf:type owl:NamedIndividual ;
                                                                       odin:describedIn odin:impactsState_Descr ;
                                                                       rdfs:comment "This relationships links an entity that impacts a Ressource State and said State. For instance, if an Actuator is updated by an Actuation, this Actuation impacts the Actuator's State." .


###  http://www.irit.fr/recherches/MELODI/ontologies/SAN.owl#isConsumedBy
<http://www.irit.fr/recherches/MELODI/ontologies/SAN.owl#isConsumedBy> rdf:type owl:NamedIndividual ;
                                                                       odin:describedIn odin:isConsumedBy_Descr ;
                                                                       rdfs:comment "Describes a relation between a consumer and a consumee" .


###  http://www.irit.fr/recherches/MELODI/ontologies/SAN.owl#receivedActuation
<http://www.irit.fr/recherches/MELODI/ontologies/SAN.owl#receivedActuation> rdf:type owl:NamedIndividual ;
                                                                            odin:describedIn odin:receivedActuation_Descr ;
                                                                            rdfs:comment "Relationship between an actuator and an Actuation it received in order to modify its action." .


###  http://www.irit.fr/recherches/MELODI/ontologies/SAN.owl#triggersTransition
<http://www.irit.fr/recherches/MELODI/ontologies/SAN.owl#triggersTransition> rdf:type owl:NamedIndividual ;
                                                                             odin:describedIn odin:triggersTransition_Descr ;
                                                                             rdfs:comment "This relationship exists between an event and a Transition between two states this event induces. For example, a new actuation updating an actuator State triggers a Transition to do so." .


###  http://www.irit.fr/recherches/MELODI/ontologies/SAN.owl#wasActuationSent
<http://www.irit.fr/recherches/MELODI/ontologies/SAN.owl#wasActuationSent> rdf:type owl:NamedIndividual ;
                                                                           odin:describedIn odin:wasActuationSent_Descr ;
                                                                           rdfs:comment "Relationship between an actuation which was sent and the actuator that received it" .


###  http://www.ontologydesignpatterns.org/cp/reaction.owl
<http://www.ontologydesignpatterns.org/cp/reaction.owl> rdf:type owl:NamedIndividual ,
                                                                 odin:ODP ;
                                                        odin:describedIn odin:reaction.owl_Descr ;
                                                        odin:hasODPComponent <http://www.ontologydesignpatterns.org/cp/reaction.owl#Action> ,
                                                                             <http://www.ontologydesignpatterns.org/cp/reaction.owl#ExternalAgent> ,
                                                                             <http://www.ontologydesignpatterns.org/cp/reaction.owl#Reaction> ,
                                                                             <http://www.ontologydesignpatterns.org/cp/reaction.owl#hasOutcome> ,
                                                                             <http://www.ontologydesignpatterns.org/cp/reaction.owl#isOutcomeOf> ;
                                                        rdfs:comment "Candidates domain: Legal, Sport, Performance, Writing." .


###  http://www.ontologydesignpatterns.org/cp/owl/bag.owl
<http://www.ontologydesignpatterns.org/cp/owl/bag.owl> rdf:type owl:NamedIndividual ,
                                                                odin:ODP ;
                                                       odin:describedIn odin:bag.owl_Descr ;
                                                       odin:hasODPComponent <http://www.ontologydesignpatterns.org/cp/owl/bag.owl#Bag> ,
                                                                            <http://www.ontologydesignpatterns.org/cp/owl/bag.owl#Item> ,
                                                                            <http://www.ontologydesignpatterns.org/cp/owl/bag.owl#hasItem> ,
                                                                            <http://www.ontologydesignpatterns.org/cp/owl/bag.owl#itemOf> ,
                                                                            <http://www.ontologydesignpatterns.org/cp/owl/bag.owl#size> ;
                                                       odin:odpType odin:Foundational ;
                                                       rdfs:comment "The Bag is characterized by a collection that can have multiple copies of each object. This is performed through the Item entity. The Item is linking exaclty one resource through the relationship itemContent." .


###  http://www.ontologydesignpatterns.org/cp/owl/basicplan.owl
<http://www.ontologydesignpatterns.org/cp/owl/basicplan.owl> rdf:type owl:NamedIndividual ,
                                                                      odin:ODP ;
                                                             odin:describedIn odin:basicplan.owl_Descr ;
                                                             odin:hasODPComponent <http://www.ontologydesignpatterns.org/cp/owl/basicplan.owl#GoalSituation> ,
                                                                                  <http://www.ontologydesignpatterns.org/cp/owl/basicplan.owl#conceptualizes> ,
                                                                                  <http://www.ontologydesignpatterns.org/cp/owl/basicplan.owl#executesTask> ,
                                                                                  <http://www.ontologydesignpatterns.org/cp/owl/basicplan.owl#isConceptualizedBy> ,
                                                                                  <http://www.ontologydesignpatterns.org/cp/owl/basicplan.owl#isExecutedIn> ,
                                                                                  <http://www.ontologydesignpatterns.org/cp/owl/basicplan.owl#isParametrizedBy> ,
                                                                                  <http://www.ontologydesignpatterns.org/cp/owl/basicplan.owl#isSatisfiedBy> ,
                                                                                  <http://www.ontologydesignpatterns.org/cp/owl/basicplan.owl#parametrizes> ,
                                                                                  <http://www.ontologydesignpatterns.org/cp/owl/basicplan.owl#satisfies> ;
                                                             odin:odpType odin:Foundational ;
                                                             rdfs:comment "The basic plans. This content ontology design patterns represents plans descriptions and their executions. It is defined by combining and expanding other CPs: basic plans description, basic plans execution, and object role. Expansion involves the partial clone of ontology elements from DOLCE Ultra Lite and Plans Lite ontologies." .


###  http://www.ontologydesignpatterns.org/cp/owl/basicplanexecution.owl
<http://www.ontologydesignpatterns.org/cp/owl/basicplanexecution.owl> rdf:type owl:NamedIndividual ,
                                                                               odin:ODP ;
                                                                      odin:describedIn odin:basicplanexecution.owl_Descr ;
                                                                      odin:hasODPComponent <http://www.ontologydesignpatterns.org/cp/owl/basicplanexecution.owl#PlanExecution> ,
                                                                                           <http://www.ontologydesignpatterns.org/cp/owl/basicplanexecution.owl#actionHasParticipant> ,
                                                                                           <http://www.ontologydesignpatterns.org/cp/owl/basicplanexecution.owl#includesAction> ,
                                                                                           <http://www.ontologydesignpatterns.org/cp/owl/basicplanexecution.owl#includesAgent> ,
                                                                                           <http://www.ontologydesignpatterns.org/cp/owl/basicplanexecution.owl#includesObject> ,
                                                                                           <http://www.ontologydesignpatterns.org/cp/owl/basicplanexecution.owl#isParticipantInAction> ;
                                                                      odin:odpType odin:Foundational ;
                                                                      rdfs:comment "The basic plans execution content ontology design pattern represents the execution of a plan and the entity that participate in such an execution. This CP is the composition of other CPs: situation and region. Furthermore, it expands such CPs with ontology elements that are partial clones of elements from the DOCLE Ultra Lite and the Plans Lite ontologies." .


###  http://www.ontologydesignpatterns.org/cp/owl/classification.owl
<http://www.ontologydesignpatterns.org/cp/owl/classification.owl> rdf:type owl:NamedIndividual ,
                                                                           odin:ODP ;
                                                                  odin:describedIn odin:classification.owl_Descr ;
                                                                  odin:hasODPComponent <http://www.ontologydesignpatterns.org/cp/owl/classification.owl#Concept> ,
                                                                                       <http://www.ontologydesignpatterns.org/cp/owl/classification.owl#classifies> ,
                                                                                       <http://www.ontologydesignpatterns.org/cp/owl/classification.owl#isClassifiedBy> ;
                                                                  rdfs:comment "The classification content ontology design pattern. This CP represents the realtions between concepts e.g., roles, task, and entities to which concepts are assigned to e.g., person, activities. The CP is extracted form DOLCE Ultra Lite ontology." .


###  http://www.ontologydesignpatterns.org/cp/owl/collectionentity.owl
<http://www.ontologydesignpatterns.org/cp/owl/collectionentity.owl> rdf:type owl:NamedIndividual ,
                                                                             odin:ODP ;
                                                                    odin:describedIn odin:collectionentity.owl_Descr ;
                                                                    odin:hasODPComponent <http://www.ontologydesignpatterns.org/cp/owl/collectionentity.owl#Collection> ,
                                                                                         <http://www.ontologydesignpatterns.org/cp/owl/collectionentity.owl#hasMember> ;
                                                                    rdfs:comment "The collection entity pattern.   It is extracted from DOLCE-UltraLite by partial clone of elements." .


###  http://www.ontologydesignpatterns.org/cp/owl/componency.owl
<http://www.ontologydesignpatterns.org/cp/owl/componency.owl> rdf:type owl:NamedIndividual ,
                                                                       odin:ODP ;
                                                              odin:describedIn odin:componency.owl_Descr ;
                                                              odin:hasODPComponent <http://www.ontologydesignpatterns.org/cp/owl/componency.owl#Object> ,
                                                                                   <http://www.ontologydesignpatterns.org/cp/owl/componency.owl#hasComponent> ,
                                                                                   <http://www.ontologydesignpatterns.org/cp/owl/componency.owl#isComponentOf> ;
                                                              rdfs:comment "The componency pattern, without temporal indexing.   This pattern re-uses the part of pattern and is extracted from DOLCE-UltraLite by partial clone." .


###  http://www.ontologydesignpatterns.org/cp/owl/constituency.owl
<http://www.ontologydesignpatterns.org/cp/owl/constituency.owl> rdf:type owl:NamedIndividual ,
                                                                         odin:ODP ;
                                                                odin:describedIn odin:constituency.owl_Descr ;
                                                                odin:hasODPComponent <http://www.ontologydesignpatterns.org/cp/owl/constituency.owl#hasConstituent> ,
                                                                                     <http://www.ontologydesignpatterns.org/cp/owl/constituency.owl#isConstituentOf> ;
                                                                rdfs:comment "The constituency pattern. It is extracted from DOLCE-UltraLite by partial clone of elements." .


###  http://www.ontologydesignpatterns.org/cp/owl/coparticipation.owl
<http://www.ontologydesignpatterns.org/cp/owl/coparticipation.owl> rdf:type owl:NamedIndividual ,
                                                                            odin:ODP ;
                                                                   odin:describedIn odin:coparticipation.owl_Descr ;
                                                                   odin:odpType odin:Foundational ;
                                                                   rdfs:comment "The co-participation pattern.   This pattern re-uses the participation pattern and is extracted from DOLCE-UltraLite by partial clone of elements.  This minimal pattern is useful to abstract from specific or domain-oriented 'thematic role' relations, such as 'agent', 'patient', 'instrument', 'product', 'provides', 'activator', etc.  A property chain allows to derive coparticipation from simple participation relations. For a more complete version of this pattern, see the functionalsituation.owl pattern." .


###  http://www.ontologydesignpatterns.org/cp/owl/description.owl
<http://www.ontologydesignpatterns.org/cp/owl/description.owl> rdf:type owl:NamedIndividual ,
                                                                        odin:ODP ;
                                                               odin:describedIn odin:description.owl_Descr ;
                                                               odin:hasODPComponent <http://www.ontologydesignpatterns.org/cp/owl/description.owl#Concept> ,
                                                                                    <http://www.ontologydesignpatterns.org/cp/owl/description.owl#Description> ,
                                                                                    <http://www.ontologydesignpatterns.org/cp/owl/description.owl#defines> ,
                                                                                    <http://www.ontologydesignpatterns.org/cp/owl/description.owl#isConceptUsedIn> ,
                                                                                    <http://www.ontologydesignpatterns.org/cp/owl/description.owl#isDefinedIn> ,
                                                                                    <http://www.ontologydesignpatterns.org/cp/owl/description.owl#usesConcept> ;
                                                               odin:odpType odin:Foundational ;
                                                               rdfs:comment "The description pattern.   It is extracted from DOLCE-UltraLite by partial clone of elements." .


###  http://www.ontologydesignpatterns.org/cp/owl/descriptionandsituation.owl
<http://www.ontologydesignpatterns.org/cp/owl/descriptionandsituation.owl> rdf:type owl:NamedIndividual ,
                                                                                    odin:ODP ;
                                                                           odin:describedIn odin:descriptionandsituation.owl_Descr ;
                                                                           odin:hasODPComponent <http://www.ontologydesignpatterns.org/cp/owl/descriptionandsituation.owl#describes> ,
                                                                                                <http://www.ontologydesignpatterns.org/cp/owl/descriptionandsituation.owl#isDescribedBy> ,
                                                                                                <http://www.ontologydesignpatterns.org/cp/owl/descriptionandsituation.owl#isSatisfiedBy> ,
                                                                                                <http://www.ontologydesignpatterns.org/cp/owl/descriptionandsituation.owl#satisfies> ;
                                                                           rdfs:comment "The Description and Situation content ontology design pattern. This CP represents conceptualizations i.e., descriptions, and corresponding groundings i.e., situations. The pattern is extracted from DOLCE+DnS Ultralite by partial cloning of elements, and is composed of three other CPs: description, situation, and classification." .


###  http://www.ontologydesignpatterns.org/cp/owl/gotop.owl
<http://www.ontologydesignpatterns.org/cp/owl/gotop.owl> rdf:type owl:NamedIndividual ,
                                                                  odin:ODP ;
                                                         odin:describedIn odin:gotop.owl_Descr ;
                                                         odin:hasODPComponent <http://www.ontologydesignpatterns.org/cp/owl/gotop.owl#All> ,
                                                                              <http://www.ontologydesignpatterns.org/cp/owl/gotop.owl#BiologicalProcess> ,
                                                                              <http://www.ontologydesignpatterns.org/cp/owl/gotop.owl#CellularComponent> ,
                                                                              <http://www.ontologydesignpatterns.org/cp/owl/gotop.owl#MolecularFunction> ;
                                                         odin:odpType odin:Core ;
                                                         rdfs:comment "This pattern is peculiar to the biomolecular domain, where types of entities, rather than specific instances, are the main focus of interest. As a result, the Gene Ontology, based on this top-level categories, is a huge TBox." .


###  http://www.ontologydesignpatterns.org/cp/owl/intensionextension.owl
<http://www.ontologydesignpatterns.org/cp/owl/intensionextension.owl> rdf:type owl:NamedIndividual ,
                                                                               odin:ODP ;
                                                                      odin:describedIn odin:intensionextension.owl_Descr ;
                                                                      odin:hasODPComponent <http://www.ontologydesignpatterns.org/cp/owl/intensionextension.owl#isAbout> ,
                                                                                           <http://www.ontologydesignpatterns.org/cp/owl/intensionextension.owl#isReferenceOf> ;
                                                                      odin:odpType odin:Foundational ;
                                                                      rdfs:comment "The intension and extension pattern. It allows to represent the intensional expression and extensional reference of information objects. This pattern is extracted from DOLCE-UltraLite by partial clone of elements." .


###  http://www.ontologydesignpatterns.org/cp/owl/linnaeantaxonomy.owl
<http://www.ontologydesignpatterns.org/cp/owl/linnaeantaxonomy.owl> rdf:type owl:NamedIndividual ,
                                                                             odin:ODP ;
                                                                    odin:describedIn odin:linnaeantaxonomy.owl_Descr ;
                                                                    odin:hasODPComponent <http://www.ontologydesignpatterns.org/cp/owl/linnaeantaxonomy.owl#Class> ,
                                                                                         <http://www.ontologydesignpatterns.org/cp/owl/linnaeantaxonomy.owl#Genus> ,
                                                                                         <http://www.ontologydesignpatterns.org/cp/owl/linnaeantaxonomy.owl#Kingdom> ,
                                                                                         <http://www.ontologydesignpatterns.org/cp/owl/linnaeantaxonomy.owl#Order> ,
                                                                                         <http://www.ontologydesignpatterns.org/cp/owl/linnaeantaxonomy.owl#Phylum> ,
                                                                                         <http://www.ontologydesignpatterns.org/cp/owl/linnaeantaxonomy.owl#Species> ,
                                                                                         <http://www.ontologydesignpatterns.org/cp/owl/linnaeantaxonomy.owl#hasDirectHigherRank> ,
                                                                                         <http://www.ontologydesignpatterns.org/cp/owl/linnaeantaxonomy.owl#hasDirectLowerRank> ,
                                                                                         <http://www.ontologydesignpatterns.org/cp/owl/linnaeantaxonomy.owl#hasHigherRank> ,
                                                                                         <http://www.ontologydesignpatterns.org/cp/owl/linnaeantaxonomy.owl#hasLowerRank> ;
                                                                    rdfs:comment "The linnaean taxonomy content ontology design pattern represents the layered classification invented by Linneus in the XVIII century. It is created by reengineering Wikipedia articles about taxa, taxonomic ranks, and linnaean taxonomy." .


###  http://www.ontologydesignpatterns.org/cp/owl/move.owl
<http://www.ontologydesignpatterns.org/cp/owl/move.owl> rdf:type owl:NamedIndividual ,
                                                                 odin:ODP ;
                                                        odin:describedIn odin:move.owl_Descr ;
                                                        odin:hasODPComponent <http://www.ontologydesignpatterns.org/cp/owl/move.owl#Move> ,
                                                                             <http://www.ontologydesignpatterns.org/cp/owl/move.owl#PhysicalObject> ,
                                                                             <http://www.ontologydesignpatterns.org/cp/owl/move.owl#Place> ,
                                                                             <http://www.ontologydesignpatterns.org/cp/owl/move.owl#consistsOf> ,
                                                                             <http://www.ontologydesignpatterns.org/cp/owl/move.owl#movedFrom> ,
                                                                             <http://www.ontologydesignpatterns.org/cp/owl/move.owl#movedTo> ,
                                                                             <http://www.ontologydesignpatterns.org/cp/owl/move.owl#tookPlaceAt> ;
                                                        rdfs:comment "The move content ontology design pattern. This CP represents the action of moving a physical object from a place to another. The move CP is extracted from the CIDOC ontology." .


###  http://www.ontologydesignpatterns.org/cp/owl/naryparticipation.owl
<http://www.ontologydesignpatterns.org/cp/owl/naryparticipation.owl> rdf:type owl:NamedIndividual ,
                                                                              odin:ODP ;
                                                                     odin:describedIn odin:naryparticipation.owl_Descr ;
                                                                     rdfs:comment "The nary participation pattern.   This pattern re-uses participation and situation patterns. It is extracted from DOLCE-UltraLite by partial clone of elements." .


###  http://www.ontologydesignpatterns.org/cp/owl/objectrole.owl
<http://www.ontologydesignpatterns.org/cp/owl/objectrole.owl> rdf:type owl:NamedIndividual ,
                                                                       odin:ODP ;
                                                              odin:describedIn odin:objectrole.owl_Descr ;
                                                              odin:hasODPComponent <http://www.ontologydesignpatterns.org/cp/owl/objectrole.owl#Object> ,
                                                                                   <http://www.ontologydesignpatterns.org/cp/owl/objectrole.owl#Role> ,
                                                                                   <http://www.ontologydesignpatterns.org/cp/owl/objectrole.owl#hasRole> ,
                                                                                   <http://www.ontologydesignpatterns.org/cp/owl/objectrole.owl#isRoleOf> ;
                                                              rdfs:comment "It is extracted from DOLCE Ultra Lite ontology and specialize the classification CP. Object is an Entity, and Role is a Concept. The hasRole relation specializes the classifies relation, while the isRoleOf specializes the isClassifiedBy relation." .


###  http://www.ontologydesignpatterns.org/cp/owl/parameter.owl
<http://www.ontologydesignpatterns.org/cp/owl/parameter.owl> rdf:type owl:NamedIndividual ,
                                                                      odin:ODP ;
                                                             odin:describedIn odin:parameter.owl_Descr ;
                                                             odin:hasODPComponent <http://www.ontologydesignpatterns.org/cp/owl/parameter.owl#Concept> ,
                                                                                  <http://www.ontologydesignpatterns.org/cp/owl/parameter.owl#hasParameter> ,
                                                                                  <http://www.ontologydesignpatterns.org/cp/owl/parameter.owl#hasParameterDataValue> ,
                                                                                  <http://www.ontologydesignpatterns.org/cp/owl/parameter.owl#isParameterFor> ;
                                                             odin:odpType odin:Foundational ;
                                                             rdfs:comment "The parameter content ontology design pattern. This CP is extracted from the DOLCE Ultra Lite ontology. It represents parameters which are constraints or selections on observable values." .


###  http://www.ontologydesignpatterns.org/cp/owl/participation.owl
<http://www.ontologydesignpatterns.org/cp/owl/participation.owl> rdf:type owl:NamedIndividual ,
                                                                          odin:ODP ;
                                                                 odin:describedIn odin:participation.owl_Descr ;
                                                                 odin:hasODPComponent <http://www.ontologydesignpatterns.org/cp/owl/participation.owl#Event> ,
                                                                                      <http://www.ontologydesignpatterns.org/cp/owl/participation.owl#Object> ;
                                                                 rdfs:comment "The basic participation pattern, without temporal indexing.   It clones equivalent elements from DOLCE-UltraLite." .


###  http://www.ontologydesignpatterns.org/cp/owl/region.owl
<http://www.ontologydesignpatterns.org/cp/owl/region.owl> rdf:type owl:NamedIndividual ,
                                                                   odin:ODP ;
                                                          odin:describedIn odin:region.owl_Descr ;
                                                          odin:hasODPComponent <http://www.ontologydesignpatterns.org/cp/owl/region.owl#Region> ,
                                                                               <http://www.ontologydesignpatterns.org/cp/owl/region.owl#hasRegion> ,
                                                                               <http://www.ontologydesignpatterns.org/cp/owl/region.owl#hasRegionDataValue> ,
                                                                               <http://www.ontologydesignpatterns.org/cp/owl/region.owl#isRegionFor> ;
                                                          rdfs:comment "The region content ontology design pattern. This CP represents regions that are portions of a dimensional space which can be used as a value for a quality of an Entity. The CP is extracted from DOLCE + DnS Ultra Lite ontology." .


###  http://www.ontologydesignpatterns.org/cp/owl/set.owl
<http://www.ontologydesignpatterns.org/cp/owl/set.owl> rdf:type owl:NamedIndividual ,
                                                                odin:ODP ;
                                                       odin:describedIn odin:set.owl_Descr ;
                                                       odin:hasODPComponent <http://www.ontologydesignpatterns.org/cp/owl/set.owl#Set> ,
                                                                            <http://www.ontologydesignpatterns.org/cp/owl/set.owl#size> ;
                                                       odin:odpType odin:Foundational ;
                                                       rdfs:comment "A Set is a collection that cannot contain duplicate elements. A Set is expressed by linking to it directly all the members (elements), multiple identical values of members (elements) will be eliminated because by default they are treated as a set." .


###  http://www.ontologydesignpatterns.org/cp/owl/tagging.owl
<http://www.ontologydesignpatterns.org/cp/owl/tagging.owl> rdf:type owl:NamedIndividual ,
                                                                    odin:ODP ;
                                                           odin:describedIn odin:tagging.owl_Descr ;
                                                           rdfs:comment "The tagging ontology drafted by Tom Gruber in FOL, and formalized here in OWL by Aldo Gangemi with pattern-based design.  A Tag is here classified as a linguistic object that is used in the context of a Tagging Situation, which also involves a (tagged) Entity, an Agent, and a Folksonomy." .


###  http://www.ontologydesignpatterns.org/cp/owl/taskrole.owl
<http://www.ontologydesignpatterns.org/cp/owl/taskrole.owl> rdf:type owl:NamedIndividual ,
                                                                     odin:ODP ;
                                                            odin:describedIn odin:taskrole.owl_Descr ;
                                                            odin:hasODPComponent <http://www.ontologydesignpatterns.org/cp/owl/taskrole.owl#Role> ,
                                                                                 <http://www.ontologydesignpatterns.org/cp/owl/taskrole.owl#Task> ,
                                                                                 <http://www.ontologydesignpatterns.org/cp/owl/taskrole.owl#hasTask> ,
                                                                                 <http://www.ontologydesignpatterns.org/cp/owl/taskrole.owl#isTaskOf> ;
                                                            rdfs:comment "The task role pattern.   This pattern is extracted from DOLCE-UltraLite by partial clone of elements." .


###  http://www.ontologydesignpatterns.org/cp/owl/timeindexedparticipation.owl
<http://www.ontologydesignpatterns.org/cp/owl/timeindexedparticipation.owl> rdf:type owl:NamedIndividual ,
                                                                                     odin:ODP ;
                                                                            odin:describedIn odin:timeindexedparticipation.owl_Descr ;
                                                                            odin:hasODPComponent <http://www.ontologydesignpatterns.org/cp/owl/timeindexedparticipation.owl#TimeIndexedParticipation> ,
                                                                                                 <http://www.ontologydesignpatterns.org/cp/owl/timeindexedparticipation.owl#includesEvent> ,
                                                                                                 <http://www.ontologydesignpatterns.org/cp/owl/timeindexedparticipation.owl#includesObject> ;
                                                                            rdfs:comment "A time-indexed pattern for participation" .


###  http://www.ontologydesignpatterns.org/cp/owl/timeindexedpartof.owl
<http://www.ontologydesignpatterns.org/cp/owl/timeindexedpartof.owl> rdf:type owl:NamedIndividual ,
                                                                              odin:ODP ;
                                                                     odin:describedIn odin:timeindexedpartof.owl_Descr ;
                                                                     odin:hasODPComponent <http://www.ontologydesignpatterns.org/cp/owl/timeindexedpartof.owl#Object> ,
                                                                                          <http://www.ontologydesignpatterns.org/cp/owl/timeindexedpartof.owl#TimeIndexedPartOf> ,
                                                                                          <http://www.ontologydesignpatterns.org/cp/owl/timeindexedpartof.owl#includesPartObject> ,
                                                                                          <http://www.ontologydesignpatterns.org/cp/owl/timeindexedpartof.owl#includesWholeObject> ,
                                                                                          <http://www.ontologydesignpatterns.org/cp/owl/timeindexedpartof.owl#isPartObjectOf> ,
                                                                                          <http://www.ontologydesignpatterns.org/cp/owl/timeindexedpartof.owl#isWholeObjectOf> ;
                                                                     rdfs:comment "The time indexed part of pattern.   This pattern re-uses part of and time-indexed situation patterns. It is extracted from DOLCE-UltraLite by partial clone of elements." .


###  http://www.ontologydesignpatterns.org/cp/owl/timeindexedsituation.owl
<http://www.ontologydesignpatterns.org/cp/owl/timeindexedsituation.owl> rdf:type owl:NamedIndividual ,
                                                                                 odin:ODP ;
                                                                        odin:describedIn odin:timeindexedsituation.owl_Descr ;
                                                                        odin:hasODPComponent <http://www.ontologydesignpatterns.org/cp/owl/timeindexedsituation.owl#TimeIndexedSituation> ;
                                                                        odin:odpType odin:Foundational ;
                                                                        rdfs:comment "A generic pattern usable for all situations that require a temporal indexing." .


###  http://www.ontologydesignpatterns.org/cp/owl/timeinterval.owl
<http://www.ontologydesignpatterns.org/cp/owl/timeinterval.owl> rdf:type owl:NamedIndividual ,
                                                                         odin:ODP ;
                                                                odin:describedIn odin:timeinterval.owl_Descr ;
                                                                odin:hasODPComponent <http://www.ontologydesignpatterns.org/cp/owl/timeinterval.owl#TimeInterval> ,
                                                                                     <http://www.ontologydesignpatterns.org/cp/owl/timeinterval.owl#hasIntervalEndDate> ;
                                                                odin:odpType odin:Foundational ;
                                                                rdfs:comment "The time interval pattern.   This pattern is extracted from DOLCE-UltraLite by partial clone of elements and expansion. Two datatype properties have been added which allow to express the boundaries of the time interval.  Ranges of datatype properties are not indicated, because otherwise specializing them with different xsd datatypes would lead to inconsistencies." .


###  http://www.ontologydesignpatterns.org/cp/owl/timeperiod.owl
<http://www.ontologydesignpatterns.org/cp/owl/timeperiod.owl> rdf:type owl:NamedIndividual ,
                                                                       odin:ODP ;
                                                              odin:describedIn odin:timeperiod.owl_Descr ;
                                                              odin:hasODPComponent <http://www.ontologydesignpatterns.org/cp/owl/timeperiod.owl#TimePeriod> ,
                                                                                   <http://www.ontologydesignpatterns.org/cp/owl/timeperiod.owl#TimePeriodMeasurementUnit> ,
                                                                                   <http://www.ontologydesignpatterns.org/cp/owl/timeperiod.owl#hasTimePeriodMeasurementUnit> ,
                                                                                   <http://www.ontologydesignpatterns.org/cp/owl/timeperiod.owl#isTimePeriodMeasurementUnitOf> ,
                                                                                   <http://www.ontologydesignpatterns.org/cp/owl/timeperiod.owl#timePeriodValue> ;
                                                              rdfs:comment "A pattern for time periods." .


###  http://www.ontologydesignpatterns.org/cp/owl/topic.owl
<http://www.ontologydesignpatterns.org/cp/owl/topic.owl> rdf:type owl:NamedIndividual ,
                                                                  odin:ODP ;
                                                         odin:describedIn odin:topic.owl_Descr ;
                                                         odin:hasODPComponent <http://www.ontologydesignpatterns.org/cp/owl/topic.owl#Concept> ,
                                                                              <http://www.ontologydesignpatterns.org/cp/owl/topic.owl#Topic> ,
                                                                              <http://www.ontologydesignpatterns.org/cp/owl/topic.owl#farTopicFrom> ,
                                                                              <http://www.ontologydesignpatterns.org/cp/owl/topic.owl#hasCoreConcept> ,
                                                                              <http://www.ontologydesignpatterns.org/cp/owl/topic.owl#hasSubTopic> ,
                                                                              <http://www.ontologydesignpatterns.org/cp/owl/topic.owl#hasTopic> ,
                                                                              <http://www.ontologydesignpatterns.org/cp/owl/topic.owl#isCoreConceptFor> ,
                                                                              <http://www.ontologydesignpatterns.org/cp/owl/topic.owl#isSubTopicOf> ,
                                                                              <http://www.ontologydesignpatterns.org/cp/owl/topic.owl#isTopicOf> ,
                                                                              <http://www.ontologydesignpatterns.org/cp/owl/topic.owl#nearTopicTo> ,
                                                                              <http://www.ontologydesignpatterns.org/cp/owl/topic.owl#overlappingTopic> ;
                                                         odin:odpType odin:Foundational ;
                                                         rdfs:comment "It is a simplified version of the ontology http://ontologydesignpatterns.org/ont/dul/ontopic.owl" .


###  http://www.ontologydesignpatterns.org/cp/owl/transition.owl
<http://www.ontologydesignpatterns.org/cp/owl/transition.owl> rdf:type owl:NamedIndividual ,
                                                                       odin:ODP ;
                                                              odin:describedIn odin:transition.owl_Descr ;
                                                              odin:hasODPComponent <http://www.ontologydesignpatterns.org/cp/owl/transition.owl#Process> ,
                                                                                   <http://www.ontologydesignpatterns.org/cp/owl/transition.owl#Transition> ,
                                                                                   <http://www.ontologydesignpatterns.org/cp/owl/transition.owl#hasFinalStateAtTime> ,
                                                                                   <http://www.ontologydesignpatterns.org/cp/owl/transition.owl#hasInitialStateAtTime> ,
                                                                                   <http://www.ontologydesignpatterns.org/cp/owl/transition.owl#includesFinalSituation> ,
                                                                                   <http://www.ontologydesignpatterns.org/cp/owl/transition.owl#includesProcess> ,
                                                                                   <http://www.ontologydesignpatterns.org/cp/owl/transition.owl#isFinalSituationIncludedIn> ,
                                                                                   <http://www.ontologydesignpatterns.org/cp/owl/transition.owl#isProcessIncludedIn> ;
                                                              rdfs:comment "A simple pattern to represent transitions between states." .


###  http://www.ontologydesignpatterns.org/cp/owl/actingfor.owl#Agent
<http://www.ontologydesignpatterns.org/cp/owl/actingfor.owl#Agent> rdf:type owl:NamedIndividual ,
                                                                            odin:ODPElement ;
                                                                   odin:describedIn odin:Agent_Descr ;
                                                                   odin:odpType odin:Foundational ;
                                                                   rdfs:comment "Additional comment: a computational agent can be considered as a PhysicalAgent that realizes a certain class of algorithms (that can be considered as instances of InformationObject) that allow to obtain some behaviors that are considered typical of agents in general. For an ontology of computational objects based on DOLCE see e.g. and http://www.loa-cnr.it/COS/COS.owl, and http://www.loa-cnr.it/KCO/KCO.owl." ,
                                                                                "Any agentive Object , either physical (e.g. a whale, a robot, an oak), or social (e.g. a corporation, an institution, a community)." .


###  http://www.ontologydesignpatterns.org/cp/owl/actingfor.owl#SocialAgent
<http://www.ontologydesignpatterns.org/cp/owl/actingfor.owl#SocialAgent> rdf:type owl:NamedIndividual ,
                                                                                  odin:ODPElement ;
                                                                         odin:describedIn odin:SocialAgent_Descr ;
                                                                         rdfs:comment "Any individual whose existence is granted simply by its social communicability and capability of action (through some PhysicalAgent)." .


###  http://www.ontologydesignpatterns.org/cp/owl/actingfor.owl#actsFor
<http://www.ontologydesignpatterns.org/cp/owl/actingfor.owl#actsFor> rdf:type owl:NamedIndividual ,
                                                                              odin:ODPElement ;
                                                                     odin:describedIn odin:actsFor_Descr ;
                                                                     odin:odpType odin:Foundational ;
                                                                     rdfs:comment "The relation holding between any Agent, and a SocialAgent. In principle, a SocialAgent requires at least one PhysicalAgent in order to act, but this dependency can be 'delegated'; e.g. a university can be acted for by a department, which on its turm is acted for by physical agents." .


###  http://www.ontologydesignpatterns.org/cp/owl/actingfor.owl#actsThrough
<http://www.ontologydesignpatterns.org/cp/owl/actingfor.owl#actsThrough> rdf:type owl:NamedIndividual ,
                                                                                  odin:ODPElement ;
                                                                         odin:describedIn odin:actsThrough_Descr ;
                                                                         rdfs:comment "The relation holding between a PhysicalAgent and a SocialAgent. In principle, a SocialAgent requires at least one PhysicalAgent in order to act, but this dependency can be 'delegated', e.g. a university can be acted for by a department, which is acted for by physical agents." .


###  http://www.ontologydesignpatterns.org/cp/owl/agentrole.owl#Agent
<http://www.ontologydesignpatterns.org/cp/owl/agentrole.owl#Agent> rdf:type owl:NamedIndividual ,
                                                                            odin:ODPElement ;
                                                                   odin:describedIn odin:Agent_Descr ;
                                                                   rdfs:comment "Any agentive Object , either physical, or social." .


###  http://www.ontologydesignpatterns.org/cp/owl/bag.owl#Bag
<http://www.ontologydesignpatterns.org/cp/owl/bag.owl#Bag> rdf:type owl:NamedIndividual ,
                                                                    odin:ODPElement ;
                                                           odin:describedIn odin:Bag_Descr ;
                                                           odin:odpType odin:Foundational ;
                                                           rdfs:comment "Bag - Collection that can have a number of copies of each object" .


###  http://www.ontologydesignpatterns.org/cp/owl/bag.owl#Item
<http://www.ontologydesignpatterns.org/cp/owl/bag.owl#Item> rdf:type owl:NamedIndividual ,
                                                                     odin:ODPElement ;
                                                            odin:describedIn odin:Item_Descr ;
                                                            odin:odpType odin:Foundational ;
                                                            rdfs:comment "Item - Element belonging to a Bag" .


###  http://www.ontologydesignpatterns.org/cp/owl/bag.owl#hasItem
<http://www.ontologydesignpatterns.org/cp/owl/bag.owl#hasItem> rdf:type owl:NamedIndividual ,
                                                                        odin:ODPElement ;
                                                               odin:describedIn odin:hasItem_Descr ;
                                                               odin:odpType odin:Foundational ;
                                                               rdfs:comment "has item - The link to every item of the Bag" .


###  http://www.ontologydesignpatterns.org/cp/owl/bag.owl#itemOf
<http://www.ontologydesignpatterns.org/cp/owl/bag.owl#itemOf> rdf:type owl:NamedIndividual ,
                                                                       odin:ODPElement ;
                                                              odin:describedIn odin:itemOf_Descr ;
                                                              odin:odpType odin:Foundational ;
                                                              rdfs:comment "item of - The link from an item to the Bag where it is contained" .


###  http://www.ontologydesignpatterns.org/cp/owl/bag.owl#size
<http://www.ontologydesignpatterns.org/cp/owl/bag.owl#size> rdf:type owl:NamedIndividual ,
                                                                     odin:ODPElement ;
                                                            odin:describedIn odin:size_Descr ;
                                                            odin:odpType odin:Foundational ;
                                                            rdfs:comment "size - The number of items belonging to a collection" .


###  http://www.ontologydesignpatterns.org/cp/owl/basicplan.owl#GoalSituation
<http://www.ontologydesignpatterns.org/cp/owl/basicplan.owl#GoalSituation> rdf:type owl:NamedIndividual ,
                                                                                    odin:ODPElement ;
                                                                           odin:describedIn odin:GoalSituation_Descr ;
                                                                           odin:odpType odin:Foundational ;
                                                                           rdfs:comment "A goal situation is a situation that satisfies a goal.Opposite to the case of subplan executions, a goal situation is not part of a plan execution.In other words, it is not true in general that any situation satisfying a part of a description, is also part of the situation that satisfies the whole description. This helps to account for the following cases: a) Execution of plans containing abort or suspension conditions (the plan would be satisfied even if the goal has not been reached, see below), b) Incidental satisfaction, like when a situation satisfies a goal without being intentionally planned (but anyway desired)." .


###  http://www.ontologydesignpatterns.org/cp/owl/basicplan.owl#conceptualizes
<http://www.ontologydesignpatterns.org/cp/owl/basicplan.owl#conceptualizes> rdf:type owl:NamedIndividual ,
                                                                                     odin:ODPElement ;
                                                                            odin:describedIn odin:conceptualizes_Descr ;
                                                                            odin:odpType odin:Foundational ;
                                                                            rdfs:comment "A relation stating that an Agent is internally representing a SocialObject . E.g., 'John believes in the conspiracy theory'; 'Niels Bohr created the solar-system metaphor for the atomic theory'; 'Jacques assumes all swans are white'; 'the task force members share the attack plan'." .


###  http://www.ontologydesignpatterns.org/cp/owl/basicplan.owl#executesTask
<http://www.ontologydesignpatterns.org/cp/owl/basicplan.owl#executesTask> rdf:type owl:NamedIndividual ,
                                                                                   odin:ODPElement ;
                                                                          odin:describedIn odin:executesTask_Descr ;
                                                                          odin:odpType odin:Foundational ;
                                                                          rdfs:comment "A relation between an action and a task, e.g. 'putting some water in a pot and putting the pot on a fire until the water starts bubbling' executes the task 'boiling'." .


###  http://www.ontologydesignpatterns.org/cp/owl/basicplan.owl#isConceptualizedBy
<http://www.ontologydesignpatterns.org/cp/owl/basicplan.owl#isConceptualizedBy> rdf:type owl:NamedIndividual ,
                                                                                         odin:ODPElement ;
                                                                                odin:describedIn odin:isConceptualizedBy_Descr ;
                                                                                odin:odpType odin:Foundational ;
                                                                                rdfs:comment "A relation stating that an Agent is internally representing a Description . E.g., 'John believes in the conspiracy theory'; 'Niels Bohr created a solar-system metaphor for his atomic theory'; 'Jacques assumes all swans are white'; 'the task force shares the attack plan'." .


###  http://www.ontologydesignpatterns.org/cp/owl/basicplan.owl#isExecutedIn
<http://www.ontologydesignpatterns.org/cp/owl/basicplan.owl#isExecutedIn> rdf:type owl:NamedIndividual ,
                                                                                   odin:ODPElement ;
                                                                          odin:describedIn odin:isExecutedIn_Descr ;
                                                                          odin:odpType odin:Foundational ;
                                                                          rdfs:comment "A relation between an action and a task, e.g. 'putting some water in a pot and putting the pot on a fire until the water starts bubbling' executes the task 'boiling'." .


###  http://www.ontologydesignpatterns.org/cp/owl/basicplan.owl#isParametrizedBy
<http://www.ontologydesignpatterns.org/cp/owl/basicplan.owl#isParametrizedBy> rdf:type owl:NamedIndividual ,
                                                                                       odin:ODPElement ;
                                                                              odin:describedIn odin:isParametrizedBy_Descr ;
                                                                              rdfs:comment "The relation between a Parameter, e.g. 'MajorAge', and a Region, e.g. '>17 year'." .


###  http://www.ontologydesignpatterns.org/cp/owl/basicplan.owl#isSatisfiedBy
<http://www.ontologydesignpatterns.org/cp/owl/basicplan.owl#isSatisfiedBy> rdf:type owl:NamedIndividual ,
                                                                                    odin:ODPElement ;
                                                                           odin:describedIn odin:isSatisfiedBy_Descr ;
                                                                           odin:odpType odin:Foundational ;
                                                                           rdfs:comment "A relation between a Situation and a Description, e.g. the execution of a Plan satisfies that plan." .


###  http://www.ontologydesignpatterns.org/cp/owl/basicplan.owl#parametrizes
<http://www.ontologydesignpatterns.org/cp/owl/basicplan.owl#parametrizes> rdf:type owl:NamedIndividual ,
                                                                                   odin:ODPElement ;
                                                                          odin:describedIn odin:parametrizes_Descr ;
                                                                          odin:odpType odin:Foundational ;
                                                                          rdfs:comment "The relation between a Parameter, e.g. 'MajorAgeLimit', and a Region, e.g. '18_year'.  For a more data-oriented relation, see hasDataValue" .


###  http://www.ontologydesignpatterns.org/cp/owl/basicplan.owl#satisfies
<http://www.ontologydesignpatterns.org/cp/owl/basicplan.owl#satisfies> rdf:type owl:NamedIndividual ,
                                                                                odin:ODPElement ;
                                                                       odin:describedIn odin:satisfies_Descr ;
                                                                       odin:odpType odin:Foundational ;
                                                                       rdfs:comment "A relation between a Situation and a Description, e.g. the execution of a Plan satisfies that plan." .


###  http://www.ontologydesignpatterns.org/cp/owl/basicplanexecution.owl#PlanExecution
<http://www.ontologydesignpatterns.org/cp/owl/basicplanexecution.owl#PlanExecution> rdf:type owl:NamedIndividual ,
                                                                                             odin:ODPElement ;
                                                                                    odin:describedIn odin:PlanExecution_Descr ;
                                                                                    rdfs:comment "Plan executions are situations that proactively satisfy a plan. Subplan executions are proper parts of the whole plan execution." .


###  http://www.ontologydesignpatterns.org/cp/owl/basicplanexecution.owl#actionHasParticipant
<http://www.ontologydesignpatterns.org/cp/owl/basicplanexecution.owl#actionHasParticipant> rdf:type owl:NamedIndividual ,
                                                                                                    odin:ODPElement ;
                                                                                           odin:describedIn odin:actionHasParticipant_Descr ;
                                                                                           odin:odpType odin:Foundational ;
                                                                                           rdfs:comment "A relation between a Process and an Object, e.g. 'the avalanche hasParticipant a mass of snow', or 'the cooking of a cake hasParticipant an agent, some sugar, flour, etc.'." .


###  http://www.ontologydesignpatterns.org/cp/owl/basicplanexecution.owl#includesAction
<http://www.ontologydesignpatterns.org/cp/owl/basicplanexecution.owl#includesAction> rdf:type owl:NamedIndividual ,
                                                                                              odin:ODPElement ;
                                                                                     odin:describedIn odin:includesAction_Descr ;
                                                                                     rdfs:comment "A relation between situations and persons, e.g. 'this morning I've prepared my coffee and had my fingers burnt' (i.e.: the preparation of my coffee this morning included a burning of my fingers)." .


###  http://www.ontologydesignpatterns.org/cp/owl/basicplanexecution.owl#includesAgent
<http://www.ontologydesignpatterns.org/cp/owl/basicplanexecution.owl#includesAgent> rdf:type owl:NamedIndividual ,
                                                                                             odin:ODPElement ;
                                                                                    odin:describedIn odin:includesAgent_Descr ;
                                                                                    odin:odpType odin:Foundational ;
                                                                                    rdfs:comment "A relation between situations and persons, e.g. 'this morning I've prepared my coffee and had my fingers burnt' (i.e.: the preparation of my coffee this morning included me)." .


###  http://www.ontologydesignpatterns.org/cp/owl/basicplanexecution.owl#includesObject
<http://www.ontologydesignpatterns.org/cp/owl/basicplanexecution.owl#includesObject> rdf:type owl:NamedIndividual ,
                                                                                              odin:ODPElement ;
                                                                                     odin:describedIn odin:includesObject_Descr ;
                                                                                     odin:odpType odin:Foundational ;
                                                                                     rdfs:comment "A relation between situations and persons, e.g. 'this morning I've prepared my coffee and had my fingers burnt' (i.e.: the preparation of my coffee this morning included me)." .


###  http://www.ontologydesignpatterns.org/cp/owl/basicplanexecution.owl#isParticipantInAction
<http://www.ontologydesignpatterns.org/cp/owl/basicplanexecution.owl#isParticipantInAction> rdf:type owl:NamedIndividual ,
                                                                                                     odin:ODPElement ;
                                                                                            odin:describedIn odin:isParticipantInAction_Descr ;
                                                                                            rdfs:comment "A relation between an object and a process, e.g. 'a mass of snow is partipant in the avalanche', or 'an agent, some sugar, flour, etc. are participant in the cooking of a cake'." .


###  http://www.ontologydesignpatterns.org/cp/owl/classification.owl#Concept
<http://www.ontologydesignpatterns.org/cp/owl/classification.owl#Concept> rdf:type owl:NamedIndividual ,
                                                                                   odin:ODPElement ;
                                                                          odin:describedIn odin:Concept_Descr ;
                                                                          rdfs:comment "A concept is a Social Object.   The classifies relation relates concepts to entities at some time, but time can only be expressed in the alternative pattern: timeindexedclassification." .


###  http://www.ontologydesignpatterns.org/cp/owl/classification.owl#classifies
<http://www.ontologydesignpatterns.org/cp/owl/classification.owl#classifies> rdf:type owl:NamedIndividual ,
                                                                                      odin:ODPElement ;
                                                                             odin:describedIn odin:classifies_Descr ;
                                                                             odin:odpType odin:Foundational ;
                                                                             rdfs:comment "A relation between a Concept and an Entity, e.g. the Role 'student' classifies a Person 'John'." .


###  http://www.ontologydesignpatterns.org/cp/owl/classification.owl#isClassifiedBy
<http://www.ontologydesignpatterns.org/cp/owl/classification.owl#isClassifiedBy> rdf:type owl:NamedIndividual ,
                                                                                          odin:ODPElement ;
                                                                                 odin:describedIn odin:isClassifiedBy_Descr ;
                                                                                 odin:odpType odin:Foundational ;
                                                                                 rdfs:comment "A relation between a Concept and an Entity, e.g. 'John is considered a typical rude man'; your last concert constitutes the achievement of a lifetime; '20-year-old means she's mature enough'." .


###  http://www.ontologydesignpatterns.org/cp/owl/collectionentity.owl#Collection
<http://www.ontologydesignpatterns.org/cp/owl/collectionentity.owl#Collection> rdf:type owl:NamedIndividual ,
                                                                                        odin:ODPElement ;
                                                                               odin:describedIn odin:Collection_Descr ;
                                                                               rdfs:comment "Any container for entities that share one or more common properties. E.g. stone objects, the nurses, the Louvre Aegyptian collection. A collection is not a logical class: a collection is a first-order entity, while a class is a second-order one." .


###  http://www.ontologydesignpatterns.org/cp/owl/collectionentity.owl#hasMember
<http://www.ontologydesignpatterns.org/cp/owl/collectionentity.owl#hasMember> rdf:type owl:NamedIndividual ,
                                                                                       odin:ODPElement ;
                                                                              odin:describedIn odin:hasMember_Descr ;
                                                                              rdfs:comment "A relation between collections and entities, e.g. 'my collection of saxophones includes an old Adolphe Sax original alto' (i.e. my collection has member an Adolphe Sax alto)." ,
                                                                                           "The link to the members of a Set" .


###  http://www.ontologydesignpatterns.org/cp/owl/communities.owl#Community
<http://www.ontologydesignpatterns.org/cp/owl/communities.owl#Community> rdf:type owl:NamedIndividual ,
                                                                                  odin:ODPElement ;
                                                                         odin:describedIn odin:Community_Descr ;
                                                                         odin:odpType odin:Foundational ;
                                                                         rdfs:comment "A Collection whose members are agents, e.g. the nurses, the Italian rockabilly fans." .


###  http://www.ontologydesignpatterns.org/cp/owl/componency.owl#Object
<http://www.ontologydesignpatterns.org/cp/owl/componency.owl#Object> rdf:type owl:NamedIndividual ,
                                                                              odin:ODPElement ;
                                                                     odin:describedIn odin:Object_Descr ;
                                                                     odin:odpType odin:Foundational ;
                                                                     rdfs:comment "Any physical, social, or mental object, or a substance" .


###  http://www.ontologydesignpatterns.org/cp/owl/componency.owl#hasComponent
<http://www.ontologydesignpatterns.org/cp/owl/componency.owl#hasComponent> rdf:type owl:NamedIndividual ,
                                                                                    odin:ODPElement ;
                                                                           odin:describedIn odin:hasComponent_Descr ;
                                                                           rdfs:comment "The hasPart relation without transitivity, holding between an entity (the system) and another (the component), and assuming a design that structures the system. For an explicit pattern encoding design, see the 'designobject' pattern.  The componency pattern uses the transitive reduction logical pattern to preserve transitive on the superproperty from the partof pattern. In practice, the partof pattern acts here as the transitive reduction of the componency pattern." .


###  http://www.ontologydesignpatterns.org/cp/owl/componency.owl#isComponentOf
<http://www.ontologydesignpatterns.org/cp/owl/componency.owl#isComponentOf> rdf:type owl:NamedIndividual ,
                                                                                     odin:ODPElement ;
                                                                            odin:describedIn odin:isComponentOf_Descr ;
                                                                            odin:odpType odin:Foundational ;
                                                                            rdfs:comment "The hasPart relation without transitivity, holding between an entity (the system) and another (the component), and assuming a design that structures the system. For an explicit pattern encoding design, see the 'designobject' pattern.  The componency pattern uses the transitive reduction logical pattern to preserve transitive on the superproperty from the partof pattern. In practice, the partof pattern acts here as the transitive reduction of the componency pattern." .


###  http://www.ontologydesignpatterns.org/cp/owl/constituency.owl#hasConstituent
<http://www.ontologydesignpatterns.org/cp/owl/constituency.owl#hasConstituent> rdf:type owl:NamedIndividual ,
                                                                                        odin:ODPElement ;
                                                                               odin:describedIn odin:hasConstituent_Descr ;
                                                                               rdfs:comment "Constituency' depends on some layering of the world described by the ontology. For example, scientific granularities (e.g. body-organ-tissue-cell) or ontological 'strata' (e.g. social-mental-biological-physical) are typical layerings.   Intuitively, a constituent is a part belonging to a lower layer. Since layering is actually a partition of the world described by the ontology, constituents are not properly classified as parts, although this kinship can be intuitive for common sense.  A desirable advantage of this distinction is that we are able to talk e.g. of physical constituents of non-physical objects (e.g. systems), while this is not possible in terms of parts.  Example of are the persons constituting a social system, the molecules constituting a person, the atoms constituting a river, etc.   In all these examples, we notice a typical discontinuity between the constituted and the constituent object: e.g. a social system is conceptualized at a different layer from the persons that constitute it, a person is conceptualized at a different layer from the molecules that constitute them, and a river is conceptualized at a different layer from the atoms that constitute it." .


###  http://www.ontologydesignpatterns.org/cp/owl/constituency.owl#isConstituentOf
<http://www.ontologydesignpatterns.org/cp/owl/constituency.owl#isConstituentOf> rdf:type owl:NamedIndividual ,
                                                                                         odin:ODPElement ;
                                                                                odin:describedIn odin:isConstituentOf_Descr ;
                                                                                odin:odpType odin:Foundational ;
                                                                                rdfs:comment "Constituency' depends on some layering of the world described by the ontology. For example, scientific granularities (e.g. body-organ-tissue-cell) or ontological 'strata' (e.g. social-mental-biological-physical) are typical layerings.   Intuitively, a constituent is a part belonging to a lower layer. Since layering is actually a partition of the world described by the ontology, constituents are not properly classified as parts, although this kinship can be intuitive for common sense.  A desirable advantage of this distinction is that we are able to talk e.g. of physical constituents of non-physical objects (e.g. systems), while this is not possible in terms of parts.  Example of are the persons constituting a social system, the molecules constituting a person, the atoms constituting a river, etc.   In all these examples, we notice a typical discontinuity between the constituted and the constituent object: e.g. a social system is conceptualized at a different layer from the persons that constitute it, a person is conceptualized at a different layer from the molecules that constitute them, and a river is conceptualized at a different layer from the atoms that constitute it." .


###  http://www.ontologydesignpatterns.org/cp/owl/controlflow.owl#AbstractMergingTask
<http://www.ontologydesignpatterns.org/cp/owl/controlflow.owl#AbstractMergingTask> rdf:type owl:NamedIndividual ,
                                                                                            odin:ODPElement ;
                                                                                   odin:describedIn odin:AbstractMergingTask_Descr ;
                                                                                   odin:odpType odin:Foundational ;
                                                                                   rdfs:comment "An abstract merging task is a merging aimed at 'formally' joining the tasks that are direct successor to a case task.  Differently from synchronization tasks, which are expected to be executed, abstract mergings only provide abstract boundaries to a task structure, because in a case task, only one action task is supposed to be executed." .


###  http://www.ontologydesignpatterns.org/cp/owl/controlflow.owl#ActivationTask
<http://www.ontologydesignpatterns.org/cp/owl/controlflow.owl#ActivationTask> rdf:type owl:NamedIndividual ,
                                                                                       odin:ODPElement ;
                                                                              odin:describedIn odin:ActivationTask_Descr ;
                                                                              rdfs:comment "A control task aimed at starting an activity. It is specialized either by a beginning task or a reactivation task." .


###  http://www.ontologydesignpatterns.org/cp/owl/controlflow.owl#BooleanCaseTask
<http://www.ontologydesignpatterns.org/cp/owl/controlflow.owl#BooleanCaseTask> rdf:type owl:NamedIndividual ,
                                                                                        odin:ODPElement ;
                                                                               odin:describedIn odin:BooleanCaseTask_Descr ;
                                                                               odin:odpType odin:Foundational ;
                                                                               rdfs:comment "E.g. a yes-or-no case task, requiring exactly two deliberation tasks." .


###  http://www.ontologydesignpatterns.org/cp/owl/controlflow.owl#BranchingTask
<http://www.ontologydesignpatterns.org/cp/owl/controlflow.owl#BranchingTask> rdf:type owl:NamedIndividual ,
                                                                                      odin:ODPElement ;
                                                                             odin:describedIn odin:BranchingTask_Descr ;
                                                                             odin:odpType odin:Foundational ;
                                                                             rdfs:comment "A task that articulates the plan into an ordered set of tasks." .


###  http://www.ontologydesignpatterns.org/cp/owl/controlflow.owl#CaseTask
<http://www.ontologydesignpatterns.org/cp/owl/controlflow.owl#CaseTask> rdf:type owl:NamedIndividual ,
                                                                                 odin:ODPElement ;
                                                                        odin:describedIn odin:CaseTask_Descr ;
                                                                        rdfs:comment "A case task is a control task branched to a set of tasks that are not executable concurrently. In order to choose which task has to be undertaken, preliminary deliberation tasks should be executed, possibly based on information-gathering and decision rationales." .


###  http://www.ontologydesignpatterns.org/cp/owl/controlflow.owl#ConcurrencyTask
<http://www.ontologydesignpatterns.org/cp/owl/controlflow.owl#ConcurrencyTask> rdf:type owl:NamedIndividual ,
                                                                                        odin:ODPElement ;
                                                                               odin:describedIn odin:ConcurrencyTask_Descr ;
                                                                               rdfs:comment "A concurrent task is a task branched to a set of tasks executable concurrently -the sequenced perdurants can overlap-, which means that no deliberation task is performed in order to choose among them. A concurrent task has at least one successor synchronization task, which is aimed at waiting for the execution of all -except the optional ones- tasks direct successor to the concurrent -or any order, see below- one.The axioms cannot be expressed fully in OWL-DL (no value mapping available)." .


###  http://www.ontologydesignpatterns.org/cp/owl/controlflow.owl#ControlTask
<http://www.ontologydesignpatterns.org/cp/owl/controlflow.owl#ControlTask> rdf:type owl:NamedIndividual ,
                                                                                    odin:ODPElement ;
                                                                           odin:describedIn odin:ControlTask_Descr ;
                                                                           odin:odpType odin:Foundational ;
                                                                           rdfs:comment "A control task is a task executed during a planning activity, e.g. an activity aimed at (cognitively or via simulation) anticipating other activities. Therefore, control tasks have usually at least one direct successor task (the controlled one), with the exception of ending tasks.The reification of control constructs allows to represent procedural knowledge into the same ontology including controlled action. Besides conceptual transparency and independency from a particular grounding system, a further advantage is enabling the representation of coordination tasks. For example, a manager that coordinates the execution of several related activities can be represented as a role with a responsibility (duty+right) towards some complex task." .


###  http://www.ontologydesignpatterns.org/cp/owl/controlflow.owl#DecisionActivity
<http://www.ontologydesignpatterns.org/cp/owl/controlflow.owl#DecisionActivity> rdf:type owl:NamedIndividual ,
                                                                                         odin:ODPElement ;
                                                                                odin:describedIn odin:DecisionActivity_Descr ;
                                                                                odin:odpType odin:Foundational ;
                                                                                rdfs:comment "An activity related to planning. It is supposed to execute a 'case task', and can contain an information gathering activity." .


###  http://www.ontologydesignpatterns.org/cp/owl/controlflow.owl#DeliberationState
<http://www.ontologydesignpatterns.org/cp/owl/controlflow.owl#DeliberationState> rdf:type owl:NamedIndividual ,
                                                                                          odin:ODPElement ;
                                                                                 odin:describedIn odin:DeliberationState_Descr ;
                                                                                 rdfs:comment "A state related to planning. It finalizes the execution of a 'deliberation task', and is preceded by a decision activity." .


###  http://www.ontologydesignpatterns.org/cp/owl/controlflow.owl#EndingTask
<http://www.ontologydesignpatterns.org/cp/owl/controlflow.owl#EndingTask> rdf:type owl:NamedIndividual ,
                                                                                   odin:ODPElement ;
                                                                          odin:describedIn odin:EndingTask_Descr ;
                                                                          odin:odpType odin:Foundational ;
                                                                          rdfs:comment "An ending task is a control task that has no successor tasks defined in the plan." .


###  http://www.ontologydesignpatterns.org/cp/owl/controlflow.owl#LoopTask
<http://www.ontologydesignpatterns.org/cp/owl/controlflow.owl#LoopTask> rdf:type owl:NamedIndividual ,
                                                                                 odin:ODPElement ;
                                                                        odin:describedIn odin:LoopTask_Descr ;
                                                                        rdfs:comment "A loop task is a control task that has as successor an action -or complex- task that sequences at least two distinct activities sharing a minimal common set of properties -they have a MinimalCommonType. Notice that MinimalCommonType cannot be formalised as a first-order predicate, and then neither in OWL-DL. It can be considered a trivial guideline: when sequencing looped actions, choose a definite action class from the ground ontology.  Some relations typically hold for loop tasks. Exit condition can be used to state what deliberation task causes to exit the cycle; iteration interval can be used to state how much time should be taken by each iteration of the looped activity; iteration cardinality can be used to state how many times the action should be repeated." .


###  http://www.ontologydesignpatterns.org/cp/owl/controlflow.owl#MergingTask
<http://www.ontologydesignpatterns.org/cp/owl/controlflow.owl#MergingTask> rdf:type owl:NamedIndividual ,
                                                                                    odin:ODPElement ;
                                                                           odin:describedIn odin:MergingTask_Descr ;
                                                                           odin:odpType odin:Foundational ;
                                                                           rdfs:comment "A task that joins a set of tasks after a branching." .


###  http://www.ontologydesignpatterns.org/cp/owl/controlflow.owl#SynchroTask
<http://www.ontologydesignpatterns.org/cp/owl/controlflow.owl#SynchroTask> rdf:type owl:NamedIndividual ,
                                                                                    odin:ODPElement ;
                                                                           odin:describedIn odin:SynchroTask_Descr ;
                                                                           rdfs:comment "A synchronization task is a merging aimed at waiting for the execution of all (except the optional ones) tasks that are direct successor to a concurrent or any order task." .


###  http://www.ontologydesignpatterns.org/cp/owl/countingas.owl#CountingAs
<http://www.ontologydesignpatterns.org/cp/owl/countingas.owl#CountingAs> rdf:type owl:NamedIndividual ,
                                                                                  odin:ODPElement ;
                                                                         odin:describedIn odin:CountingAs_Descr ;
                                                                         rdfs:comment "A Situation that represents the classification of an entity 'as' something (a Concept).  Inspired by Searle's 'counts as' relation." .


###  http://www.ontologydesignpatterns.org/cp/owl/description.owl#Concept
<http://www.ontologydesignpatterns.org/cp/owl/description.owl#Concept> rdf:type owl:NamedIndividual ,
                                                                                odin:ODPElement ;
                                                                       odin:describedIn odin:Concept_Descr ;
                                                                       odin:odpType odin:Foundational ;
                                                                       rdfs:comment "A concept can be an idea, notion, role, or even a reified class, and isDefinedIn a Description .   Once defined, a Concept can be used in other descriptions.   The classifies relation (see 'classification' pattern) relates concepts to entities at some time." .


###  http://www.ontologydesignpatterns.org/cp/owl/description.owl#Description
<http://www.ontologydesignpatterns.org/cp/owl/description.owl#Description> rdf:type owl:NamedIndividual ,
                                                                                    odin:ODPElement ;
                                                                           odin:describedIn odin:Description_Descr ;
                                                                           rdfs:comment "A Description represents a conceptualization. It can be thought also as a 'descriptive context' that defines concepts in order to see a 'relational context' out of a set of data or observations. For example, a Plan is a description of some actions to be executed by agents in a certain way, with certain parameters; a Diagnosis is a description that provides an interpretation to a set of observed entities, etc.  A Description typically defines at least one Concept, for example the 'preparing a coffee' Description could define concepts such as 'Heater', 'AmountOfWater', 'CoffeeMix', etc.  With respect to other patterns, descriptions are 'abstractions' of situations (cf. the 'situation' pattern), and in some complex use cases (e.g. matching executions to plan models), the two patterns can be composed (see the descriptionsituation pattern)." .


###  http://www.ontologydesignpatterns.org/cp/owl/description.owl#defines
<http://www.ontologydesignpatterns.org/cp/owl/description.owl#defines> rdf:type owl:NamedIndividual ,
                                                                                odin:ODPElement ;
                                                                       odin:describedIn odin:defines_Descr ;
                                                                       rdfs:comment "A relation between a Description and a Concept, e.g. a Workflow for a governmental Organization defines the Role 'officer', or 'the Italian Traffic Law defines the role Vehicle'." .


###  http://www.ontologydesignpatterns.org/cp/owl/description.owl#isConceptUsedIn
<http://www.ontologydesignpatterns.org/cp/owl/description.owl#isConceptUsedIn> rdf:type owl:NamedIndividual ,
                                                                                        odin:ODPElement ;
                                                                               odin:describedIn odin:isConceptUsedIn_Descr ;
                                                                               rdfs:comment "A more generic relation holding between a Description and a Concept. In order to be used, a Concept must be previously definedIn another Description" .


###  http://www.ontologydesignpatterns.org/cp/owl/description.owl#isDefinedIn
<http://www.ontologydesignpatterns.org/cp/owl/description.owl#isDefinedIn> rdf:type owl:NamedIndividual ,
                                                                                    odin:ODPElement ;
                                                                           odin:describedIn odin:isDefinedIn_Descr ;
                                                                           odin:odpType odin:Foundational ;
                                                                           rdfs:comment "A relation between a Description and a Concept, e.g. a Workflow for a governmental Organization defines the Role 'officer', or 'the Italian Traffic Law defines the role Vehicle'." .


###  http://www.ontologydesignpatterns.org/cp/owl/description.owl#usesConcept
<http://www.ontologydesignpatterns.org/cp/owl/description.owl#usesConcept> rdf:type owl:NamedIndividual ,
                                                                                    odin:ODPElement ;
                                                                           odin:describedIn odin:usesConcept_Descr ;
                                                                           odin:odpType odin:Foundational ;
                                                                           rdfs:comment "A generic relation holding between a Description and a Concept. In order to be used, a Concept must be previously definedIn another Description. This last condition cannot be encoded for object properties in OWL." .


###  http://www.ontologydesignpatterns.org/cp/owl/descriptionandsituation.owl#describes
<http://www.ontologydesignpatterns.org/cp/owl/descriptionandsituation.owl#describes> rdf:type owl:NamedIndividual ,
                                                                                              odin:ODPElement ;
                                                                                     odin:describedIn odin:describes_Descr ;
                                                                                     odin:odpType odin:Foundational ;
                                                                                     rdfs:comment "The relation between a Description and an Entity : a Description gives a unity to a Collection of parts (the components), or constituents, by assigning a Role to each of them in the context of a whole Object (the system).  A same Entity can be given different descriptions, for example, an old cradle can be given a unifying Description based on the original aesthetic design, the functionality it was built for, or a new aesthetic functionality in which it can be used as a flower pot." .


###  http://www.ontologydesignpatterns.org/cp/owl/descriptionandsituation.owl#isDescribedBy
<http://www.ontologydesignpatterns.org/cp/owl/descriptionandsituation.owl#isDescribedBy> rdf:type owl:NamedIndividual ,
                                                                                                  odin:ODPElement ;
                                                                                         odin:describedIn odin:isDescribedBy_Descr ;
                                                                                         odin:odpType odin:Foundational ;
                                                                                         rdfs:comment "The relation between any Thing and a Description: a Description gives a unity to a Collection of parts (the components), or constituents, by assigning a Role to each of them in the context of a whole Object (the system).  A same Thing can be given different descriptions, for example, an old cradle can be given a unifying Description based on the original aesthetic design, the functionality it was built for, or a new aesthetic functionality in which it can be used as a flower pot." .


###  http://www.ontologydesignpatterns.org/cp/owl/descriptionandsituation.owl#isSatisfiedBy
<http://www.ontologydesignpatterns.org/cp/owl/descriptionandsituation.owl#isSatisfiedBy> rdf:type owl:NamedIndividual ,
                                                                                                  odin:ODPElement ;
                                                                                         odin:describedIn odin:isSatisfiedBy_Descr ;
                                                                                         rdfs:comment "A relation between a Situation and a Description, e.g. the execution of a Plan satisfies that plan." .


###  http://www.ontologydesignpatterns.org/cp/owl/descriptionandsituation.owl#satisfies
<http://www.ontologydesignpatterns.org/cp/owl/descriptionandsituation.owl#satisfies> rdf:type owl:NamedIndividual ,
                                                                                              odin:ODPElement ;
                                                                                     odin:describedIn odin:satisfies_Descr ;
                                                                                     odin:odpType odin:Foundational ;
                                                                                     rdfs:comment "A relation between a Situation and a Description, e.g. the execution of a Plan satisfies that plan." .


###  http://www.ontologydesignpatterns.org/cp/owl/eventprocessing.owl#EventObject
<http://www.ontologydesignpatterns.org/cp/owl/eventprocessing.owl#EventObject> rdf:type owl:NamedIndividual ,
                                                                                        odin:ODPElement ;
                                                                               odin:describedIn odin:EventObject_Descr ;
                                                                               rdfs:comment "An object that represents, encodes, or records an event, generally for the purpose of computer processing.      An event object may consist of an event object header and a body, where the header is defined as the part of the event object that can be interpreted by the event processing system, i.e. and event object needs to contain at least some information (e.g. with a known vocabulary) that can be used by the event processing system. Note that the open world assumption allows us to choose not to explicitly specify a header, despite the restriction that it exists.      An event object is either a complex event, i.e. an event object that has some relation (either through abstraction or componency) to other event objects, or a simple event.      An event object records information about an actual event, which is then by implication a documented event (i.e. participating in an event documentation situation)." .


###  http://www.ontologydesignpatterns.org/cp/owl/eventprocessing.owl#EventObjectBody
<http://www.ontologydesignpatterns.org/cp/owl/eventprocessing.owl#EventObjectBody> rdf:type owl:NamedIndividual ,
                                                                                            odin:ODPElement ;
                                                                                   odin:describedIn odin:EventObjectBody_Descr ;
                                                                                   rdfs:comment "Some event processing systems need to distinguish between an event object header and its body, where the event object header is the part of the event object with known content (e.g. known vocabulary) that can be directly processed by the event processing system, and the body is the rest of the event object. The body may always be empty or missing." .


###  http://www.ontologydesignpatterns.org/cp/owl/eventprocessing.owl#EventObjectHeader
<http://www.ontologydesignpatterns.org/cp/owl/eventprocessing.owl#EventObjectHeader> rdf:type owl:NamedIndividual ,
                                                                                              odin:ODPElement ;
                                                                                     odin:describedIn odin:EventObjectHeader_Descr ;
                                                                                     rdfs:comment "Some event processing systems need to distinguish between an event object header and its body, where the event object header is the part of the event object with known content (e.g. known vocabulary) that can be directly processed by the event processing system. Although a header is considered mandatory for an event object, if not specified what the header consists of, it can be inferred by the system through the fact that it contains the known part, as opposed to the body that may contain a payload that the system cannot interpret." .


###  http://www.ontologydesignpatterns.org/cp/owl/eventprocessing.owl#hasDirectSubEventObject
<http://www.ontologydesignpatterns.org/cp/owl/eventprocessing.owl#hasDirectSubEventObject> rdf:type owl:NamedIndividual ,
                                                                                                    odin:ODPElement ;
                                                                                           odin:describedIn odin:hasDirectSubEventObject_Descr ;
                                                                                           rdfs:comment "A relation that connects a complex event with the low-level events it is a higher-level representation of. This is a non-transitive relation that can be used to create a hierarchy of levels of sub-events, that represents the reasoning/triggering or abstraction process that led up to the creation or detection of a complex event. The transitive superproperty hasSubEventObject allows for direclty querying for the transitive closure of sub-events, regardless of the hierarchy, even if only this non-transitive sub-property is used in the data." .


###  http://www.ontologydesignpatterns.org/cp/owl/eventprocessing.owl#hasEventDuration
<http://www.ontologydesignpatterns.org/cp/owl/eventprocessing.owl#hasEventDuration> rdf:type owl:NamedIndividual ,
                                                                                             odin:ODPElement ;
                                                                                    odin:describedIn odin:hasEventDuration_Descr ;
                                                                                    rdfs:comment "Property for represting a time interval of an event object, rather than a time point. Alternative is to define several time points, using the subproperties of the datatype property hasEventObjectTime." .


###  http://www.ontologydesignpatterns.org/cp/owl/eventprocessing.owl#hasEventObjectApplicationTime
<http://www.ontologydesignpatterns.org/cp/owl/eventprocessing.owl#hasEventObjectApplicationTime> rdf:type owl:NamedIndividual ,
                                                                                                          odin:ODPElement ;
                                                                                                 odin:describedIn odin:hasEventObjectApplicationTime_Descr ;
                                                                                                 rdfs:comment "The timestamp assigned by the source of the data when it was transmitted, i.e. when it entered the stream." .


###  http://www.ontologydesignpatterns.org/cp/owl/eventprocessing.owl#hasEventObjectBody
<http://www.ontologydesignpatterns.org/cp/owl/eventprocessing.owl#hasEventObjectBody> rdf:type owl:NamedIndividual ,
                                                                                               odin:ODPElement ;
                                                                                      odin:describedIn odin:hasEventObjectBody_Descr ;
                                                                                      rdfs:comment "Some event processing systems need to distinguish between an event object header and its body, where the event object header is the part of the event object with known content (e.g. known vocabulary) that can be directly processed by the event processing system. This property relates an event object to its body part." .


###  http://www.ontologydesignpatterns.org/cp/owl/eventprocessing.owl#hasEventObjectComponent
<http://www.ontologydesignpatterns.org/cp/owl/eventprocessing.owl#hasEventObjectComponent> rdf:type owl:NamedIndividual ,
                                                                                                    odin:ODPElement ;
                                                                                           odin:describedIn odin:hasEventObjectComponent_Descr ;
                                                                                           rdfs:comment "This non-transitive property expresses the direct relation between an event object and its direct parts, i.e. its components. Using this property a hierarchy of components can be expressed for an event object. The components of the event object do not exist on their own, but exist to make up the whole of the encapsulating event, likewise the encapsulating event is not complete without its parts. Please note the difference between this stronger relation, compared to the hasSubEvent-property which merely relates event objects to each other, e.g. expressing the triggering of abstractions, but without implying that the events are parts of each other." .


###  http://www.ontologydesignpatterns.org/cp/owl/eventprocessing.owl#hasEventObjectHeader
<http://www.ontologydesignpatterns.org/cp/owl/eventprocessing.owl#hasEventObjectHeader> rdf:type owl:NamedIndividual ,
                                                                                                 odin:ODPElement ;
                                                                                        odin:describedIn odin:hasEventObjectHeader_Descr ;
                                                                                        rdfs:comment "Some event processing systems need to distinguish between an event object header and its body, where the event object header is the part of the event object with known content (e.g. known vocabulary) that can be directly processed by the event processing system. This property relates an event object to its header part." .


###  http://www.ontologydesignpatterns.org/cp/owl/eventprocessing.owl#hasEventObjectPart
<http://www.ontologydesignpatterns.org/cp/owl/eventprocessing.owl#hasEventObjectPart> rdf:type owl:NamedIndividual ,
                                                                                               odin:ODPElement ;
                                                                                      odin:describedIn odin:hasEventObjectPart_Descr ;
                                                                                      rdfs:comment "This transitive property represents a partonomy relation between event objects. An event object can consist of several partial events that together make up the complete event object. The parts of the event object do not exist on their own, but exist to make up the whole of the encapsulating event, likewise the encapsulating event is not complete without its parts. Please note the difference between this stronger relation, compared to the hasSubEvent-property which merely relates event objects to each other, e.g. expressing the triggering of abstractions, but without implying that the events are parts of each other." .


###  http://www.ontologydesignpatterns.org/cp/owl/eventprocessing.owl#hasEventObjectSystemTime
<http://www.ontologydesignpatterns.org/cp/owl/eventprocessing.owl#hasEventObjectSystemTime> rdf:type owl:NamedIndividual ,
                                                                                                     odin:ODPElement ;
                                                                                            odin:describedIn odin:hasEventObjectSystemTime_Descr ;
                                                                                            rdfs:comment "The timestamp of the event according to the event processing system (in terms of its internal clock time), i.e. when the event object was received byt the event processing system through the stream." .


###  http://www.ontologydesignpatterns.org/cp/owl/eventprocessing.owl#hasSensorReadingValue
<http://www.ontologydesignpatterns.org/cp/owl/eventprocessing.owl#hasSensorReadingValue> rdf:type owl:NamedIndividual ,
                                                                                                  odin:ODPElement ;
                                                                                         odin:describedIn odin:hasSensorReadingValue_Descr ;
                                                                                         rdfs:comment "Property for expresseing the alignemet to the SSN ontology, equivalent to ssn:hasValue." .


###  http://www.ontologydesignpatterns.org/cp/owl/eventprocessing.owl#hasSubEventObject
<http://www.ontologydesignpatterns.org/cp/owl/eventprocessing.owl#hasSubEventObject> rdf:type owl:NamedIndividual ,
                                                                                              odin:ODPElement ;
                                                                                     odin:describedIn odin:hasSubEventObject_Descr ;
                                                                                     rdfs:comment "A relation that connects a complex event with the low-level events it is a higher-level representation of. An event object may reference another event, on a lower level of abstraction or granularity, upon which is it is based or from which it was derived or triggered, making that other event a sub event of this aggregated or more abstract event object. Note that for modelling instance data, normally, the non-transitive sub-property hasDirectSubEventObject should be used, based on which the presence of this transitive relation can be inferred." .


###  http://www.ontologydesignpatterns.org/cp/owl/eventprocessing.owl#refersToEventObjectComponent
<http://www.ontologydesignpatterns.org/cp/owl/eventprocessing.owl#refersToEventObjectComponent> rdf:type owl:NamedIndividual ,
                                                                                                         odin:ODPElement ;
                                                                                                odin:describedIn odin:refersToEventObjectComponent_Descr ;
                                                                                                rdfs:comment "Event objects that use a header/body structure can use this property to refer to the components (i.e. direct parts) of the event object. Through a property chain axiom, the presence of a hasEventObjectComponent relation can be inferred." .


###  http://www.ontologydesignpatterns.org/cp/owl/eventprocessing.owl#refersToEventObjectConstituent
<http://www.ontologydesignpatterns.org/cp/owl/eventprocessing.owl#refersToEventObjectConstituent> rdf:type owl:NamedIndividual ,
                                                                                                           odin:ODPElement ;
                                                                                                  odin:describedIn odin:refersToEventObjectConstituent_Descr ;
                                                                                                  rdfs:comment "Event objects that use a header/body structure can use this property to refer to the constituents (i.e. direct sub-events in an abstraction hierarchy) of the event object. Through a property chain axiom, the presence of a hasDirectSubEventObject relation can be inferred." .


###  http://www.ontologydesignpatterns.org/cp/owl/fsdas/aquaticresourceobservation.owl
<http://www.ontologydesignpatterns.org/cp/owl/fsdas/aquaticresourceobservation.owl> rdf:type owl:NamedIndividual ,
                                                                                             odin:ODP ;
                                                                                    odin:describedIn odin:aquaticresourceobservation.owl_Descr ;
                                                                                    odin:hasODPComponent <http://www.ontologydesignpatterns.org/cp/owl/fsdas/aquaticresourceobservation.owl#AquaticResource> ,
                                                                                                         <http://www.ontologydesignpatterns.org/cp/owl/fsdas/aquaticresourceobservation.owl#AquaticResourceObservation> ;
                                                                                    rdfs:comment "An ontology that represents the semantics of a database view about observations for an aquatic resource, aggregated once a year." .


###  http://www.ontologydesignpatterns.org/cp/owl/fsdas/catchrecord.owl
<http://www.ontologydesignpatterns.org/cp/owl/fsdas/catchrecord.owl> rdf:type owl:NamedIndividual ,
                                                                              odin:ODP ;
                                                                     odin:describedIn odin:catchrecord.owl_Descr ;
                                                                     odin:hasODPComponent <http://www.ontologydesignpatterns.org/cp/owl/fsdas/catchrecord.owl#CatchRecord> ,
                                                                                          <http://www.ontologydesignpatterns.org/cp/owl/fsdas/catchrecord.owl#countryOfRecord> ,
                                                                                          <http://www.ontologydesignpatterns.org/cp/owl/fsdas/catchrecord.owl#fishingAreaOfRecord> ,
                                                                                          <http://www.ontologydesignpatterns.org/cp/owl/fsdas/catchrecord.owl#forCountry> ,
                                                                                          <http://www.ontologydesignpatterns.org/cp/owl/fsdas/catchrecord.owl#fromFishingArea> ,
                                                                                          <http://www.ontologydesignpatterns.org/cp/owl/fsdas/catchrecord.owl#hasCatchRecord> ,
                                                                                          <http://www.ontologydesignpatterns.org/cp/owl/fsdas/catchrecord.owl#isCatchRecordFor> ,
                                                                                          <http://www.ontologydesignpatterns.org/cp/owl/fsdas/catchrecord.owl#referenceYear> ,
                                                                                          <http://www.ontologydesignpatterns.org/cp/owl/fsdas/catchrecord.owl#reportingYear> ,
                                                                                          <http://www.ontologydesignpatterns.org/cp/owl/fsdas/catchrecord.owl#unitUsedInRecord> ,
                                                                                          <http://www.ontologydesignpatterns.org/cp/owl/fsdas/catchrecord.owl#withUnit> ;
                                                                     rdfs:comment "A design pattern for populating an ontology of aquatic species catching records." .


###  http://www.ontologydesignpatterns.org/cp/owl/fsdas/gearwaterarea.owl
<http://www.ontologydesignpatterns.org/cp/owl/fsdas/gearwaterarea.owl> rdf:type owl:NamedIndividual ,
                                                                                odin:ODP ;
                                                                       odin:describedIn odin:gearwaterarea.owl_Descr ;
                                                                       odin:hasODPComponent <http://www.ontologydesignpatterns.org/cp/owl/fsdas/gearwaterarea.owl#isSuitableForGearType> ,
                                                                                            <http://www.ontologydesignpatterns.org/cp/owl/fsdas/gearwaterarea.owl#isUsedInWaterArea> ;
                                                                       rdfs:comment "This pattern composes aquaticresources.owl and gearspecies.owl.  This must be inferred compositionally, and requires either more sophisticated logical pattern, like 'property chain', available in OWL2 (but not in OWL1), or a complex reasoning pattern, like 'DL classifier+SPARQL', or 'DL classifier+SWRL rule firing'." .


###  http://www.ontologydesignpatterns.org/cp/owl/fsdas/speciesbathymetry.owl
<http://www.ontologydesignpatterns.org/cp/owl/fsdas/speciesbathymetry.owl> rdf:type owl:NamedIndividual ,
                                                                                    odin:ODP ;
                                                                           odin:describedIn odin:speciesbathymetry.owl_Descr ;
                                                                           odin:hasODPComponent <http://www.ontologydesignpatterns.org/cp/owl/fsdas/speciesbathymetry.owl#BathymetricRange> ,
                                                                                                <http://www.ontologydesignpatterns.org/cp/owl/fsdas/speciesbathymetry.owl#hasBathymetricRange> ,
                                                                                                <http://www.ontologydesignpatterns.org/cp/owl/fsdas/speciesbathymetry.owl#isBathymetricRangeOf> ;
                                                                           rdfs:comment "This pattern encodes a FSDAS competency question, with an indication to use some AquaticSpecies class, and some hasBathymetricRange property, with range BathymetricRange." .


###  http://www.ontologydesignpatterns.org/cp/owl/fsdas/speciesconditions.owl
<http://www.ontologydesignpatterns.org/cp/owl/fsdas/speciesconditions.owl> rdf:type owl:NamedIndividual ,
                                                                                    odin:ODP ;
                                                                           odin:describedIn odin:speciesconditions.owl_Descr ;
                                                                           odin:hasODPComponent <http://www.ontologydesignpatterns.org/cp/owl/fsdas/speciesconditions.owl#AquaticSpecies> ,
                                                                                                <http://www.ontologydesignpatterns.org/cp/owl/fsdas/speciesconditions.owl#BathymetricRange> ,
                                                                                                <http://www.ontologydesignpatterns.org/cp/owl/fsdas/speciesconditions.owl#Habitat> ,
                                                                                                <http://www.ontologydesignpatterns.org/cp/owl/fsdas/speciesconditions.owl#SpeciesConditions> ;
                                                                           rdfs:comment "A pattern, based on situation.owl, which allow to express the typical 'conditions' (habitat, bathymetric range) of a species for a certain water area." .


###  http://www.ontologydesignpatterns.org/cp/owl/fsdas/specieshabitat.owl
<http://www.ontologydesignpatterns.org/cp/owl/fsdas/specieshabitat.owl> rdf:type owl:NamedIndividual ,
                                                                                 odin:ODP ;
                                                                        odin:describedIn odin:specieshabitat.owl_Descr ;
                                                                        odin:hasODPComponent <http://www.ontologydesignpatterns.org/cp/owl/fsdas/specieshabitat.owl#Habitat> ;
                                                                        rdfs:comment "This pattern encodes a FSDAS competency question, with an indication to use some Species class, and some hasHabitat property, with range xsd:string.  Since the application task of FSDAS is to jointly query FIGIS factsheet data and RTMS time series data, the pattern must encode elements that can be easily mapped to FIGIS and RTMS schemas/ontologies.  Issue (1) mapping Species to FIGIS schema, since the needed schema elements are two instead of one.  Issue (2) representation of habitats in the pattern is intuitively with objects, since habitats are typically objects, and points in a value space (as the referents of xsd datatypes typically are). The suggestion in the competencey question is to use xsd.string though." .


###  http://www.ontologydesignpatterns.org/cp/owl/fsdas/vesselspecies.owl
<http://www.ontologydesignpatterns.org/cp/owl/fsdas/vesselspecies.owl> rdf:type owl:NamedIndividual ,
                                                                                odin:ODP ;
                                                                       odin:describedIn odin:vesselspecies.owl_Descr ;
                                                                       odin:hasODPComponent <http://www.ontologydesignpatterns.org/cp/owl/fsdas/vesselspecies.owl#catchesSpecies> ,
                                                                                            <http://www.ontologydesignpatterns.org/cp/owl/fsdas/vesselspecies.owl#isCaughtBy> ;
                                                                       rdfs:comment "This pattern composes gearvessel.owl and gearspecies.owl.  This must be inferred compositionally, and requires either more sophisticated logical pattern, like 'property chain', available in OWL2 (but not in OWL1), or a complex reasoning pattern, like 'DL classifier+SPARQL', or 'DL classifier+SWRL rule firing'." .


###  http://www.ontologydesignpatterns.org/cp/owl/fsdas/vesselwaterarea.owl
<http://www.ontologydesignpatterns.org/cp/owl/fsdas/vesselwaterarea.owl> rdf:type owl:NamedIndividual ,
                                                                                  odin:ODP ;
                                                                         odin:describedIn odin:vesselwaterarea.owl_Descr ;
                                                                         odin:hasODPComponent <http://www.ontologydesignpatterns.org/cp/owl/fsdas/vesselwaterarea.owl#canBeCrossedByVesselType> ,
                                                                                              <http://www.ontologydesignpatterns.org/cp/owl/fsdas/vesselwaterarea.owl#canCrossWaterArea> ;
                                                                         rdfs:comment "This pattern composes gearvessel.owl and gearwaterarea.owl.  This must be inferred compositionally, and requires either more sophisticated logical pattern, like 'property chain', available in OWL2 (but not in OWL1), or a complex reasoning pattern, like 'DL classifier+SPARQL', or 'DL classifier+SWRL rule firing'." .


###  http://www.ontologydesignpatterns.org/cp/owl/fsdas/aquaticresourceobservation.owl#AquaticResource
<http://www.ontologydesignpatterns.org/cp/owl/fsdas/aquaticresourceobservation.owl#AquaticResource> rdf:type owl:NamedIndividual ,
                                                                                                             odin:ODPElement ;
                                                                                                    odin:describedIn odin:AquaticResource_Descr ;
                                                                                                    rdfs:comment "An aquatic resource." .


###  http://www.ontologydesignpatterns.org/cp/owl/fsdas/aquaticresourceobservation.owl#AquaticResourceObservation
<http://www.ontologydesignpatterns.org/cp/owl/fsdas/aquaticresourceobservation.owl#AquaticResourceObservation> rdf:type owl:NamedIndividual ,
                                                                                                                        odin:ODPElement ;
                                                                                                               odin:describedIn odin:AquaticResourceObservation_Descr ;
                                                                                                               rdfs:comment "An observation singled out of reported data, once a year, about an aquatic resource." .


###  http://www.ontologydesignpatterns.org/cp/owl/fsdas/aquaticresources.owl#AquaticSpecies
<http://www.ontologydesignpatterns.org/cp/owl/fsdas/aquaticresources.owl#AquaticSpecies> rdf:type owl:NamedIndividual ,
                                                                                                  odin:ODPElement ;
                                                                                         odin:describedIn odin:AquaticSpecies_Descr ;
                                                                                         rdfs:comment "Aquatic species are conceptual entities that are characterized together with resources and water areas.   Mappable to fi:Species, fi:SpeciesRef, fi:SpeciesFeature, etc.  It has related axioms from FIGIS Schema that are included in the classes linked to the fi:Species class, such as fi:SpeciesRef (holding association with fi:AqResRef, which holds association with fi:WaterAreaRef)." ,
                                                                                                      "Here also the complex type SpeciesFeature (holding association with BathymetricRange) is the schema mapping required to refer to BathymetricRange. Any mapping has to take care of that, e.g. maps(AquaticSpecies, owl:unionOf(SpeciesRef, SpeciesFeature))." ,
                                                                                                      "Here also the complex type SpeciesFeature (holding association with HabitatBio) is the schema mapping required to refer to Habitat. Any mapping has to take care of that, e.g. maps(AquaticSpecies, owl:unionOf(SpeciesRef, SpeciesFeature))." .


###  http://www.ontologydesignpatterns.org/cp/owl/fsdas/aquaticresources.owl#WaterArea
<http://www.ontologydesignpatterns.org/cp/owl/fsdas/aquaticresources.owl#WaterArea> rdf:type owl:NamedIndividual ,
                                                                                             odin:ODPElement ;
                                                                                    odin:describedIn odin:WaterArea_Descr ;
                                                                                    rdfs:comment "A physical water area. Mappable to fi:WaterAreaRef" .


###  http://www.ontologydesignpatterns.org/cp/owl/fsdas/aquaticresources.owl#hasSpecies
<http://www.ontologydesignpatterns.org/cp/owl/fsdas/aquaticresources.owl#hasSpecies> rdf:type owl:NamedIndividual ,
                                                                                              odin:ODPElement ;
                                                                                     odin:describedIn odin:hasSpecies_Descr ;
                                                                                     rdfs:comment "has species" .


###  http://www.ontologydesignpatterns.org/cp/owl/fsdas/catchrecord.owl#CatchRecord
<http://www.ontologydesignpatterns.org/cp/owl/fsdas/catchrecord.owl#CatchRecord> rdf:type owl:NamedIndividual ,
                                                                                          odin:ODPElement ;
                                                                                 odin:describedIn odin:CatchRecord_Descr ;
                                                                                 rdfs:comment "A design pattern representing the semantics of the data contained in a database view (record) about catches of species in certain fishing areas for a certain reference year." .


###  http://www.ontologydesignpatterns.org/cp/owl/fsdas/catchrecord.owl#countryOfRecord
<http://www.ontologydesignpatterns.org/cp/owl/fsdas/catchrecord.owl#countryOfRecord> rdf:type owl:NamedIndividual ,
                                                                                              odin:ODPElement ;
                                                                                     odin:describedIn odin:countryOfRecord_Descr ;
                                                                                     rdfs:comment "The country parameter for a species catch record." .


###  http://www.ontologydesignpatterns.org/cp/owl/fsdas/catchrecord.owl#fishingAreaOfRecord
<http://www.ontologydesignpatterns.org/cp/owl/fsdas/catchrecord.owl#fishingAreaOfRecord> rdf:type owl:NamedIndividual ,
                                                                                                  odin:ODPElement ;
                                                                                         odin:describedIn odin:fishingAreaOfRecord_Descr ;
                                                                                         rdfs:comment "The area parameter for a species catch record." .


###  http://www.ontologydesignpatterns.org/cp/owl/fsdas/catchrecord.owl#forCountry
<http://www.ontologydesignpatterns.org/cp/owl/fsdas/catchrecord.owl#forCountry> rdf:type owl:NamedIndividual ,
                                                                                         odin:ODPElement ;
                                                                                odin:describedIn odin:forCountry_Descr ;
                                                                                rdfs:comment "The country parameter for a species catch record." .


###  http://www.ontologydesignpatterns.org/cp/owl/fsdas/catchrecord.owl#fromFishingArea
<http://www.ontologydesignpatterns.org/cp/owl/fsdas/catchrecord.owl#fromFishingArea> rdf:type owl:NamedIndividual ,
                                                                                              odin:ODPElement ;
                                                                                     odin:describedIn odin:fromFishingArea_Descr ;
                                                                                     rdfs:comment "The area parameter for a species catch record." .


###  http://www.ontologydesignpatterns.org/cp/owl/fsdas/catchrecord.owl#hasCatchRecord
<http://www.ontologydesignpatterns.org/cp/owl/fsdas/catchrecord.owl#hasCatchRecord> rdf:type owl:NamedIndividual ,
                                                                                             odin:ODPElement ;
                                                                                    odin:describedIn odin:hasCatchRecord_Descr ;
                                                                                    rdfs:comment "The catch record of a species, i.e. its statistical observation over a reference year." .


###  http://www.ontologydesignpatterns.org/cp/owl/fsdas/catchrecord.owl#isCatchRecordFor
<http://www.ontologydesignpatterns.org/cp/owl/fsdas/catchrecord.owl#isCatchRecordFor> rdf:type owl:NamedIndividual ,
                                                                                               odin:ODPElement ;
                                                                                      odin:describedIn odin:isCatchRecordFor_Descr ;
                                                                                      rdfs:comment "The catch record of a species, i.e. its statistical observation over a reference year." .


###  http://www.ontologydesignpatterns.org/cp/owl/fsdas/catchrecord.owl#referenceYear
<http://www.ontologydesignpatterns.org/cp/owl/fsdas/catchrecord.owl#referenceYear> rdf:type owl:NamedIndividual ,
                                                                                            odin:ODPElement ;
                                                                                   odin:describedIn odin:referenceYear_Descr ;
                                                                                   rdfs:comment "The year for which the status of the target object (e.g. Marine Resource, Fishery...) has been evaluated." .


###  http://www.ontologydesignpatterns.org/cp/owl/fsdas/catchrecord.owl#reportingYear
<http://www.ontologydesignpatterns.org/cp/owl/fsdas/catchrecord.owl#reportingYear> rdf:type owl:NamedIndividual ,
                                                                                            odin:ODPElement ;
                                                                                   odin:describedIn odin:reportingYear_Descr ;
                                                                                   rdfs:comment "The year in which a catch record has been officially reported (different from its reference year, i.e. the year of the actual observation)." .


###  http://www.ontologydesignpatterns.org/cp/owl/fsdas/catchrecord.owl#unitUsedInRecord
<http://www.ontologydesignpatterns.org/cp/owl/fsdas/catchrecord.owl#unitUsedInRecord> rdf:type owl:NamedIndividual ,
                                                                                               odin:ODPElement ;
                                                                                      odin:describedIn odin:unitUsedInRecord_Descr ;
                                                                                      rdfs:comment "The unit of measure parameter for a species catch record." .


###  http://www.ontologydesignpatterns.org/cp/owl/fsdas/catchrecord.owl#withUnit
<http://www.ontologydesignpatterns.org/cp/owl/fsdas/catchrecord.owl#withUnit> rdf:type owl:NamedIndividual ,
                                                                                       odin:ODPElement ;
                                                                              odin:describedIn odin:withUnit_Descr ;
                                                                              rdfs:comment "The unit of measure parameter for a species catch record." .


###  http://www.ontologydesignpatterns.org/cp/owl/fsdas/climaticzone.owl#AquaticResource
<http://www.ontologydesignpatterns.org/cp/owl/fsdas/climaticzone.owl#AquaticResource> rdf:type owl:NamedIndividual ,
                                                                                               odin:ODPElement ;
                                                                                      odin:describedIn odin:AquaticResource_Descr ;
                                                                                      rdfs:comment "A fishery resource (a collection of actual aquatic organisms) that can include aquatic organisms from different AquaticSpecies, and is localized in some WaterArea.  It can be mapped to fi:AqResRef" .


###  http://www.ontologydesignpatterns.org/cp/owl/fsdas/climaticzone.owl#AquaticResourceObservation
<http://www.ontologydesignpatterns.org/cp/owl/fsdas/climaticzone.owl#AquaticResourceObservation> rdf:type owl:NamedIndividual ,
                                                                                                          odin:ODPElement ;
                                                                                                 odin:describedIn odin:AquaticResourceObservation_Descr ;
                                                                                                 rdfs:comment "An observation of a resource characterised by different parameters." .


###  http://www.ontologydesignpatterns.org/cp/owl/fsdas/gearvessel.owl#GearType
<http://www.ontologydesignpatterns.org/cp/owl/fsdas/gearvessel.owl#GearType> rdf:type owl:NamedIndividual ,
                                                                                      odin:ODPElement ;
                                                                             odin:describedIn odin:GearType_Descr ;
                                                                             rdfs:comment "Gear types are conceptual entities that are characterized together with AquaticSpecies that are either targeted or can be incidentally caught.   Mappable to fi:GeartypeRef" .


###  http://www.ontologydesignpatterns.org/cp/owl/fsdas/gearvessel.owl#VesselType
<http://www.ontologydesignpatterns.org/cp/owl/fsdas/gearvessel.owl#VesselType> rdf:type owl:NamedIndividual ,
                                                                                        odin:ODPElement ;
                                                                               odin:describedIn odin:VesselType_Descr ;
                                                                               rdfs:comment "Vessel types are conceptual entities.   Mappable to fi:VesseltypeRef" .


###  http://www.ontologydesignpatterns.org/cp/owl/fsdas/gearwaterarea.owl#isSuitableForGearType
<http://www.ontologydesignpatterns.org/cp/owl/fsdas/gearwaterarea.owl#isSuitableForGearType> rdf:type owl:NamedIndividual ,
                                                                                                      odin:ODPElement ;
                                                                                             odin:describedIn odin:isSuitableForGearType_Descr ;
                                                                                             rdfs:comment "Actually a composed property: this needs either a property chain, a SPARQL query, or a SWRL rule to gather a value. E.g. in SPARQL:     CONSTRUCT {?x :isUsedInWaterArea ?y . ?y :isSuitableForGearType ?x}  WHERE {  ?x gearspecies:targetsSpecies ?z .  ?z aquaticresources:isSpeciesPresentIn ?w .  ?w aquaticresources:hasWaterArea ?y  }" .


###  http://www.ontologydesignpatterns.org/cp/owl/fsdas/gearwaterarea.owl#isUsedInWaterArea
<http://www.ontologydesignpatterns.org/cp/owl/fsdas/gearwaterarea.owl#isUsedInWaterArea> rdf:type owl:NamedIndividual ,
                                                                                                  odin:ODPElement ;
                                                                                         odin:describedIn odin:isUsedInWaterArea_Descr ;
                                                                                         rdfs:comment "Actually a composed property: this needs either a property chain, a SPARQL query, or a SWRL rule to gather a value. E.g. in SPARQL:     CONSTRUCT {?x :isUsedInWaterArea ?y . ?y :isSuitableForGearType ?x}  WHERE {  ?x gearspecies:targetsSpecies ?z .  ?z aquaticresources:isSpeciesPresentIn ?w .  ?w aquaticresources:hasWaterArea ?y  }" .


###  http://www.ontologydesignpatterns.org/cp/owl/fsdas/resourceabundanceobservation.owl#ResourceAbundanceObservation
<http://www.ontologydesignpatterns.org/cp/owl/fsdas/resourceabundanceobservation.owl#ResourceAbundanceObservation> rdf:type owl:NamedIndividual ,
                                                                                                                            odin:ODPElement ;
                                                                                                                   odin:describedIn odin:ResourceAbundanceObservation_Descr ;
                                                                                                                   rdfs:comment "An observation of a resource characterised by different parameters." .


###  http://www.ontologydesignpatterns.org/cp/owl/fsdas/resourceexploitationobservation.owl#ResourceExploitationObservation
<http://www.ontologydesignpatterns.org/cp/owl/fsdas/resourceexploitationobservation.owl#ResourceExploitationObservation> rdf:type owl:NamedIndividual ,
                                                                                                                                  odin:ODPElement ;
                                                                                                                         odin:describedIn odin:ResourceExploitationObservation_Descr ;
                                                                                                                         rdfs:comment "An observation of a resource characterised by different parameters." .


###  http://www.ontologydesignpatterns.org/cp/owl/fsdas/rtmsmapping.owl#RTMS_Code
<http://www.ontologydesignpatterns.org/cp/owl/fsdas/rtmsmapping.owl#RTMS_Code> rdf:type owl:NamedIndividual ,
                                                                                        odin:ODPElement ;
                                                                               odin:describedIn odin:RTMS_Code_Descr ;
                                                                               rdfs:comment "Any code RTMS relational database that is linked from the FIGIS XML.  For species, it can be possibly mapped to fi:FAO3AlphaCode, fi:FAOTaxonomicCode, or fi:ISSCAAPCode" .


###  http://www.ontologydesignpatterns.org/cp/owl/fsdas/speciesbathymetry.owl#BathymetricRange
<http://www.ontologydesignpatterns.org/cp/owl/fsdas/speciesbathymetry.owl#BathymetricRange> rdf:type owl:NamedIndividual ,
                                                                                                     odin:ODPElement ;
                                                                                            odin:describedIn odin:BathymetricRange_Descr ;
                                                                                            rdfs:comment "This class contains the set of bathymetric ranges. Bathymetry is numeric depth information about the ranges in which an aquatic species is found.  It can be mapped to fi:Bathymetry." .


###  http://www.ontologydesignpatterns.org/cp/owl/fsdas/speciesbathymetry.owl#hasBathymetricRange
<http://www.ontologydesignpatterns.org/cp/owl/fsdas/speciesbathymetry.owl#hasBathymetricRange> rdf:type owl:NamedIndividual ,
                                                                                                        odin:ODPElement ;
                                                                                               odin:describedIn odin:hasBathymetricRange_Descr ;
                                                                                               rdfs:comment "has bathymetric range" .


###  http://www.ontologydesignpatterns.org/cp/owl/fsdas/speciesbathymetry.owl#isBathymetricRangeOf
<http://www.ontologydesignpatterns.org/cp/owl/fsdas/speciesbathymetry.owl#isBathymetricRangeOf> rdf:type owl:NamedIndividual ,
                                                                                                         odin:ODPElement ;
                                                                                                odin:describedIn odin:isBathymetricRangeOf_Descr ;
                                                                                                rdfs:comment "is bathymetric range of" .


###  http://www.ontologydesignpatterns.org/cp/owl/fsdas/speciesconditions.owl#AquaticSpecies
<http://www.ontologydesignpatterns.org/cp/owl/fsdas/speciesconditions.owl#AquaticSpecies> rdf:type owl:NamedIndividual ,
                                                                                                   odin:ODPElement ;
                                                                                          odin:describedIn odin:AquaticSpecies_Descr ;
                                                                                          rdfs:comment "Aquatic species is characterized together with resources and water areas.   Mappable to fi:Species, fi:SpeciesRef, fi:SpeciesFeature, etc.  It has related axioms from FIGIS Schema that are included in the classes linked to the fi:Species class, such as fi:SpeciesRef (holding association with fi:AqResRef, which holds association with fi:WaterAreaRef)." .


###  http://www.ontologydesignpatterns.org/cp/owl/fsdas/speciesconditions.owl#BathymetricRange
<http://www.ontologydesignpatterns.org/cp/owl/fsdas/speciesconditions.owl#BathymetricRange> rdf:type owl:NamedIndividual ,
                                                                                                     odin:ODPElement ;
                                                                                            odin:describedIn odin:BathymetricRange_Descr ;
                                                                                            rdfs:comment "This class contains the set of bathymetric ranges. Bathymetry is numeric depth information about the ranges in which an aquatic species is found.  It can be mapped to fi:Bathymetry." .


###  http://www.ontologydesignpatterns.org/cp/owl/fsdas/speciesconditions.owl#Habitat
<http://www.ontologydesignpatterns.org/cp/owl/fsdas/speciesconditions.owl#Habitat> rdf:type owl:NamedIndividual ,
                                                                                            odin:ODPElement ;
                                                                                   odin:describedIn odin:Habitat_Descr ;
                                                                                   rdfs:comment "Habitat is the biological and ecological context of a species in the area of an aquatic resource." .


###  http://www.ontologydesignpatterns.org/cp/owl/fsdas/speciesconditions.owl#SpeciesConditions
<http://www.ontologydesignpatterns.org/cp/owl/fsdas/speciesconditions.owl#SpeciesConditions> rdf:type owl:NamedIndividual ,
                                                                                                      odin:ODPElement ;
                                                                                             odin:describedIn odin:SpeciesConditions_Descr ;
                                                                                             rdfs:comment "A class that allows to represent the typical physic conditions (bathymetry, habitat) of an aquatic species for a certain water area." .


###  http://www.ontologydesignpatterns.org/cp/owl/fsdas/speciesconservation.owl#AquaticSpecies
<http://www.ontologydesignpatterns.org/cp/owl/fsdas/speciesconservation.owl#AquaticSpecies> rdf:type owl:NamedIndividual ,
                                                                                                     odin:ODPElement ;
                                                                                            odin:describedIn odin:AquaticSpecies_Descr ;
                                                                                            rdfs:comment "Aquatic species are conceptual entities that are characterized together with resources and water areas.   Mappable to fi:Species, fi:SpeciesRef, fi:SpeciesFeature, etc.  It has related axioms from FIGIS Schema that are included in the classes linked to the fi:Species class, such as fi:SpeciesRef (holding association with fi:AqResRef, which holds association with fi:WaterAreaRef)." .


###  http://www.ontologydesignpatterns.org/cp/owl/fsdas/specieseat.owl#AquaticSpecies
<http://www.ontologydesignpatterns.org/cp/owl/fsdas/specieseat.owl#AquaticSpecies> rdf:type owl:NamedIndividual ,
                                                                                            odin:ODPElement ;
                                                                                   odin:describedIn odin:AquaticSpecies_Descr ;
                                                                                   rdfs:comment "Aquatic species are conceptual entities that are characterized together with resources and water areas.   Mappable to fi:Species, fi:SpeciesRef, fi:SpeciesFeature, etc.  It has related axioms from FIGIS Schema that are included in the classes linked to the fi:Species class, such as fi:SpeciesRef (holding association with fi:AqResRef, which holds association with fi:WaterAreaRef)." .


###  http://www.ontologydesignpatterns.org/cp/owl/fsdas/specieshabitat.owl#Habitat
<http://www.ontologydesignpatterns.org/cp/owl/fsdas/specieshabitat.owl#Habitat> rdf:type owl:NamedIndividual ,
                                                                                         odin:ODPElement ;
                                                                                odin:describedIn odin:Habitat_Descr ;
                                                                                rdfs:comment "Habitat is the biological and ecological context of a species in the area of an aquatic resource." .


###  http://www.ontologydesignpatterns.org/cp/owl/fsdas/speciesnames.owl#AquaticSpecies
<http://www.ontologydesignpatterns.org/cp/owl/fsdas/speciesnames.owl#AquaticSpecies> rdf:type owl:NamedIndividual ,
                                                                                              odin:ODPElement ;
                                                                                     odin:describedIn odin:AquaticSpecies_Descr ;
                                                                                     rdfs:comment "Aquatic species are conceptual entities that are characterized together with resources and water areas.   Mappable to fi:Species, fi:SpeciesRef, fi:SpeciesFeature, etc.  It has related axioms from FIGIS Schema that are included in the classes linked to the fi:Species class, such as fi:SpeciesRef (holding association with fi:AqResRef, which holds association with fi:WaterAreaRef)." .


###  http://www.ontologydesignpatterns.org/cp/owl/fsdas/speciesnames.owl#canBeConfusedWith
<http://www.ontologydesignpatterns.org/cp/owl/fsdas/speciesnames.owl#canBeConfusedWith> rdf:type owl:NamedIndividual ,
                                                                                                 odin:ODPElement ;
                                                                                        odin:describedIn odin:canBeConfusedWith_Descr ;
                                                                                        rdfs:comment "A property for expressing a description of why a species may be confused with another. It may instead/also contain a list of other species with which a species may be confused." .


###  http://www.ontologydesignpatterns.org/cp/owl/fsdas/speciesnames.owl#hasLocalName
<http://www.ontologydesignpatterns.org/cp/owl/fsdas/speciesnames.owl#hasLocalName> rdf:type owl:NamedIndividual ,
                                                                                            odin:ODPElement ;
                                                                                   odin:describedIn odin:hasLocalName_Descr ;
                                                                                   rdfs:comment "Property to express a species' localname , where it is used , and any additional information like the name of the dialect or more detailed geographical information on where exactly the local-common name is used for the aquatic species in a given country." .


###  http://www.ontologydesignpatterns.org/cp/owl/fsdas/speciesnames.owl#hasSynonym
<http://www.ontologydesignpatterns.org/cp/owl/fsdas/speciesnames.owl#hasSynonym> rdf:type owl:NamedIndividual ,
                                                                                          odin:ODPElement ;
                                                                                 odin:describedIn odin:hasSynonym_Descr ;
                                                                                 rdfs:comment "Expresses the scientific names that exist for a species but are no longer valid." .


###  http://www.ontologydesignpatterns.org/cp/owl/fsdas/verticaldistribution.owl#AquaticResource
<http://www.ontologydesignpatterns.org/cp/owl/fsdas/verticaldistribution.owl#AquaticResource> rdf:type owl:NamedIndividual ,
                                                                                                       odin:ODPElement ;
                                                                                              odin:describedIn odin:AquaticResource_Descr ;
                                                                                              rdfs:comment "A fishery resource (a collection of actual aquatic organisms) that can include aquatic organisms from different AquaticSpecies, and is localized in some WaterArea.  It can be mapped to fi:AqResRef" .


###  http://www.ontologydesignpatterns.org/cp/owl/fsdas/verticaldistribution.owl#AquaticResourceObservation
<http://www.ontologydesignpatterns.org/cp/owl/fsdas/verticaldistribution.owl#AquaticResourceObservation> rdf:type owl:NamedIndividual ,
                                                                                                                  odin:ODPElement ;
                                                                                                         odin:describedIn odin:AquaticResourceObservation_Descr ;
                                                                                                         rdfs:comment "An observation of a resource characterised by different parameters." .


###  http://www.ontologydesignpatterns.org/cp/owl/fsdas/vesselspecies.owl#catchesSpecies
<http://www.ontologydesignpatterns.org/cp/owl/fsdas/vesselspecies.owl#catchesSpecies> rdf:type owl:NamedIndividual ,
                                                                                               odin:ODPElement ;
                                                                                      odin:describedIn odin:catchesSpecies_Descr ;
                                                                                      rdfs:comment "Actually a composed property: this needs either a property chain, a SPARQL query, or a SWRL rule to gather a value. E.g. in SPARQL:     CONSTRUCT {?x :catchesSpecies ?y . ?y isCaughtBy ?x}  WHERE {  ?x gearvessel:usesGearType ?z .  ?z gearspecies:catchesSpecies ?y  }" .


###  http://www.ontologydesignpatterns.org/cp/owl/fsdas/vesselspecies.owl#isCaughtBy
<http://www.ontologydesignpatterns.org/cp/owl/fsdas/vesselspecies.owl#isCaughtBy> rdf:type owl:NamedIndividual ,
                                                                                           odin:ODPElement ;
                                                                                  odin:describedIn odin:isCaughtBy_Descr ;
                                                                                  rdfs:comment "Actually a composed property: this needs either a property chain, a SPARQL query, or a SWRL rule to gather a value. E.g. in SPARQL:     CONSTRUCT {?x :catchesSpecies ?y . ?y isCaughtBy ?x}  WHERE {  ?x gearvessel:usesGearType ?z .  ?z gearspecies:catchesSpecies ?y  }" .


###  http://www.ontologydesignpatterns.org/cp/owl/fsdas/vesselwaterarea.owl#canBeCrossedByVesselType
<http://www.ontologydesignpatterns.org/cp/owl/fsdas/vesselwaterarea.owl#canBeCrossedByVesselType> rdf:type owl:NamedIndividual ,
                                                                                                           odin:ODPElement ;
                                                                                                  odin:describedIn odin:canBeCrossedByVesselType_Descr ;
                                                                                                  rdfs:comment "Actually a composed property: this needs either a property chain, a SPARQL query, or a SWRL rule to gather a value. E.g. in SPARQL:     CONSTRUCT {?x :canCrossWaterArea ?y . ?y canBeCrossedByVesselType ?x}  WHERE {  ?x gearvessel:usesGearType ?z .  ?z gearwaterarea:isUsedInWaterArea ?y  }" .


###  http://www.ontologydesignpatterns.org/cp/owl/fsdas/vesselwaterarea.owl#canCrossWaterArea
<http://www.ontologydesignpatterns.org/cp/owl/fsdas/vesselwaterarea.owl#canCrossWaterArea> rdf:type owl:NamedIndividual ,
                                                                                                    odin:ODPElement ;
                                                                                           odin:describedIn odin:canCrossWaterArea_Descr ;
                                                                                           rdfs:comment "Actually a composed property: this needs either a property chain, a SPARQL query, or a SWRL rule to gather a value. E.g. in SPARQL:     CONSTRUCT {?x :canCrossWaterArea ?y . ?y canBeCrossedByVesselType ?x}  WHERE {  ?x gearvessel:usesGearType ?z .  ?z gearwaterarea:isUsedInWaterArea ?y  }" .


###  http://www.ontologydesignpatterns.org/cp/owl/gotop.owl#All
<http://www.ontologydesignpatterns.org/cp/owl/gotop.owl#All> rdf:type owl:NamedIndividual ,
                                                                      odin:ODPElement ;
                                                             odin:describedIn odin:All_Descr ;
                                                             rdfs:comment "This term is the most general term possible" .


###  http://www.ontologydesignpatterns.org/cp/owl/gotop.owl#BiologicalProcess
<http://www.ontologydesignpatterns.org/cp/owl/gotop.owl#BiologicalProcess> rdf:type owl:NamedIndividual ,
                                                                                    odin:ODPElement ;
                                                                           odin:describedIn odin:BiologicalProcess_Descr ;
                                                                           rdfs:comment "Those processes specifically pertinent to the functioning of integrated living units: cells, tissues, organs, and organisms. A process is a collection of molecular events with a defined beginning and end." .


###  http://www.ontologydesignpatterns.org/cp/owl/gotop.owl#CellularComponent
<http://www.ontologydesignpatterns.org/cp/owl/gotop.owl#CellularComponent> rdf:type owl:NamedIndividual ,
                                                                                    odin:ODPElement ;
                                                                           odin:describedIn odin:CellularComponent_Descr ;
                                                                           odin:odpType odin:Core ;
                                                                           rdfs:comment "The part of a cell or its extracellular environment in which a gene product is located. A gene product may be located in one or more parts of a cell and its location may be as specific as a particular macromolecular complex, that is, a stable, persistent association of macromolecules that function together." .


###  http://www.ontologydesignpatterns.org/cp/owl/gotop.owl#MolecularFunction
<http://www.ontologydesignpatterns.org/cp/owl/gotop.owl#MolecularFunction> rdf:type owl:NamedIndividual ,
                                                                                    odin:ODPElement ;
                                                                           odin:describedIn odin:MolecularFunction_Descr ;
                                                                           rdfs:comment "Elemental activities, such as catalysis or binding, describing the actions of a gene product at the molecular level. A given gene product may exhibit one or more molecular functions." .


###  http://www.ontologydesignpatterns.org/cp/owl/informationobjectsandrepresentationlanguages.owl#FormalExpression
<http://www.ontologydesignpatterns.org/cp/owl/informationobjectsandrepresentationlanguages.owl#FormalExpression> rdf:type owl:NamedIndividual ,
                                                                                                                          odin:ODPElement ;
                                                                                                                 odin:describedIn odin:FormalExpression_Descr ;
                                                                                                                 odin:odpType odin:Foundational ;
                                                                                                                 rdfs:comment "Any information object represented in a FormalLanguage, usually having a formal interpretation by a dul:FormalEntity, and used to formally represent any Entity" .


###  http://www.ontologydesignpatterns.org/cp/owl/informationobjectsandrepresentationlanguages.owl#FormalLanguage
<http://www.ontologydesignpatterns.org/cp/owl/informationobjectsandrepresentationlanguages.owl#FormalLanguage> rdf:type owl:NamedIndividual ,
                                                                                                                        odin:ODPElement ;
                                                                                                               odin:describedIn odin:FormalLanguage_Descr ;
                                                                                                               odin:odpType odin:Foundational ;
                                                                                                               rdfs:comment "A formal language, created by some human, with a fixed grammar, and usually with an explicit formal semantics (i.e. its elements have an interpretation wrt to formal entities such as sets, categories, etc.)." .


###  http://www.ontologydesignpatterns.org/cp/owl/informationobjectsandrepresentationlanguages.owl#IconicLanguage
<http://www.ontologydesignpatterns.org/cp/owl/informationobjectsandrepresentationlanguages.owl#IconicLanguage> rdf:type owl:NamedIndividual ,
                                                                                                                        odin:ODPElement ;
                                                                                                               odin:describedIn odin:IconicLanguage_Descr ;
                                                                                                               odin:odpType odin:Foundational ;
                                                                                                               rdfs:comment "A language made up of graphical elements. It can be natural, artificial, and even formal." .


###  http://www.ontologydesignpatterns.org/cp/owl/informationobjectsandrepresentationlanguages.owl#IconicObject
<http://www.ontologydesignpatterns.org/cp/owl/informationobjectsandrepresentationlanguages.owl#IconicObject> rdf:type owl:NamedIndividual ,
                                                                                                                      odin:ODPElement ;
                                                                                                             odin:describedIn odin:IconicObject_Descr ;
                                                                                                             rdfs:comment "An information object represented in an IconicLanguage" .


###  http://www.ontologydesignpatterns.org/cp/owl/informationobjectsandrepresentationlanguages.owl#Language
<http://www.ontologydesignpatterns.org/cp/owl/informationobjectsandrepresentationlanguages.owl#Language> rdf:type owl:NamedIndividual ,
                                                                                                                  odin:ODPElement ;
                                                                                                         odin:describedIn odin:Language_Descr ;
                                                                                                         rdfs:comment "A natural or artificial language, provided with an alphabet (or vocabulary) and combinatorial rules. In the case of natural languages, their components are 'temporary' and 'reconstructed' out of actual usage. For example, a grammar for a natural language has the status of a theory for that language, and alternative ones can exist (e.g. generative vs. construction grammars).  Another distinction, between the general (systemic) rules for a language, and the local (contextual) rules for e.g. a certain context, speaker, place, etc., can be made separately.  The most comprehensive classification of languages ha probably been made by Umberto Eco, based on the production modes of the 'signs' that are represented in a certain language. It uses several semiotic dimensions, and will be modeled in a forthcoming ontology." .


###  http://www.ontologydesignpatterns.org/cp/owl/informationobjectsandrepresentationlanguages.owl#LinguisticObject
<http://www.ontologydesignpatterns.org/cp/owl/informationobjectsandrepresentationlanguages.owl#LinguisticObject> rdf:type owl:NamedIndividual ,
                                                                                                                          odin:ODPElement ;
                                                                                                                 odin:describedIn odin:LinguisticObject_Descr ;
                                                                                                                 odin:odpType odin:Foundational ;
                                                                                                                 rdfs:comment "An information object represented in a NaturalLanguage" .


###  http://www.ontologydesignpatterns.org/cp/owl/informationobjectsandrepresentationlanguages.owl#NaturalLanguage
<http://www.ontologydesignpatterns.org/cp/owl/informationobjectsandrepresentationlanguages.owl#NaturalLanguage> rdf:type owl:NamedIndividual ,
                                                                                                                         odin:ODPElement ;
                                                                                                                odin:describedIn odin:NaturalLanguage_Descr ;
                                                                                                                odin:odpType odin:Foundational ;
                                                                                                                rdfs:comment "A natural language, evolved and used in a community across time.  Natural languages components are 'temporary' and 'reconstructed' out of actual usage. For example, a grammar for a (part of a) natural language has the status of a theory for that language, but alternative ones can exist (e.g. generative vs. construction grammars)." .


###  http://www.ontologydesignpatterns.org/cp/owl/informationobjectsandrepresentationlanguages.owl#formallyRepresents
<http://www.ontologydesignpatterns.org/cp/owl/informationobjectsandrepresentationlanguages.owl#formallyRepresents> rdf:type owl:NamedIndividual ,
                                                                                                                            odin:ODPElement ;
                                                                                                                   odin:describedIn odin:formallyRepresents_Descr ;
                                                                                                                   odin:odpType odin:Foundational ;
                                                                                                                   rdfs:comment "The relation between formal expressions, and anything that they are supposed to represent.  E.g., 'the predicate 'MariachiInTijuana' formallyRepresents the dul:Collection of all mariachis in Tijuana'; 'the equivalence relation '<=>' formallyRepresents the concept of two entities having the same properties'.  Notice that formal expressions are formally interpreted by instances of dul:FormalEntity" .


###  http://www.ontologydesignpatterns.org/cp/owl/informationobjectsandrepresentationlanguages.owl#isConceptualizedBy
<http://www.ontologydesignpatterns.org/cp/owl/informationobjectsandrepresentationlanguages.owl#isConceptualizedBy> rdf:type owl:NamedIndividual ,
                                                                                                                            odin:ODPElement ;
                                                                                                                   odin:describedIn odin:isConceptualizedBy_Descr ;
                                                                                                                   odin:odpType odin:Foundational ;
                                                                                                                   rdfs:comment "A relation stating that an Agent is internally representing a Description . E.g., 'John believes in the conspiracy theory'; 'Niels Bohr created a solar-system metaphor for his atomic theory'; 'Jacques assumes all swans are white'; 'the task force shares the attack plan'." .


###  http://www.ontologydesignpatterns.org/cp/owl/informationobjectsandrepresentationlanguages.owl#isFormallyRepresentedIn
<http://www.ontologydesignpatterns.org/cp/owl/informationobjectsandrepresentationlanguages.owl#isFormallyRepresentedIn> rdf:type owl:NamedIndividual ,
                                                                                                                                 odin:ODPElement ;
                                                                                                                        odin:describedIn odin:isFormallyRepresentedIn_Descr ;
                                                                                                                        odin:odpType odin:Foundational ;
                                                                                                                        rdfs:comment "The relation between formal expressions, and anything that they are supposed to represent.  E.g., 'the predicate 'MariachiInTijuana' formallyRepresents the dul:Collection of all mariachis in Tijuana'; 'the equivalence relation '<=>' formallyRepresents the concept of two entities having the same properties'.  Notice that formal expressions are formally interpreted by instances of dul:FormalEntity" .


###  http://www.ontologydesignpatterns.org/cp/owl/informationrealization.owl#InformationRealization
<http://www.ontologydesignpatterns.org/cp/owl/informationrealization.owl#InformationRealization> rdf:type owl:NamedIndividual ,
                                                                                                          odin:ODPElement ;
                                                                                                 odin:describedIn odin:InformationRealization_Descr ;
                                                                                                 odin:odpType odin:Foundational ;
                                                                                                 rdfs:comment "A concrete realization of an information object, e.g. the written document containing the text of a law." .


###  http://www.ontologydesignpatterns.org/cp/owl/informationrealization.owl#isRealizedBy
<http://www.ontologydesignpatterns.org/cp/owl/informationrealization.owl#isRealizedBy> rdf:type owl:NamedIndividual ,
                                                                                                odin:ODPElement ;
                                                                                       odin:describedIn odin:isRealizedBy_Descr ;
                                                                                       odin:odpType odin:Foundational ;
                                                                                       rdfs:comment "A relation between an information realization and an information object, e.g. the paper copy of the Italian Constitution realizes the text of the Constitution." .


###  http://www.ontologydesignpatterns.org/cp/owl/informationrealization.owl#realizes
<http://www.ontologydesignpatterns.org/cp/owl/informationrealization.owl#realizes> rdf:type owl:NamedIndividual ,
                                                                                            odin:ODPElement ;
                                                                                   odin:describedIn odin:realizes_Descr ;
                                                                                   odin:odpType odin:Foundational ;
                                                                                   rdfs:comment "A relation between an information realization and an information object, e.g. the paper copy of the Italian Constitution realizes the text of the Constitution." .


###  http://www.ontologydesignpatterns.org/cp/owl/intensionextension.owl#isAbout
<http://www.ontologydesignpatterns.org/cp/owl/intensionextension.owl#isAbout> rdf:type owl:NamedIndividual ,
                                                                                       odin:ODPElement ;
                                                                              odin:describedIn odin:isAbout_Descr ;
                                                                              rdfs:comment "A relation between information objects and any Entity (including information objects). It can be used to talk about e.g. entities are references of proper nouns: the proper noun 'Leonardo da Vinci' isAbout the Person Leonardo da Vinci; as well as to talk about sets of entities that can be described by a common noun: the common noun 'person' isAbout the set of all persons in a domain of discourse, which can be represented bu reusing the pattern CollectionEntity." .


###  http://www.ontologydesignpatterns.org/cp/owl/intensionextension.owl#isReferenceOf
<http://www.ontologydesignpatterns.org/cp/owl/intensionextension.owl#isReferenceOf> rdf:type owl:NamedIndividual ,
                                                                                             odin:ODPElement ;
                                                                                    odin:describedIn odin:isReferenceOf_Descr ;
                                                                                    odin:odpType odin:Foundational ;
                                                                                    rdfs:comment "A relation between information objects and any Entity (including information objects). It can be used to talk about e.g. entities are references of proper nouns: the proper noun 'Leonardo da Vinci' isAbout the Person Leonardo da Vinci; as well as to talk about sets of entities that can be described by a common noun: the common noun 'person' isAbout the set of all persons in a domain of discourse, which can be represented in DOLCE-Ultralite as an individual of the class: Collection ." .


###  http://www.ontologydesignpatterns.org/cp/owl/linnaeantaxonomy.owl#Class
<http://www.ontologydesignpatterns.org/cp/owl/linnaeantaxonomy.owl#Class> rdf:type owl:NamedIndividual ,
                                                                                   odin:ODPElement ;
                                                                          odin:describedIn odin:Class_Descr ;
                                                                          rdfs:comment "Class is the third highest traditional taxon. E.g., in the case of humans the class is 'Mammalia'." .


###  http://www.ontologydesignpatterns.org/cp/owl/linnaeantaxonomy.owl#Genus
<http://www.ontologydesignpatterns.org/cp/owl/linnaeantaxonomy.owl#Genus> rdf:type owl:NamedIndividual ,
                                                                                   odin:ODPElement ;
                                                                          odin:describedIn odin:Genus_Descr ;
                                                                          rdfs:comment "Genus is the sixth highest traditional taxon. E.g., in the case of humans the genus is 'Homo'." .


###  http://www.ontologydesignpatterns.org/cp/owl/linnaeantaxonomy.owl#Kingdom
<http://www.ontologydesignpatterns.org/cp/owl/linnaeantaxonomy.owl#Kingdom> rdf:type owl:NamedIndividual ,
                                                                                     odin:ODPElement ;
                                                                            odin:describedIn odin:Kingdom_Descr ;
                                                                            rdfs:comment "Kingdom is the highest traditional taxon. E.g., in the case of humans the kingdom is 'Animalia'." .


###  http://www.ontologydesignpatterns.org/cp/owl/linnaeantaxonomy.owl#Order
<http://www.ontologydesignpatterns.org/cp/owl/linnaeantaxonomy.owl#Order> rdf:type owl:NamedIndividual ,
                                                                                   odin:ODPElement ;
                                                                          odin:describedIn odin:Order_Descr ;
                                                                          rdfs:comment "Order is the fourth highest traditional taxon. E.g., in the case of humans the phylum is 'Primates'." .


###  http://www.ontologydesignpatterns.org/cp/owl/linnaeantaxonomy.owl#Phylum
<http://www.ontologydesignpatterns.org/cp/owl/linnaeantaxonomy.owl#Phylum> rdf:type owl:NamedIndividual ,
                                                                                    odin:ODPElement ;
                                                                           odin:describedIn odin:Phylum_Descr ;
                                                                           rdfs:comment "Phylum is the second highest traditional taxon. E.g., in the case of humans the phylum is 'Chordata'." .


###  http://www.ontologydesignpatterns.org/cp/owl/linnaeantaxonomy.owl#Species
<http://www.ontologydesignpatterns.org/cp/owl/linnaeantaxonomy.owl#Species> rdf:type owl:NamedIndividual ,
                                                                                     odin:ODPElement ;
                                                                            odin:describedIn odin:Species_Descr ;
                                                                            rdfs:comment "Species is the lowest traditional taxon. E.g., in the case of humans the species is 'Homo sapiens'." .


###  http://www.ontologydesignpatterns.org/cp/owl/linnaeantaxonomy.owl#hasDirectHigherRank
<http://www.ontologydesignpatterns.org/cp/owl/linnaeantaxonomy.owl#hasDirectHigherRank> rdf:type owl:NamedIndividual ,
                                                                                                 odin:ODPElement ;
                                                                                        odin:describedIn odin:hasDirectHigherRank_Descr ;
                                                                                        odin:odpType odin:Foundational ;
                                                                                        rdfs:comment "This property relates two taxa, where the first is more specific then the second and there is no other taxon that is both more general than the first and more specific than the second." .


###  http://www.ontologydesignpatterns.org/cp/owl/linnaeantaxonomy.owl#hasDirectLowerRank
<http://www.ontologydesignpatterns.org/cp/owl/linnaeantaxonomy.owl#hasDirectLowerRank> rdf:type owl:NamedIndividual ,
                                                                                                odin:ODPElement ;
                                                                                       odin:describedIn odin:hasDirectLowerRank_Descr ;
                                                                                       rdfs:comment "This property relates two taxa, where the first is less specific then the second and there is no other taxon that is both more specific than the first and more general than the second." .


###  http://www.ontologydesignpatterns.org/cp/owl/linnaeantaxonomy.owl#hasHigherRank
<http://www.ontologydesignpatterns.org/cp/owl/linnaeantaxonomy.owl#hasHigherRank> rdf:type owl:NamedIndividual ,
                                                                                           odin:ODPElement ;
                                                                                  odin:describedIn odin:hasHigherRank_Descr ;
                                                                                  rdfs:comment "This property relates two taxa, where the first is more specific than the second." .


###  http://www.ontologydesignpatterns.org/cp/owl/linnaeantaxonomy.owl#hasLowerRank
<http://www.ontologydesignpatterns.org/cp/owl/linnaeantaxonomy.owl#hasLowerRank> rdf:type owl:NamedIndividual ,
                                                                                          odin:ODPElement ;
                                                                                 odin:describedIn odin:hasLowerRank_Descr ;
                                                                                 rdfs:comment "This property relates two taxa, where the first is less specific than the second." .


###  http://www.ontologydesignpatterns.org/cp/owl/list.owl#List
<http://www.ontologydesignpatterns.org/cp/owl/list.owl#List> rdf:type owl:NamedIndividual ,
                                                                      odin:ODPElement ;
                                                             odin:describedIn odin:List_Descr ;
                                                             rdfs:comment "List - An ordered array of items, that can be present in multiple copies" .


###  http://www.ontologydesignpatterns.org/cp/owl/list.owl#ListItem
<http://www.ontologydesignpatterns.org/cp/owl/list.owl#ListItem> rdf:type owl:NamedIndividual ,
                                                                          odin:ODPElement ;
                                                                 odin:describedIn odin:ListItem_Descr ;
                                                                 rdfs:comment "ListItem - Element belonging to a list" .


###  http://www.ontologydesignpatterns.org/cp/owl/list.owl#hasFirstItem
<http://www.ontologydesignpatterns.org/cp/owl/list.owl#hasFirstItem> rdf:type owl:NamedIndividual ,
                                                                              odin:ODPElement ;
                                                                     odin:describedIn odin:hasFirstItem_Descr ;
                                                                     odin:odpType odin:Foundational ;
                                                                     rdfs:comment "first item - The link to the first item of the list" .


###  http://www.ontologydesignpatterns.org/cp/owl/list.owl#hasLastItem
<http://www.ontologydesignpatterns.org/cp/owl/list.owl#hasLastItem> rdf:type owl:NamedIndividual ,
                                                                             odin:ODPElement ;
                                                                    odin:describedIn odin:hasLastItem_Descr ;
                                                                    odin:odpType odin:Foundational ;
                                                                    rdfs:comment "last item - The link to the last item of the list" .


###  http://www.ontologydesignpatterns.org/cp/owl/list.owl#nextItem
<http://www.ontologydesignpatterns.org/cp/owl/list.owl#nextItem> rdf:type owl:NamedIndividual ,
                                                                          odin:ODPElement ;
                                                                 odin:describedIn odin:nextItem_Descr ;
                                                                 rdfs:comment "next item - The link to the next item in a list (ordered collection)" .


###  http://www.ontologydesignpatterns.org/cp/owl/list.owl#previousItem
<http://www.ontologydesignpatterns.org/cp/owl/list.owl#previousItem> rdf:type owl:NamedIndividual ,
                                                                              odin:ODPElement ;
                                                                     odin:describedIn odin:previousItem_Descr ;
                                                                     odin:odpType odin:Foundational ;
                                                                     rdfs:comment "previous item - The link to the previous item in a list (ordered collection)" .


###  http://www.ontologydesignpatterns.org/cp/owl/move.owl#Move
<http://www.ontologydesignpatterns.org/cp/owl/move.owl#Move> rdf:type owl:NamedIndividual ,
                                                                      odin:ODPElement ;
                                                             odin:describedIn odin:Move_Descr ;
                                                             odin:odpType odin:Foundational ;
                                                             rdfs:comment "This class comprises changes of the physical location of the instances of Physical Object.      Note, that the class Move inherits the property 'took place at' (witnessed): Place. This property should be used to describe the trajectory or a larger area within which a move takes place, whereas the properties moved to (was destination of), moved from (was origin of) describe the start and end points only. Moves may also be documented to consistsOf other moves (via consistsOf (formsPartOf)), in order to describe intermediate stages on a trajectory. In that case, start and end points of the partial moves should match appropriately between each other and with the overall event. {@en}" .


###  http://www.ontologydesignpatterns.org/cp/owl/move.owl#PhysicalObject
<http://www.ontologydesignpatterns.org/cp/owl/move.owl#PhysicalObject> rdf:type owl:NamedIndividual ,
                                                                                odin:ODPElement ;
                                                                       odin:describedIn odin:PhysicalObject_Descr ;
                                                                       odin:odpType odin:Foundational ;
                                                                       rdfs:comment "This class comprises items of a material nature that are units for documentation and have physical boundaries that separate them completely in an objective way from other objects.      The class also includes all aggregates of objects made for functional purposes of whatever kind, independent of physical coherence, such as a set of chessmen. Typically, instances of E19 Physical Object can be moved (if not too heavy).     In some contexts, such objects, except for aggregates, are also called bona fide objects (Smith and Varzi, 2000, pp.401-420), i.e. naturally defined objects.      The decision as to what is documented as a complete item, rather than by its parts or components, may be a purely administrative decision or may be a result of the order in which the item was acquired." .


###  http://www.ontologydesignpatterns.org/cp/owl/move.owl#Place
<http://www.ontologydesignpatterns.org/cp/owl/move.owl#Place> rdf:type owl:NamedIndividual ,
                                                                       odin:ODPElement ;
                                                              odin:describedIn odin:Place_Descr ;
                                                              rdfs:comment "This class comprises extents in space, in particular on the surface of the earth, in the pure sense of physics: independent from temporal phenomena and matter. The instances of E53 Place are usually determined by reference to the position of immobile objects such as buildings, cities, mountains, rivers, or dedicated geodetic marks. A Place can be determined by combining a frame of reference and a location with respect to this frame. It may be identified by one or more instances of E44 Place Appellation. It is sometimes argued that instances of E53 Place are best identified by global coordinates or absolute reference systems. However, relative references are often more relevant in the context of cultural documentation and tend to be more precise. In particular, we are often interested in position in relation to large, mobile objects, such as ships. For example, the Place at which Nelson died is known with reference to a large mobile object, H.M.S Victory. A resolution of this Place in terms of absolute coordinates would require knowledge of the movements of the vessel and the precise time of death, either of which may be revised, and the result would lack historical and cultural relevance.  Any object can serve as a frame of reference for E53 Place determination. The model foresees the notion of a section of an E19 Physical Object as a valid E53 Place determination. {@en}" .


###  http://www.ontologydesignpatterns.org/cp/owl/move.owl#consistsOf
<http://www.ontologydesignpatterns.org/cp/owl/move.owl#consistsOf> rdf:type owl:NamedIndividual ,
                                                                            odin:ODPElement ;
                                                                   odin:describedIn odin:consistsOf_Descr ;
                                                                   odin:odpType odin:Foundational ;
                                                                   rdfs:comment "This property describes the decomposition of an instance of Move into discrete, subsidiary move.     The sub-moves into which the move is decomposed form a logical whole, although the entire picture may not be completely known, and the sub-moves are constitutive of the general move." .


###  http://www.ontologydesignpatterns.org/cp/owl/move.owl#movedFrom
<http://www.ontologydesignpatterns.org/cp/owl/move.owl#movedFrom> rdf:type owl:NamedIndividual ,
                                                                           odin:ODPElement ;
                                                                  odin:describedIn odin:movedFrom_Descr ;
                                                                  rdfs:comment "This property identifies the starting Place of an Move.     A move will be linked to an origin, such as the move of an artefact from storage to display. A move may be linked to many origins. In this case the move describes the picking up of a set of objects. The area of the move includes the origin, route and destination." .


###  http://www.ontologydesignpatterns.org/cp/owl/move.owl#movedTo
<http://www.ontologydesignpatterns.org/cp/owl/move.owl#movedTo> rdf:type owl:NamedIndividual ,
                                                                         odin:ODPElement ;
                                                                odin:describedIn odin:movedTo_Descr ;
                                                                odin:odpType odin:Foundational ;
                                                                rdfs:comment "This property identifies the destination of a Move.      A move will be linked to a destination, such as the move of an artefact from storage to display. A move may be linked to many terminal instances of E53 Places. In this case the move describes a distribution of a set of objects. The area of the move includes the origin, route and destination." .


###  http://www.ontologydesignpatterns.org/cp/owl/move.owl#tookPlaceAt
<http://www.ontologydesignpatterns.org/cp/owl/move.owl#tookPlaceAt> rdf:type owl:NamedIndividual ,
                                                                             odin:ODPElement ;
                                                                    odin:describedIn odin:tookPlaceAt_Descr ;
                                                                    rdfs:comment "This property describes the spatial location of an instance of a Move.      The related Place should be seen as an approximation of the geographical area within which the phenomena that characterise the move in question occurred. took place at (witnessed) does not convey any meaning other than spatial positioning (generally on the surface of the earth)." .


###  http://www.ontologydesignpatterns.org/cp/owl/objectrole.owl#Object
<http://www.ontologydesignpatterns.org/cp/owl/objectrole.owl#Object> rdf:type owl:NamedIndividual ,
                                                                              odin:ODPElement ;
                                                                     odin:describedIn odin:Object_Descr ;
                                                                     odin:odpType odin:Foundational ;
                                                                     rdfs:comment "Any physical, social, or mental object, or a substance" .


###  http://www.ontologydesignpatterns.org/cp/owl/objectrole.owl#Role
<http://www.ontologydesignpatterns.org/cp/owl/objectrole.owl#Role> rdf:type owl:NamedIndividual ,
                                                                            odin:ODPElement ;
                                                                   odin:describedIn odin:Role_Descr ;
                                                                   rdfs:comment "A Concept that classifies an Object" .


###  http://www.ontologydesignpatterns.org/cp/owl/objectrole.owl#hasRole
<http://www.ontologydesignpatterns.org/cp/owl/objectrole.owl#hasRole> rdf:type owl:NamedIndividual ,
                                                                               odin:ODPElement ;
                                                                      odin:describedIn odin:hasRole_Descr ;
                                                                      odin:odpType odin:Foundational ;
                                                                      rdfs:comment "A relation between an object and a role, e.g. the person 'John' has role 'student'." .


###  http://www.ontologydesignpatterns.org/cp/owl/objectrole.owl#isRoleOf
<http://www.ontologydesignpatterns.org/cp/owl/objectrole.owl#isRoleOf> rdf:type owl:NamedIndividual ,
                                                                                odin:ODPElement ;
                                                                       odin:describedIn odin:isRoleOf_Descr ;
                                                                       rdfs:comment "A relation between an object and a role, e.g. the 'student' is the role of 'John'." .


###  http://www.ontologydesignpatterns.org/cp/owl/observation.owl#Parameter
<http://www.ontologydesignpatterns.org/cp/owl/observation.owl#Parameter> rdf:type owl:NamedIndividual ,
                                                                                  odin:ODPElement ;
                                                                         odin:describedIn odin:Parameter_Descr ;
                                                                         odin:odpType odin:Foundational ;
                                                                         rdfs:comment "The parameters of an observation describe the context and content of the observation. For example in a medical context an observation of a patient may contain a set of symptoms, that are the parameters of that observation." .


###  http://www.ontologydesignpatterns.org/cp/owl/parameter.owl#Concept
<http://www.ontologydesignpatterns.org/cp/owl/parameter.owl#Concept> rdf:type owl:NamedIndividual ,
                                                                              odin:ODPElement ;
                                                                     odin:describedIn odin:Concept_Descr ;
                                                                     rdfs:comment "A concept is a SocialObject, and isDefinedIn a Description .   Once defined, a Concept can be used in other descriptions.   The classifies relation relates concepts to entities at some time" .


###  http://www.ontologydesignpatterns.org/cp/owl/parameter.owl#hasParameter
<http://www.ontologydesignpatterns.org/cp/owl/parameter.owl#hasParameter> rdf:type owl:NamedIndividual ,
                                                                                   odin:ODPElement ;
                                                                          odin:describedIn odin:hasParameter_Descr ;
                                                                          rdfs:comment "A Concept can have a Parameter that constrains the attributes that a classified Entity can have in a certain Situation, e.g. a 4WheelDriver Role definedIn the ItalianTrafficLaw has a MinimumAge parameter on the Amount 16." .


###  http://www.ontologydesignpatterns.org/cp/owl/parameter.owl#hasParameterDataValue
<http://www.ontologydesignpatterns.org/cp/owl/parameter.owl#hasParameterDataValue> rdf:type owl:NamedIndividual ,
                                                                                            odin:ODPElement ;
                                                                                   odin:describedIn odin:hasParameterDataValue_Descr ;
                                                                                   odin:odpType odin:Foundational ;
                                                                                   rdfs:comment "Parametrizes values from a datatype. For example, a Parameter AgeForDriving hasParameterDataValue 18 on datatype xsd:int, in the Italian traffic code. In this example, AgeForDriving isDefinedIn the Norm ItalianTrafficCodeAgeDriving.  More complex parametrization requires workarounds. E.g. AgeRangeForDrugUsage could parametrize data value: 14 to 50 on the datatype: xsd:int. Since complex datatypes are not allowed in OWL1.0, a solution to this can only work by creating two 'sub-parameters': MinimumAgeRangeForDrugUsage (that hasParameterDataValue 14) and MaximumAgeRangeForDrugUsage (that hasParameterDataValue 50), which are components of the main Parameter AgeRangeForDrugUsage.  Ordering on subparameters can be created by using or specializing the object property 'precedes'." .


###  http://www.ontologydesignpatterns.org/cp/owl/parameter.owl#isParameterFor
<http://www.ontologydesignpatterns.org/cp/owl/parameter.owl#isParameterFor> rdf:type owl:NamedIndividual ,
                                                                                     odin:ODPElement ;
                                                                            odin:describedIn odin:isParameterFor_Descr ;
                                                                            odin:odpType odin:Foundational ;
                                                                            rdfs:comment "A Concept can have a Parameter that constrains the attributes that a classified Entity can have in a certain Situation, e.g. a 4WheelDriver Role definedIn the ItalianTrafficLaw has a MinimumAge parameter on the Amount 16." .


###  http://www.ontologydesignpatterns.org/cp/owl/participation.owl#Event
<http://www.ontologydesignpatterns.org/cp/owl/participation.owl#Event> rdf:type owl:NamedIndividual ,
                                                                                odin:ODPElement ;
                                                                       odin:describedIn odin:Event_Descr ;
                                                                       rdfs:comment "In this pattern, it is the cause for the transition." .


###  http://www.ontologydesignpatterns.org/cp/owl/participation.owl#Object
<http://www.ontologydesignpatterns.org/cp/owl/participation.owl#Object> rdf:type owl:NamedIndividual ,
                                                                                 odin:ODPElement ;
                                                                        odin:describedIn odin:Object_Descr ;
                                                                        rdfs:comment "Any physical, social, or mental object, or substance" .


###  http://www.ontologydesignpatterns.org/cp/owl/partof.owl#hasPart
<http://www.ontologydesignpatterns.org/cp/owl/partof.owl#hasPart> rdf:type owl:NamedIndividual ,
                                                                           odin:ODPElement ;
                                                                  odin:describedIn odin:hasPart_Descr ;
                                                                  rdfs:comment "A transitive relation expressing parthood between any entities, e.g. 'the human body has a brain as part'. When specializing this pattern, take care of restricting the domain and range appropriately, since it could be counterintuitive to use this relation arbitrarily, e.g. between animals and planets. For an intransitive partof pattern, see 'componency'." .


###  http://www.ontologydesignpatterns.org/cp/owl/partof.owl#isPartOf
<http://www.ontologydesignpatterns.org/cp/owl/partof.owl#isPartOf> rdf:type owl:NamedIndividual ,
                                                                            odin:ODPElement ;
                                                                   odin:describedIn odin:isPartOf_Descr ;
                                                                   odin:odpType odin:Foundational ;
                                                                   rdfs:comment "A transitive relation expressing parthood between any entities, e.g. 'brain is a part of the human body'. When specializing this pattern, take care of restricting the domain and range appropriately, since it could be counterintuitive to use this relation arbitrarily, e.g. between animals and planets. For an intransitive partof pattern, see 'componency'." .


###  http://www.ontologydesignpatterns.org/cp/owl/persons.owl#NaturalPerson
<http://www.ontologydesignpatterns.org/cp/owl/persons.owl#NaturalPerson> rdf:type owl:NamedIndividual ,
                                                                                  odin:ODPElement ;
                                                                         odin:describedIn odin:NaturalPerson_Descr ;
                                                                         odin:odpType odin:Foundational ;
                                                                         rdfs:comment "A Person in the physical commonsense intuition: 'have you seen that person walking down the street?'" .


###  http://www.ontologydesignpatterns.org/cp/owl/persons.owl#Person
<http://www.ontologydesignpatterns.org/cp/owl/persons.owl#Person> rdf:type owl:NamedIndividual ,
                                                                           odin:ODPElement ;
                                                                  odin:describedIn odin:Person_Descr ;
                                                                  odin:odpType odin:Foundational ;
                                                                  rdfs:comment "Persons in commonsense intuition, which does not apparently distinguish between either natural or social persons." .


###  http://www.ontologydesignpatterns.org/cp/owl/persons.owl#SocialPerson
<http://www.ontologydesignpatterns.org/cp/owl/persons.owl#SocialPerson> rdf:type owl:NamedIndividual ,
                                                                                 odin:ODPElement ;
                                                                        odin:describedIn odin:SocialPerson_Descr ;
                                                                        odin:odpType odin:Foundational ;
                                                                        rdfs:comment "A Person that needs the existence of a specific NaturalPerson in order to act (but the lifetime of the NaturalPerson has only to overlap that of the SocialPerson). The NaturalPerson through which it acts can be also indirectly related, e.g. an organization that acts through another organization, which actsThrough one or more NaturalPerson(s)." .


###  http://www.ontologydesignpatterns.org/cp/owl/persons.owl#actsFor
<http://www.ontologydesignpatterns.org/cp/owl/persons.owl#actsFor> rdf:type owl:NamedIndividual ,
                                                                            odin:ODPElement ;
                                                                   odin:describedIn odin:actsFor_Descr ;
                                                                   rdfs:comment "The relation holding between any Agent, and a SocialPerson. In principle, a SocialPerson requires at least one NaturalPerson in order to act, but this dependency can be 'delegated'; e.g. a university can be acted for by a department, which on its turm is acted for by natural persons." .


###  http://www.ontologydesignpatterns.org/cp/owl/persons.owl#actsThrough
<http://www.ontologydesignpatterns.org/cp/owl/persons.owl#actsThrough> rdf:type owl:NamedIndividual ,
                                                                                odin:ODPElement ;
                                                                       odin:describedIn odin:actsThrough_Descr ;
                                                                       odin:odpType odin:Foundational ;
                                                                       rdfs:comment "The relation holding between any Agent, and a SocialPerson. In principle, a SocialPerson requires at least one NaturalPerson in order to act, but this dependency can be 'delegated'; e.g. a university can be acted for by a department, which on its turm is acted for by natural persons." .


###  http://www.ontologydesignpatterns.org/cp/owl/persons.owl#introduces
<http://www.ontologydesignpatterns.org/cp/owl/persons.owl#introduces> rdf:type owl:NamedIndividual ,
                                                                               odin:ODPElement ;
                                                                      odin:describedIn odin:introduces_Descr ;
                                                                      odin:odpType odin:Foundational ;
                                                                      rdfs:comment "A relation between a Description and a SocialPerson, e.g. a Constitutional Charter that introduces the SocialPerson 'PresidentOfRepublic'." .


###  http://www.ontologydesignpatterns.org/cp/owl/persons.owl#isIntroducedBy
<http://www.ontologydesignpatterns.org/cp/owl/persons.owl#isIntroducedBy> rdf:type owl:NamedIndividual ,
                                                                                   odin:ODPElement ;
                                                                          odin:describedIn odin:isIntroducedBy_Descr ;
                                                                          odin:odpType odin:Foundational ;
                                                                          rdfs:comment "A relation between a Description and a SocialPerson, e.g. a Constitutional Charter that introduces the SocialPerson 'PresidentOfRepublic'." .


###  http://www.ontologydesignpatterns.org/cp/owl/place.owl#Place
<http://www.ontologydesignpatterns.org/cp/owl/place.owl#Place> rdf:type owl:NamedIndividual ,
                                                                        odin:ODPElement ;
                                                               odin:describedIn odin:Place_Descr ;
                                                               rdfs:comment "A location, in a very generic sense: a political geographic entity (Roma, Lesotho), a location determined by the presence of other entities ('the area close to Roma'), pivot events or signs (the area where the helicopter fell), complements of other entities ('the area under the table'), as well as physical objects conceptualized as locations as their main identity criterion ('the territory of Italy').  In this generic sense, a Place is an 'approximate', relative location. For an 'absolute', abstract location, cf. the pattern spaceregion.owl.  Formally, a Place is defined by the fact of having something located in it; a Place is located in itself." .


###  http://www.ontologydesignpatterns.org/cp/owl/place.owl#hasLocation
<http://www.ontologydesignpatterns.org/cp/owl/place.owl#hasLocation> rdf:type owl:NamedIndividual ,
                                                                              odin:ODPElement ;
                                                                     odin:describedIn odin:hasLocation_Descr ;
                                                                     odin:odpType odin:Foundational ;
                                                                     rdfs:comment "A generic, relative localization, holding between any entities. E.g. 'the cat is on the mat', 'Omar is in Samarcanda', 'the wound is close to the femural artery'.  For 'absolute' locations, see SpaceRegion" .


###  http://www.ontologydesignpatterns.org/cp/owl/place.owl#isLocationOf
<http://www.ontologydesignpatterns.org/cp/owl/place.owl#isLocationOf> rdf:type owl:NamedIndividual ,
                                                                               odin:ODPElement ;
                                                                      odin:describedIn odin:isLocationOf_Descr ;
                                                                      odin:odpType odin:Foundational ;
                                                                      rdfs:comment "A generic, relative localization, holding between any entities. E.g. 'Rome is the seat of the Pope', 'the liver is the location of the tumor'.  As a very general notion of localization, it is assumed as transitive.  For 'absolute' locations, see SpaceRegion" .


###  http://www.ontologydesignpatterns.org/cp/owl/price.owl#Currency
<http://www.ontologydesignpatterns.org/cp/owl/price.owl#Currency> rdf:type owl:NamedIndividual ,
                                                                           odin:ODPElement ;
                                                                  odin:describedIn odin:Currency_Descr ;
                                                                  rdfs:comment "A system of money in general use in a particular country." .


###  http://www.ontologydesignpatterns.org/cp/owl/price.owl#Price
<http://www.ontologydesignpatterns.org/cp/owl/price.owl#Price> rdf:type owl:NamedIndividual ,
                                                                        odin:ODPElement ;
                                                               odin:describedIn odin:Price_Descr ;
                                                               rdfs:comment "The amount of money expected, required, or given in payment for something." .


###  http://www.ontologydesignpatterns.org/cp/owl/recurrenteventseries.owl#RecurrentEventSeries
<http://www.ontologydesignpatterns.org/cp/owl/recurrenteventseries.owl#RecurrentEventSeries> rdf:type owl:NamedIndividual ,
                                                                                                      odin:ODPElement ;
                                                                                             odin:describedIn odin:RecurrentEventSeries_Descr ;
                                                                                             odin:odpType odin:Foundational ;
                                                                                             rdfs:comment "Recurrent event series is modeled as an intersection of the classes Collection and :Situation. Indeed, a recurrent event is seen as a collection, since it contains entities that share one or more common properties and are unified conceptually. These entities are member of the collection, and are all consecutive events, in such a manner that each event has either a previous event, or a next event, or both. At the same time, a recurrent event is a situation, intended as a relational context in which the contextualized things are based on a frame: a recurrent event is similar to a plan that defines how the things involved in that plan (i.e. the specific events) shall be carried out, e.g. where the events shall be located, in which time of the year, etc." .


###  http://www.ontologydesignpatterns.org/cp/owl/recurrenteventseries.owl#TimePeriod
<http://www.ontologydesignpatterns.org/cp/owl/recurrenteventseries.owl#TimePeriod> rdf:type owl:NamedIndividual ,
                                                                                            odin:ODPElement ;
                                                                                   odin:describedIn odin:TimePeriod_Descr ;
                                                                                   odin:odpType odin:Foundational ;
                                                                                   rdfs:comment "This class represents a Time Period (e.g. 1 week)." .


###  http://www.ontologydesignpatterns.org/cp/owl/recurrenteventseries.owl#UnifyingFactor
<http://www.ontologydesignpatterns.org/cp/owl/recurrenteventseries.owl#UnifyingFactor> rdf:type owl:NamedIndividual ,
                                                                                                odin:ODPElement ;
                                                                                       odin:describedIn odin:UnifyingFactor_Descr ;
                                                                                       odin:odpType odin:Foundational ;
                                                                                       rdfs:comment "A Unifying Factor is an element or property occurring in each event member of a recurrent event series, which unifies the collection and makes all the events attributable to a homogeneous collection." .


###  http://www.ontologydesignpatterns.org/cp/owl/recurrenteventseries.owl#hasTimePeriod
<http://www.ontologydesignpatterns.org/cp/owl/recurrenteventseries.owl#hasTimePeriod> rdf:type owl:NamedIndividual ,
                                                                                               odin:ODPElement ;
                                                                                      odin:describedIn odin:hasTimePeriod_Descr ;
                                                                                      rdfs:comment "This property relates a recurrent event series to a time period." .


###  http://www.ontologydesignpatterns.org/cp/owl/recurrenteventseries.owl#hasTimePeriodBeforeNextEvent
<http://www.ontologydesignpatterns.org/cp/owl/recurrenteventseries.owl#hasTimePeriodBeforeNextEvent> rdf:type owl:NamedIndividual ,
                                                                                                              odin:ODPElement ;
                                                                                                     odin:describedIn odin:hasTimePeriodBeforeNextEvent_Descr ;
                                                                                                     odin:odpType odin:Foundational ;
                                                                                                     rdfs:comment "This property relates an event member of a recurrent event series to the time period elapsing before its next event." .


###  http://www.ontologydesignpatterns.org/cp/owl/recurrenteventseries.owl#hasUnifyingFactor
<http://www.ontologydesignpatterns.org/cp/owl/recurrenteventseries.owl#hasUnifyingFactor> rdf:type owl:NamedIndividual ,
                                                                                                   odin:ODPElement ;
                                                                                          odin:describedIn odin:hasUnifyingFactor_Descr ;
                                                                                          odin:odpType odin:Foundational ;
                                                                                          rdfs:comment "This property relates a recurrent event series to a unifying factor." .


###  http://www.ontologydesignpatterns.org/cp/owl/recurrenteventseries.owl#isLocallyInconsistentWith
<http://www.ontologydesignpatterns.org/cp/owl/recurrenteventseries.owl#isLocallyInconsistentWith> rdf:type owl:NamedIndividual ,
                                                                                                           odin:ODPElement ;
                                                                                                  odin:describedIn odin:isLocallyInconsistentWith_Descr ;
                                                                                                  rdfs:comment "This property relates two entities that are considered locally inconsistent." .


###  http://www.ontologydesignpatterns.org/cp/owl/recurrenteventseries.owl#isTimePeriodBeforeNextEventOf
<http://www.ontologydesignpatterns.org/cp/owl/recurrenteventseries.owl#isTimePeriodBeforeNextEventOf> rdf:type owl:NamedIndividual ,
                                                                                                               odin:ODPElement ;
                                                                                                      odin:describedIn odin:isTimePeriodBeforeNextEventOf_Descr ;
                                                                                                      rdfs:comment "This property relates a time period, elapsing before the next event of an event member of a recurrent event series, to one of the member events." .


###  http://www.ontologydesignpatterns.org/cp/owl/recurrenteventseries.owl#isTimePeriodOf
<http://www.ontologydesignpatterns.org/cp/owl/recurrenteventseries.owl#isTimePeriodOf> rdf:type owl:NamedIndividual ,
                                                                                                odin:ODPElement ;
                                                                                       odin:describedIn odin:isTimePeriodOf_Descr ;
                                                                                       rdfs:comment "This property relates a time period to a recurrent event series having that time period." .


###  http://www.ontologydesignpatterns.org/cp/owl/recurrenteventseries.owl#isUnifyingFactorOf
<http://www.ontologydesignpatterns.org/cp/owl/recurrenteventseries.owl#isUnifyingFactorOf> rdf:type owl:NamedIndividual ,
                                                                                                    odin:ODPElement ;
                                                                                           odin:describedIn odin:isUnifyingFactorOf_Descr ;
                                                                                           rdfs:comment "This property relates a unifying factor to the recurrent event series that is unified by that factor." .


###  http://www.ontologydesignpatterns.org/cp/owl/region.owl#Region
<http://www.ontologydesignpatterns.org/cp/owl/region.owl#Region> rdf:type owl:NamedIndividual ,
                                                                          odin:ODPElement ;
                                                                 odin:describedIn odin:Region_Descr ;
                                                                 odin:odpType odin:Foundational ;
                                                                 rdfs:comment "Any region in a dimensional space (a dimensional space is a maximal Region), which can be used as a value for a quality of an Entity . For example, TimeInterval, SpaceRegion, PhysicalAttribute, Amount, SocialAttribute are all subclasses of Region.   Regions are not data values in the ordinary knowledge representation sense; in order to get patterns for modelling data, see the properties: representsDataValue and hasDataValue" .


###  http://www.ontologydesignpatterns.org/cp/owl/region.owl#hasRegion
<http://www.ontologydesignpatterns.org/cp/owl/region.owl#hasRegion> rdf:type owl:NamedIndividual ,
                                                                             odin:ODPElement ;
                                                                    odin:describedIn odin:hasRegion_Descr ;
                                                                    rdfs:comment "A relation between entities and regions, e.g. 'the number of wheels of that truck is 12'." .


###  http://www.ontologydesignpatterns.org/cp/owl/region.owl#hasRegionDataValue
<http://www.ontologydesignpatterns.org/cp/owl/region.owl#hasRegionDataValue> rdf:type owl:NamedIndividual ,
                                                                                      odin:ODPElement ;
                                                                             odin:describedIn odin:hasRegionDataValue_Descr ;
                                                                             odin:odpType odin:Foundational ;
                                                                             rdfs:comment "A datatype property that encodes values for a Region, e.g. a float for the Region Height." .


###  http://www.ontologydesignpatterns.org/cp/owl/region.owl#isRegionFor
<http://www.ontologydesignpatterns.org/cp/owl/region.owl#isRegionFor> rdf:type owl:NamedIndividual ,
                                                                               odin:ODPElement ;
                                                                      odin:describedIn odin:isRegionFor_Descr ;
                                                                      rdfs:comment "A relation between entities and regions, e.g. 'the color of my car is red'." .


###  http://www.ontologydesignpatterns.org/cp/owl/sequence.owl#directlyFollows
<http://www.ontologydesignpatterns.org/cp/owl/sequence.owl#directlyFollows> rdf:type owl:NamedIndividual ,
                                                                                     odin:ODPElement ;
                                                                            odin:describedIn odin:directlyFollows_Descr ;
                                                                            odin:odpType odin:Foundational ;
                                                                            rdfs:comment "The intransitive follows relation. For example, Wednesday directly precedes Thursday. Directness of precedence depends on the designer conceptualization." .


###  http://www.ontologydesignpatterns.org/cp/owl/sequence.owl#directlyPrecedes
<http://www.ontologydesignpatterns.org/cp/owl/sequence.owl#directlyPrecedes> rdf:type owl:NamedIndividual ,
                                                                                      odin:ODPElement ;
                                                                             odin:describedIn odin:directlyPrecedes_Descr ;
                                                                             odin:odpType odin:Foundational ;
                                                                             rdfs:comment "The intransitive precedes relation. For example, Monday directly precedes Tuesday. Directness of precedence depends on the designer conceptualization." .


###  http://www.ontologydesignpatterns.org/cp/owl/sequence.owl#follows
<http://www.ontologydesignpatterns.org/cp/owl/sequence.owl#follows> rdf:type owl:NamedIndividual ,
                                                                             odin:ODPElement ;
                                                                    odin:describedIn odin:follows_Descr ;
                                                                    rdfs:comment "A relation between entities, expressing a 'sequence' schema.   E.g. 'year 2000 follows 1999', 'preparing coffee' follows 'deciding what coffee to use', 'II World War follows I World War', etc.   It can be used between tasks, processes or time intervals, and subproperties would fit best in order to distinguish the different uses." .


###  http://www.ontologydesignpatterns.org/cp/owl/sequence.owl#precedes
<http://www.ontologydesignpatterns.org/cp/owl/sequence.owl#precedes> rdf:type owl:NamedIndividual ,
                                                                              odin:ODPElement ;
                                                                     odin:describedIn odin:precedes_Descr ;
                                                                     rdfs:comment "A relation between entities, expressing a 'sequence' schema.   E.g. 'year 1999 precedes 2000', 'deciding what coffee to use' precedes 'preparing coffee', 'World War II follows World War I', 'in the Milan to Rome autoroute, Bologna precedes Florence', etc.  It can then be used between tasks, processes, time intervals, spatially locate objects, situations, etc.   Subproperties can be defined in order to distinguish the different uses." .


###  http://www.ontologydesignpatterns.org/cp/owl/set.owl#Set
<http://www.ontologydesignpatterns.org/cp/owl/set.owl#Set> rdf:type owl:NamedIndividual ,
                                                                    odin:ODPElement ;
                                                           odin:describedIn odin:Set_Descr ;
                                                           rdfs:comment "Set - A collection that cannot contain duplicate elements." .


###  http://www.ontologydesignpatterns.org/cp/owl/set.owl#size
<http://www.ontologydesignpatterns.org/cp/owl/set.owl#size> rdf:type owl:NamedIndividual ,
                                                                     odin:ODPElement ;
                                                            odin:describedIn odin:size_Descr ;
                                                            odin:odpType odin:Foundational ;
                                                            rdfs:comment "size - The number of items belonging to a collection" .


###  http://www.ontologydesignpatterns.org/cp/owl/situation.owl#hasSetting
<http://www.ontologydesignpatterns.org/cp/owl/situation.owl#hasSetting> rdf:type owl:NamedIndividual ,
                                                                                 odin:ODPElement ;
                                                                        odin:describedIn odin:hasSetting_Descr ;
                                                                        odin:odpType odin:Foundational ;
                                                                        rdfs:comment "A relation between entities and situations, e.g. 'this morning I've prepared my coffee with a new fantastic Arabica' (i.e.: (an amount of) a new fantastic Arabica hasSetting the preparation of my coffee this morning)." .


###  http://www.ontologydesignpatterns.org/cp/owl/taskexecution.owl#executesTask
<http://www.ontologydesignpatterns.org/cp/owl/taskexecution.owl#executesTask> rdf:type owl:NamedIndividual ,
                                                                                       odin:ODPElement ;
                                                                              odin:describedIn odin:executesTask_Descr ;
                                                                              odin:odpType odin:Foundational ;
                                                                              rdfs:comment "A relation between an action and a task, e.g. 'putting some water in a pot and putting the pot on a fire until the water starts bubbling' executes the task 'boiling'." .


###  http://www.ontologydesignpatterns.org/cp/owl/taskexecution.owl#isExecutedIn
<http://www.ontologydesignpatterns.org/cp/owl/taskexecution.owl#isExecutedIn> rdf:type owl:NamedIndividual ,
                                                                                       odin:ODPElement ;
                                                                              odin:describedIn odin:isExecutedIn_Descr ;
                                                                              odin:odpType odin:Foundational ;
                                                                              rdfs:comment "A relation between an action and a task, e.g. 'putting some water in a pot and putting the pot on a fire until the water starts bubbling' executes the task 'boiling'." .


###  http://www.ontologydesignpatterns.org/cp/owl/taskrole.owl#Role
<http://www.ontologydesignpatterns.org/cp/owl/taskrole.owl#Role> rdf:type owl:NamedIndividual ,
                                                                          odin:ODPElement ;
                                                                 odin:describedIn odin:Role_Descr ;
                                                                 odin:odpType odin:Foundational ;
                                                                 rdfs:comment "A concept that classifies an object. For example, the role developer classifies a person, the role server classifies a computer machine. A hasTask only Tasks." .


###  http://www.ontologydesignpatterns.org/cp/owl/taskrole.owl#Task
<http://www.ontologydesignpatterns.org/cp/owl/taskrole.owl#Task> rdf:type owl:NamedIndividual ,
                                                                          odin:ODPElement ;
                                                                 odin:describedIn odin:Task_Descr ;
                                                                 odin:odpType odin:Foundational ;
                                                                 rdfs:comment "A piece of work to be done or undertaken. A Task is assigned to only Roles through the property isTaskOf." .


###  http://www.ontologydesignpatterns.org/cp/owl/taskrole.owl#hasTask
<http://www.ontologydesignpatterns.org/cp/owl/taskrole.owl#hasTask> rdf:type owl:NamedIndividual ,
                                                                             odin:ODPElement ;
                                                                    odin:describedIn odin:hasTask_Descr ;
                                                                    odin:odpType odin:Foundational ;
                                                                    rdfs:comment "A relation between roles and tasks, e.g. 'students have the duty of giving exams' (i.e. the Role 'student' hasTask the Task 'giving exams')." .


###  http://www.ontologydesignpatterns.org/cp/owl/taskrole.owl#isTaskOf
<http://www.ontologydesignpatterns.org/cp/owl/taskrole.owl#isTaskOf> rdf:type owl:NamedIndividual ,
                                                                              odin:ODPElement ;
                                                                     odin:describedIn odin:isTaskOf_Descr ;
                                                                     odin:odpType odin:Foundational ;
                                                                     rdfs:comment "A relation between roles and tasks, e.g. 'students have the duty of giving exams' (i.e. the Role 'student' hasTask the Task 'giving exams')." .


###  http://www.ontologydesignpatterns.org/cp/owl/timeindexedclassification.owl#TimeIndexedClassification
<http://www.ontologydesignpatterns.org/cp/owl/timeindexedclassification.owl#TimeIndexedClassification> rdf:type owl:NamedIndividual ,
                                                                                                                odin:ODPElement ;
                                                                                                       odin:describedIn odin:TimeIndexedClassification_Descr ;
                                                                                                       odin:odpType odin:Foundational ;
                                                                                                       rdfs:comment "A Situation to represent classification ('counting as') of an entity at some time." .


###  http://www.ontologydesignpatterns.org/cp/owl/timeindexedparticipation.owl#TimeIndexedParticipation
<http://www.ontologydesignpatterns.org/cp/owl/timeindexedparticipation.owl#TimeIndexedParticipation> rdf:type owl:NamedIndividual ,
                                                                                                              odin:ODPElement ;
                                                                                                     odin:describedIn odin:TimeIndexedParticipation_Descr ;
                                                                                                     odin:odpType odin:Foundational ;
                                                                                                     rdfs:comment "A Situation that represents participation of Object(s) in Event(s) at some Time." .


###  http://www.ontologydesignpatterns.org/cp/owl/timeindexedparticipation.owl#includesEvent
<http://www.ontologydesignpatterns.org/cp/owl/timeindexedparticipation.owl#includesEvent> rdf:type owl:NamedIndividual ,
                                                                                                   odin:ODPElement ;
                                                                                          odin:describedIn odin:includesEvent_Descr ;
                                                                                          odin:odpType odin:Foundational ;
                                                                                          rdfs:comment "A relation between situations and events, e.g. 'this morning I've prepared my coffee and had my fingers burnt' (i.e.: the preparation of my coffee this morning included a burning of my fingers)." .


###  http://www.ontologydesignpatterns.org/cp/owl/timeindexedparticipation.owl#includesObject
<http://www.ontologydesignpatterns.org/cp/owl/timeindexedparticipation.owl#includesObject> rdf:type owl:NamedIndividual ,
                                                                                                    odin:ODPElement ;
                                                                                           odin:describedIn odin:includesObject_Descr ;
                                                                                           odin:odpType odin:Foundational ;
                                                                                           rdfs:comment "A relation between situations and objects, e.g. 'this morning I've prepared my coffee and had my fingers burnt' (i.e.: the preparation of my coffee this morning included me)." .


###  http://www.ontologydesignpatterns.org/cp/owl/timeindexedpartof.owl#Object
<http://www.ontologydesignpatterns.org/cp/owl/timeindexedpartof.owl#Object> rdf:type owl:NamedIndividual ,
                                                                                     odin:ODPElement ;
                                                                            odin:describedIn odin:Object_Descr ;
                                                                            odin:odpType odin:Foundational ;
                                                                            rdfs:comment "Any physical, social, or mental object, or a substance" .


###  http://www.ontologydesignpatterns.org/cp/owl/timeindexedpartof.owl#TimeIndexedPartOf
<http://www.ontologydesignpatterns.org/cp/owl/timeindexedpartof.owl#TimeIndexedPartOf> rdf:type owl:NamedIndividual ,
                                                                                                odin:ODPElement ;
                                                                                       odin:describedIn odin:TimeIndexedPartOf_Descr ;
                                                                                       odin:odpType odin:Foundational ;
                                                                                       rdfs:comment "A situation that includes at least two Objects, one having the role of whole object, the other(s) being a part(s) of it, and one TimeInterval." .


###  http://www.ontologydesignpatterns.org/cp/owl/timeindexedpartof.owl#includesPartObject
<http://www.ontologydesignpatterns.org/cp/owl/timeindexedpartof.owl#includesPartObject> rdf:type owl:NamedIndividual ,
                                                                                                 odin:ODPElement ;
                                                                                        odin:describedIn odin:includesPartObject_Descr ;
                                                                                        odin:odpType odin:Foundational ;
                                                                                        rdfs:comment "A relation between a temporary part-of situation and the part(s) involved." .


###  http://www.ontologydesignpatterns.org/cp/owl/timeindexedpartof.owl#includesWholeObject
<http://www.ontologydesignpatterns.org/cp/owl/timeindexedpartof.owl#includesWholeObject> rdf:type owl:NamedIndividual ,
                                                                                                  odin:ODPElement ;
                                                                                         odin:describedIn odin:includesWholeObject_Descr ;
                                                                                         odin:odpType odin:Foundational ;
                                                                                         rdfs:comment "A relation between a temporary part-of situation and the whole object involved." .


###  http://www.ontologydesignpatterns.org/cp/owl/timeindexedpartof.owl#isPartObjectOf
<http://www.ontologydesignpatterns.org/cp/owl/timeindexedpartof.owl#isPartObjectOf> rdf:type owl:NamedIndividual ,
                                                                                             odin:ODPElement ;
                                                                                    odin:describedIn odin:isPartObjectOf_Descr ;
                                                                                    rdfs:comment "A relation between object part(s) and the temporary part-of situation they are involved in." .


###  http://www.ontologydesignpatterns.org/cp/owl/timeindexedpartof.owl#isWholeObjectOf
<http://www.ontologydesignpatterns.org/cp/owl/timeindexedpartof.owl#isWholeObjectOf> rdf:type owl:NamedIndividual ,
                                                                                              odin:ODPElement ;
                                                                                     odin:describedIn odin:isWholeObjectOf_Descr ;
                                                                                     rdfs:comment "A relation between a whole object and the temporary part-of situation it is involved in." .


###  http://www.ontologydesignpatterns.org/cp/owl/timeindexedpersonrole.owl#Person
<http://www.ontologydesignpatterns.org/cp/owl/timeindexedpersonrole.owl#Person> rdf:type owl:NamedIndividual ,
                                                                                         odin:ODPElement ;
                                                                                odin:describedIn odin:Person_Descr ;
                                                                                odin:odpType odin:Foundational ;
                                                                                rdfs:comment "Persons in commonsense intuition, i.e. either as physical agents (humans) or social persons." .


###  http://www.ontologydesignpatterns.org/cp/owl/timeindexedpersonrole.owl#TimeIndexedPersonRole
<http://www.ontologydesignpatterns.org/cp/owl/timeindexedpersonrole.owl#TimeIndexedPersonRole> rdf:type owl:NamedIndividual ,
                                                                                                        odin:ODPElement ;
                                                                                               odin:describedIn odin:TimeIndexedPersonRole_Descr ;
                                                                                               odin:odpType odin:Foundational ;
                                                                                               rdfs:comment "A situation that expresses time indexing for the relation between persons and roles they play." .


###  http://www.ontologydesignpatterns.org/cp/owl/timeindexedsituation.owl#TimeIndexedSituation
<http://www.ontologydesignpatterns.org/cp/owl/timeindexedsituation.owl#TimeIndexedSituation> rdf:type owl:NamedIndividual ,
                                                                                                      odin:ODPElement ;
                                                                                             odin:describedIn odin:TimeIndexedSituation_Descr ;
                                                                                             rdfs:comment "A Situation that is explicitly indexed at some time for at least one entity." .


###  http://www.ontologydesignpatterns.org/cp/owl/timeinterval.owl#TimeInterval
<http://www.ontologydesignpatterns.org/cp/owl/timeinterval.owl#TimeInterval> rdf:type owl:NamedIndividual ,
                                                                                      odin:ODPElement ;
                                                                             odin:describedIn odin:TimeInterval_Descr ;
                                                                             rdfs:comment "Any Region in a dimensional space that aims at representing time.  It should be used when you want to talk about time as an object having some characteristics." .


###  http://www.ontologydesignpatterns.org/cp/owl/timeinterval.owl#hasIntervalEndDate
<http://www.ontologydesignpatterns.org/cp/owl/timeinterval.owl#hasIntervalEndDate> rdf:type owl:NamedIndividual ,
                                                                                            odin:ODPElement ;
                                                                                   odin:describedIn odin:hasIntervalEndDate_Descr ;
                                                                                   odin:odpType odin:Foundational ;
                                                                                   rdfs:comment "The end date of a time interval." .


###  http://www.ontologydesignpatterns.org/cp/owl/timeperiod.owl#TimePeriod
<http://www.ontologydesignpatterns.org/cp/owl/timeperiod.owl#TimePeriod> rdf:type owl:NamedIndividual ,
                                                                                  odin:ODPElement ;
                                                                         odin:describedIn odin:TimePeriod_Descr ;
                                                                         odin:odpType odin:Foundational ;
                                                                         rdfs:comment "A Time Period is a temporal distance, even approximated, that elapses between two events or situations." .


###  http://www.ontologydesignpatterns.org/cp/owl/timeperiod.owl#TimePeriodMeasurementUnit
<http://www.ontologydesignpatterns.org/cp/owl/timeperiod.owl#TimePeriodMeasurementUnit> rdf:type owl:NamedIndividual ,
                                                                                                 odin:ODPElement ;
                                                                                        odin:describedIn odin:TimePeriodMeasurementUnit_Descr ;
                                                                                        rdfs:comment "The Time Period Measurement Unit is the unit for measuring a Time Period (e.g. year, month, week)." .


###  http://www.ontologydesignpatterns.org/cp/owl/timeperiod.owl#hasTimePeriodMeasurementUnit
<http://www.ontologydesignpatterns.org/cp/owl/timeperiod.owl#hasTimePeriodMeasurementUnit> rdf:type owl:NamedIndividual ,
                                                                                                    odin:ODPElement ;
                                                                                           odin:describedIn odin:hasTimePeriodMeasurementUnit_Descr ;
                                                                                           rdfs:comment "This property relates a time period to its measurement unit." .


###  http://www.ontologydesignpatterns.org/cp/owl/timeperiod.owl#isTimePeriodMeasurementUnitOf
<http://www.ontologydesignpatterns.org/cp/owl/timeperiod.owl#isTimePeriodMeasurementUnitOf> rdf:type owl:NamedIndividual ,
                                                                                                     odin:ODPElement ;
                                                                                            odin:describedIn odin:isTimePeriodMeasurementUnitOf_Descr ;
                                                                                            odin:odpType odin:Foundational ;
                                                                                            rdfs:comment "This property relates the measurement unit to the time period." .


###  http://www.ontologydesignpatterns.org/cp/owl/timeperiod.owl#timePeriodValue
<http://www.ontologydesignpatterns.org/cp/owl/timeperiod.owl#timePeriodValue> rdf:type owl:NamedIndividual ,
                                                                                       odin:ODPElement ;
                                                                              odin:describedIn odin:timePeriodValue_Descr ;
                                                                              rdfs:comment "This property represents the value of a time period." .


###  http://www.ontologydesignpatterns.org/cp/owl/topic.owl#Concept
<http://www.ontologydesignpatterns.org/cp/owl/topic.owl#Concept> rdf:type owl:NamedIndividual ,
                                                                          odin:ODPElement ;
                                                                 odin:describedIn odin:Concept_Descr ;
                                                                 rdfs:comment "A Concept is a social object, which is used to classify entities. Differently from a Topic  Both concepts and topics are used to classify entities, but concepts typically have an is a relation to the entities; e.g.   (1) A biography of Brigitte Bardot hasTopic 'star system' (Topic)  (2) A biography of Brigitte Bardot is a Biography (Concept)  (3) A biography of Claude Chabrol hasTopic 'Nouvelle Vague' (Topic)  (4) The Nouvelle Vague is a CulturalMovement (Concept)" .


###  http://www.ontologydesignpatterns.org/cp/owl/topic.owl#Topic
<http://www.ontologydesignpatterns.org/cp/owl/topic.owl#Topic> rdf:type owl:NamedIndividual ,
                                                                        odin:ODPElement ;
                                                               odin:describedIn odin:Topic_Descr ;
                                                               rdfs:comment "A topic, or subject, argument, domain, theme, subject area, etc.  Topics have a controversial intuition across common sense, document management systems, knowledge organization systems, etc.     There is an interesting duality of topics: they are commonly interpreted as areas of shared knowledge within a Community (therefore as collections of social objects). On the other hand, existing directories and thesauri use 'topic' (or 'subject') more restrictively, as a relation between a document and a concept.      For example, thesauri do not usually distinguish when their 'concepts' (cf. skos:Concept) are actually intended as concepts (in the sense of Concept in this pattern) and when they are intended as topics. The distinction is clear when you compare these two sample sentences: 'the football topic is part of the sport topic' vs. 'the concept of football is part of the concept of sport'.   While the first is perfectly acceptable, the second is counterintuitive and even possibly wrong. This effect is due to the fact that concepts are 'intensional' notions and are not intended as areas of knowledge, document spaces, etc., which are 'extensional' notions.     Accordingly to these basic observations, in this pattern Concept and Topic result to be disjoint, and an appropriate representation should be in place in order to model thesauri. E.g. skos:Concept should be mapped to the union of Concept and Topic." .


###  http://www.ontologydesignpatterns.org/cp/owl/topic.owl#farTopicFrom
<http://www.ontologydesignpatterns.org/cp/owl/topic.owl#farTopicFrom> rdf:type owl:NamedIndividual ,
                                                                               odin:ODPElement ;
                                                                      odin:describedIn odin:farTopicFrom_Descr ;
                                                                      rdfs:comment "The opposite to vicinity relation between two topics, e.g. 'star system' (as a Topic) is farTopicFrom 'geology' (as a Topic).  Distance is typically established with reference to a threshold on the number of concepts or entities that are common between the two topics. Alternatively, it can be established with reference to the a geometrical semantics applied to the spaces (super-topics) of which topics are part (cf. ontopic.owl ontology)." .


###  http://www.ontologydesignpatterns.org/cp/owl/topic.owl#hasCoreConcept
<http://www.ontologydesignpatterns.org/cp/owl/topic.owl#hasCoreConcept> rdf:type owl:NamedIndividual ,
                                                                                 odin:ODPElement ;
                                                                        odin:describedIn odin:hasCoreConcept_Descr ;
                                                                        odin:odpType odin:Foundational ;
                                                                        rdfs:comment "A Concept is a core concept for a Topic when it can classify many entities that have that Topic.  For example, Saxophone (as a Concept) isCoreConceptFor Saxophones (as a Topic)." .


###  http://www.ontologydesignpatterns.org/cp/owl/topic.owl#hasSubTopic
<http://www.ontologydesignpatterns.org/cp/owl/topic.owl#hasSubTopic> rdf:type owl:NamedIndividual ,
                                                                              odin:ODPElement ;
                                                                     odin:describedIn odin:hasSubTopic_Descr ;
                                                                     rdfs:comment "The relation between two instances of a Topic, in terms of their cultural coverage. For example, Sport hasSubTopic Football.   It can be used widely to talk about document annotations, subject directories, etc." .


###  http://www.ontologydesignpatterns.org/cp/owl/topic.owl#hasTopic
<http://www.ontologydesignpatterns.org/cp/owl/topic.owl#hasTopic> rdf:type owl:NamedIndividual ,
                                                                           odin:ODPElement ;
                                                                  odin:describedIn odin:hasTopic_Descr ;
                                                                  odin:odpType odin:Foundational ;
                                                                  rdfs:comment "The relation between something and its Topic (subject, argument, domain, theme, subject area, etc.). It can be used widely to talk about document annotations, subject directories, etc.  hasTopic is very general. For example, consider the following cases:  (1) A biography of Brigitte Bardot hasTopic 'star system'  (2) The concept of 'starlet' hasTopic 'cinema'  (3) A biography of Claude Chabrol hasTopic 'Nouvelle Vague'." .


###  http://www.ontologydesignpatterns.org/cp/owl/topic.owl#isCoreConceptFor
<http://www.ontologydesignpatterns.org/cp/owl/topic.owl#isCoreConceptFor> rdf:type owl:NamedIndividual ,
                                                                                   odin:ODPElement ;
                                                                          odin:describedIn odin:isCoreConceptFor_Descr ;
                                                                          rdfs:comment "A Concept is a core concept for a Topic when it can classify many entities that have that Topic.  For example, Saxophone (as a Concept) isCoreConceptFor Saxophones (as a Topic)." .


###  http://www.ontologydesignpatterns.org/cp/owl/topic.owl#isSubTopicOf
<http://www.ontologydesignpatterns.org/cp/owl/topic.owl#isSubTopicOf> rdf:type owl:NamedIndividual ,
                                                                               odin:ODPElement ;
                                                                      odin:describedIn odin:isSubTopicOf_Descr ;
                                                                      rdfs:comment "The relation between two Topic(s), in terms of their cultural coverage. For example, Football isSubTopicOf Sport.   It can be used widely to talk about document annotations, subject directories, etc." .


###  http://www.ontologydesignpatterns.org/cp/owl/topic.owl#isTopicOf
<http://www.ontologydesignpatterns.org/cp/owl/topic.owl#isTopicOf> rdf:type owl:NamedIndividual ,
                                                                            odin:ODPElement ;
                                                                   odin:describedIn odin:isTopicOf_Descr ;
                                                                   rdfs:comment "The relation between something and its Topic (subject, argument, domain, theme, subject area, etc.). It can be used widely to talk about document annotations, subject directories, etc.  hasTopic is very general. For example, consider the following cases:  (1) A biography of Brigitte Bardot hasTopic 'star system'  (2) The concept of 'starlet' hasTopic 'cinema'  (3) A biography of Claude Chabrol hasTopic 'Nouvelle Vague'." .


###  http://www.ontologydesignpatterns.org/cp/owl/topic.owl#nearTopicTo
<http://www.ontologydesignpatterns.org/cp/owl/topic.owl#nearTopicTo> rdf:type owl:NamedIndividual ,
                                                                              odin:ODPElement ;
                                                                     odin:describedIn odin:nearTopicTo_Descr ;
                                                                     odin:odpType odin:Foundational ;
                                                                     rdfs:comment "The vicinity relation between two topics, e.g. 'star system' (as a Topic) is nearTopicTo 'cinema' (as a Topic).  Vicinity is typically established with reference to a threshold on the number of concepts or entities that are common to the two Topic(s), or based on a geometrical semantics applied to the spaces common between two topics (cf. ontopic.owl ontology)." .


###  http://www.ontologydesignpatterns.org/cp/owl/topic.owl#overlappingTopic
<http://www.ontologydesignpatterns.org/cp/owl/topic.owl#overlappingTopic> rdf:type owl:NamedIndividual ,
                                                                                   odin:ODPElement ;
                                                                          odin:describedIn odin:overlappingTopic_Descr ;
                                                                          rdfs:comment "The relation between two topics, e.g. 'star system' (as a Topic) is overlappingTopic with 'Bollywood movies' (as a Topic).  Overlap is typically established with reference to a threshold on the number of concepts or entities that are common between the two topics. Alternatively, it can be established with reference to the a geometrical semantics applied to the spaces (super-topics) of which topics are part (cf. ontopic.owl ontology)." .


###  http://www.ontologydesignpatterns.org/cp/owl/transition.owl#Process
<http://www.ontologydesignpatterns.org/cp/owl/transition.owl#Process> rdf:type owl:NamedIndividual ,
                                                                               odin:ODPElement ;
                                                                      odin:describedIn odin:Process_Descr ;
                                                                      odin:odpType odin:Foundational ;
                                                                      rdfs:comment "The invariance under some different transitions (including the one represented here), in which at least one Object is situated." .


###  http://www.ontologydesignpatterns.org/cp/owl/transition.owl#Transition
<http://www.ontologydesignpatterns.org/cp/owl/transition.owl#Transition> rdf:type owl:NamedIndividual ,
                                                                                  odin:ODPElement ;
                                                                         odin:describedIn odin:Transition_Descr ;
                                                                         odin:odpType odin:Foundational ;
                                                                         rdfs:comment "A transition is a Situation that creates a context for three TimeInterval(s), two additional different Situation(s), one Event, one Process, and at least one Object: the Event is observed as the cause for the transition, one Situation is the state before the transition, the second Situation is the state after the transition, the Process is the invariance under some different transitions (including the one represented here), in which at least one Object is situated. Finally, the time intervals position the situations and the transitional event in time.  This class of situations partly encodes the ontology underlying typical engineering algebras for processes, e.g. Petri Nets.   A full representation of the transition ontology is outside the expressivity of OWL, because we would need qualified cardinality restrictions, coreference, property equivalence, and property composition." .


###  http://www.ontologydesignpatterns.org/cp/owl/transition.owl#hasFinalStateAtTime
<http://www.ontologydesignpatterns.org/cp/owl/transition.owl#hasFinalStateAtTime> rdf:type owl:NamedIndividual ,
                                                                                           odin:ODPElement ;
                                                                                  odin:describedIn odin:hasFinalStateAtTime_Descr ;
                                                                                  rdfs:comment "The time of the final state of the transition." .


###  http://www.ontologydesignpatterns.org/cp/owl/transition.owl#hasInitialStateAtTime
<http://www.ontologydesignpatterns.org/cp/owl/transition.owl#hasInitialStateAtTime> rdf:type owl:NamedIndividual ,
                                                                                             odin:ODPElement ;
                                                                                    odin:describedIn odin:hasInitialStateAtTime_Descr ;
                                                                                    odin:odpType odin:Foundational ;
                                                                                    rdfs:comment "The time of the initial state in the transition." .


###  http://www.ontologydesignpatterns.org/cp/owl/transition.owl#includesFinalSituation
<http://www.ontologydesignpatterns.org/cp/owl/transition.owl#includesFinalSituation> rdf:type owl:NamedIndividual ,
                                                                                              odin:ODPElement ;
                                                                                     odin:describedIn odin:includesFinalSituation_Descr ;
                                                                                     rdfs:comment "A relation between a transition situation and the situation resulting from the transition." .


###  http://www.ontologydesignpatterns.org/cp/owl/transition.owl#includesProcess
<http://www.ontologydesignpatterns.org/cp/owl/transition.owl#includesProcess> rdf:type owl:NamedIndividual ,
                                                                                       odin:ODPElement ;
                                                                              odin:describedIn odin:includesProcess_Descr ;
                                                                              odin:odpType odin:Foundational ;
                                                                              rdfs:comment "A relation between a transition situation and the underlying process that is invariant for the object(s) included in the transition." .


###  http://www.ontologydesignpatterns.org/cp/owl/transition.owl#isFinalSituationIncludedIn
<http://www.ontologydesignpatterns.org/cp/owl/transition.owl#isFinalSituationIncludedIn> rdf:type owl:NamedIndividual ,
                                                                                                  odin:ODPElement ;
                                                                                         odin:describedIn odin:isFinalSituationIncludedIn_Descr ;
                                                                                         odin:odpType odin:Foundational ;
                                                                                         rdfs:comment "A relation between a transition situation and the situation resulting from the transition." .


###  http://www.ontologydesignpatterns.org/cp/owl/transition.owl#isProcessIncludedIn
<http://www.ontologydesignpatterns.org/cp/owl/transition.owl#isProcessIncludedIn> rdf:type owl:NamedIndividual ,
                                                                                           odin:ODPElement ;
                                                                                  odin:describedIn odin:isProcessIncludedIn_Descr ;
                                                                                  rdfs:comment "A relation between a transition situation and the underlying process that is invariant for the object(s) included in the transition." .


###  http://www.ontologydesignpatterns.org/cp/owl/typesofentities.owl#Abstract
<http://www.ontologydesignpatterns.org/cp/owl/typesofentities.owl#Abstract> rdf:type owl:NamedIndividual ,
                                                                                     odin:ODPElement ;
                                                                            odin:describedIn odin:Abstract_Descr ;
                                                                            rdfs:comment "Any Entity that cannot be located in space-time. E.g. mathematical entities: formal semantics elements, regions within dimensional spaces, etc." .


###  http://www.ontologydesignpatterns.org/cp/owl/typesofentities.owl#Entity
<http://www.ontologydesignpatterns.org/cp/owl/typesofentities.owl#Entity> rdf:type owl:NamedIndividual ,
                                                                                   odin:ODPElement ;
                                                                          odin:describedIn odin:Entity_Descr ;
                                                                          odin:odpType odin:Foundational ;
                                                                          rdfs:comment "Anything: real, possible, or imaginary, which some modeller wants to talk about for some purpose." .


###  http://www.ontologydesignpatterns.org/cp/owl/typesofentities.owl#Object
<http://www.ontologydesignpatterns.org/cp/owl/typesofentities.owl#Object> rdf:type owl:NamedIndividual ,
                                                                                   odin:ODPElement ;
                                                                          odin:describedIn odin:Object_Descr ;
                                                                          odin:odpType odin:Foundational ;
                                                                          rdfs:comment "Any physical, social, or mental object, or a substance" .


###  http://www.ontologydesignpatterns.org/cp/owl/typesofentities.owl#Quality
<http://www.ontologydesignpatterns.org/cp/owl/typesofentities.owl#Quality> rdf:type owl:NamedIndividual ,
                                                                                    odin:ODPElement ;
                                                                           odin:describedIn odin:Quality_Descr ;
                                                                           odin:odpType odin:Foundational ;
                                                                           rdfs:comment "Any aspect of an Entity (but not a part of it), which cannot exist without that Entity. For example, the way the surface of a specific PhysicalObject looks like is a Quality, while the encoding of that quality into e.g. a PhysicalAttribute is a Region" .


###  http://www.ontologydesignpatterns.org/cp/reaction.owl#Action
<http://www.ontologydesignpatterns.org/cp/reaction.owl#Action> rdf:type owl:NamedIndividual ,
                                                                        odin:ODPElement ;
                                                               odin:describedIn odin:Action_Descr ;
                                                               odin:odpType odin:Foundational ;
                                                               rdfs:comment "Action can produce more than a single event. Mutiple events can share the same position in the sequence." .


###  http://www.ontologydesignpatterns.org/cp/reaction.owl#ExternalAgent
<http://www.ontologydesignpatterns.org/cp/reaction.owl#ExternalAgent> rdf:type owl:NamedIndividual ,
                                                                               odin:ODPElement ;
                                                                      odin:describedIn odin:ExternalAgent_Descr ;
                                                                      odin:odpType odin:Foundational ;
                                                                      rdfs:comment "External agents cannot react to anything!" .


###  http://www.ontologydesignpatterns.org/cp/reaction.owl#Reaction
<http://www.ontologydesignpatterns.org/cp/reaction.owl#Reaction> rdf:type owl:NamedIndividual ,
                                                                          odin:ODPElement ;
                                                                 odin:describedIn odin:Reaction_Descr ;
                                                                 odin:odpType odin:Foundational ;
                                                                 rdfs:comment "This class is not intended to be instantiated." .


###  http://www.ontologydesignpatterns.org/cp/reaction.owl#hasOutcome
<http://www.ontologydesignpatterns.org/cp/reaction.owl#hasOutcome> rdf:type owl:NamedIndividual ,
                                                                            odin:ODPElement ;
                                                                   odin:describedIn odin:hasOutcome_Descr ;
                                                                   rdfs:comment "Is also true that some action directly preceeds its outcome" .


###  http://www.ontologydesignpatterns.org/cp/reaction.owl#isOutcomeOf
<http://www.ontologydesignpatterns.org/cp/reaction.owl#isOutcomeOf> rdf:type owl:NamedIndividual ,
                                                                             odin:ODPElement ;
                                                                    odin:describedIn odin:isOutcomeOf_Descr ;
                                                                    rdfs:comment "Is also true that some outcome follows some action" .


###  http://www.ontologydesignpatterns.org/ont/dul/tagging.owl#Folksonomy
<http://www.ontologydesignpatterns.org/ont/dul/tagging.owl#Folksonomy> rdf:type owl:NamedIndividual ;
                                                                       odin:describedIn odin:Folksonomy_Descr ;
                                                                       odin:odpType odin:Foundational ;
                                                                       rdfs:comment "A collection of tags or metadata that have no formal semantics, and are typically used sparsely to annotate texts, images, bookmarks, etc. Folksonomies are typically maintained by communities through web-based services or systems, and do not have any systematic intent, such as that shared by KOS(es)." .


###  http://www.ontologydesignpatterns.org/ont/dul/tagging.owl#Tag
<http://www.ontologydesignpatterns.org/ont/dul/tagging.owl#Tag> rdf:type owl:NamedIndividual ;
                                                                odin:describedIn odin:Tag_Descr ;
                                                                odin:odpType odin:Foundational ;
                                                                rdfs:comment "The typical elements of folksonomies, used to add a hint for the interpretation of web resources in so-called situations of 'Tagging'.  Tags are considered here as InformationObject(s) that have a folksonomy as their schema.  A Tag is typically used to add an element of interpretation to some document, i.e. 'forcing' the reader to see that document from the viewpoint that can be built by pairing the Tag interpretation with the document interpretation. For example, an image of St. Peter's dome can be tagged as 'Michelangelo', 'Big ovoid', 'trip to Rome', etc., thus forcing the interpretation of the dome image towards artistic design, geometry, or private memories." .


###  http://www.ontologydesignpatterns.org/ont/fred/domain.owl#activator_1
<http://www.ontologydesignpatterns.org/ont/fred/domain.owl#activator_1> rdf:type owl:NamedIndividual .


###  http://www.ontologydesignpatterns.org/ont/is/isaac_vanilla.owl#BLOCKAGE
<http://www.ontologydesignpatterns.org/ont/is/isaac_vanilla.owl#BLOCKAGE> rdf:type owl:NamedIndividual .


###  http://www.ontologydesignpatterns.org/ont/is/isaac_vanilla.owl#CENTER
<http://www.ontologydesignpatterns.org/ont/is/isaac_vanilla.owl#CENTER> rdf:type owl:NamedIndividual .


###  http://www.ontologydesignpatterns.org/ont/is/isaac_vanilla.owl#CENTER_PERIPHERY
<http://www.ontologydesignpatterns.org/ont/is/isaac_vanilla.owl#CENTER_PERIPHERY> rdf:type owl:NamedIndividual .


###  http://www.ontologydesignpatterns.org/ont/is/isaac_vanilla.owl#CONTAINER
<http://www.ontologydesignpatterns.org/ont/is/isaac_vanilla.owl#CONTAINER> rdf:type owl:NamedIndividual .


###  http://www.ontologydesignpatterns.org/ont/is/isaac_vanilla.owl#CONTAINMENT
<http://www.ontologydesignpatterns.org/ont/is/isaac_vanilla.owl#CONTAINMENT> rdf:type owl:NamedIndividual .


###  http://www.ontologydesignpatterns.org/ont/is/isaac_vanilla.owl#GOAL
<http://www.ontologydesignpatterns.org/ont/is/isaac_vanilla.owl#GOAL> rdf:type owl:NamedIndividual .


###  http://www.ontologydesignpatterns.org/ont/is/isaac_vanilla.owl#PART_WHOLE
<http://www.ontologydesignpatterns.org/ont/is/isaac_vanilla.owl#PART_WHOLE> rdf:type owl:NamedIndividual .


###  http://www.ontologydesignpatterns.org/ont/is/isaac_vanilla.owl#PATH
<http://www.ontologydesignpatterns.org/ont/is/isaac_vanilla.owl#PATH> rdf:type owl:NamedIndividual .


###  http://www.ontologydesignpatterns.org/ont/is/isaac_vanilla.owl#PERIPHERY
<http://www.ontologydesignpatterns.org/ont/is/isaac_vanilla.owl#PERIPHERY> rdf:type owl:NamedIndividual .


###  http://www.ontologydesignpatterns.org/ont/is/isaac_vanilla.owl#SOURCE_PATH_GOAL
<http://www.ontologydesignpatterns.org/ont/is/isaac_vanilla.owl#SOURCE_PATH_GOAL> rdf:type owl:NamedIndividual .


###  http://www.ontologydesignpatterns.org/ont/is/isaac_vanilla.owl#SUPPORT
<http://www.ontologydesignpatterns.org/ont/is/isaac_vanilla.owl#SUPPORT> rdf:type owl:NamedIndividual .


###  http://www.ontologydesignpatterns.org/ont/is/isaac_vanilla.owl#SUPPORTER
<http://www.ontologydesignpatterns.org/ont/is/isaac_vanilla.owl#SUPPORTER> rdf:type owl:NamedIndividual .


###  http://www.ontologydesignpatterns.org/ont/is/isaac_vanilla.owl#WHOLE
<http://www.ontologydesignpatterns.org/ont/is/isaac_vanilla.owl#WHOLE> rdf:type owl:NamedIndividual .


###  http://www.ontologydesignpatterns.org/ont/mario/affordance.owl#Affordance
<http://www.ontologydesignpatterns.org/ont/mario/affordance.owl#Affordance> rdf:type owl:NamedIndividual ,
                                                                                     odin:ODPElement ;
                                                                            odin:describedIn odin:Affordance_Descr ;
                                                                            odin:odpType odin:Foundational ;
                                                                            rdfs:comment "An affordance is modelled in DnS fashion and is an n-ary that relates state of the world (i.e., situations) to tasks according to specific weights or affordance strengths." .


###  http://www.ontologydesignpatterns.org/ont/mario/affordance.owl#BehaviorParameter
<http://www.ontologydesignpatterns.org/ont/mario/affordance.owl#BehaviorParameter> rdf:type owl:NamedIndividual ,
                                                                                            odin:ODPElement ;
                                                                                   odin:describedIn odin:BehaviorParameter_Descr ;
                                                                                   odin:odpType odin:Foundational ;
                                                                                   rdfs:comment "A parameter of a behavior." .


###  http://www.ontologydesignpatterns.org/ont/mario/affordance.owl#Situation
<http://www.ontologydesignpatterns.org/ont/mario/affordance.owl#Situation> rdf:type owl:NamedIndividual ,
                                                                                    odin:ODPElement ;
                                                                           odin:describedIn odin:Situation_Descr ;
                                                                           rdfs:comment "A state of the world." .


###  http://www.ontologydesignpatterns.org/ont/mario/affordance.owl#affordanceStrength
<http://www.ontologydesignpatterns.org/ont/mario/affordance.owl#affordanceStrength> rdf:type owl:NamedIndividual ,
                                                                                             odin:ODPElement ;
                                                                                    odin:describedIn odin:affordanceStrength_Descr ;
                                                                                    rdfs:comment "It encodes the strength of the Affordance." .


###  http://www.ontologydesignpatterns.org/ont/mario/affordance.owl#hasParameter
<http://www.ontologydesignpatterns.org/ont/mario/affordance.owl#hasParameter> rdf:type owl:NamedIndividual ,
                                                                                       odin:ODPElement ;
                                                                              odin:describedIn odin:hasParameter_Descr ;
                                                                              odin:odpType odin:Foundational ;
                                                                              rdfs:comment "It associates the Task with its parameters." .


###  http://www.ontologydesignpatterns.org/ont/mario/affordance.owl#hasTask
<http://www.ontologydesignpatterns.org/ont/mario/affordance.owl#hasTask> rdf:type owl:NamedIndividual ,
                                                                                  odin:ODPElement ;
                                                                         odin:describedIn odin:hasTask_Descr ;
                                                                         rdfs:comment "It associates an Affordance to the Task it refers to." .


###  http://www.ontologydesignpatterns.org/ont/mario/affordance.owl#holds
<http://www.ontologydesignpatterns.org/ont/mario/affordance.owl#holds> rdf:type owl:NamedIndividual ,
                                                                                odin:ODPElement ;
                                                                       odin:describedIn odin:holds_Descr ;
                                                                       rdfs:comment "It associates an Affordance with the Frame in which it holds." .


###  http://www.ontologydesignpatterns.org/ont/mario/affordance.owl#isHeldBy
<http://www.ontologydesignpatterns.org/ont/mario/affordance.owl#isHeldBy> rdf:type owl:NamedIndividual ,
                                                                                   odin:ODPElement ;
                                                                          odin:describedIn odin:isHeldBy_Descr ;
                                                                          odin:odpType odin:Foundational ;
                                                                          rdfs:comment "It associates a Frame with the Affordance it enables." .


###  http://www.ontologydesignpatterns.org/ont/odin/odin.owl#AAE_Descr
odin:AAE_Descr rdf:type owl:NamedIndividual .


###  http://www.ontologydesignpatterns.org/ont/odin/odin.owl#AbstractMergingTask_Descr
odin:AbstractMergingTask_Descr rdf:type owl:NamedIndividual ;
                               isnet:activates <http://www.ontologydesignpatterns.org/ont/is/isaac_vanilla.owl#CONTAINMENT> ,
                                               <http://www.ontologydesignpatterns.org/ont/is/isaac_vanilla.owl#SOURCE_PATH_GOAL> ,
                                               <http://www.ontologydesignpatterns.org/ont/is/isaac_vanilla.owl#SUPPORT> ;
                               isnet:hasActivator <https://w3id.org/framester/data/framestercore/Aiming> ,
                                                  <https://w3id.org/framester/data/framestercore/Assistance> ,
                                                  <https://w3id.org/framester/data/framestercore/Goal> ,
                                                  <https://w3id.org/framester/data/framestercore/Placing> ,
                                                  <https://w3id.org/framester/data/framestercore/Purpose> ,
                                                  <https://w3id.org/framester/data/framestercore/Supply> ,
                                                  <https://w3id.org/framester/vn/vn31/data/Aim_62000000> ,
                                                  <https://w3id.org/framester/wn/wn30/instances/synset-supply-verb-1> .


###  http://www.ontologydesignpatterns.org/ont/odin/odin.owl#Abstract_Descr
odin:Abstract_Descr rdf:type owl:NamedIndividual .


###  http://www.ontologydesignpatterns.org/ont/odin/odin.owl#Action_Descr
odin:Action_Descr rdf:type owl:NamedIndividual .


###  http://www.ontologydesignpatterns.org/ont/odin/odin.owl#ActivationTask_Descr
odin:ActivationTask_Descr rdf:type owl:NamedIndividual .


###  http://www.ontologydesignpatterns.org/ont/odin/odin.owl#ActivityPattern_Descr
odin:ActivityPattern_Descr rdf:type owl:NamedIndividual .


###  http://www.ontologydesignpatterns.org/ont/odin/odin.owl#ActualEventViewContext_Descr
odin:ActualEventViewContext_Descr rdf:type owl:NamedIndividual .


###  http://www.ontologydesignpatterns.org/ont/odin/odin.owl#ActualEvent_Descr
odin:ActualEvent_Descr rdf:type owl:NamedIndividual ;
                       isnet:activates <http://www.ontologydesignpatterns.org/ont/is/isaac_vanilla.owl#CONTAINER> ,
                                       <http://www.ontologydesignpatterns.org/ont/is/isaac_vanilla.owl#PERIPHERY> ;
                       isnet:hasActivator <https://w3id.org/framester/wn/wn30/instances/supersense-noun_location> ,
                                          <https://w3id.org/framester/wn/wn30/instances/synset-there-noun-1> .


###  http://www.ontologydesignpatterns.org/ont/odin/odin.owl#ActuatingCapability_Descr
odin:ActuatingCapability_Descr rdf:type owl:NamedIndividual .


###  http://www.ontologydesignpatterns.org/ont/odin/odin.owl#ActuatingDevice_Descr
odin:ActuatingDevice_Descr rdf:type owl:NamedIndividual .


###  http://www.ontologydesignpatterns.org/ont/odin/odin.owl#ActuatingRange_Descr
odin:ActuatingRange_Descr rdf:type owl:NamedIndividual .


###  http://www.ontologydesignpatterns.org/ont/odin/odin.owl#ActuatingTime_Descr
odin:ActuatingTime_Descr rdf:type owl:NamedIndividual .


###  http://www.ontologydesignpatterns.org/ont/odin/odin.owl#ActuatorInput_Descr
odin:ActuatorInput_Descr rdf:type owl:NamedIndividual ;
                         isnet:activates <http://www.ontologydesignpatterns.org/ont/is/isaac_vanilla.owl#PART_WHOLE> ,
                                         <http://www.ontologydesignpatterns.org/ont/is/isaac_vanilla.owl#SOURCE_PATH_GOAL> ,
                                         <http://www.ontologydesignpatterns.org/ont/is/isaac_vanilla.owl#SUPPORT> ;
                         isnet:hasActivator <https://w3id.org/framester/data/framestercore/Assistance> ,
                                            <https://w3id.org/framester/data/framestercore/Conduct> ,
                                            <https://w3id.org/framester/data/framestercore/Supply> ,
                                            <https://w3id.org/framester/wn/wn30/instances/synset-piece-noun-1> .


###  http://www.ontologydesignpatterns.org/ont/odin/odin.owl#ActuatorOutput_Descr
odin:ActuatorOutput_Descr rdf:type owl:NamedIndividual ;
                          isnet:activates <http://www.ontologydesignpatterns.org/ont/is/isaac_vanilla.owl#CONTAINMENT> ;
                          isnet:hasActivator <https://w3id.org/framester/data/framestercore/Ingestion> ,
                                             <https://w3id.org/framester/data/framestercore/Placing> ,
                                             <https://w3id.org/framester/wn/wn30/instances/synset-lodge-verb-2> .


###  http://www.ontologydesignpatterns.org/ont/odin/odin.owl#Actuator_Descr
odin:Actuator_Descr rdf:type owl:NamedIndividual ;
                    isnet:activates <http://www.ontologydesignpatterns.org/ont/is/isaac_vanilla.owl#PART_WHOLE> ,
                                    <http://www.ontologydesignpatterns.org/ont/is/isaac_vanilla.owl#PATH> ,
                                    <http://www.ontologydesignpatterns.org/ont/is/isaac_vanilla.owl#SUPPORTER> ;
                    isnet:hasActivator <https://w3id.org/framester/wn/wn30/instances/synset-bulb-noun-1> ,
                                       <https://w3id.org/framester/wn/wn30/instances/synset-light-adjective-1> .


###  http://www.ontologydesignpatterns.org/ont/odin/odin.owl#Affordance_Descr
odin:Affordance_Descr rdf:type owl:NamedIndividual .


###  http://www.ontologydesignpatterns.org/ont/odin/odin.owl#Agent_Descr
odin:Agent_Descr rdf:type owl:NamedIndividual ;
                 isnet:activates <http://www.ontologydesignpatterns.org/ont/is/isaac_vanilla.owl#PART_WHOLE> ;
                 isnet:hasActivator <https://w3id.org/framester/wn/wn30/instances/supersense-noun_group> .


###  http://www.ontologydesignpatterns.org/ont/odin/odin.owl#AggregatedObject_Descr
odin:AggregatedObject_Descr rdf:type owl:NamedIndividual ;
                            isnet:activates <http://www.ontologydesignpatterns.org/ont/is/isaac_vanilla.owl#CONTAINER> ,
                                            <http://www.ontologydesignpatterns.org/ont/is/isaac_vanilla.owl#PART_WHOLE> ;
                            isnet:hasActivator <https://w3id.org/framester/wn/wn30/instances/supersense-noun_group> ,
                                               <https://w3id.org/framester/wn/wn30/instances/supersense-noun_location> .


###  http://www.ontologydesignpatterns.org/ont/odin/odin.owl#Airline.owl_Descr
odin:Airline.owl_Descr rdf:type owl:NamedIndividual .


###  http://www.ontologydesignpatterns.org/ont/odin/odin.owl#All_Descr
odin:All_Descr rdf:type owl:NamedIndividual ;
               isnet:activates <http://www.ontologydesignpatterns.org/ont/is/isaac_vanilla.owl#PART_WHOLE> ;
               isnet:hasActivator <https://w3id.org/framester/wn/wn30/instances/synset-term-noun-1> .


###  http://www.ontologydesignpatterns.org/ont/odin/odin.owl#AnalogBroadcastStandard_Descr
odin:AnalogBroadcastStandard_Descr rdf:type owl:NamedIndividual .


###  http://www.ontologydesignpatterns.org/ont/odin/odin.owl#AquaticResourceObservation_Descr
odin:AquaticResourceObservation_Descr rdf:type owl:NamedIndividual .


###  http://www.ontologydesignpatterns.org/ont/odin/odin.owl#AquaticResource_Descr
odin:AquaticResource_Descr rdf:type owl:NamedIndividual ;
                           isnet:activates <http://www.ontologydesignpatterns.org/ont/is/isaac_vanilla.owl#PART_WHOLE> ;
                           isnet:hasActivator <https://w3id.org/framester/wn/wn30/instances/supersense-noun_group> .


###  http://www.ontologydesignpatterns.org/ont/odin/odin.owl#AquaticSpecies_Descr
odin:AquaticSpecies_Descr rdf:type owl:NamedIndividual ;
                          isnet:activates <http://www.ontologydesignpatterns.org/ont/is/isaac_vanilla.owl#CONTAINMENT> ,
                                          <http://www.ontologydesignpatterns.org/ont/is/isaac_vanilla.owl#PART_WHOLE> ;
                          isnet:hasActivator <https://w3id.org/framester/data/framestercore/Ingestion> ,
                                             <https://w3id.org/framester/wn/wn30/instances/supersense-noun_group> .


###  http://www.ontologydesignpatterns.org/ont/odin/odin.owl#AspectRatio_Descr
odin:AspectRatio_Descr rdf:type owl:NamedIndividual .


###  http://www.ontologydesignpatterns.org/ont/odin/odin.owl#Attribute_Descr
odin:Attribute_Descr rdf:type owl:NamedIndividual .


###  http://www.ontologydesignpatterns.org/ont/odin/odin.owl#AudioCodec_Descr
odin:AudioCodec_Descr rdf:type owl:NamedIndividual ;
                      isnet:activates <http://www.ontologydesignpatterns.org/ont/is/isaac_vanilla.owl#GOAL> ,
                                      <http://www.ontologydesignpatterns.org/ont/is/isaac_vanilla.owl#SOURCE_PATH_GOAL> ;
                      isnet:hasActivator <https://w3id.org/framester/data/framestercore/Purpose> ,
                                         <https://w3id.org/framester/wn/wn30/instances/synset-plan-noun-1> .


###  http://www.ontologydesignpatterns.org/ont/odin/odin.owl#AudioStream_Descr
odin:AudioStream_Descr rdf:type owl:NamedIndividual ;
                       isnet:activates <http://www.ontologydesignpatterns.org/ont/is/isaac_vanilla.owl#PART_WHOLE> ,
                                       <http://www.ontologydesignpatterns.org/ont/is/isaac_vanilla.owl#SOURCE_PATH_GOAL> ;
                       isnet:hasActivator <https://w3id.org/framester/data/framestercore/Motion> ,
                                          <https://w3id.org/framester/vn/vn31/data/Carry_11040000> ,
                                          <https://w3id.org/framester/wn/wn30/instances/supersense-noun_group> .


###  http://www.ontologydesignpatterns.org/ont/odin/odin.owl#AutomationStatus_Descr
odin:AutomationStatus_Descr rdf:type owl:NamedIndividual ;
                            isnet:activates <http://www.ontologydesignpatterns.org/ont/is/isaac_vanilla.owl#GOAL> ;
                            isnet:hasActivator <https://w3id.org/framester/wn/wn30/instances/synset-automation-noun-1> ,
                                               <https://w3id.org/framester/wn/wn30/instances/synset-policy-noun-1> .


###  http://www.ontologydesignpatterns.org/ont/odin/odin.owl#Bag_Descr
odin:Bag_Descr rdf:type owl:NamedIndividual ;
               isnet:activates <http://www.ontologydesignpatterns.org/ont/is/isaac_vanilla.owl#CONTAINMENT> ,
                               <http://www.ontologydesignpatterns.org/ont/is/isaac_vanilla.owl#PART_WHOLE> ;
               isnet:hasActivator <https://w3id.org/framester/data/framestercore/Ingestion> ,
                                  <https://w3id.org/framester/wn/wn30/instances/supersense-noun_group> .


###  http://www.ontologydesignpatterns.org/ont/odin/odin.owl#BathymetricRange_Descr
odin:BathymetricRange_Descr rdf:type owl:NamedIndividual ;
                            isnet:activates <http://www.ontologydesignpatterns.org/ont/is/isaac_vanilla.owl#CONTAINMENT> ,
                                            <http://www.ontologydesignpatterns.org/ont/is/isaac_vanilla.owl#PART_WHOLE> ;
                            isnet:hasActivator <https://w3id.org/framester/data/framestercore/Containing> ,
                                               <https://w3id.org/framester/data/framestercore/Placing> ,
                                               <https://w3id.org/framester/vn/vn31/data/Contain_54030000> ,
                                               <https://w3id.org/framester/wn/wn30/instances/supersense-noun_group> .


###  http://www.ontologydesignpatterns.org/ont/odin/odin.owl#BehaviorParameter_Descr
odin:BehaviorParameter_Descr rdf:type owl:NamedIndividual .


###  http://www.ontologydesignpatterns.org/ont/odin/odin.owl#BiologicalProcess_Descr
odin:BiologicalProcess_Descr rdf:type owl:NamedIndividual .


###  http://www.ontologydesignpatterns.org/ont/odin/odin.owl#BitRate_Descr
odin:BitRate_Descr rdf:type owl:NamedIndividual ;
                   isnet:activates <http://www.ontologydesignpatterns.org/ont/is/isaac_vanilla.owl#CONTAINMENT> ;
                   isnet:hasActivator <https://w3id.org/framester/data/framestercore/Ingestion> ,
                                      <https://w3id.org/framester/data/framestercore/Placing> .


###  http://www.ontologydesignpatterns.org/ont/odin/odin.owl#BooleanCaseTask_Descr
odin:BooleanCaseTask_Descr rdf:type owl:NamedIndividual .


###  http://www.ontologydesignpatterns.org/ont/odin/odin.owl#BranchingTask_Descr
odin:BranchingTask_Descr rdf:type owl:NamedIndividual ;
                         isnet:activates <http://www.ontologydesignpatterns.org/ont/is/isaac_vanilla.owl#GOAL> ,
                                         <http://www.ontologydesignpatterns.org/ont/is/isaac_vanilla.owl#PART_WHOLE> ,
                                         <http://www.ontologydesignpatterns.org/ont/is/isaac_vanilla.owl#SOURCE_PATH_GOAL> ;
                         isnet:hasActivator <https://w3id.org/framester/data/framestercore/Motion> ,
                                            <https://w3id.org/framester/data/framestercore/Purpose> ,
                                            <https://w3id.org/framester/wn/wn30/instances/supersense-noun_group> ,
                                            <https://w3id.org/framester/wn/wn30/instances/synset-plan-noun-1> .


###  http://www.ontologydesignpatterns.org/ont/odin/odin.owl#CaseTask_Descr
odin:CaseTask_Descr rdf:type owl:NamedIndividual ;
                    isnet:activates <http://www.ontologydesignpatterns.org/ont/is/isaac_vanilla.owl#CONTAINMENT> ,
                                    <http://www.ontologydesignpatterns.org/ont/is/isaac_vanilla.owl#PART_WHOLE> ,
                                    <http://www.ontologydesignpatterns.org/ont/is/isaac_vanilla.owl#SOURCE_PATH_GOAL> ;
                    isnet:hasActivator <https://w3id.org/framester/data/framestercore/Ingestion> ,
                                       <https://w3id.org/framester/data/framestercore/SelfMotion> ,
                                       <https://w3id.org/framester/vn/vn31/data/Undertake_98000000> ,
                                       <https://w3id.org/framester/wn/wn30/instances/supersense-noun_group> .


###  http://www.ontologydesignpatterns.org/ont/odin/odin.owl#CatchRecord_Descr
odin:CatchRecord_Descr rdf:type owl:NamedIndividual ;
                       isnet:activates <http://www.ontologydesignpatterns.org/ont/is/isaac_vanilla.owl#CENTER_PERIPHERY> ,
                                       <http://www.ontologydesignpatterns.org/ont/is/isaac_vanilla.owl#CONTAINMENT> ,
                                       <http://www.ontologydesignpatterns.org/ont/is/isaac_vanilla.owl#PART_WHOLE> ;
                       isnet:hasActivator <https://w3id.org/framester/data/framestercore/Containing> ,
                                          <https://w3id.org/framester/data/framestercore/Placing> ,
                                          <https://w3id.org/framester/data/framestercore/Range> ,
                                          <https://w3id.org/framester/vn/vn31/data/Contain_54030000> ,
                                          <https://w3id.org/framester/wn/wn30/instances/supersense-noun_group> ,
                                          <https://w3id.org/framester/wn/wn30/instances/synset-position-noun-3> .


###  http://www.ontologydesignpatterns.org/ont/odin/odin.owl#CellularComponent_Descr
odin:CellularComponent_Descr rdf:type owl:NamedIndividual .


###  http://www.ontologydesignpatterns.org/ont/odin/odin.owl#ChromaFormat_Descr
odin:ChromaFormat_Descr rdf:type owl:NamedIndividual .


###  http://www.ontologydesignpatterns.org/ont/odin/odin.owl#City_Descr
odin:City_Descr rdf:type owl:NamedIndividual ;
                isnet:activates <http://www.ontologydesignpatterns.org/ont/is/isaac_vanilla.owl#PART_WHOLE> ;
                isnet:hasActivator <https://w3id.org/framester/wn/wn30/instances/supersense-noun_group> ,
                                   <https://w3id.org/framester/wn/wn30/instances/synset-colony-noun-1> .


###  http://www.ontologydesignpatterns.org/ont/odin/odin.owl#Class_Descr
odin:Class_Descr rdf:type owl:NamedIndividual .


###  http://www.ontologydesignpatterns.org/ont/odin/odin.owl#Codec_Descr
odin:Codec_Descr rdf:type owl:NamedIndividual ;
                 isnet:activates <http://www.ontologydesignpatterns.org/ont/is/isaac_vanilla.owl#GOAL> ,
                                 <http://www.ontologydesignpatterns.org/ont/is/isaac_vanilla.owl#SOURCE_PATH_GOAL> ;
                 isnet:hasActivator <https://w3id.org/framester/data/framestercore/Purpose> ,
                                    <https://w3id.org/framester/wn/wn30/instances/synset-plan-noun-1> .


###  http://www.ontologydesignpatterns.org/ont/odin/odin.owl#CodingStandard_Descr
odin:CodingStandard_Descr rdf:type owl:NamedIndividual .


###  http://www.ontologydesignpatterns.org/ont/odin/odin.owl#Collection_Descr
odin:Collection_Descr rdf:type owl:NamedIndividual .


###  http://www.ontologydesignpatterns.org/ont/odin/odin.owl#ColourSpaceType_Descr
odin:ColourSpaceType_Descr rdf:type owl:NamedIndividual ;
                           isnet:activates <http://www.ontologydesignpatterns.org/ont/is/isaac_vanilla.owl#PART_WHOLE> ;
                           isnet:hasActivator <https://w3id.org/framester/wn/wn30/instances/supersense-noun_group> .


###  http://www.ontologydesignpatterns.org/ont/odin/odin.owl#Community_Descr
odin:Community_Descr rdf:type owl:NamedIndividual ;
                     isnet:activates <http://www.ontologydesignpatterns.org/ont/is/isaac_vanilla.owl#PART_WHOLE> ;
                     isnet:hasActivator <https://w3id.org/framester/wn/wn30/instances/supersense-noun_group> .


###  http://www.ontologydesignpatterns.org/ont/odin/odin.owl#CompressionType_Descr
odin:CompressionType_Descr rdf:type owl:NamedIndividual .


###  http://www.ontologydesignpatterns.org/ont/odin/odin.owl#Computer_Descr
odin:Computer_Descr rdf:type owl:NamedIndividual .


###  http://www.ontologydesignpatterns.org/ont/odin/odin.owl#Concept_Descr
odin:Concept_Descr rdf:type owl:NamedIndividual ;
                   isnet:activates <http://www.ontologydesignpatterns.org/ont/is/isaac_vanilla.owl#CONTAINMENT> ,
                                   <http://www.ontologydesignpatterns.org/ont/is/isaac_vanilla.owl#PART_WHOLE> ,
                                   <http://www.ontologydesignpatterns.org/ont/is/isaac_vanilla.owl#SOURCE_PATH_GOAL> ;
                   isnet:hasActivator <https://w3id.org/framester/data/framestercore/Sending> ,
                                      <https://w3id.org/framester/wn/wn30/instances/supersense-noun_group> ,
                                      <https://w3id.org/framester/wn/wn30/instances/synset-concept-noun-1> ,
                                      <https://w3id.org/framester/wn/wn30/instances/synset-idea-noun-1> ,
                                      <https://w3id.org/framester/wn/wn30/instances/synset-notion-noun-2> .


###  http://www.ontologydesignpatterns.org/ont/odin/odin.owl#ConcurrencyTask_Descr
odin:ConcurrencyTask_Descr rdf:type owl:NamedIndividual ;
                           isnet:activates <http://www.ontologydesignpatterns.org/ont/is/isaac_vanilla.owl#CONTAINMENT> ,
                                           <http://www.ontologydesignpatterns.org/ont/is/isaac_vanilla.owl#PART_WHOLE> ,
                                           <http://www.ontologydesignpatterns.org/ont/is/isaac_vanilla.owl#SOURCE_PATH_GOAL> ;
                           isnet:hasActivator <https://w3id.org/framester/data/framestercore/Aiming> ,
                                              <https://w3id.org/framester/data/framestercore/Goal> ,
                                              <https://w3id.org/framester/data/framestercore/Ingestion> ,
                                              <https://w3id.org/framester/data/framestercore/Placing> ,
                                              <https://w3id.org/framester/data/framestercore/Purpose> ,
                                              <https://w3id.org/framester/data/framestercore/Sending> ,
                                              <https://w3id.org/framester/vn/vn31/data/Aim_62000000> ,
                                              <https://w3id.org/framester/wn/wn30/instances/supersense-noun_group> .


###  http://www.ontologydesignpatterns.org/ont/odin/odin.owl#ConfigurationProcedure_Descr
odin:ConfigurationProcedure_Descr rdf:type owl:NamedIndividual ;
                                  isnet:activates <http://www.ontologydesignpatterns.org/ont/is/isaac_vanilla.owl#PART_WHOLE> ;
                                  isnet:hasActivator <https://w3id.org/framester/wn/wn30/instances/synset-context-noun-1> .


###  http://www.ontologydesignpatterns.org/ont/odin/odin.owl#Container_Descr
odin:Container_Descr rdf:type owl:NamedIndividual .


###  http://www.ontologydesignpatterns.org/ont/odin/odin.owl#ControlTask_Descr
odin:ControlTask_Descr rdf:type owl:NamedIndividual ;
                       isnet:activates <http://www.ontologydesignpatterns.org/ont/is/isaac_vanilla.owl#CONTAINMENT> ,
                                       <http://www.ontologydesignpatterns.org/ont/is/isaac_vanilla.owl#SOURCE_PATH_GOAL> ;
                       isnet:hasActivator <https://w3id.org/framester/data/framestercore/Aiming> ,
                                          <https://w3id.org/framester/data/framestercore/Goal> ,
                                          <https://w3id.org/framester/data/framestercore/Ingestion> ,
                                          <https://w3id.org/framester/data/framestercore/Placing> ,
                                          <https://w3id.org/framester/data/framestercore/Purpose> ,
                                          <https://w3id.org/framester/vn/vn31/data/Aim_62000000> .


###  http://www.ontologydesignpatterns.org/ont/odin/odin.owl#Core
odin:Core rdf:type owl:NamedIndividual ,
                   odin:ODPType .


###  http://www.ontologydesignpatterns.org/ont/odin/odin.owl#CountingAs_Descr
odin:CountingAs_Descr rdf:type owl:NamedIndividual .


###  http://www.ontologydesignpatterns.org/ont/odin/odin.owl#Currency_Descr
odin:Currency_Descr rdf:type owl:NamedIndividual .


###  http://www.ontologydesignpatterns.org/ont/odin/odin.owl#DASE_RULE_Descr
odin:DASE_RULE_Descr rdf:type owl:NamedIndividual .


###  http://www.ontologydesignpatterns.org/ont/odin/odin.owl#DataReceiverNode_Descr
odin:DataReceiverNode_Descr rdf:type owl:NamedIndividual .


###  http://www.ontologydesignpatterns.org/ont/odin/odin.owl#DataSenderNode_Descr
odin:DataSenderNode_Descr rdf:type owl:NamedIndividual ;
                          isnet:activates <http://www.ontologydesignpatterns.org/ont/is/isaac_vanilla.owl#PART_WHOLE> ,
                                          <http://www.ontologydesignpatterns.org/ont/is/isaac_vanilla.owl#SOURCE_PATH_GOAL> ;
                          isnet:hasActivator <https://w3id.org/framester/data/framestercore/Membership> ,
                                             <https://w3id.org/framester/data/framestercore/Sending> ,
                                             <https://w3id.org/framester/wn/wn30/instances/synset-part-noun-1> .


###  http://www.ontologydesignpatterns.org/ont/odin/odin.owl#DecisionActivity_Descr
odin:DecisionActivity_Descr rdf:type owl:NamedIndividual .


###  http://www.ontologydesignpatterns.org/ont/odin/odin.owl#DeliberationState_Descr
odin:DeliberationState_Descr rdf:type owl:NamedIndividual .


###  http://www.ontologydesignpatterns.org/ont/odin/odin.owl#DescriptionInRange_Descr
odin:DescriptionInRange_Descr rdf:type owl:NamedIndividual .


###  http://www.ontologydesignpatterns.org/ont/odin/odin.owl#Description_Descr
odin:Description_Descr rdf:type owl:NamedIndividual ;
                       isnet:activates <http://www.ontologydesignpatterns.org/ont/is/isaac_vanilla.owl#CONTAINMENT> ,
                                       <http://www.ontologydesignpatterns.org/ont/is/isaac_vanilla.owl#GOAL> ,
                                       <http://www.ontologydesignpatterns.org/ont/is/isaac_vanilla.owl#PART_WHOLE> ,
                                       <http://www.ontologydesignpatterns.org/ont/is/isaac_vanilla.owl#SOURCE_PATH_GOAL> ,
                                       <http://www.ontologydesignpatterns.org/ont/is/isaac_vanilla.owl#SUPPORT> ;
                       isnet:hasActivator <https://w3id.org/framester/data/framestercore/Assistance> ,
                                          <https://w3id.org/framester/data/framestercore/Purpose> ,
                                          <https://w3id.org/framester/data/framestercore/Supply> ,
                                          <https://w3id.org/framester/vn/vn31/data/Plan_62000000> ,
                                          <https://w3id.org/framester/wn/wn30/instances/supersense-noun_group> ,
                                          <https://w3id.org/framester/wn/wn30/instances/synset-concept-noun-1> ,
                                          <https://w3id.org/framester/wn/wn30/instances/synset-context-noun-1> ,
                                          <https://w3id.org/framester/wn/wn30/instances/synset-interpretation-noun-1> ,
                                          <https://w3id.org/framester/wn/wn30/instances/synset-out-noun-1> ,
                                          <https://w3id.org/framester/wn/wn30/instances/synset-plan-verb-1> ,
                                          <https://w3id.org/framester/wn/wn30/instances/synset-use-noun-1> .


###  http://www.ontologydesignpatterns.org/ont/odin/odin.owl#Descriptor_Descr
odin:Descriptor_Descr rdf:type owl:NamedIndividual ;
                      isnet:activates <http://www.ontologydesignpatterns.org/ont/is/isaac_vanilla.owl#CONTAINMENT> ,
                                      <http://www.ontologydesignpatterns.org/ont/is/isaac_vanilla.owl#GOAL> ;
                      isnet:hasActivator <https://w3id.org/framester/data/framestercore/Containers> ,
                                         <https://w3id.org/framester/wn/wn30/instances/synset-container-noun-1> ,
                                         <https://w3id.org/framester/wn/wn30/instances/synset-policy-noun-1> .


###  http://www.ontologydesignpatterns.org/ont/odin/odin.owl#DigitalVideo_Descr
odin:DigitalVideo_Descr rdf:type owl:NamedIndividual ;
                        isnet:activates <http://www.ontologydesignpatterns.org/ont/is/isaac_vanilla.owl#CONTAINMENT> ;
                        isnet:hasActivator <https://w3id.org/framester/data/framestercore/Placing> .


###  http://www.ontologydesignpatterns.org/ont/odin/odin.owl#Effect_Descr
odin:Effect_Descr rdf:type owl:NamedIndividual ;
                  isnet:activates <http://www.ontologydesignpatterns.org/ont/is/isaac_vanilla.owl#CONTAINMENT> ;
                  isnet:hasActivator <https://w3id.org/framester/wn/wn30/instances/synset-concept-noun-1> ,
                                     <https://w3id.org/framester/wn/wn30/instances/synset-kind-noun-1> .


###  http://www.ontologydesignpatterns.org/ont/odin/odin.owl#EmbeddingType_Descr
odin:EmbeddingType_Descr rdf:type owl:NamedIndividual .


###  http://www.ontologydesignpatterns.org/ont/odin/odin.owl#EndingFix_Descr
odin:EndingFix_Descr rdf:type owl:NamedIndividual .


###  http://www.ontologydesignpatterns.org/ont/odin/odin.owl#EndingTask_Descr
odin:EndingTask_Descr rdf:type owl:NamedIndividual .


###  http://www.ontologydesignpatterns.org/ont/odin/odin.owl#Entity_Descr
odin:Entity_Descr rdf:type owl:NamedIndividual .


###  http://www.ontologydesignpatterns.org/ont/odin/odin.owl#EventCondition_Descr
odin:EventCondition_Descr rdf:type owl:NamedIndividual ;
                          isnet:activates <http://www.ontologydesignpatterns.org/ont/is/isaac_vanilla.owl#CENTER_PERIPHERY> ;
                          isnet:hasActivator <https://w3id.org/framester/data/framestercore/Range> ,
                                             <https://w3id.org/framester/wn/wn30/instances/synset-distance-noun-1> .


###  http://www.ontologydesignpatterns.org/ont/odin/odin.owl#EventObjectBody_Descr
odin:EventObjectBody_Descr rdf:type owl:NamedIndividual ;
                           isnet:activates <http://www.ontologydesignpatterns.org/ont/is/isaac_vanilla.owl#PART_WHOLE> ,
                                           <http://www.ontologydesignpatterns.org/ont/is/isaac_vanilla.owl#SUPPORT> ;
                           isnet:hasActivator <https://w3id.org/framester/data/framestercore/Membership> ,
                                              <https://w3id.org/framester/data/framestercore/Needing> ,
                                              <https://w3id.org/framester/wn/wn30/instances/supersense-noun_group> ,
                                              <https://w3id.org/framester/wn/wn30/instances/synset-body-noun-1> ,
                                              <https://w3id.org/framester/wn/wn30/instances/synset-part-noun-1> .


###  http://www.ontologydesignpatterns.org/ont/odin/odin.owl#EventObjectHeader_Descr
odin:EventObjectHeader_Descr rdf:type owl:NamedIndividual .


###  http://www.ontologydesignpatterns.org/ont/odin/odin.owl#EventObject_Descr
odin:EventObject_Descr rdf:type owl:NamedIndividual ;
                       isnet:activates <http://www.ontologydesignpatterns.org/ont/is/isaac_vanilla.owl#BLOCKAGE> ,
                                       <http://www.ontologydesignpatterns.org/ont/is/isaac_vanilla.owl#CONTAINMENT> ,
                                       <http://www.ontologydesignpatterns.org/ont/is/isaac_vanilla.owl#GOAL> ,
                                       <http://www.ontologydesignpatterns.org/ont/is/isaac_vanilla.owl#PART_WHOLE> ,
                                       <http://www.ontologydesignpatterns.org/ont/is/isaac_vanilla.owl#SOURCE_PATH_GOAL> ;
                       isnet:hasActivator <https://w3id.org/framester/data/framestercore/Containing> ,
                                          <https://w3id.org/framester/data/framestercore/Ingestion> ,
                                          <https://w3id.org/framester/data/framestercore/Membership> ,
                                          <https://w3id.org/framester/data/framestercore/Placing> ,
                                          <https://w3id.org/framester/data/framestercore/Purpose> ,
                                          <https://w3id.org/framester/vn/vn31/data/Contain_54030000> ,
                                          <https://w3id.org/framester/wn/wn30/instances/synset-abstraction-noun-1> ,
                                          <https://w3id.org/framester/wn/wn30/instances/synset-body-noun-1> ,
                                          <https://w3id.org/framester/wn/wn30/instances/synset-incorporate-verb-2> ,
                                          <https://w3id.org/framester/wn/wn30/instances/synset-part-noun-1> ,
                                          <https://w3id.org/framester/wn/wn30/instances/synset-purpose-noun-1> ,
                                          <https://w3id.org/framester/wn/wn30/instances/synset-restriction-noun-1> .


###  http://www.ontologydesignpatterns.org/ont/odin/odin.owl#Event_Descr
odin:Event_Descr rdf:type owl:NamedIndividual ;
                 isnet:activates <http://www.ontologydesignpatterns.org/ont/is/isaac_vanilla.owl#CONTAINMENT> ,
                                 <http://www.ontologydesignpatterns.org/ont/is/isaac_vanilla.owl#SUPPORT> ;
                 isnet:hasActivator <https://w3id.org/framester/data/framestercore/Assistance> ,
                                    <https://w3id.org/framester/data/framestercore/Ingestion> ,
                                    <https://w3id.org/framester/data/framestercore/Supply> ,
                                    <https://w3id.org/framester/wn/wn30/instances/synset-kind-noun-1> .


###  http://www.ontologydesignpatterns.org/ont/odin/odin.owl#ExternalAgent_Descr
odin:ExternalAgent_Descr rdf:type owl:NamedIndividual .


###  http://www.ontologydesignpatterns.org/ont/odin/odin.owl#File_Descr
odin:File_Descr rdf:type owl:NamedIndividual .


###  http://www.ontologydesignpatterns.org/ont/odin/odin.owl#Fix_Descr
odin:Fix_Descr rdf:type owl:NamedIndividual ;
               isnet:activates <http://www.ontologydesignpatterns.org/ont/is/isaac_vanilla.owl#BLOCKAGE> ,
                               <http://www.ontologydesignpatterns.org/ont/is/isaac_vanilla.owl#PART_WHOLE> ;
               isnet:hasActivator <https://w3id.org/framester/data/framestercore/Predicament> ,
                                  <https://w3id.org/framester/wn/wn30/instances/supersense-noun_group> ,
                                  <https://w3id.org/framester/wn/wn30/instances/synset-fix-noun-1> ,
                                  <https://w3id.org/framester/wn/wn30/instances/synset-point-noun-1> .


###  http://www.ontologydesignpatterns.org/ont/odin/odin.owl#Folksonomy_Descr
odin:Folksonomy_Descr rdf:type owl:NamedIndividual ;
                      isnet:activates <http://www.ontologydesignpatterns.org/ont/is/isaac_vanilla.owl#CONTAINMENT> ,
                                      <http://www.ontologydesignpatterns.org/ont/is/isaac_vanilla.owl#GOAL> ,
                                      <http://www.ontologydesignpatterns.org/ont/is/isaac_vanilla.owl#PART_WHOLE> ,
                                      <http://www.ontologydesignpatterns.org/ont/is/isaac_vanilla.owl#SOURCE_PATH_GOAL> ;
                      isnet:hasActivator <https://w3id.org/framester/data/framestercore/Ingestion> ,
                                         <https://w3id.org/framester/data/framestercore/Purpose> ,
                                         <https://w3id.org/framester/wn/wn30/instances/supersense-noun_group> ,
                                         <https://w3id.org/framester/wn/wn30/instances/synset-purpose-noun-1> .


###  http://www.ontologydesignpatterns.org/ont/odin/odin.owl#Fonds_Descr
odin:Fonds_Descr rdf:type owl:NamedIndividual ;
                 isnet:activates <http://www.ontologydesignpatterns.org/ont/is/isaac_vanilla.owl#PART_WHOLE> ,
                                 <http://www.ontologydesignpatterns.org/ont/is/isaac_vanilla.owl#PATH> ,
                                 <http://www.ontologydesignpatterns.org/ont/is/isaac_vanilla.owl#WHOLE> ;
                 isnet:hasActivator <https://w3id.org/framester/wn/wn30/instances/supersense-noun_group> ,
                                    <https://w3id.org/framester/wn/wn30/instances/synset-body-noun-1> ,
                                    <https://w3id.org/framester/wn/wn30/instances/synset-course-noun-1> ,
                                    <https://w3id.org/framester/wn/wn30/instances/synset-form-noun-1> ,
                                    <https://w3id.org/framester/wn/wn30/instances/synset-whole-noun-1> .


###  http://www.ontologydesignpatterns.org/ont/odin/odin.owl#FormalExpression_Descr
odin:FormalExpression_Descr rdf:type owl:NamedIndividual ;
                            isnet:activates <http://www.ontologydesignpatterns.org/ont/is/isaac_vanilla.owl#CONTAINMENT> ;
                            isnet:hasActivator <https://w3id.org/framester/data/framestercore/Ingestion> ,
                                               <https://w3id.org/framester/wn/wn30/instances/synset-interpretation-noun-1> .


###  http://www.ontologydesignpatterns.org/ont/odin/odin.owl#FormalLanguage_Descr
odin:FormalLanguage_Descr rdf:type owl:NamedIndividual ;
                          isnet:activates <http://www.ontologydesignpatterns.org/ont/is/isaac_vanilla.owl#CONTAINMENT> ;
                          isnet:hasActivator <https://w3id.org/framester/data/framestercore/Ingestion> ,
                                             <https://w3id.org/framester/wn/wn30/instances/synset-interpretation-noun-1> .


###  http://www.ontologydesignpatterns.org/ont/odin/odin.owl#Foundational
odin:Foundational rdf:type owl:NamedIndividual ,
                           odin:ODPType .


###  http://www.ontologydesignpatterns.org/ont/odin/odin.owl#FrameRate_Descr
odin:FrameRate_Descr rdf:type owl:NamedIndividual .


###  http://www.ontologydesignpatterns.org/ont/odin/odin.owl#FrameSize_Descr
odin:FrameSize_Descr rdf:type owl:NamedIndividual .


###  http://www.ontologydesignpatterns.org/ont/odin/odin.owl#GearType_Descr
odin:GearType_Descr rdf:type owl:NamedIndividual .


###  http://www.ontologydesignpatterns.org/ont/odin/odin.owl#Genus_Descr
odin:Genus_Descr rdf:type owl:NamedIndividual ;
                 isnet:activates <http://www.ontologydesignpatterns.org/ont/is/isaac_vanilla.owl#CONTAINMENT> ,
                                 <http://www.ontologydesignpatterns.org/ont/is/isaac_vanilla.owl#PART_WHOLE> ;
                 isnet:hasActivator <https://w3id.org/framester/wn/wn30/instances/supersense-noun_group> ,
                                    <https://w3id.org/framester/wn/wn30/instances/synset-genus-noun-1> .


###  http://www.ontologydesignpatterns.org/ont/odin/odin.owl#GoalSituation_Descr
odin:GoalSituation_Descr rdf:type owl:NamedIndividual .


###  http://www.ontologydesignpatterns.org/ont/odin/odin.owl#Habitat_Descr
odin:Habitat_Descr rdf:type owl:NamedIndividual ;
                   isnet:activates <http://www.ontologydesignpatterns.org/ont/is/isaac_vanilla.owl#CONTAINER> ,
                                   <http://www.ontologydesignpatterns.org/ont/is/isaac_vanilla.owl#PART_WHOLE> ;
                   isnet:hasActivator <https://w3id.org/framester/wn/wn30/instances/supersense-noun_group> ,
                                      <https://w3id.org/framester/wn/wn30/instances/supersense-noun_location> ,
                                      <https://w3id.org/framester/wn/wn30/instances/synset-context-noun-1> .


###  http://www.ontologydesignpatterns.org/ont/odin/odin.owl#Hardware_Descr
odin:Hardware_Descr rdf:type owl:NamedIndividual ;
                    isnet:activates <http://www.ontologydesignpatterns.org/ont/is/isaac_vanilla.owl#CONTAINER> ,
                                    <http://www.ontologydesignpatterns.org/ont/is/isaac_vanilla.owl#PART_WHOLE> ;
                    isnet:hasActivator <https://w3id.org/framester/wn/wn30/instances/supersense-noun_group> ,
                                       <https://w3id.org/framester/wn/wn30/instances/supersense-noun_location> ,
                                       <https://w3id.org/framester/wn/wn30/instances/synset-component-noun-1> .


###  http://www.ontologydesignpatterns.org/ont/odin/odin.owl#IconicLanguage_Descr
odin:IconicLanguage_Descr rdf:type owl:NamedIndividual .


###  http://www.ontologydesignpatterns.org/ont/odin/odin.owl#IconicObject_Descr
odin:IconicObject_Descr rdf:type owl:NamedIndividual .


###  http://www.ontologydesignpatterns.org/ont/odin/odin.owl#ImplementationStatus_Descr
odin:ImplementationStatus_Descr rdf:type owl:NamedIndividual ;
                                isnet:activates <http://www.ontologydesignpatterns.org/ont/is/isaac_vanilla.owl#GOAL> ;
                                isnet:hasActivator <https://w3id.org/framester/wn/wn30/instances/synset-policy-noun-1> .


###  http://www.ontologydesignpatterns.org/ont/odin/odin.owl#InformationObject_Descr
odin:InformationObject_Descr rdf:type owl:NamedIndividual .


###  http://www.ontologydesignpatterns.org/ont/odin/odin.owl#InformationRealization_Descr
odin:InformationRealization_Descr rdf:type owl:NamedIndividual ;
                                  isnet:activates <http://www.ontologydesignpatterns.org/ont/is/isaac_vanilla.owl#CONTAINMENT> ,
                                                  <http://www.ontologydesignpatterns.org/ont/is/isaac_vanilla.owl#PART_WHOLE> ;
                                  isnet:hasActivator <https://w3id.org/framester/data/framestercore/Containing> ,
                                                     <https://w3id.org/framester/data/framestercore/Placing> ,
                                                     <https://w3id.org/framester/vn/vn31/data/Contain_54030000> ,
                                                     <https://w3id.org/framester/wn/wn30/instances/supersense-noun_group> .


###  http://www.ontologydesignpatterns.org/ont/odin/odin.owl#Instant_Descr
odin:Instant_Descr rdf:type owl:NamedIndividual .


###  http://www.ontologydesignpatterns.org/ont/odin/odin.owl#Interval_Descr
odin:Interval_Descr rdf:type owl:NamedIndividual .


###  http://www.ontologydesignpatterns.org/ont/odin/odin.owl#Item_Descr
odin:Item_Descr rdf:type owl:NamedIndividual ;
                isnet:activates <http://www.ontologydesignpatterns.org/ont/is/isaac_vanilla.owl#CONTAINMENT> ;
                isnet:hasActivator <https://w3id.org/framester/data/framestercore/Containers> ,
                                   <https://w3id.org/framester/wn/wn30/instances/synset-bag-noun-1> .


###  http://www.ontologydesignpatterns.org/ont/odin/odin.owl#Kingdom_Descr
odin:Kingdom_Descr rdf:type owl:NamedIndividual ;
                   isnet:activates <http://www.ontologydesignpatterns.org/ont/is/isaac_vanilla.owl#PART_WHOLE> ;
                   isnet:hasActivator <https://w3id.org/framester/wn/wn30/instances/supersense-noun_group> .


###  http://www.ontologydesignpatterns.org/ont/odin/odin.owl#Language_Descr
odin:Language_Descr rdf:type owl:NamedIndividual ;
                    isnet:activates <http://www.ontologydesignpatterns.org/ont/is/isaac_vanilla.owl#GOAL> ;
                    isnet:hasActivator <https://w3id.org/framester/wn/wn30/instances/synset-policy-noun-1> .


###  http://www.ontologydesignpatterns.org/ont/odin/odin.owl#LinguisticObject_Descr
odin:LinguisticObject_Descr rdf:type owl:NamedIndividual .


###  http://www.ontologydesignpatterns.org/ont/odin/odin.owl#ListItem_Descr
odin:ListItem_Descr rdf:type owl:NamedIndividual .


###  http://www.ontologydesignpatterns.org/ont/odin/odin.owl#List_Descr
odin:List_Descr rdf:type owl:NamedIndividual .


###  http://www.ontologydesignpatterns.org/ont/odin/odin.owl#LoopTask_Descr
odin:LoopTask_Descr rdf:type owl:NamedIndividual .


###  http://www.ontologydesignpatterns.org/ont/odin/odin.owl#Manifestation_Descr
odin:Manifestation_Descr rdf:type owl:NamedIndividual ;
                         isnet:activates <http://www.ontologydesignpatterns.org/ont/is/isaac_vanilla.owl#SOURCE_PATH_GOAL> ;
                         isnet:hasActivator <https://w3id.org/framester/data/framestercore/Replacing> .


###  http://www.ontologydesignpatterns.org/ont/odin/odin.owl#MeanOfTransportation_Descr
odin:MeanOfTransportation_Descr rdf:type owl:NamedIndividual .


###  http://www.ontologydesignpatterns.org/ont/odin/odin.owl#Media_Descr
odin:Media_Descr rdf:type owl:NamedIndividual .


###  http://www.ontologydesignpatterns.org/ont/odin/odin.owl#MergingTask_Descr
odin:MergingTask_Descr rdf:type owl:NamedIndividual ;
                       isnet:activates <http://www.ontologydesignpatterns.org/ont/is/isaac_vanilla.owl#PART_WHOLE> ;
                       isnet:hasActivator <https://w3id.org/framester/wn/wn30/instances/supersense-noun_group> .


###  http://www.ontologydesignpatterns.org/ont/odin/odin.owl#MobileObject_Descr
odin:MobileObject_Descr rdf:type owl:NamedIndividual ;
                        isnet:activates <http://www.ontologydesignpatterns.org/ont/is/isaac_vanilla.owl#CONTAINMENT> ,
                                        <http://www.ontologydesignpatterns.org/ont/is/isaac_vanilla.owl#PATH> ,
                                        <http://www.ontologydesignpatterns.org/ont/is/isaac_vanilla.owl#SOURCE_PATH_GOAL> ;
                        isnet:hasActivator <https://w3id.org/framester/data/framestercore/BodyMovement> ,
                                           <https://w3id.org/framester/data/framestercore/Ingestion> ,
                                           <https://w3id.org/framester/data/framestercore/Motion> ,
                                           <https://w3id.org/framester/data/framestercore/Travel> ,
                                           <https://w3id.org/framester/wn/wn30/instances/synset-travel-verb-1> .


###  http://www.ontologydesignpatterns.org/ont/odin/odin.owl#MolecularFunction_Descr
odin:MolecularFunction_Descr rdf:type owl:NamedIndividual ;
                             isnet:activates <http://www.ontologydesignpatterns.org/ont/is/isaac_vanilla.owl#CONTAINMENT> ;
                             isnet:hasActivator <https://w3id.org/framester/data/framestercore/Ingestion> .


###  http://www.ontologydesignpatterns.org/ont/odin/odin.owl#Move_Descr
odin:Move_Descr rdf:type owl:NamedIndividual ;
                isnet:activates <http://www.ontologydesignpatterns.org/ont/is/isaac_vanilla.owl#CONTAINER> ,
                                <http://www.ontologydesignpatterns.org/ont/is/isaac_vanilla.owl#PART_WHOLE> ,
                                <http://www.ontologydesignpatterns.org/ont/is/isaac_vanilla.owl#SOURCE_PATH_GOAL> ;
                isnet:hasActivator <https://w3id.org/framester/data/framestercore/BodyMovement> ,
                                   <https://w3id.org/framester/data/framestercore/Motion> ,
                                   <https://w3id.org/framester/data/framestercore/Origin> ,
                                   <https://w3id.org/framester/data/framestercore/ProcessEnd> ,
                                   <https://w3id.org/framester/data/framestercore/Removing> ,
                                   <https://w3id.org/framester/data/framestercore/SelfMotion> ,
                                   <https://w3id.org/framester/data/framestercore/Travel> ,
                                   <https://w3id.org/framester/vn/vn31/data/Move_11020000> ,
                                   <https://w3id.org/framester/vn/vn31/data/Take_10050000> ,
                                   <https://w3id.org/framester/wn/wn30/instances/supersense-noun_group> ,
                                   <https://w3id.org/framester/wn/wn30/instances/supersense-noun_location> ,
                                   <https://w3id.org/framester/wn/wn30/instances/synset-end-noun-1> .


###  http://www.ontologydesignpatterns.org/ont/odin/odin.owl#MovingObject_Descr
odin:MovingObject_Descr rdf:type owl:NamedIndividual ;
                        isnet:activates <http://www.ontologydesignpatterns.org/ont/is/isaac_vanilla.owl#SOURCE_PATH_GOAL> ;
                        isnet:hasActivator <https://w3id.org/framester/data/framestercore/BodyMovement> ,
                                           <https://w3id.org/framester/data/framestercore/Motion> ,
                                           <https://w3id.org/framester/data/framestercore/SelfMotion> ,
                                           <https://w3id.org/framester/data/framestercore/Travel> ,
                                           <https://w3id.org/framester/vn/vn31/data/Move_11020000> .


###  http://www.ontologydesignpatterns.org/ont/odin/odin.owl#NaturalLanguage_Descr
odin:NaturalLanguage_Descr rdf:type owl:NamedIndividual .


###  http://www.ontologydesignpatterns.org/ont/odin/odin.owl#NaturalPerson_Descr
odin:NaturalPerson_Descr rdf:type owl:NamedIndividual .


###  http://www.ontologydesignpatterns.org/ont/odin/odin.owl#NetworkModule_Descr
odin:NetworkModule_Descr rdf:type owl:NamedIndividual ;
                         isnet:activates <http://www.ontologydesignpatterns.org/ont/is/isaac_vanilla.owl#PART_WHOLE> ,
                                         <http://www.ontologydesignpatterns.org/ont/is/isaac_vanilla.owl#SOURCE_PATH_GOAL> ;
                         isnet:hasActivator <https://w3id.org/framester/data/framestercore/Sending> ,
                                            <https://w3id.org/framester/wn/wn30/instances/supersense-noun_group> ,
                                            <https://w3id.org/framester/wn/wn30/instances/synset-context-noun-1> ,
                                            <https://w3id.org/framester/wn/wn30/instances/synset-form-noun-1> .


###  http://www.ontologydesignpatterns.org/ont/odin/odin.owl#Network_Descr
odin:Network_Descr rdf:type owl:NamedIndividual ;
                   isnet:activates <http://www.ontologydesignpatterns.org/ont/is/isaac_vanilla.owl#PART_WHOLE> ;
                   isnet:hasActivator <https://w3id.org/framester/wn/wn30/instances/supersense-noun_group> .


###  http://www.ontologydesignpatterns.org/ont/odin/odin.owl#NewsEventReporter_Descr
odin:NewsEventReporter_Descr rdf:type owl:NamedIndividual .


###  http://www.ontologydesignpatterns.org/ont/odin/odin.owl#NewsPresentationContext_Descr
odin:NewsPresentationContext_Descr rdf:type owl:NamedIndividual ;
                                   isnet:activates <http://www.ontologydesignpatterns.org/ont/is/isaac_vanilla.owl#CONTAINER> ,
                                                   <http://www.ontologydesignpatterns.org/ont/is/isaac_vanilla.owl#PART_WHOLE> ,
                                                   <http://www.ontologydesignpatterns.org/ont/is/isaac_vanilla.owl#SOURCE_PATH_GOAL> ;
                                   isnet:hasActivator <https://w3id.org/framester/data/framestercore/ProcessEnd> ,
                                                      <https://w3id.org/framester/wn/wn30/instances/supersense-noun_group> ,
                                                      <https://w3id.org/framester/wn/wn30/instances/supersense-noun_location> ,
                                                      <https://w3id.org/framester/wn/wn30/instances/synset-end-noun-1> .


###  http://www.ontologydesignpatterns.org/ont/odin/odin.owl#NewsProvider_Descr
odin:NewsProvider_Descr rdf:type owl:NamedIndividual .


###  http://www.ontologydesignpatterns.org/ont/odin/odin.owl#NewsReportingEvent_Descr
odin:NewsReportingEvent_Descr rdf:type owl:NamedIndividual .


###  http://www.ontologydesignpatterns.org/ont/odin/odin.owl#NodeHolder_Descr
odin:NodeHolder_Descr rdf:type owl:NamedIndividual ;
                      isnet:activates <http://www.ontologydesignpatterns.org/ont/is/isaac_vanilla.owl#PART_WHOLE> ;
                      isnet:hasActivator <https://w3id.org/framester/wn/wn30/instances/supersense-noun_group> .


###  http://www.ontologydesignpatterns.org/ont/odin/odin.owl#NodeStation_Descr
odin:NodeStation_Descr rdf:type owl:NamedIndividual ;
                       isnet:activates <http://www.ontologydesignpatterns.org/ont/is/isaac_vanilla.owl#CONTAINMENT> ,
                                       <http://www.ontologydesignpatterns.org/ont/is/isaac_vanilla.owl#PART_WHOLE> ;
                       isnet:hasActivator <https://w3id.org/framester/data/framestercore/Containing> ,
                                          <https://w3id.org/framester/data/framestercore/Placing> ,
                                          <https://w3id.org/framester/vn/vn31/data/Contain_54030000> ,
                                          <https://w3id.org/framester/wn/wn30/instances/supersense-noun_group> ,
                                          <https://w3id.org/framester/wn/wn30/instances/synset-module-noun-4> .


###  http://www.ontologydesignpatterns.org/ont/odin/odin.owl#Node_Descr
odin:Node_Descr rdf:type owl:NamedIndividual .


###  http://www.ontologydesignpatterns.org/ont/odin/odin.owl#ObjectWithStates.owl_Descr
odin:ObjectWithStates.owl_Descr rdf:type owl:NamedIndividual .


###  http://www.ontologydesignpatterns.org/ont/odin/odin.owl#Object_Descr
odin:Object_Descr rdf:type owl:NamedIndividual .


###  http://www.ontologydesignpatterns.org/ont/odin/odin.owl#Observation_Descr
odin:Observation_Descr rdf:type owl:NamedIndividual .


###  http://www.ontologydesignpatterns.org/ont/odin/odin.owl#Order_Descr
odin:Order_Descr rdf:type owl:NamedIndividual ;
                 isnet:activates <http://www.ontologydesignpatterns.org/ont/is/isaac_vanilla.owl#PART_WHOLE> ;
                 isnet:hasActivator <https://w3id.org/framester/wn/wn30/instances/supersense-noun_group> .


###  http://www.ontologydesignpatterns.org/ont/odin/odin.owl#Parameter_Descr
odin:Parameter_Descr rdf:type owl:NamedIndividual .


###  http://www.ontologydesignpatterns.org/ont/odin/odin.owl#PeriodicInterval.owl_Descr
odin:PeriodicInterval.owl_Descr rdf:type owl:NamedIndividual .


###  http://www.ontologydesignpatterns.org/ont/odin/odin.owl#Person_Descr
odin:Person_Descr rdf:type owl:NamedIndividual .


###  http://www.ontologydesignpatterns.org/ont/odin/odin.owl#Phylum_Descr
odin:Phylum_Descr rdf:type owl:NamedIndividual .


###  http://www.ontologydesignpatterns.org/ont/odin/odin.owl#PhysicalObject_Descr
odin:PhysicalObject_Descr rdf:type owl:NamedIndividual ;
                          isnet:activates <http://www.ontologydesignpatterns.org/ont/is/isaac_vanilla.owl#CONTAINMENT> ,
                                          <http://www.ontologydesignpatterns.org/ont/is/isaac_vanilla.owl#PART_WHOLE> ,
                                          <http://www.ontologydesignpatterns.org/ont/is/isaac_vanilla.owl#SOURCE_PATH_GOAL> ;
                          isnet:hasActivator <https://w3id.org/framester/data/framestercore/BodyMovement> ,
                                             <https://w3id.org/framester/data/framestercore/Ingestion> ,
                                             <https://w3id.org/framester/data/framestercore/Motion> ,
                                             <https://w3id.org/framester/data/framestercore/Travel> ,
                                             <https://w3id.org/framester/wn/wn30/instances/supersense-noun_group> ,
                                             <https://w3id.org/framester/wn/wn30/instances/synset-complete-adjective-1> ,
                                             <https://w3id.org/framester/wn/wn30/instances/synset-kind-noun-1> ,
                                             <https://w3id.org/framester/wn/wn30/instances/synset-separate-verb-1> .


###  http://www.ontologydesignpatterns.org/ont/odin/odin.owl#Place_Descr
odin:Place_Descr rdf:type owl:NamedIndividual ;
                 isnet:activates <http://www.ontologydesignpatterns.org/ont/is/isaac_vanilla.owl#CENTER_PERIPHERY> ,
                                 <http://www.ontologydesignpatterns.org/ont/is/isaac_vanilla.owl#CONTAINER> ,
                                 <http://www.ontologydesignpatterns.org/ont/is/isaac_vanilla.owl#CONTAINMENT> ,
                                 <http://www.ontologydesignpatterns.org/ont/is/isaac_vanilla.owl#PART_WHOLE> ,
                                 <http://www.ontologydesignpatterns.org/ont/is/isaac_vanilla.owl#SOURCE_PATH_GOAL> ,
                                 <http://www.ontologydesignpatterns.org/ont/is/isaac_vanilla.owl#SUPPORT> ;
                 isnet:hasActivator <https://w3id.org/framester/data/framestercore/Assistance> ,
                                    <https://w3id.org/framester/data/framestercore/LocativeRelation> ,
                                    <https://w3id.org/framester/data/framestercore/Motion> ,
                                    <https://w3id.org/framester/data/framestercore/PartInnerOuter> ,
                                    <https://w3id.org/framester/data/framestercore/Roadways> ,
                                    <https://w3id.org/framester/data/framestercore/Travel> ,
                                    <https://w3id.org/framester/wn/wn30/instances/supersense-noun_group> ,
                                    <https://w3id.org/framester/wn/wn30/instances/supersense-noun_location> ,
                                    <https://w3id.org/framester/wn/wn30/instances/synset-context-noun-1> ,
                                    <https://w3id.org/framester/wn/wn30/instances/synset-notion-noun-2> ,
                                    <https://w3id.org/framester/wn/wn30/instances/synset-surface-noun-1> .


###  http://www.ontologydesignpatterns.org/ont/odin/odin.owl#PlanExecution_Descr
odin:PlanExecution_Descr rdf:type owl:NamedIndividual ;
                         isnet:activates <http://www.ontologydesignpatterns.org/ont/is/isaac_vanilla.owl#GOAL> ,
                                         <http://www.ontologydesignpatterns.org/ont/is/isaac_vanilla.owl#SOURCE_PATH_GOAL> ;
                         isnet:hasActivator <https://w3id.org/framester/data/framestercore/Purpose> ,
                                            <https://w3id.org/framester/wn/wn30/instances/synset-plan-noun-1> .


###  http://www.ontologydesignpatterns.org/ont/odin/odin.owl#PlaybackDuration_Descr
odin:PlaybackDuration_Descr rdf:type owl:NamedIndividual .


###  http://www.ontologydesignpatterns.org/ont/odin/odin.owl#PolicyType_Descr
odin:PolicyType_Descr rdf:type owl:NamedIndividual ;
                      isnet:activates <http://www.ontologydesignpatterns.org/ont/is/isaac_vanilla.owl#GOAL> ,
                                      <http://www.ontologydesignpatterns.org/ont/is/isaac_vanilla.owl#PART_WHOLE> ,
                                      <http://www.ontologydesignpatterns.org/ont/is/isaac_vanilla.owl#SOURCE_PATH_GOAL> ;
                      isnet:hasActivator <https://w3id.org/framester/data/framestercore/ComeTogether> ,
                                         <https://w3id.org/framester/data/framestercore/SelfMotion> ,
                                         <https://w3id.org/framester/wn/wn30/instances/supersense-noun_group> ,
                                         <https://w3id.org/framester/wn/wn30/instances/synset-policy-noun-1> .


###  http://www.ontologydesignpatterns.org/ont/odin/odin.owl#Policy_Descr
odin:Policy_Descr rdf:type owl:NamedIndividual ;
                  isnet:activates <http://www.ontologydesignpatterns.org/ont/is/isaac_vanilla.owl#GOAL> ,
                                  <http://www.ontologydesignpatterns.org/ont/is/isaac_vanilla.owl#SOURCE_PATH_GOAL> ;
                  isnet:hasActivator <https://w3id.org/framester/data/framestercore/Accomplishment> ,
                                     <https://w3id.org/framester/data/framestercore/Purpose> ,
                                     <https://w3id.org/framester/vn/vn31/data/Achieve_55020000> ,
                                     <https://w3id.org/framester/wn/wn30/instances/synset-achieve-verb-1> ,
                                     <https://w3id.org/framester/wn/wn30/instances/synset-policy-noun-1> ,
                                     <https://w3id.org/framester/wn/wn30/instances/synset-purpose-noun-1> .


###  http://www.ontologydesignpatterns.org/ont/odin/odin.owl#PresentationContext_Descr
odin:PresentationContext_Descr rdf:type owl:NamedIndividual ;
                               isnet:activates <http://www.ontologydesignpatterns.org/ont/is/isaac_vanilla.owl#CONTAINMENT> ,
                                               <http://www.ontologydesignpatterns.org/ont/is/isaac_vanilla.owl#PART_WHOLE> ;
                               isnet:hasActivator <https://w3id.org/framester/data/framestercore/Containers> ,
                                                  <https://w3id.org/framester/wn/wn30/instances/supersense-noun_group> ,
                                                  <https://w3id.org/framester/wn/wn30/instances/synset-dish-noun-1> .


###  http://www.ontologydesignpatterns.org/ont/odin/odin.owl#Price_Descr
odin:Price_Descr rdf:type owl:NamedIndividual ;
                 isnet:activates <http://www.ontologydesignpatterns.org/ont/is/isaac_vanilla.owl#CONTAINMENT> ;
                 isnet:hasActivator <https://w3id.org/framester/data/framestercore/Ingestion> .


###  http://www.ontologydesignpatterns.org/ont/odin/odin.owl#Process_Descr
odin:Process_Descr rdf:type owl:NamedIndividual ;
                   isnet:activates <http://www.ontologydesignpatterns.org/ont/is/isaac_vanilla.owl#CONTAINMENT> ;
                   isnet:hasActivator <https://w3id.org/framester/data/framestercore/Placing> .


###  http://www.ontologydesignpatterns.org/ont/odin/odin.owl#Quality_Descr
odin:Quality_Descr rdf:type owl:NamedIndividual ;
                   isnet:activates <http://www.ontologydesignpatterns.org/ont/is/isaac_vanilla.owl#CENTER_PERIPHERY> ,
                                   <http://www.ontologydesignpatterns.org/ont/is/isaac_vanilla.owl#CONTAINER> ,
                                   <http://www.ontologydesignpatterns.org/ont/is/isaac_vanilla.owl#CONTAINMENT> ,
                                   <http://www.ontologydesignpatterns.org/ont/is/isaac_vanilla.owl#PART_WHOLE> ;
                   isnet:hasActivator <https://w3id.org/framester/data/framestercore/PartInnerOuter> ,
                                      <https://w3id.org/framester/wn/wn30/instances/supersense-noun_location> ,
                                      <https://w3id.org/framester/wn/wn30/instances/synset-surface-noun-1> .


###  http://www.ontologydesignpatterns.org/ont/odin/odin.owl#RTMS_Code_Descr
odin:RTMS_Code_Descr rdf:type owl:NamedIndividual ;
                     isnet:activates <http://www.ontologydesignpatterns.org/ont/is/isaac_vanilla.owl#PART_WHOLE> ;
                     isnet:hasActivator <https://w3id.org/framester/wn/wn30/instances/supersense-noun_group> .


###  http://www.ontologydesignpatterns.org/ont/odin/odin.owl#RangeType_Descr
odin:RangeType_Descr rdf:type owl:NamedIndividual ;
                     isnet:activates <http://www.ontologydesignpatterns.org/ont/is/isaac_vanilla.owl#CONTAINMENT> ;
                     isnet:hasActivator <https://w3id.org/framester/data/framestercore/Fullness> ,
                                        <https://w3id.org/framester/wn/wn30/instances/synset-full-adjective-1> .


###  http://www.ontologydesignpatterns.org/ont/odin/odin.owl#Reaction_Descr
odin:Reaction_Descr rdf:type owl:NamedIndividual .


###  http://www.ontologydesignpatterns.org/ont/odin/odin.owl#ReceiverNodeStation_Descr
odin:ReceiverNodeStation_Descr rdf:type owl:NamedIndividual ;
                               isnet:activates <http://www.ontologydesignpatterns.org/ont/is/isaac_vanilla.owl#PART_WHOLE> ;
                               isnet:hasActivator <https://w3id.org/framester/data/framestercore/Membership> ,
                                                  <https://w3id.org/framester/wn/wn30/instances/synset-part-noun-1> .


###  http://www.ontologydesignpatterns.org/ont/odin/odin.owl#RecurrentEventSeries_Descr
odin:RecurrentEventSeries_Descr rdf:type owl:NamedIndividual ;
                                isnet:activates <http://www.ontologydesignpatterns.org/ont/is/isaac_vanilla.owl#CONTAINMENT> ,
                                                <http://www.ontologydesignpatterns.org/ont/is/isaac_vanilla.owl#PART_WHOLE> ;
                                isnet:hasActivator <https://w3id.org/framester/data/framestercore/Containing> ,
                                                   <https://w3id.org/framester/data/framestercore/Grasp> ,
                                                   <https://w3id.org/framester/data/framestercore/Ingestion> ,
                                                   <https://w3id.org/framester/data/framestercore/Membership> ,
                                                   <https://w3id.org/framester/data/framestercore/Placing> ,
                                                   <https://w3id.org/framester/vn/vn31/data/Contain_54030000> ,
                                                   <https://w3id.org/framester/wn/wn30/instances/supersense-noun_group> ,
                                                   <https://w3id.org/framester/wn/wn30/instances/synset-intersection-noun-1> ,
                                                   <https://w3id.org/framester/wn/wn30/instances/synset-member-noun-1> .


###  http://www.ontologydesignpatterns.org/ont/odin/odin.owl#Region_Descr
odin:Region_Descr rdf:type owl:NamedIndividual ;
                  isnet:activates <http://www.ontologydesignpatterns.org/ont/is/isaac_vanilla.owl#CONTAINER> ,
                                  <http://www.ontologydesignpatterns.org/ont/is/isaac_vanilla.owl#CONTAINMENT> ;
                  isnet:hasActivator <https://w3id.org/framester/data/framestercore/Grasp> ,
                                     <https://w3id.org/framester/wn/wn30/instances/supersense-noun_location> .


###  http://www.ontologydesignpatterns.org/ont/odin/odin.owl#RequirementLevel_Descr
odin:RequirementLevel_Descr rdf:type owl:NamedIndividual .


###  http://www.ontologydesignpatterns.org/ont/odin/odin.owl#ResourceAbundanceObservation_Descr
odin:ResourceAbundanceObservation_Descr rdf:type owl:NamedIndividual .


###  http://www.ontologydesignpatterns.org/ont/odin/odin.owl#ResourceExploitationObservation_Descr
odin:ResourceExploitationObservation_Descr rdf:type owl:NamedIndividual .


###  http://www.ontologydesignpatterns.org/ont/odin/odin.owl#River_Descr
odin:River_Descr rdf:type owl:NamedIndividual .


###  http://www.ontologydesignpatterns.org/ont/odin/odin.owl#Role_Descr
odin:Role_Descr rdf:type owl:NamedIndividual ;
                isnet:activates <http://www.ontologydesignpatterns.org/ont/is/isaac_vanilla.owl#CONTAINMENT> ;
                isnet:hasActivator <https://w3id.org/framester/wn/wn30/instances/synset-concept-noun-1> .


###  http://www.ontologydesignpatterns.org/ont/odin/odin.owl#SampleRate_Descr
odin:SampleRate_Descr rdf:type owl:NamedIndividual ;
                      isnet:activates <http://www.ontologydesignpatterns.org/ont/is/isaac_vanilla.owl#SOURCE_PATH_GOAL> ;
                      isnet:hasActivator <https://w3id.org/framester/data/framestercore/Motion> ,
                                         <https://w3id.org/framester/data/framestercore/Sending> ,
                                         <https://w3id.org/framester/vn/vn31/data/Carry_11040000> .


###  http://www.ontologydesignpatterns.org/ont/odin/odin.owl#ScanType_Descr
odin:ScanType_Descr rdf:type owl:NamedIndividual .


###  http://www.ontologydesignpatterns.org/ont/odin/odin.owl#Section_Descr
odin:Section_Descr rdf:type owl:NamedIndividual .


###  http://www.ontologydesignpatterns.org/ont/odin/odin.owl#Segment_Descr
odin:Segment_Descr rdf:type owl:NamedIndividual ;
                   isnet:activates <http://www.ontologydesignpatterns.org/ont/is/isaac_vanilla.owl#BLOCKAGE> ,
                                   <http://www.ontologydesignpatterns.org/ont/is/isaac_vanilla.owl#CENTER_PERIPHERY> ,
                                   <http://www.ontologydesignpatterns.org/ont/is/isaac_vanilla.owl#PART_WHOLE> ,
                                   <http://www.ontologydesignpatterns.org/ont/is/isaac_vanilla.owl#SOURCE_PATH_GOAL> ;
                   isnet:hasActivator <https://w3id.org/framester/data/framestercore/BodyMovement> ,
                                      <https://w3id.org/framester/data/framestercore/Departing> ,
                                      <https://w3id.org/framester/data/framestercore/IntentionalTraversing> ,
                                      <https://w3id.org/framester/data/framestercore/Motion> ,
                                      <https://w3id.org/framester/data/framestercore/PathShape> ,
                                      <https://w3id.org/framester/data/framestercore/Predicament> ,
                                      <https://w3id.org/framester/data/framestercore/SelfMotion> ,
                                      <https://w3id.org/framester/data/framestercore/Travel> ,
                                      <https://w3id.org/framester/data/framestercore/Traversing> ,
                                      <https://w3id.org/framester/vn/vn31/data/Move_11020000> ,
                                      <https://w3id.org/framester/vn/vn31/data/Traverse_47080000> ,
                                      <https://w3id.org/framester/wn/wn30/instances/supersense-noun_group> ,
                                      <https://w3id.org/framester/wn/wn30/instances/synset-fix-noun-1> ,
                                      <https://w3id.org/framester/wn/wn30/instances/synset-section-noun-4> .


###  http://www.ontologydesignpatterns.org/ont/odin/odin.owl#SenderNodeStation_Descr
odin:SenderNodeStation_Descr rdf:type owl:NamedIndividual ;
                             isnet:activates <http://www.ontologydesignpatterns.org/ont/is/isaac_vanilla.owl#CONTAINMENT> ;
                             isnet:hasActivator <https://w3id.org/framester/data/framestercore/Containing> ,
                                                <https://w3id.org/framester/data/framestercore/Placing> ,
                                                <https://w3id.org/framester/vn/vn31/data/Contain_54030000> ,
                                                <https://w3id.org/framester/wn/wn30/instances/synset-incorporate-verb-2> .


###  http://www.ontologydesignpatterns.org/ont/odin/odin.owl#Sensor_Descr
odin:Sensor_Descr rdf:type owl:NamedIndividual .


###  http://www.ontologydesignpatterns.org/ont/odin/odin.owl#Series_Descr
odin:Series_Descr rdf:type owl:NamedIndividual ;
                  isnet:activates <http://www.ontologydesignpatterns.org/ont/is/isaac_vanilla.owl#CONTAINMENT> ,
                                  <http://www.ontologydesignpatterns.org/ont/is/isaac_vanilla.owl#GOAL> ,
                                  <http://www.ontologydesignpatterns.org/ont/is/isaac_vanilla.owl#PART_WHOLE> ,
                                  <http://www.ontologydesignpatterns.org/ont/is/isaac_vanilla.owl#SOURCE_PATH_GOAL> ;
                  isnet:hasActivator <https://w3id.org/framester/data/framestercore/Ingestion> ,
                                     <https://w3id.org/framester/data/framestercore/Origin> ,
                                     <https://w3id.org/framester/data/framestercore/Placing> ,
                                     <https://w3id.org/framester/data/framestercore/Purpose> ,
                                     <https://w3id.org/framester/vn/vn31/data/Arrange_26010000> ,
                                     <https://w3id.org/framester/wn/wn30/instances/supersense-noun_group> ,
                                     <https://w3id.org/framester/wn/wn30/instances/synset-form-noun-1> ,
                                     <https://w3id.org/framester/wn/wn30/instances/synset-use-noun-1> .


###  http://www.ontologydesignpatterns.org/ont/odin/odin.owl#SetOfStandards_Descr
odin:SetOfStandards_Descr rdf:type owl:NamedIndividual .


###  http://www.ontologydesignpatterns.org/ont/odin/odin.owl#Set_Descr
odin:Set_Descr rdf:type owl:NamedIndividual .


###  http://www.ontologydesignpatterns.org/ont/odin/odin.owl#SimpleObject_Descr
odin:SimpleObject_Descr rdf:type owl:NamedIndividual ;
                        isnet:activates <http://www.ontologydesignpatterns.org/ont/is/isaac_vanilla.owl#CONTAINMENT> ;
                        isnet:hasActivator <https://w3id.org/framester/data/framestercore/Ingestion> .


###  http://www.ontologydesignpatterns.org/ont/odin/odin.owl#Situation_Descr
odin:Situation_Descr rdf:type owl:NamedIndividual ;
                     isnet:activates <http://www.ontologydesignpatterns.org/ont/is/isaac_vanilla.owl#CONTAINER> ,
                                     <http://www.ontologydesignpatterns.org/ont/is/isaac_vanilla.owl#PART_WHOLE> ,
                                     <http://www.ontologydesignpatterns.org/ont/is/isaac_vanilla.owl#SOURCE_PATH_GOAL> ;
                     isnet:hasActivator <https://w3id.org/framester/data/framestercore/Sending> ,
                                        <https://w3id.org/framester/wn/wn30/instances/supersense-noun_location> ,
                                        <https://w3id.org/framester/wn/wn30/instances/synset-context-noun-1> ,
                                        <https://w3id.org/framester/wn/wn30/instances/synset-form-noun-1> .


###  http://www.ontologydesignpatterns.org/ont/odin/odin.owl#SmartEnvironment_Descr
odin:SmartEnvironment_Descr rdf:type owl:NamedIndividual ;
                            isnet:activates <http://www.ontologydesignpatterns.org/ont/is/isaac_vanilla.owl#CENTER_PERIPHERY> ,
                                            <http://www.ontologydesignpatterns.org/ont/is/isaac_vanilla.owl#CONTAINER> ,
                                            <http://www.ontologydesignpatterns.org/ont/is/isaac_vanilla.owl#PART_WHOLE> ;
                            isnet:hasActivator <https://w3id.org/framester/wn/wn30/instances/supersense-noun_group> ,
                                               <https://w3id.org/framester/wn/wn30/instances/supersense-noun_location> ,
                                               <https://w3id.org/framester/wn/wn30/instances/synset-platform-noun-1> .


###  http://www.ontologydesignpatterns.org/ont/odin/odin.owl#SmartHomeSection_Descr
odin:SmartHomeSection_Descr rdf:type owl:NamedIndividual .


###  http://www.ontologydesignpatterns.org/ont/odin/odin.owl#SmartHome_Object.owl_Descr
odin:SmartHome_Object.owl_Descr rdf:type owl:NamedIndividual ;
                                isnet:activates <http://www.ontologydesignpatterns.org/ont/is/isaac_vanilla.owl#BLOCKAGE> ,
                                                <http://www.ontologydesignpatterns.org/ont/is/isaac_vanilla.owl#CONTAINER> ,
                                                <http://www.ontologydesignpatterns.org/ont/is/isaac_vanilla.owl#PART_WHOLE> ;
                                isnet:hasActivator <https://w3id.org/framester/wn/wn30/instances/supersense-noun_group> ,
                                                   <https://w3id.org/framester/wn/wn30/instances/supersense-noun_location> ,
                                                   <https://w3id.org/framester/wn/wn30/instances/synset-context-noun-1> ,
                                                   <https://w3id.org/framester/wn/wn30/instances/synset-door-noun-1> ,
                                                   <https://w3id.org/framester/wn/wn30/instances/synset-part-noun-1> ,
                                                   <https://w3id.org/framester/wn/wn30/instances/synset-sol-noun-3> .


###  http://www.ontologydesignpatterns.org/ont/odin/odin.owl#SmartObject_Descr
odin:SmartObject_Descr rdf:type owl:NamedIndividual .


###  http://www.ontologydesignpatterns.org/ont/odin/odin.owl#SocialAgent_Descr
odin:SocialAgent_Descr rdf:type owl:NamedIndividual .


###  http://www.ontologydesignpatterns.org/ont/odin/odin.owl#SocialPerson_Descr
odin:SocialPerson_Descr rdf:type owl:NamedIndividual ;
                        isnet:activates <http://www.ontologydesignpatterns.org/ont/is/isaac_vanilla.owl#CONTAINMENT> ,
                                        <http://www.ontologydesignpatterns.org/ont/is/isaac_vanilla.owl#PART_WHOLE> ;
                        isnet:hasActivator <https://w3id.org/framester/data/framestercore/Ingestion> ,
                                           <https://w3id.org/framester/wn/wn30/instances/supersense-noun_group> .


###  http://www.ontologydesignpatterns.org/ont/odin/odin.owl#SourceActivity_Descr
odin:SourceActivity_Descr rdf:type owl:NamedIndividual .


###  http://www.ontologydesignpatterns.org/ont/odin/odin.owl#SourceObject_Descr
odin:SourceObject_Descr rdf:type owl:NamedIndividual .


###  http://www.ontologydesignpatterns.org/ont/odin/odin.owl#SpatialObject_Descr
odin:SpatialObject_Descr rdf:type owl:NamedIndividual .


###  http://www.ontologydesignpatterns.org/ont/odin/odin.owl#SpatioTemporalExtent_Descr
odin:SpatioTemporalExtent_Descr rdf:type owl:NamedIndividual ;
                                isnet:activates <http://www.ontologydesignpatterns.org/ont/is/isaac_vanilla.owl#BLOCKAGE> ,
                                                <http://www.ontologydesignpatterns.org/ont/is/isaac_vanilla.owl#CONTAINMENT> ,
                                                <http://www.ontologydesignpatterns.org/ont/is/isaac_vanilla.owl#PART_WHOLE> ,
                                                <http://www.ontologydesignpatterns.org/ont/is/isaac_vanilla.owl#SOURCE_PATH_GOAL> ;
                                isnet:hasActivator <https://w3id.org/framester/data/framestercore/Adorning> ,
                                                   <https://w3id.org/framester/data/framestercore/Eclipse> ,
                                                   <https://w3id.org/framester/data/framestercore/Filling> ,
                                                   <https://w3id.org/framester/data/framestercore/Ingestion> ,
                                                   <https://w3id.org/framester/data/framestercore/Purpose> ,
                                                   <https://w3id.org/framester/vn/vn31/data/Intend_61000000> ,
                                                   <https://w3id.org/framester/wn/wn30/instances/supersense-noun_group> ,
                                                   <https://w3id.org/framester/wn/wn30/instances/synset-cover-verb-1> ,
                                                   <https://w3id.org/framester/wn/wn30/instances/synset-notion-noun-2> ,
                                                   <https://w3id.org/framester/wn/wn30/instances/synset-overlap-noun-1> .


###  http://www.ontologydesignpatterns.org/ont/odin/odin.owl#SpeciesConditions_Descr
odin:SpeciesConditions_Descr rdf:type owl:NamedIndividual .


###  http://www.ontologydesignpatterns.org/ont/odin/odin.owl#Species_Descr
odin:Species_Descr rdf:type owl:NamedIndividual .


###  http://www.ontologydesignpatterns.org/ont/odin/odin.owl#StartingFix_Descr
odin:StartingFix_Descr rdf:type owl:NamedIndividual ;
                       isnet:activates <http://www.ontologydesignpatterns.org/ont/is/isaac_vanilla.owl#BLOCKAGE> ,
                                       <http://www.ontologydesignpatterns.org/ont/is/isaac_vanilla.owl#PART_WHOLE> ;
                       isnet:hasActivator <https://w3id.org/framester/data/framestercore/Predicament> ,
                                          <https://w3id.org/framester/wn/wn30/instances/supersense-noun_group> ,
                                          <https://w3id.org/framester/wn/wn30/instances/synset-fix-noun-1> .


###  http://www.ontologydesignpatterns.org/ont/odin/odin.owl#StateSet_Descr
odin:StateSet_Descr rdf:type owl:NamedIndividual ;
                    isnet:activates <http://www.ontologydesignpatterns.org/ont/is/isaac_vanilla.owl#CONTAINER> ;
                    isnet:hasActivator <https://w3id.org/framester/wn/wn30/instances/supersense-noun_location> .


###  http://www.ontologydesignpatterns.org/ont/odin/odin.owl#State_Descr
odin:State_Descr rdf:type owl:NamedIndividual .


###  http://www.ontologydesignpatterns.org/ont/odin/odin.owl#Statement_Descr
odin:Statement_Descr rdf:type owl:NamedIndividual ;
                     isnet:activates <http://www.ontologydesignpatterns.org/ont/is/isaac_vanilla.owl#GOAL> ;
                     isnet:hasActivator <https://w3id.org/framester/wn/wn30/instances/synset-policy-noun-1> .


###  http://www.ontologydesignpatterns.org/ont/odin/odin.owl#Stream_Descr
odin:Stream_Descr rdf:type owl:NamedIndividual .


###  http://www.ontologydesignpatterns.org/ont/odin/odin.owl#SubtitleStream_Descr
odin:SubtitleStream_Descr rdf:type owl:NamedIndividual ;
                          isnet:activates <http://www.ontologydesignpatterns.org/ont/is/isaac_vanilla.owl#PART_WHOLE> ,
                                          <http://www.ontologydesignpatterns.org/ont/is/isaac_vanilla.owl#SOURCE_PATH_GOAL> ;
                          isnet:hasActivator <https://w3id.org/framester/data/framestercore/Motion> ,
                                             <https://w3id.org/framester/vn/vn31/data/Carry_11040000> ,
                                             <https://w3id.org/framester/wn/wn30/instances/supersense-noun_group> .


###  http://www.ontologydesignpatterns.org/ont/odin/odin.owl#SubtitleTextFormat_Descr
odin:SubtitleTextFormat_Descr rdf:type owl:NamedIndividual .


###  http://www.ontologydesignpatterns.org/ont/odin/odin.owl#SynchroTask_Descr
odin:SynchroTask_Descr rdf:type owl:NamedIndividual .


###  http://www.ontologydesignpatterns.org/ont/odin/odin.owl#Tag_Descr
odin:Tag_Descr rdf:type owl:NamedIndividual ;
               isnet:activates <http://www.ontologydesignpatterns.org/ont/is/isaac_vanilla.owl#CONTAINMENT> ,
                               <http://www.ontologydesignpatterns.org/ont/is/isaac_vanilla.owl#PART_WHOLE> ,
                               <http://www.ontologydesignpatterns.org/ont/is/isaac_vanilla.owl#PATH> ,
                               <http://www.ontologydesignpatterns.org/ont/is/isaac_vanilla.owl#SOURCE_PATH_GOAL> ;
               isnet:hasActivator <https://w3id.org/framester/data/framestercore/Ingestion> ,
                                  <https://w3id.org/framester/data/framestercore/Travel> ,
                                  <https://w3id.org/framester/wn/wn30/instances/synset-component-noun-1> ,
                                  <https://w3id.org/framester/wn/wn30/instances/synset-image-noun-1> ,
                                  <https://w3id.org/framester/wn/wn30/instances/synset-interpretation-noun-1> ,
                                  <https://w3id.org/framester/wn/wn30/instances/synset-schema-noun-1> ,
                                  <https://w3id.org/framester/wn/wn30/instances/synset-trip-noun-1> .


###  http://www.ontologydesignpatterns.org/ont/odin/odin.owl#Task_Descr
odin:Task_Descr rdf:type owl:NamedIndividual ;
                isnet:activates <http://www.ontologydesignpatterns.org/ont/is/isaac_vanilla.owl#PART_WHOLE> ,
                                <http://www.ontologydesignpatterns.org/ont/is/isaac_vanilla.owl#SOURCE_PATH_GOAL> ;
                isnet:hasActivator <https://w3id.org/framester/data/framestercore/SelfMotion> ,
                                   <https://w3id.org/framester/vn/vn31/data/Undertake_98000000> ,
                                   <https://w3id.org/framester/wn/wn30/instances/synset-piece-noun-1> .


###  http://www.ontologydesignpatterns.org/ont/odin/odin.owl#TemporalDistance_Descr
odin:TemporalDistance_Descr rdf:type owl:NamedIndividual ;
                            isnet:activates <http://www.ontologydesignpatterns.org/ont/is/isaac_vanilla.owl#CENTER_PERIPHERY> ,
                                            <http://www.ontologydesignpatterns.org/ont/is/isaac_vanilla.owl#CONTAINMENT> ,
                                            <http://www.ontologydesignpatterns.org/ont/is/isaac_vanilla.owl#PART_WHOLE> ;
                            isnet:hasActivator <https://w3id.org/framester/data/framestercore/Ingestion> ,
                                               <https://w3id.org/framester/data/framestercore/Range> ,
                                               <https://w3id.org/framester/wn/wn30/instances/supersense-noun_group> ,
                                               <https://w3id.org/framester/wn/wn30/instances/synset-distance-noun-1> .


###  http://www.ontologydesignpatterns.org/ont/odin/odin.owl#TemporalEntity_Descr
odin:TemporalEntity_Descr rdf:type owl:NamedIndividual .


###  http://www.ontologydesignpatterns.org/ont/odin/odin.owl#TimeDuration_Descr
odin:TimeDuration_Descr rdf:type owl:NamedIndividual .


###  http://www.ontologydesignpatterns.org/ont/odin/odin.owl#TimeEntity_Descr
odin:TimeEntity_Descr rdf:type owl:NamedIndividual ;
                      isnet:activates <http://www.ontologydesignpatterns.org/ont/is/isaac_vanilla.owl#PART_WHOLE> ,
                                      <http://www.ontologydesignpatterns.org/ont/is/isaac_vanilla.owl#SUPPORT> ;
                      isnet:hasActivator <https://w3id.org/framester/data/framestercore/Assistance> ,
                                         <https://w3id.org/framester/data/framestercore/Supply> ,
                                         <https://w3id.org/framester/wn/wn30/instances/supersense-noun_group> .


###  http://www.ontologydesignpatterns.org/ont/odin/odin.owl#TimeIndexedClassification_Descr
odin:TimeIndexedClassification_Descr rdf:type owl:NamedIndividual .


###  http://www.ontologydesignpatterns.org/ont/odin/odin.owl#TimeIndexedPartOf_Descr
odin:TimeIndexedPartOf_Descr rdf:type owl:NamedIndividual .


###  http://www.ontologydesignpatterns.org/ont/odin/odin.owl#TimeIndexedParticipation_Descr
odin:TimeIndexedParticipation_Descr rdf:type owl:NamedIndividual .


###  http://www.ontologydesignpatterns.org/ont/odin/odin.owl#TimeIndexedPersonRole_Descr
odin:TimeIndexedPersonRole_Descr rdf:type owl:NamedIndividual .


###  http://www.ontologydesignpatterns.org/ont/odin/odin.owl#TimeIndexedSituation_Descr
odin:TimeIndexedSituation_Descr rdf:type owl:NamedIndividual .


###  http://www.ontologydesignpatterns.org/ont/odin/odin.owl#TimeInterval_Descr
odin:TimeInterval_Descr rdf:type owl:NamedIndividual ;
                        isnet:activates <http://www.ontologydesignpatterns.org/ont/is/isaac_vanilla.owl#CONTAINER> ,
                                        <http://www.ontologydesignpatterns.org/ont/is/isaac_vanilla.owl#CONTAINMENT> ,
                                        <http://www.ontologydesignpatterns.org/ont/is/isaac_vanilla.owl#SOURCE_PATH_GOAL> ;
                        isnet:hasActivator <https://w3id.org/framester/data/framestercore/Aiming> ,
                                           <https://w3id.org/framester/data/framestercore/Goal> ,
                                           <https://w3id.org/framester/data/framestercore/Ingestion> ,
                                           <https://w3id.org/framester/data/framestercore/Placing> ,
                                           <https://w3id.org/framester/data/framestercore/Purpose> ,
                                           <https://w3id.org/framester/vn/vn31/data/Aim_62000000> ,
                                           <https://w3id.org/framester/wn/wn30/instances/supersense-noun_location> .


###  http://www.ontologydesignpatterns.org/ont/odin/odin.owl#TimePeriodMeasurementUnit_Descr
odin:TimePeriodMeasurementUnit_Descr rdf:type owl:NamedIndividual .


###  http://www.ontologydesignpatterns.org/ont/odin/odin.owl#TimePeriod_Descr
odin:TimePeriod_Descr rdf:type owl:NamedIndividual ;
                      isnet:activates <http://www.ontologydesignpatterns.org/ont/is/isaac_vanilla.owl#CENTER_PERIPHERY> ,
                                      <http://www.ontologydesignpatterns.org/ont/is/isaac_vanilla.owl#PART_WHOLE> ;
                      isnet:hasActivator <https://w3id.org/framester/data/framestercore/Range> ,
                                         <https://w3id.org/framester/wn/wn30/instances/supersense-noun_group> ,
                                         <https://w3id.org/framester/wn/wn30/instances/synset-distance-noun-1> .


###  http://www.ontologydesignpatterns.org/ont/odin/odin.owl#Topic_Descr
odin:Topic_Descr rdf:type owl:NamedIndividual ;
                 isnet:activates <http://www.ontologydesignpatterns.org/ont/is/isaac_vanilla.owl#CONTAINER> ,
                                 <http://www.ontologydesignpatterns.org/ont/is/isaac_vanilla.owl#CONTAINMENT> ,
                                 <http://www.ontologydesignpatterns.org/ont/is/isaac_vanilla.owl#PART_WHOLE> ,
                                 <http://www.ontologydesignpatterns.org/ont/is/isaac_vanilla.owl#PERIPHERY> ,
                                 <http://www.ontologydesignpatterns.org/ont/is/isaac_vanilla.owl#SOURCE_PATH_GOAL> ;
                 isnet:hasActivator <https://w3id.org/framester/data/framestercore/Ingestion> ,
                                    <https://w3id.org/framester/data/framestercore/Membership> ,
                                    <https://w3id.org/framester/data/framestercore/Purpose> ,
                                    <https://w3id.org/framester/vn/vn31/data/Intend_61000000> ,
                                    <https://w3id.org/framester/wn/wn30/instances/supersense-noun_group> ,
                                    <https://w3id.org/framester/wn/wn30/instances/supersense-noun_location> ,
                                    <https://w3id.org/framester/wn/wn30/instances/synset-concept-noun-1> ,
                                    <https://w3id.org/framester/wn/wn30/instances/synset-hand-noun-1> ,
                                    <https://w3id.org/framester/wn/wn30/instances/synset-part-noun-1> ,
                                    <https://w3id.org/framester/wn/wn30/instances/synset-there-noun-1> .


###  http://www.ontologydesignpatterns.org/ont/odin/odin.owl#Town_Descr
odin:Town_Descr rdf:type owl:NamedIndividual ;
                isnet:activates <http://www.ontologydesignpatterns.org/ont/is/isaac_vanilla.owl#CONTAINER> ,
                                <http://www.ontologydesignpatterns.org/ont/is/isaac_vanilla.owl#PART_WHOLE> ,
                                <http://www.ontologydesignpatterns.org/ont/is/isaac_vanilla.owl#PERIPHERY> ;
                isnet:hasActivator <https://w3id.org/framester/wn/wn30/instances/supersense-noun_group> ,
                                   <https://w3id.org/framester/wn/wn30/instances/supersense-noun_location> ,
                                   <https://w3id.org/framester/wn/wn30/instances/synset-several-adjectivesatellite-1> ,
                                   <https://w3id.org/framester/wn/wn30/instances/synset-there-noun-1> .


###  http://www.ontologydesignpatterns.org/ont/odin/odin.owl#Trajectory_Descr
odin:Trajectory_Descr rdf:type owl:NamedIndividual .


###  http://www.ontologydesignpatterns.org/ont/odin/odin.owl#Transition_Descr
odin:Transition_Descr rdf:type owl:NamedIndividual ;
                      isnet:activates <http://www.ontologydesignpatterns.org/ont/is/isaac_vanilla.owl#CONTAINMENT> ,
                                      <http://www.ontologydesignpatterns.org/ont/is/isaac_vanilla.owl#GOAL> ,
                                      <http://www.ontologydesignpatterns.org/ont/is/isaac_vanilla.owl#PART_WHOLE> ,
                                      <http://www.ontologydesignpatterns.org/ont/is/isaac_vanilla.owl#SUPPORT> ;
                      isnet:hasActivator <https://w3id.org/framester/data/framestercore/Fullness> ,
                                         <https://w3id.org/framester/data/framestercore/Ingestion> ,
                                         <https://w3id.org/framester/data/framestercore/Needing> ,
                                         <https://w3id.org/framester/data/framestercore/Placing> ,
                                         <https://w3id.org/framester/vn/vn31/data/Underlie_47080000> ,
                                         <https://w3id.org/framester/wn/wn30/instances/supersense-noun_group> ,
                                         <https://w3id.org/framester/wn/wn30/instances/synset-full-adjective-1> ,
                                         <https://w3id.org/framester/wn/wn30/instances/synset-technology-noun-1> .


###  http://www.ontologydesignpatterns.org/ont/odin/odin.owl#TransportEntity_Descr
odin:TransportEntity_Descr rdf:type owl:NamedIndividual ;
                           isnet:activates <http://www.ontologydesignpatterns.org/ont/is/isaac_vanilla.owl#CONTAINMENT> ,
                                           <http://www.ontologydesignpatterns.org/ont/is/isaac_vanilla.owl#PART_WHOLE> ,
                                           <http://www.ontologydesignpatterns.org/ont/is/isaac_vanilla.owl#SOURCE_PATH_GOAL> ;
                           isnet:hasActivator <https://w3id.org/framester/data/framestercore/BodyMovement> ,
                                              <https://w3id.org/framester/data/framestercore/Membership> ,
                                              <https://w3id.org/framester/data/framestercore/Motion> ,
                                              <https://w3id.org/framester/data/framestercore/SelfMotion> ,
                                              <https://w3id.org/framester/data/framestercore/Travel> ,
                                              <https://w3id.org/framester/vn/vn31/data/Move_11020000> ,
                                              <https://w3id.org/framester/wn/wn30/instances/synset-concept-noun-1> ,
                                              <https://w3id.org/framester/wn/wn30/instances/synset-part-noun-1> .


###  http://www.ontologydesignpatterns.org/ont/odin/odin.owl#TransportEvent_Descr
odin:TransportEvent_Descr rdf:type owl:NamedIndividual .


###  http://www.ontologydesignpatterns.org/ont/odin/odin.owl#TransportMechanim_Descr
odin:TransportMechanim_Descr rdf:type owl:NamedIndividual ;
                             isnet:activates <http://www.ontologydesignpatterns.org/ont/is/isaac_vanilla.owl#CONTAINER> ,
                                             <http://www.ontologydesignpatterns.org/ont/is/isaac_vanilla.owl#CONTAINMENT> ,
                                             <http://www.ontologydesignpatterns.org/ont/is/isaac_vanilla.owl#SOURCE_PATH_GOAL> ;
                             isnet:hasActivator <https://w3id.org/framester/data/framestercore/Origin> ,
                                                <https://w3id.org/framester/wn/wn30/instances/supersense-noun_location> ,
                                                <https://w3id.org/framester/wn/wn30/instances/synset-concept-noun-1> .


###  http://www.ontologydesignpatterns.org/ont/odin/odin.owl#UnifyingFactor_Descr
odin:UnifyingFactor_Descr rdf:type owl:NamedIndividual ;
                          isnet:activates <http://www.ontologydesignpatterns.org/ont/is/isaac_vanilla.owl#PART_WHOLE> ;
                          isnet:hasActivator <https://w3id.org/framester/data/framestercore/Membership> ,
                                             <https://w3id.org/framester/wn/wn30/instances/supersense-noun_group> ,
                                             <https://w3id.org/framester/wn/wn30/instances/synset-component-noun-1> ,
                                             <https://w3id.org/framester/wn/wn30/instances/synset-member-noun-1> .


###  http://www.ontologydesignpatterns.org/ont/odin/odin.owl#Version_Descr
odin:Version_Descr rdf:type owl:NamedIndividual .


###  http://www.ontologydesignpatterns.org/ont/odin/odin.owl#VesselType_Descr
odin:VesselType_Descr rdf:type owl:NamedIndividual .


###  http://www.ontologydesignpatterns.org/ont/odin/odin.owl#VideoCodecLevel_Descr
odin:VideoCodecLevel_Descr rdf:type owl:NamedIndividual ;
                           isnet:activates <http://www.ontologydesignpatterns.org/ont/is/isaac_vanilla.owl#PART_WHOLE> ;
                           isnet:hasActivator <https://w3id.org/framester/wn/wn30/instances/supersense-noun_group> .


###  http://www.ontologydesignpatterns.org/ont/odin/odin.owl#VideoCodecProfile_Descr
odin:VideoCodecProfile_Descr rdf:type owl:NamedIndividual ;
                             isnet:activates <http://www.ontologydesignpatterns.org/ont/is/isaac_vanilla.owl#PART_WHOLE> ;
                             isnet:hasActivator <https://w3id.org/framester/wn/wn30/instances/supersense-noun_group> .


###  http://www.ontologydesignpatterns.org/ont/odin/odin.owl#VideoCodec_Descr
odin:VideoCodec_Descr rdf:type owl:NamedIndividual ;
                      isnet:activates <http://www.ontologydesignpatterns.org/ont/is/isaac_vanilla.owl#CONTAINMENT> ;
                      isnet:hasActivator <https://w3id.org/framester/data/framestercore/Filling> ,
                                         <https://w3id.org/framester/data/framestercore/Placing> .


###  http://www.ontologydesignpatterns.org/ont/odin/odin.owl#VideoQualityMeasurement_Descr
odin:VideoQualityMeasurement_Descr rdf:type owl:NamedIndividual .


###  http://www.ontologydesignpatterns.org/ont/odin/odin.owl#VideoQualityMetric_Descr
odin:VideoQualityMetric_Descr rdf:type owl:NamedIndividual .


###  http://www.ontologydesignpatterns.org/ont/odin/odin.owl#VideoStream_Descr
odin:VideoStream_Descr rdf:type owl:NamedIndividual .


###  http://www.ontologydesignpatterns.org/ont/odin/odin.owl#WaterArea_Descr
odin:WaterArea_Descr rdf:type owl:NamedIndividual ;
                     isnet:activates <http://www.ontologydesignpatterns.org/ont/is/isaac_vanilla.owl#CONTAINER> ;
                     isnet:hasActivator <https://w3id.org/framester/wn/wn30/instances/supersense-noun_location> .


###  http://www.ontologydesignpatterns.org/ont/odin/odin.owl#YUVSampleRange_Descr
odin:YUVSampleRange_Descr rdf:type owl:NamedIndividual .


###  http://www.ontologydesignpatterns.org/ont/odin/odin.owl#actionHasParticipant_Descr
odin:actionHasParticipant_Descr rdf:type owl:NamedIndividual .


###  http://www.ontologydesignpatterns.org/ont/odin/odin.owl#actsFor_Descr
odin:actsFor_Descr rdf:type owl:NamedIndividual ;
                   isnet:activates <http://www.ontologydesignpatterns.org/ont/is/isaac_vanilla.owl#CONTAINMENT> ,
                                   <http://www.ontologydesignpatterns.org/ont/is/isaac_vanilla.owl#PART_WHOLE> ;
                   isnet:hasActivator <https://w3id.org/framester/wn/wn30/instances/supersense-noun_group> ,
                                      <https://w3id.org/framester/wn/wn30/instances/synset-principle-noun-1> .


###  http://www.ontologydesignpatterns.org/ont/odin/odin.owl#actsOn_Descr
odin:actsOn_Descr rdf:type owl:NamedIndividual .


###  http://www.ontologydesignpatterns.org/ont/odin/odin.owl#actsThrough_Descr
odin:actsThrough_Descr rdf:type owl:NamedIndividual ;
                       isnet:activates <http://www.ontologydesignpatterns.org/ont/is/isaac_vanilla.owl#CONTAINMENT> ,
                                       <http://www.ontologydesignpatterns.org/ont/is/isaac_vanilla.owl#PART_WHOLE> ;
                       isnet:hasActivator <https://w3id.org/framester/wn/wn30/instances/supersense-noun_group> ,
                                          <https://w3id.org/framester/wn/wn30/instances/synset-principle-noun-1> .


###  http://www.ontologydesignpatterns.org/ont/odin/odin.owl#actuationResults_Descr
odin:actuationResults_Descr rdf:type owl:NamedIndividual .


###  http://www.ontologydesignpatterns.org/ont/odin/odin.owl#affordanceStrength_Descr
odin:affordanceStrength_Descr rdf:type owl:NamedIndividual .


###  http://www.ontologydesignpatterns.org/ont/odin/odin.owl#aquaticresourceobservation.owl_Descr
odin:aquaticresourceobservation.owl_Descr rdf:type owl:NamedIndividual ;
                                          isnet:activates <http://www.ontologydesignpatterns.org/ont/is/isaac_vanilla.owl#CENTER_PERIPHERY> ;
                                          isnet:hasActivator <https://w3id.org/framester/data/framestercore/Range> ,
                                                             <https://w3id.org/framester/wn/wn30/instances/synset-position-noun-3> .


###  http://www.ontologydesignpatterns.org/ont/odin/odin.owl#assignedTo_Descr
odin:assignedTo_Descr rdf:type owl:NamedIndividual ;
                      isnet:activates <http://www.ontologydesignpatterns.org/ont/is/isaac_vanilla.owl#GOAL> ,
                                      <http://www.ontologydesignpatterns.org/ont/is/isaac_vanilla.owl#SOURCE_PATH_GOAL> ;
                      isnet:hasActivator <https://w3id.org/framester/data/framestercore/Purpose> ,
                                         <https://w3id.org/framester/wn/wn30/instances/synset-application-noun-1> ,
                                         <https://w3id.org/framester/wn/wn30/instances/synset-policy-noun-1> .


###  http://www.ontologydesignpatterns.org/ont/odin/odin.owl#atPlace_Descr
odin:atPlace_Descr rdf:type owl:NamedIndividual ;
                   isnet:activates <http://www.ontologydesignpatterns.org/ont/is/isaac_vanilla.owl#CONTAINMENT> ;
                   isnet:hasActivator <https://w3id.org/framester/data/framestercore/Placing> ,
                                      <https://w3id.org/framester/wn/wn30/instances/synset-put-verb-1> .


###  http://www.ontologydesignpatterns.org/ont/odin/odin.owl#atTime_Descr
odin:atTime_Descr rdf:type owl:NamedIndividual .


###  http://www.ontologydesignpatterns.org/ont/odin/odin.owl#bag.owl_Descr
odin:bag.owl_Descr rdf:type owl:NamedIndividual ;
                   isnet:activates <http://www.ontologydesignpatterns.org/ont/is/isaac_vanilla.owl#CONTAINMENT> ,
                                   <http://www.ontologydesignpatterns.org/ont/is/isaac_vanilla.owl#PART_WHOLE> ;
                   isnet:hasActivator <https://w3id.org/framester/data/framestercore/Ingestion> ,
                                      <https://w3id.org/framester/wn/wn30/instances/supersense-noun_group> .


###  http://www.ontologydesignpatterns.org/ont/odin/odin.owl#basicplan.owl_Descr
odin:basicplan.owl_Descr rdf:type owl:NamedIndividual ;
                         isnet:activates <http://www.ontologydesignpatterns.org/ont/is/isaac_vanilla.owl#PART_WHOLE> ;
                         isnet:hasActivator <https://w3id.org/framester/wn/wn30/instances/supersense-noun_group> ,
                                            <https://w3id.org/framester/wn/wn30/instances/synset-partial-adjectivesatellite-1> .


###  http://www.ontologydesignpatterns.org/ont/odin/odin.owl#basicplanexecution.owl_Descr
odin:basicplanexecution.owl_Descr rdf:type owl:NamedIndividual ;
                                  isnet:activates <http://www.ontologydesignpatterns.org/ont/is/isaac_vanilla.owl#CONTAINER> ,
                                                  <http://www.ontologydesignpatterns.org/ont/is/isaac_vanilla.owl#GOAL> ,
                                                  <http://www.ontologydesignpatterns.org/ont/is/isaac_vanilla.owl#PART_WHOLE> ,
                                                  <http://www.ontologydesignpatterns.org/ont/is/isaac_vanilla.owl#SOURCE_PATH_GOAL> ;
                                  isnet:hasActivator <https://w3id.org/framester/data/framestercore/Purpose> ,
                                                     <https://w3id.org/framester/wn/wn30/instances/supersense-noun_group> ,
                                                     <https://w3id.org/framester/wn/wn30/instances/supersense-noun_location> ,
                                                     <https://w3id.org/framester/wn/wn30/instances/synset-plan-noun-1> .


###  http://www.ontologydesignpatterns.org/ont/odin/odin.owl#canBeConfusedWith_Descr
odin:canBeConfusedWith_Descr rdf:type owl:NamedIndividual .


###  http://www.ontologydesignpatterns.org/ont/odin/odin.owl#canBeCrossedByVesselType_Descr
odin:canBeCrossedByVesselType_Descr rdf:type owl:NamedIndividual ;
                                    isnet:activates <http://www.ontologydesignpatterns.org/ont/is/isaac_vanilla.owl#CONTAINMENT> ,
                                                    <http://www.ontologydesignpatterns.org/ont/is/isaac_vanilla.owl#PART_WHOLE> ;
                                    isnet:hasActivator <https://w3id.org/framester/data/framestercore/ComeTogether> ,
                                                       <https://w3id.org/framester/data/framestercore/Ingestion> ,
                                                       <https://w3id.org/framester/wn/wn30/instances/supersense-noun_group> .


###  http://www.ontologydesignpatterns.org/ont/odin/odin.owl#canCrossWaterArea_Descr
odin:canCrossWaterArea_Descr rdf:type owl:NamedIndividual ;
                             isnet:activates <http://www.ontologydesignpatterns.org/ont/is/isaac_vanilla.owl#CONTAINMENT> ,
                                             <http://www.ontologydesignpatterns.org/ont/is/isaac_vanilla.owl#PART_WHOLE> ;
                             isnet:hasActivator <https://w3id.org/framester/data/framestercore/ComeTogether> ,
                                                <https://w3id.org/framester/data/framestercore/Ingestion> ,
                                                <https://w3id.org/framester/wn/wn30/instances/supersense-noun_group> .


###  http://www.ontologydesignpatterns.org/ont/odin/odin.owl#catchesSpecies_Descr
odin:catchesSpecies_Descr rdf:type owl:NamedIndividual ;
                          isnet:activates <http://www.ontologydesignpatterns.org/ont/is/isaac_vanilla.owl#CONTAINMENT> ,
                                          <http://www.ontologydesignpatterns.org/ont/is/isaac_vanilla.owl#PART_WHOLE> ;
                          isnet:hasActivator <https://w3id.org/framester/data/framestercore/ComeTogether> ,
                                             <https://w3id.org/framester/data/framestercore/Ingestion> ,
                                             <https://w3id.org/framester/wn/wn30/instances/supersense-noun_group> .


###  http://www.ontologydesignpatterns.org/ont/odin/odin.owl#catchrecord.owl_Descr
odin:catchrecord.owl_Descr rdf:type owl:NamedIndividual ;
                           isnet:activates <http://www.ontologydesignpatterns.org/ont/is/isaac_vanilla.owl#PART_WHOLE> ;
                           isnet:hasActivator <https://w3id.org/framester/wn/wn30/instances/supersense-noun_group> .


###  http://www.ontologydesignpatterns.org/ont/odin/odin.owl#classification.owl_Descr
odin:classification.owl_Descr rdf:type owl:NamedIndividual .


###  http://www.ontologydesignpatterns.org/ont/odin/odin.owl#classifies_Descr
odin:classifies_Descr rdf:type owl:NamedIndividual .


###  http://www.ontologydesignpatterns.org/ont/odin/odin.owl#collectionentity.owl_Descr
odin:collectionentity.owl_Descr rdf:type owl:NamedIndividual ;
                                isnet:activates <http://www.ontologydesignpatterns.org/ont/is/isaac_vanilla.owl#PART_WHOLE> ,
                                                <http://www.ontologydesignpatterns.org/ont/is/isaac_vanilla.owl#SOURCE_PATH_GOAL> ;
                                isnet:hasActivator <https://w3id.org/framester/data/framestercore/Removing> ,
                                                   <https://w3id.org/framester/vn/vn31/data/Extract_10010000> ,
                                                   <https://w3id.org/framester/wn/wn30/instances/supersense-noun_group> ,
                                                   <https://w3id.org/framester/wn/wn30/instances/synset-partial-adjectivesatellite-1> .


###  http://www.ontologydesignpatterns.org/ont/odin/odin.owl#componency.owl_Descr
odin:componency.owl_Descr rdf:type owl:NamedIndividual ;
                          isnet:activates <http://www.ontologydesignpatterns.org/ont/is/isaac_vanilla.owl#PART_WHOLE> ,
                                          <http://www.ontologydesignpatterns.org/ont/is/isaac_vanilla.owl#SOURCE_PATH_GOAL> ;
                          isnet:hasActivator <https://w3id.org/framester/data/framestercore/Membership> ,
                                             <https://w3id.org/framester/data/framestercore/Removing> ,
                                             <https://w3id.org/framester/vn/vn31/data/Extract_10010000> ,
                                             <https://w3id.org/framester/wn/wn30/instances/supersense-noun_group> ,
                                             <https://w3id.org/framester/wn/wn30/instances/synset-part-noun-1> ,
                                             <https://w3id.org/framester/wn/wn30/instances/synset-partial-adjectivesatellite-1> .


###  http://www.ontologydesignpatterns.org/ont/odin/odin.owl#conceptualizes_Descr
odin:conceptualizes_Descr rdf:type owl:NamedIndividual ;
                          isnet:activates <http://www.ontologydesignpatterns.org/ont/is/isaac_vanilla.owl#GOAL> ,
                                          <http://www.ontologydesignpatterns.org/ont/is/isaac_vanilla.owl#PART_WHOLE> ;
                          isnet:hasActivator <https://w3id.org/framester/wn/wn30/instances/supersense-noun_group> ,
                                             <https://w3id.org/framester/wn/wn30/instances/synset-conspiracy-noun-2> .


###  http://www.ontologydesignpatterns.org/ont/odin/odin.owl#consistsOf_Descr
odin:consistsOf_Descr rdf:type owl:NamedIndividual .


###  http://www.ontologydesignpatterns.org/ont/odin/odin.owl#constituency.owl_Descr
odin:constituency.owl_Descr rdf:type owl:NamedIndividual .


###  http://www.ontologydesignpatterns.org/ont/odin/odin.owl#consumes_Descr
odin:consumes_Descr rdf:type owl:NamedIndividual ;
                    isnet:activates <http://www.ontologydesignpatterns.org/ont/is/isaac_vanilla.owl#CONTAINMENT> ;
                    isnet:hasActivator <https://w3id.org/framester/data/framestercore/Ingestion> ,
                                       <https://w3id.org/framester/vn/vn31/data/Consume_66000000> .


###  http://www.ontologydesignpatterns.org/ont/odin/odin.owl#controlledBy_Descr
odin:controlledBy_Descr rdf:type owl:NamedIndividual .


###  http://www.ontologydesignpatterns.org/ont/odin/odin.owl#coparticipation.owl_Descr
odin:coparticipation.owl_Descr rdf:type owl:NamedIndividual ;
                               isnet:activates <http://www.ontologydesignpatterns.org/ont/is/isaac_vanilla.owl#PART_WHOLE> ,
                                               <http://www.ontologydesignpatterns.org/ont/is/isaac_vanilla.owl#SOURCE_PATH_GOAL> ,
                                               <http://www.ontologydesignpatterns.org/ont/is/isaac_vanilla.owl#SUPPORT> ;
                               isnet:hasActivator <http://www.ontologydesignpatterns.org/ont/fred/domain.owl#activator_1> ,
                                                  <https://w3id.org/framester/data/framestercore/Assistance> ,
                                                  <https://w3id.org/framester/data/framestercore/Removing> ,
                                                  <https://w3id.org/framester/data/framestercore/Supply> ,
                                                  <https://w3id.org/framester/vn/vn31/data/Extract_10010000> ,
                                                  <https://w3id.org/framester/wn/wn30/instances/supersense-noun_group> ,
                                                  <https://w3id.org/framester/wn/wn30/instances/synset-complete-adjective-1> ,
                                                  <https://w3id.org/framester/wn/wn30/instances/synset-partial-adjectivesatellite-1> .


###  http://www.ontologydesignpatterns.org/ont/odin/odin.owl#countryOfRecord_Descr
odin:countryOfRecord_Descr rdf:type owl:NamedIndividual .


###  http://www.ontologydesignpatterns.org/ont/odin/odin.owl#defines_Descr
odin:defines_Descr rdf:type owl:NamedIndividual .


###  http://www.ontologydesignpatterns.org/ont/odin/odin.owl#describes_Descr
odin:describes_Descr rdf:type owl:NamedIndividual ;
                     isnet:activates <http://www.ontologydesignpatterns.org/ont/is/isaac_vanilla.owl#CONTAINMENT> ,
                                     <http://www.ontologydesignpatterns.org/ont/is/isaac_vanilla.owl#PART_WHOLE> ,
                                     <http://www.ontologydesignpatterns.org/ont/is/isaac_vanilla.owl#WHOLE> ;
                     isnet:hasActivator <https://w3id.org/framester/data/framestercore/Containers> ,
                                        <https://w3id.org/framester/data/framestercore/Ingestion> ,
                                        <https://w3id.org/framester/wn/wn30/instances/supersense-noun_group> ,
                                        <https://w3id.org/framester/wn/wn30/instances/synset-context-noun-1> ,
                                        <https://w3id.org/framester/wn/wn30/instances/synset-pot-noun-1> ,
                                        <https://w3id.org/framester/wn/wn30/instances/synset-whole-adjective-1> .


###  http://www.ontologydesignpatterns.org/ont/odin/odin.owl#description.owl_Descr
odin:description.owl_Descr rdf:type owl:NamedIndividual ;
                           isnet:activates <http://www.ontologydesignpatterns.org/ont/is/isaac_vanilla.owl#PART_WHOLE> ,
                                           <http://www.ontologydesignpatterns.org/ont/is/isaac_vanilla.owl#SOURCE_PATH_GOAL> ;
                           isnet:hasActivator <https://w3id.org/framester/data/framestercore/Removing> ,
                                              <https://w3id.org/framester/vn/vn31/data/Extract_10010000> ,
                                              <https://w3id.org/framester/wn/wn30/instances/supersense-noun_group> ,
                                              <https://w3id.org/framester/wn/wn30/instances/synset-partial-adjectivesatellite-1> .


###  http://www.ontologydesignpatterns.org/ont/odin/odin.owl#descriptionandsituation.owl_Descr
odin:descriptionandsituation.owl_Descr rdf:type owl:NamedIndividual ;
                                       isnet:activates <http://www.ontologydesignpatterns.org/ont/is/isaac_vanilla.owl#PART_WHOLE> ,
                                                       <http://www.ontologydesignpatterns.org/ont/is/isaac_vanilla.owl#SOURCE_PATH_GOAL> ;
                                       isnet:hasActivator <https://w3id.org/framester/data/framestercore/Removing> ,
                                                          <https://w3id.org/framester/vn/vn31/data/Extract_10010000> ,
                                                          <https://w3id.org/framester/wn/wn30/instances/supersense-noun_group> ,
                                                          <https://w3id.org/framester/wn/wn30/instances/synset-partial-adjectivesatellite-1> .


###  http://www.ontologydesignpatterns.org/ont/odin/odin.owl#directlyFollows_Descr
odin:directlyFollows_Descr rdf:type owl:NamedIndividual .


###  http://www.ontologydesignpatterns.org/ont/odin/odin.owl#directlyPrecedes_Descr
odin:directlyPrecedes_Descr rdf:type owl:NamedIndividual .


###  http://www.ontologydesignpatterns.org/ont/odin/odin.owl#encodedAsSAN_Descr
odin:encodedAsSAN_Descr rdf:type owl:NamedIndividual .


###  http://www.ontologydesignpatterns.org/ont/odin/odin.owl#endsAt_Descr
odin:endsAt_Descr rdf:type owl:NamedIndividual .


###  http://www.ontologydesignpatterns.org/ont/odin/odin.owl#event.owl_Descr
odin:event.owl_Descr rdf:type owl:NamedIndividual ;
                     isnet:activates <http://www.ontologydesignpatterns.org/ont/is/isaac_vanilla.owl#CONTAINMENT> ,
                                     <http://www.ontologydesignpatterns.org/ont/is/isaac_vanilla.owl#PART_WHOLE> ,
                                     <http://www.ontologydesignpatterns.org/ont/is/isaac_vanilla.owl#SUPPORT> ;
                     isnet:hasActivator <https://w3id.org/framester/vn/vn31/data/Happen_48030000> ,
                                        <https://w3id.org/framester/vn/vn31/data/Sit_50000000> ,
                                        <https://w3id.org/framester/wn/wn30/instances/synset-context-noun-1> .


###  http://www.ontologydesignpatterns.org/ont/odin/odin.owl#executesTask_Descr
odin:executesTask_Descr rdf:type owl:NamedIndividual ;
                        isnet:activates <http://www.ontologydesignpatterns.org/ont/is/isaac_vanilla.owl#CENTER_PERIPHERY> ,
                                        <http://www.ontologydesignpatterns.org/ont/is/isaac_vanilla.owl#CONTAINMENT> ,
                                        <http://www.ontologydesignpatterns.org/ont/is/isaac_vanilla.owl#SOURCE_PATH_GOAL> ;
                        isnet:hasActivator <https://w3id.org/framester/data/framestercore/Containers> ,
                                           <https://w3id.org/framester/data/framestercore/Departing> ,
                                           <https://w3id.org/framester/data/framestercore/Placing> ,
                                           <https://w3id.org/framester/wn/wn30/instances/synset-pot-noun-1> .


###  http://www.ontologydesignpatterns.org/ont/odin/odin.owl#farTopicFrom_Descr
odin:farTopicFrom_Descr rdf:type owl:NamedIndividual .


###  http://www.ontologydesignpatterns.org/ont/odin/odin.owl#fishingAreaOfRecord_Descr
odin:fishingAreaOfRecord_Descr rdf:type owl:NamedIndividual ;
                               isnet:activates <http://www.ontologydesignpatterns.org/ont/is/isaac_vanilla.owl#CONTAINER> ,
                                               <http://www.ontologydesignpatterns.org/ont/is/isaac_vanilla.owl#PART_WHOLE> ;
                               isnet:hasActivator <https://w3id.org/framester/wn/wn30/instances/supersense-noun_group> ,
                                                  <https://w3id.org/framester/wn/wn30/instances/supersense-noun_location> .


###  http://www.ontologydesignpatterns.org/ont/odin/odin.owl#follows_Descr
odin:follows_Descr rdf:type owl:NamedIndividual ;
                   isnet:activates <http://www.ontologydesignpatterns.org/ont/is/isaac_vanilla.owl#CONTAINMENT> ,
                                   <http://www.ontologydesignpatterns.org/ont/is/isaac_vanilla.owl#GOAL> ,
                                   <http://www.ontologydesignpatterns.org/ont/is/isaac_vanilla.owl#PART_WHOLE> ,
                                   <http://www.ontologydesignpatterns.org/ont/is/isaac_vanilla.owl#SOURCE_PATH_GOAL> ;
                   isnet:hasActivator <https://w3id.org/framester/data/framestercore/Purpose> ,
                                      <https://w3id.org/framester/data/framestercore/Sending> ,
                                      <https://w3id.org/framester/wn/wn30/instances/supersense-noun_group> ,
                                      <https://w3id.org/framester/wn/wn30/instances/synset-schema-noun-1> ,
                                      <https://w3id.org/framester/wn/wn30/instances/synset-use-noun-1> .


###  http://www.ontologydesignpatterns.org/ont/odin/odin.owl#forCountry_Descr
odin:forCountry_Descr rdf:type owl:NamedIndividual ;
                      isnet:activates <http://www.ontologydesignpatterns.org/ont/is/isaac_vanilla.owl#PART_WHOLE> ;
                      isnet:hasActivator <https://w3id.org/framester/wn/wn30/instances/supersense-noun_group> .


###  http://www.ontologydesignpatterns.org/ont/odin/odin.owl#formallyRepresents_Descr
odin:formallyRepresents_Descr rdf:type owl:NamedIndividual ;
                              isnet:activates <http://www.ontologydesignpatterns.org/ont/is/isaac_vanilla.owl#CONTAINMENT> ,
                                              <http://www.ontologydesignpatterns.org/ont/is/isaac_vanilla.owl#PART_WHOLE> ;
                              isnet:hasActivator <https://w3id.org/framester/data/framestercore/Ingestion> ,
                                                 <https://w3id.org/framester/wn/wn30/instances/supersense-noun_group> ,
                                                 <https://w3id.org/framester/wn/wn30/instances/synset-concept-noun-1> .


###  http://www.ontologydesignpatterns.org/ont/odin/odin.owl#freshProp1_Descr
odin:freshProp1_Descr rdf:type owl:NamedIndividual .


###  http://www.ontologydesignpatterns.org/ont/odin/odin.owl#freshProp2_Descr
odin:freshProp2_Descr rdf:type owl:NamedIndividual .


###  http://www.ontologydesignpatterns.org/ont/odin/odin.owl#fromFishingArea_Descr
odin:fromFishingArea_Descr rdf:type owl:NamedIndividual ;
                           isnet:activates <http://www.ontologydesignpatterns.org/ont/is/isaac_vanilla.owl#CONTAINER> ,
                                           <http://www.ontologydesignpatterns.org/ont/is/isaac_vanilla.owl#PART_WHOLE> ;
                           isnet:hasActivator <https://w3id.org/framester/wn/wn30/instances/supersense-noun_group> ,
                                              <https://w3id.org/framester/wn/wn30/instances/supersense-noun_location> .


###  http://www.ontologydesignpatterns.org/ont/odin/odin.owl#gearwaterarea.owl_Descr
odin:gearwaterarea.owl_Descr rdf:type owl:NamedIndividual ;
                             isnet:activates <http://www.ontologydesignpatterns.org/ont/is/isaac_vanilla.owl#PART_WHOLE> ;
                             isnet:hasActivator <https://w3id.org/framester/wn/wn30/instances/supersense-noun_group> .


###  http://www.ontologydesignpatterns.org/ont/odin/odin.owl#gotop.owl_Descr
odin:gotop.owl_Descr rdf:type owl:NamedIndividual .


###  http://www.ontologydesignpatterns.org/ont/odin/odin.owl#hasActuatingCapability_Descr
odin:hasActuatingCapability_Descr rdf:type owl:NamedIndividual .


###  http://www.ontologydesignpatterns.org/ont/odin/odin.owl#hasActuatingProperty_Descr
odin:hasActuatingProperty_Descr rdf:type owl:NamedIndividual .


###  http://www.ontologydesignpatterns.org/ont/odin/odin.owl#hasAircraft_Descr
odin:hasAircraft_Descr rdf:type owl:NamedIndividual .


###  http://www.ontologydesignpatterns.org/ont/odin/odin.owl#hasAnalogBroadcastStandard_Descr
odin:hasAnalogBroadcastStandard_Descr rdf:type owl:NamedIndividual .


###  http://www.ontologydesignpatterns.org/ont/odin/odin.owl#hasAspectRatio_Descr
odin:hasAspectRatio_Descr rdf:type owl:NamedIndividual .


###  http://www.ontologydesignpatterns.org/ont/odin/odin.owl#hasAttribute_Descr
odin:hasAttribute_Descr rdf:type owl:NamedIndividual .


###  http://www.ontologydesignpatterns.org/ont/odin/odin.owl#hasAudioStream_Descr
odin:hasAudioStream_Descr rdf:type owl:NamedIndividual .


###  http://www.ontologydesignpatterns.org/ont/odin/odin.owl#hasAutomationStatus_Descr
odin:hasAutomationStatus_Descr rdf:type owl:NamedIndividual ;
                               isnet:activates <http://www.ontologydesignpatterns.org/ont/is/isaac_vanilla.owl#GOAL> ;
                               isnet:hasActivator <https://w3id.org/framester/wn/wn30/instances/synset-automation-noun-1> ,
                                                  <https://w3id.org/framester/wn/wn30/instances/synset-policy-noun-1> .


###  http://www.ontologydesignpatterns.org/ont/odin/odin.owl#hasBathymetricRange_Descr
odin:hasBathymetricRange_Descr rdf:type owl:NamedIndividual .


###  http://www.ontologydesignpatterns.org/ont/odin/odin.owl#hasBitRate_Descr
odin:hasBitRate_Descr rdf:type owl:NamedIndividual .


###  http://www.ontologydesignpatterns.org/ont/odin/odin.owl#hasCatchRecord_Descr
odin:hasCatchRecord_Descr rdf:type owl:NamedIndividual ;
                          isnet:activates <http://www.ontologydesignpatterns.org/ont/is/isaac_vanilla.owl#PART_WHOLE> ;
                          isnet:hasActivator <https://w3id.org/framester/wn/wn30/instances/supersense-noun_group> .


###  http://www.ontologydesignpatterns.org/ont/odin/odin.owl#hasChromaFormat_Descr
odin:hasChromaFormat_Descr rdf:type owl:NamedIndividual .


###  http://www.ontologydesignpatterns.org/ont/odin/odin.owl#hasCodingStandard_Descr
odin:hasCodingStandard_Descr rdf:type owl:NamedIndividual .


###  http://www.ontologydesignpatterns.org/ont/odin/odin.owl#hasColourSpaceType_Descr
odin:hasColourSpaceType_Descr rdf:type owl:NamedIndividual ;
                              isnet:activates <http://www.ontologydesignpatterns.org/ont/is/isaac_vanilla.owl#CONTAINMENT> ;
                              isnet:hasActivator <https://w3id.org/framester/wn/wn30/instances/synset-type-noun-1> .


###  http://www.ontologydesignpatterns.org/ont/odin/odin.owl#hasComponent_Descr
odin:hasComponent_Descr rdf:type owl:NamedIndividual ;
                        isnet:activates <http://www.ontologydesignpatterns.org/ont/is/isaac_vanilla.owl#PART_WHOLE> ;
                        isnet:hasActivator <https://w3id.org/framester/wn/wn30/instances/synset-component-noun-1> .


###  http://www.ontologydesignpatterns.org/ont/odin/odin.owl#hasCompressionType_Descr
odin:hasCompressionType_Descr rdf:type owl:NamedIndividual ;
                              isnet:activates <http://www.ontologydesignpatterns.org/ont/is/isaac_vanilla.owl#CONTAINMENT> ;
                              isnet:hasActivator <https://w3id.org/framester/wn/wn30/instances/synset-type-noun-1> .


###  http://www.ontologydesignpatterns.org/ont/odin/odin.owl#hasConstituent_Descr
odin:hasConstituent_Descr rdf:type owl:NamedIndividual .


###  http://www.ontologydesignpatterns.org/ont/odin/odin.owl#hasContext_Descr
odin:hasContext_Descr rdf:type owl:NamedIndividual .


###  http://www.ontologydesignpatterns.org/ont/odin/odin.owl#hasCoreConcept_Descr
odin:hasCoreConcept_Descr rdf:type owl:NamedIndividual ;
                          isnet:activates <http://www.ontologydesignpatterns.org/ont/is/isaac_vanilla.owl#CENTER> ,
                                          <http://www.ontologydesignpatterns.org/ont/is/isaac_vanilla.owl#CONTAINMENT> ,
                                          <http://www.ontologydesignpatterns.org/ont/is/isaac_vanilla.owl#PART_WHOLE> ;
                          isnet:hasActivator <https://w3id.org/framester/wn/wn30/instances/supersense-noun_group> ,
                                             <https://w3id.org/framester/wn/wn30/instances/synset-concept-noun-1> ,
                                             <https://w3id.org/framester/wn/wn30/instances/synset-core-noun-1> .


###  http://www.ontologydesignpatterns.org/ont/odin/odin.owl#hasCreator_Descr
odin:hasCreator_Descr rdf:type owl:NamedIndividual .


###  http://www.ontologydesignpatterns.org/ont/odin/odin.owl#hasDescriptiveSpatialRelation_Descr
odin:hasDescriptiveSpatialRelation_Descr rdf:type owl:NamedIndividual .


###  http://www.ontologydesignpatterns.org/ont/odin/odin.owl#hasDirectHigherRank_Descr
odin:hasDirectHigherRank_Descr rdf:type owl:NamedIndividual ;
                               isnet:activates <http://www.ontologydesignpatterns.org/ont/is/isaac_vanilla.owl#CONTAINER> ,
                                               <http://www.ontologydesignpatterns.org/ont/is/isaac_vanilla.owl#PART_WHOLE> ,
                                               <http://www.ontologydesignpatterns.org/ont/is/isaac_vanilla.owl#PERIPHERY> ;
                               isnet:hasActivator <https://w3id.org/framester/wn/wn30/instances/supersense-noun_group> ,
                                                  <https://w3id.org/framester/wn/wn30/instances/supersense-noun_location> ,
                                                  <https://w3id.org/framester/wn/wn30/instances/synset-there-noun-1> .


###  http://www.ontologydesignpatterns.org/ont/odin/odin.owl#hasDirectLowerRank_Descr
odin:hasDirectLowerRank_Descr rdf:type owl:NamedIndividual ;
                              isnet:activates <http://www.ontologydesignpatterns.org/ont/is/isaac_vanilla.owl#CONTAINER> ,
                                              <http://www.ontologydesignpatterns.org/ont/is/isaac_vanilla.owl#PART_WHOLE> ,
                                              <http://www.ontologydesignpatterns.org/ont/is/isaac_vanilla.owl#PERIPHERY> ;
                              isnet:hasActivator <https://w3id.org/framester/wn/wn30/instances/supersense-noun_group> ,
                                                 <https://w3id.org/framester/wn/wn30/instances/supersense-noun_location> ,
                                                 <https://w3id.org/framester/wn/wn30/instances/synset-there-noun-1> .


###  http://www.ontologydesignpatterns.org/ont/odin/odin.owl#hasDirectSubEventObject_Descr
odin:hasDirectSubEventObject_Descr rdf:type owl:NamedIndividual .


###  http://www.ontologydesignpatterns.org/ont/odin/odin.owl#hasECOCode_Descr
odin:hasECOCode_Descr rdf:type owl:NamedIndividual .


###  http://www.ontologydesignpatterns.org/ont/odin/odin.owl#hasEffect_Descr
odin:hasEffect_Descr rdf:type owl:NamedIndividual .


###  http://www.ontologydesignpatterns.org/ont/odin/odin.owl#hasEmbeddingType_Descr
odin:hasEmbeddingType_Descr rdf:type owl:NamedIndividual ;
                            isnet:activates <http://www.ontologydesignpatterns.org/ont/is/isaac_vanilla.owl#CONTAINMENT> ;
                            isnet:hasActivator <https://w3id.org/framester/data/framestercore/Placing> .


###  http://www.ontologydesignpatterns.org/ont/odin/odin.owl#hasEventDuration_Descr
odin:hasEventDuration_Descr rdf:type owl:NamedIndividual ;
                            isnet:activates <http://www.ontologydesignpatterns.org/ont/is/isaac_vanilla.owl#PART_WHOLE> ;
                            isnet:hasActivator <https://w3id.org/framester/wn/wn30/instances/synset-point-noun-1> .


###  http://www.ontologydesignpatterns.org/ont/odin/odin.owl#hasEventObjectApplicationTime_Descr
odin:hasEventObjectApplicationTime_Descr rdf:type owl:NamedIndividual .


###  http://www.ontologydesignpatterns.org/ont/odin/odin.owl#hasEventObjectBody_Descr
odin:hasEventObjectBody_Descr rdf:type owl:NamedIndividual ;
                              isnet:activates <http://www.ontologydesignpatterns.org/ont/is/isaac_vanilla.owl#PART_WHOLE> ,
                                              <http://www.ontologydesignpatterns.org/ont/is/isaac_vanilla.owl#SUPPORT> ;
                              isnet:hasActivator <https://w3id.org/framester/data/framestercore/Membership> ,
                                                 <https://w3id.org/framester/data/framestercore/Needing> ,
                                                 <https://w3id.org/framester/wn/wn30/instances/supersense-noun_group> ,
                                                 <https://w3id.org/framester/wn/wn30/instances/synset-body-noun-1> ,
                                                 <https://w3id.org/framester/wn/wn30/instances/synset-part-noun-1> .


###  http://www.ontologydesignpatterns.org/ont/odin/odin.owl#hasEventObjectComponent_Descr
odin:hasEventObjectComponent_Descr rdf:type owl:NamedIndividual .


###  http://www.ontologydesignpatterns.org/ont/odin/odin.owl#hasEventObjectHeader_Descr
odin:hasEventObjectHeader_Descr rdf:type owl:NamedIndividual .


###  http://www.ontologydesignpatterns.org/ont/odin/odin.owl#hasEventObjectPart_Descr
odin:hasEventObjectPart_Descr rdf:type owl:NamedIndividual .


###  http://www.ontologydesignpatterns.org/ont/odin/odin.owl#hasEventObjectSystemTime_Descr
odin:hasEventObjectSystemTime_Descr rdf:type owl:NamedIndividual .


###  http://www.ontologydesignpatterns.org/ont/odin/odin.owl#hasFinalStateAtTime_Descr
odin:hasFinalStateAtTime_Descr rdf:type owl:NamedIndividual ;
                               isnet:activates <http://www.ontologydesignpatterns.org/ont/is/isaac_vanilla.owl#CONTAINER> ,
                                               <http://www.ontologydesignpatterns.org/ont/is/isaac_vanilla.owl#SOURCE_PATH_GOAL> ;
                               isnet:hasActivator <https://w3id.org/framester/data/framestercore/ProcessEnd> ,
                                                  <https://w3id.org/framester/wn/wn30/instances/supersense-noun_location> .


###  http://www.ontologydesignpatterns.org/ont/odin/odin.owl#hasFirstItem_Descr
odin:hasFirstItem_Descr rdf:type owl:NamedIndividual .


###  http://www.ontologydesignpatterns.org/ont/odin/odin.owl#hasFix_Descr
odin:hasFix_Descr rdf:type owl:NamedIndividual .


###  http://www.ontologydesignpatterns.org/ont/odin/odin.owl#hasFrameRate_Descr
odin:hasFrameRate_Descr rdf:type owl:NamedIndividual .


###  http://www.ontologydesignpatterns.org/ont/odin/odin.owl#hasFrameSize_Descr
odin:hasFrameSize_Descr rdf:type owl:NamedIndividual .


###  http://www.ontologydesignpatterns.org/ont/odin/odin.owl#hasHigherRank_Descr
odin:hasHigherRank_Descr rdf:type owl:NamedIndividual .


###  http://www.ontologydesignpatterns.org/ont/odin/odin.owl#hasImplementationStatus_Descr
odin:hasImplementationStatus_Descr rdf:type owl:NamedIndividual ;
                                   isnet:activates <http://www.ontologydesignpatterns.org/ont/is/isaac_vanilla.owl#GOAL> ;
                                   isnet:hasActivator <https://w3id.org/framester/wn/wn30/instances/synset-policy-noun-1> .


###  http://www.ontologydesignpatterns.org/ont/odin/odin.owl#hasInclusiveLowerBoundValue_Descr
odin:hasInclusiveLowerBoundValue_Descr rdf:type owl:NamedIndividual ;
                                       isnet:activates <http://www.ontologydesignpatterns.org/ont/is/isaac_vanilla.owl#CONTAINMENT> ,
                                                       <http://www.ontologydesignpatterns.org/ont/is/isaac_vanilla.owl#SOURCE_PATH_GOAL> ;
                                       isnet:hasActivator <https://w3id.org/framester/data/framestercore/Closure> ,
                                                          <https://w3id.org/framester/data/framestercore/SelfMotion> ,
                                                          <https://w3id.org/framester/wn/wn30/instances/synset-concept-noun-1> .


###  http://www.ontologydesignpatterns.org/ont/odin/odin.owl#hasInclusiveUpperBoundValue_Descr
odin:hasInclusiveUpperBoundValue_Descr rdf:type owl:NamedIndividual ;
                                       isnet:activates <http://www.ontologydesignpatterns.org/ont/is/isaac_vanilla.owl#CONTAINMENT> ;
                                       isnet:hasActivator <https://w3id.org/framester/wn/wn30/instances/synset-concept-noun-1> .


###  http://www.ontologydesignpatterns.org/ont/odin/odin.owl#hasInformationObject_Descr
odin:hasInformationObject_Descr rdf:type owl:NamedIndividual .


###  http://www.ontologydesignpatterns.org/ont/odin/odin.owl#hasInitialStateAtTime_Descr
odin:hasInitialStateAtTime_Descr rdf:type owl:NamedIndividual ;
                                 isnet:activates <http://www.ontologydesignpatterns.org/ont/is/isaac_vanilla.owl#CONTAINER> ;
                                 isnet:hasActivator <https://w3id.org/framester/wn/wn30/instances/supersense-noun_location> .


###  http://www.ontologydesignpatterns.org/ont/odin/odin.owl#hasIntervalEndDate_Descr
odin:hasIntervalEndDate_Descr rdf:type owl:NamedIndividual ;
                              isnet:activates <http://www.ontologydesignpatterns.org/ont/is/isaac_vanilla.owl#CONTAINER> ,
                                              <http://www.ontologydesignpatterns.org/ont/is/isaac_vanilla.owl#SOURCE_PATH_GOAL> ;
                              isnet:hasActivator <https://w3id.org/framester/data/framestercore/ProcessEnd> ,
                                                 <https://w3id.org/framester/wn/wn30/instances/supersense-noun_location> ,
                                                 <https://w3id.org/framester/wn/wn30/instances/synset-end-noun-1> .


###  http://www.ontologydesignpatterns.org/ont/odin/odin.owl#hasItem_Descr
odin:hasItem_Descr rdf:type owl:NamedIndividual .


###  http://www.ontologydesignpatterns.org/ont/odin/odin.owl#hasLanguage_Descr
odin:hasLanguage_Descr rdf:type owl:NamedIndividual .


###  http://www.ontologydesignpatterns.org/ont/odin/odin.owl#hasLastItem_Descr
odin:hasLastItem_Descr rdf:type owl:NamedIndividual .


###  http://www.ontologydesignpatterns.org/ont/odin/odin.owl#hasLocalName_Descr
odin:hasLocalName_Descr rdf:type owl:NamedIndividual ;
                        isnet:activates <http://www.ontologydesignpatterns.org/ont/is/isaac_vanilla.owl#CONTAINMENT> ,
                                        <http://www.ontologydesignpatterns.org/ont/is/isaac_vanilla.owl#PART_WHOLE> ,
                                        <http://www.ontologydesignpatterns.org/ont/is/isaac_vanilla.owl#SOURCE_PATH_GOAL> ;
                        isnet:hasActivator <https://w3id.org/framester/data/framestercore/Ingestion> ,
                                           <https://w3id.org/framester/data/framestercore/Sending> ,
                                           <https://w3id.org/framester/wn/wn30/instances/supersense-noun_group> ,
                                           <https://w3id.org/framester/wn/wn30/instances/synset-name-noun-1> .


###  http://www.ontologydesignpatterns.org/ont/odin/odin.owl#hasLocation_Descr
odin:hasLocation_Descr rdf:type owl:NamedIndividual .


###  http://www.ontologydesignpatterns.org/ont/odin/odin.owl#hasLowerRank_Descr
odin:hasLowerRank_Descr rdf:type owl:NamedIndividual .


###  http://www.ontologydesignpatterns.org/ont/odin/odin.owl#hasMember_Descr
odin:hasMember_Descr rdf:type owl:NamedIndividual .


###  http://www.ontologydesignpatterns.org/ont/odin/odin.owl#hasNonInclusiveLowerBoundValue_Descr
odin:hasNonInclusiveLowerBoundValue_Descr rdf:type owl:NamedIndividual ;
                                          isnet:activates <http://www.ontologydesignpatterns.org/ont/is/isaac_vanilla.owl#CONTAINMENT> ,
                                                          <http://www.ontologydesignpatterns.org/ont/is/isaac_vanilla.owl#SOURCE_PATH_GOAL> ;
                                          isnet:hasActivator <https://w3id.org/framester/data/framestercore/Closure> ,
                                                             <https://w3id.org/framester/data/framestercore/SelfMotion> ,
                                                             <https://w3id.org/framester/wn/wn30/instances/synset-concept-noun-1> .


###  http://www.ontologydesignpatterns.org/ont/odin/odin.owl#hasNonInclusiveUpperBoundValue_Descr
odin:hasNonInclusiveUpperBoundValue_Descr rdf:type owl:NamedIndividual .


###  http://www.ontologydesignpatterns.org/ont/odin/odin.owl#hasOutcome_Descr
odin:hasOutcome_Descr rdf:type owl:NamedIndividual .


###  http://www.ontologydesignpatterns.org/ont/odin/odin.owl#hasPGNFile_Descr
odin:hasPGNFile_Descr rdf:type owl:NamedIndividual .


###  http://www.ontologydesignpatterns.org/ont/odin/odin.owl#hasParameterDataValue_Descr
odin:hasParameterDataValue_Descr rdf:type owl:NamedIndividual .


###  http://www.ontologydesignpatterns.org/ont/odin/odin.owl#hasParameter_Descr
odin:hasParameter_Descr rdf:type owl:NamedIndividual ;
                        isnet:activates <http://www.ontologydesignpatterns.org/ont/is/isaac_vanilla.owl#BLOCKAGE> ,
                                        <http://www.ontologydesignpatterns.org/ont/is/isaac_vanilla.owl#CONTAINMENT> ;
                        isnet:hasActivator <https://w3id.org/framester/data/framestercore/Hindering> ,
                                           <https://w3id.org/framester/data/framestercore/Ingestion> ,
                                           <https://w3id.org/framester/vn/vn31/data/Constrain_76000000> ,
                                           <https://w3id.org/framester/wn/wn30/instances/synset-concept-noun-1> .


###  http://www.ontologydesignpatterns.org/ont/odin/odin.owl#hasPart_Descr
odin:hasPart_Descr rdf:type owl:NamedIndividual .


###  http://www.ontologydesignpatterns.org/ont/odin/odin.owl#hasPlaybackDuration_Descr
odin:hasPlaybackDuration_Descr rdf:type owl:NamedIndividual .


###  http://www.ontologydesignpatterns.org/ont/odin/odin.owl#hasPolicyType_Descr
odin:hasPolicyType_Descr rdf:type owl:NamedIndividual ;
                         isnet:activates <http://www.ontologydesignpatterns.org/ont/is/isaac_vanilla.owl#CONTAINMENT> ,
                                         <http://www.ontologydesignpatterns.org/ont/is/isaac_vanilla.owl#GOAL> ;
                         isnet:hasActivator <https://w3id.org/framester/wn/wn30/instances/synset-policy-noun-1> ,
                                            <https://w3id.org/framester/wn/wn30/instances/synset-type-noun-1> .


###  http://www.ontologydesignpatterns.org/ont/odin/odin.owl#hasPowerConsumption_Descr
odin:hasPowerConsumption_Descr rdf:type owl:NamedIndividual ;
                               isnet:activates <http://www.ontologydesignpatterns.org/ont/is/isaac_vanilla.owl#CONTAINER> ,
                                               <http://www.ontologydesignpatterns.org/ont/is/isaac_vanilla.owl#SOURCE_PATH_GOAL> ;
                               isnet:hasActivator <https://w3id.org/framester/data/framestercore/Sending> ,
                                                  <https://w3id.org/framester/wn/wn30/instances/supersense-noun_location> .


###  http://www.ontologydesignpatterns.org/ont/odin/odin.owl#hasPresentationContext_Descr
odin:hasPresentationContext_Descr rdf:type owl:NamedIndividual .


###  http://www.ontologydesignpatterns.org/ont/odin/odin.owl#hasRangeType_Descr
odin:hasRangeType_Descr rdf:type owl:NamedIndividual ;
                        isnet:activates <http://www.ontologydesignpatterns.org/ont/is/isaac_vanilla.owl#CONTAINMENT> ;
                        isnet:hasActivator <https://w3id.org/framester/wn/wn30/instances/synset-type-noun-1> .


###  http://www.ontologydesignpatterns.org/ont/odin/odin.owl#hasRegionDataValue_Descr
odin:hasRegionDataValue_Descr rdf:type owl:NamedIndividual .


###  http://www.ontologydesignpatterns.org/ont/odin/odin.owl#hasRegion_Descr
odin:hasRegion_Descr rdf:type owl:NamedIndividual ;
                     isnet:activates <http://www.ontologydesignpatterns.org/ont/is/isaac_vanilla.owl#CONTAINMENT> ;
                     isnet:hasActivator <https://w3id.org/framester/wn/wn30/instances/synset-truck-noun-1> .


###  http://www.ontologydesignpatterns.org/ont/odin/odin.owl#hasRequirementLevel_Descr
odin:hasRequirementLevel_Descr rdf:type owl:NamedIndividual ;
                               isnet:activates <http://www.ontologydesignpatterns.org/ont/is/isaac_vanilla.owl#GOAL> ;
                               isnet:hasActivator <https://w3id.org/framester/wn/wn30/instances/synset-policy-noun-1> .


###  http://www.ontologydesignpatterns.org/ont/odin/odin.owl#hasRole_Descr
odin:hasRole_Descr rdf:type owl:NamedIndividual ;
                   isnet:activates <http://www.ontologydesignpatterns.org/ont/is/isaac_vanilla.owl#CONTAINMENT> ;
                   isnet:hasActivator <https://w3id.org/framester/data/framestercore/Ingestion> .


###  http://www.ontologydesignpatterns.org/ont/odin/odin.owl#hasSANRecord_Descr
odin:hasSANRecord_Descr rdf:type owl:NamedIndividual .


###  http://www.ontologydesignpatterns.org/ont/odin/odin.owl#hasSampleRate_Descr
odin:hasSampleRate_Descr rdf:type owl:NamedIndividual .


###  http://www.ontologydesignpatterns.org/ont/odin/odin.owl#hasScanType_Descr
odin:hasScanType_Descr rdf:type owl:NamedIndividual ;
                       isnet:activates <http://www.ontologydesignpatterns.org/ont/is/isaac_vanilla.owl#CONTAINMENT> ;
                       isnet:hasActivator <https://w3id.org/framester/wn/wn30/instances/synset-type-noun-1> .


###  http://www.ontologydesignpatterns.org/ont/odin/odin.owl#hasSegment_Descr
odin:hasSegment_Descr rdf:type owl:NamedIndividual .


###  http://www.ontologydesignpatterns.org/ont/odin/odin.owl#hasSensorReadingValue_Descr
odin:hasSensorReadingValue_Descr rdf:type owl:NamedIndividual .


###  http://www.ontologydesignpatterns.org/ont/odin/odin.owl#hasSetOfStandards_Descr
odin:hasSetOfStandards_Descr rdf:type owl:NamedIndividual ;
                             isnet:activates <http://www.ontologydesignpatterns.org/ont/is/isaac_vanilla.owl#PART_WHOLE> ;
                             isnet:hasActivator <https://w3id.org/framester/wn/wn30/instances/supersense-noun_group> .


###  http://www.ontologydesignpatterns.org/ont/odin/odin.owl#hasSetting_Descr
odin:hasSetting_Descr rdf:type owl:NamedIndividual .


###  http://www.ontologydesignpatterns.org/ont/odin/odin.owl#hasSpatialRelation_Descr
odin:hasSpatialRelation_Descr rdf:type owl:NamedIndividual .


###  http://www.ontologydesignpatterns.org/ont/odin/odin.owl#hasSpatioTemporalExtent_Descr
odin:hasSpatioTemporalExtent_Descr rdf:type owl:NamedIndividual .


###  http://www.ontologydesignpatterns.org/ont/odin/odin.owl#hasSpecies_Descr
odin:hasSpecies_Descr rdf:type owl:NamedIndividual ;
                      isnet:activates <http://www.ontologydesignpatterns.org/ont/is/isaac_vanilla.owl#CONTAINMENT> ,
                                      <http://www.ontologydesignpatterns.org/ont/is/isaac_vanilla.owl#PART_WHOLE> ;
                      isnet:hasActivator <https://w3id.org/framester/data/framestercore/Ingestion> ,
                                         <https://w3id.org/framester/wn/wn30/instances/supersense-noun_group> .


###  http://www.ontologydesignpatterns.org/ont/odin/odin.owl#hasState_Descr
odin:hasState_Descr rdf:type owl:NamedIndividual ;
                    isnet:activates <http://www.ontologydesignpatterns.org/ont/is/isaac_vanilla.owl#CONTAINER> ;
                    isnet:hasActivator <https://w3id.org/framester/wn/wn30/instances/supersense-noun_location> .


###  http://www.ontologydesignpatterns.org/ont/odin/odin.owl#hasStatement_Descr
odin:hasStatement_Descr rdf:type owl:NamedIndividual ;
                        isnet:activates <http://www.ontologydesignpatterns.org/ont/is/isaac_vanilla.owl#GOAL> ;
                        isnet:hasActivator <https://w3id.org/framester/wn/wn30/instances/synset-policy-noun-1> .


###  http://www.ontologydesignpatterns.org/ont/odin/odin.owl#hasStream_Descr
odin:hasStream_Descr rdf:type owl:NamedIndividual .


###  http://www.ontologydesignpatterns.org/ont/odin/odin.owl#hasSubEventObject_Descr
odin:hasSubEventObject_Descr rdf:type owl:NamedIndividual .


###  http://www.ontologydesignpatterns.org/ont/odin/odin.owl#hasSubPolicy_Descr
odin:hasSubPolicy_Descr rdf:type owl:NamedIndividual ;
                        isnet:activates <http://www.ontologydesignpatterns.org/ont/is/isaac_vanilla.owl#CONTAINMENT> ,
                                        <http://www.ontologydesignpatterns.org/ont/is/isaac_vanilla.owl#GOAL> ;
                        isnet:hasActivator <https://w3id.org/framester/vn/vn31/data/Contain_54030000> ,
                                           <https://w3id.org/framester/wn/wn30/instances/synset-policy-noun-1> .


###  http://www.ontologydesignpatterns.org/ont/odin/odin.owl#hasSubTopic_Descr
odin:hasSubTopic_Descr rdf:type owl:NamedIndividual .


###  http://www.ontologydesignpatterns.org/ont/odin/odin.owl#hasSubtitleStream_Descr
odin:hasSubtitleStream_Descr rdf:type owl:NamedIndividual .


###  http://www.ontologydesignpatterns.org/ont/odin/odin.owl#hasSubtitleTextFormat_Descr
odin:hasSubtitleTextFormat_Descr rdf:type owl:NamedIndividual .


###  http://www.ontologydesignpatterns.org/ont/odin/odin.owl#hasSynonym_Descr
odin:hasSynonym_Descr rdf:type owl:NamedIndividual ;
                      isnet:activates <http://www.ontologydesignpatterns.org/ont/is/isaac_vanilla.owl#PART_WHOLE> ,
                                      <http://www.ontologydesignpatterns.org/ont/is/isaac_vanilla.owl#SOURCE_PATH_GOAL> ;
                      isnet:hasActivator <https://w3id.org/framester/data/framestercore/Sending> ,
                                         <https://w3id.org/framester/wn/wn30/instances/supersense-noun_group> .


###  http://www.ontologydesignpatterns.org/ont/odin/odin.owl#hasTask_Descr
odin:hasTask_Descr rdf:type owl:NamedIndividual .


###  http://www.ontologydesignpatterns.org/ont/odin/odin.owl#hasTimePeriodBeforeNextEvent_Descr
odin:hasTimePeriodBeforeNextEvent_Descr rdf:type owl:NamedIndividual ;
                                        isnet:activates <http://www.ontologydesignpatterns.org/ont/is/isaac_vanilla.owl#PART_WHOLE> ;
                                        isnet:hasActivator <https://w3id.org/framester/data/framestercore/Membership> ,
                                                           <https://w3id.org/framester/wn/wn30/instances/supersense-noun_group> ,
                                                           <https://w3id.org/framester/wn/wn30/instances/synset-member-noun-1> .


###  http://www.ontologydesignpatterns.org/ont/odin/odin.owl#hasTimePeriodMeasurementUnit_Descr
odin:hasTimePeriodMeasurementUnit_Descr rdf:type owl:NamedIndividual .


###  http://www.ontologydesignpatterns.org/ont/odin/odin.owl#hasTimePeriod_Descr
odin:hasTimePeriod_Descr rdf:type owl:NamedIndividual .


###  http://www.ontologydesignpatterns.org/ont/odin/odin.owl#hasTopic_Descr
odin:hasTopic_Descr rdf:type owl:NamedIndividual ;
                    isnet:activates <http://www.ontologydesignpatterns.org/ont/is/isaac_vanilla.owl#CONTAINER> ;
                    isnet:hasActivator <https://w3id.org/framester/wn/wn30/instances/supersense-noun_location> .


###  http://www.ontologydesignpatterns.org/ont/odin/odin.owl#hasTrajectory_Descr
odin:hasTrajectory_Descr rdf:type owl:NamedIndividual .


###  http://www.ontologydesignpatterns.org/ont/odin/odin.owl#hasUnifyingFactor_Descr
odin:hasUnifyingFactor_Descr rdf:type owl:NamedIndividual ;
                             isnet:activates <http://www.ontologydesignpatterns.org/ont/is/isaac_vanilla.owl#PART_WHOLE> ;
                             isnet:hasActivator <https://w3id.org/framester/wn/wn30/instances/supersense-noun_group> .


###  http://www.ontologydesignpatterns.org/ont/odin/odin.owl#hasValidationProcess_Descr
odin:hasValidationProcess_Descr rdf:type owl:NamedIndividual ;
                                isnet:activates <http://www.ontologydesignpatterns.org/ont/is/isaac_vanilla.owl#GOAL> ;
                                isnet:hasActivator <https://w3id.org/framester/wn/wn30/instances/synset-policy-noun-1> .


###  http://www.ontologydesignpatterns.org/ont/odin/odin.owl#hasVersion_Descr
odin:hasVersion_Descr rdf:type owl:NamedIndividual ;
                      isnet:activates <http://www.ontologydesignpatterns.org/ont/is/isaac_vanilla.owl#GOAL> ;
                      isnet:hasActivator <https://w3id.org/framester/wn/wn30/instances/synset-policy-noun-1> .


###  http://www.ontologydesignpatterns.org/ont/odin/odin.owl#hasVideoCodecLevel_Descr
odin:hasVideoCodecLevel_Descr rdf:type owl:NamedIndividual .


###  http://www.ontologydesignpatterns.org/ont/odin/odin.owl#hasVideoCodecProfile_Descr
odin:hasVideoCodecProfile_Descr rdf:type owl:NamedIndividual .


###  http://www.ontologydesignpatterns.org/ont/odin/odin.owl#hasVideoQualityMeasurement_Descr
odin:hasVideoQualityMeasurement_Descr rdf:type owl:NamedIndividual .


###  http://www.ontologydesignpatterns.org/ont/odin/odin.owl#hasVideoQualityMetric_Descr
odin:hasVideoQualityMetric_Descr rdf:type owl:NamedIndividual .


###  http://www.ontologydesignpatterns.org/ont/odin/odin.owl#hasVideoStream_Descr
odin:hasVideoStream_Descr rdf:type owl:NamedIndividual .


###  http://www.ontologydesignpatterns.org/ont/odin/odin.owl#hasYUVSampleRange_Descr
odin:hasYUVSampleRange_Descr rdf:type owl:NamedIndividual .


###  http://www.ontologydesignpatterns.org/ont/odin/odin.owl#holds_Descr
odin:holds_Descr rdf:type owl:NamedIndividual ;
                 isnet:activates <http://www.ontologydesignpatterns.org/ont/is/isaac_vanilla.owl#CONTAINMENT> ;
                 isnet:hasActivator <https://w3id.org/framester/data/framestercore/Containing> ,
                                    <https://w3id.org/framester/vn/vn31/data/Hold_54030000> .


###  http://www.ontologydesignpatterns.org/ont/odin/odin.owl#impactsState_Descr
odin:impactsState_Descr rdf:type owl:NamedIndividual ;
                        isnet:activates <http://www.ontologydesignpatterns.org/ont/is/isaac_vanilla.owl#CONTAINER> ;
                        isnet:hasActivator <https://w3id.org/framester/wn/wn30/instances/supersense-noun_location> .


###  http://www.ontologydesignpatterns.org/ont/odin/odin.owl#impacts_Descr
odin:impacts_Descr rdf:type owl:NamedIndividual .


###  http://www.ontologydesignpatterns.org/ont/odin/odin.owl#implementedBy_Descr
odin:implementedBy_Descr rdf:type owl:NamedIndividual .


###  http://www.ontologydesignpatterns.org/ont/odin/odin.owl#includesAction_Descr
odin:includesAction_Descr rdf:type owl:NamedIndividual .


###  http://www.ontologydesignpatterns.org/ont/odin/odin.owl#includesAgent_Descr
odin:includesAgent_Descr rdf:type owl:NamedIndividual ;
                         isnet:activates <http://www.ontologydesignpatterns.org/ont/is/isaac_vanilla.owl#CONTAINMENT> ;
                         isnet:hasActivator <https://w3id.org/framester/data/framestercore/Ingestion> .


###  http://www.ontologydesignpatterns.org/ont/odin/odin.owl#includesEvent_Descr
odin:includesEvent_Descr rdf:type owl:NamedIndividual .


###  http://www.ontologydesignpatterns.org/ont/odin/odin.owl#includesFinalSituation_Descr
odin:includesFinalSituation_Descr rdf:type owl:NamedIndividual .


###  http://www.ontologydesignpatterns.org/ont/odin/odin.owl#includesObject_Descr
odin:includesObject_Descr rdf:type owl:NamedIndividual ;
                          isnet:activates <http://www.ontologydesignpatterns.org/ont/is/isaac_vanilla.owl#CONTAINMENT> ;
                          isnet:hasActivator <https://w3id.org/framester/data/framestercore/Ingestion> .


###  http://www.ontologydesignpatterns.org/ont/odin/odin.owl#includesPartObject_Descr
odin:includesPartObject_Descr rdf:type owl:NamedIndividual ;
                              isnet:activates <http://www.ontologydesignpatterns.org/ont/is/isaac_vanilla.owl#PART_WHOLE> ;
                              isnet:hasActivator <https://w3id.org/framester/data/framestercore/Membership> ,
                                                 <https://w3id.org/framester/wn/wn30/instances/synset-part-noun-1> .


###  http://www.ontologydesignpatterns.org/ont/odin/odin.owl#includesProcess_Descr
odin:includesProcess_Descr rdf:type owl:NamedIndividual .


###  http://www.ontologydesignpatterns.org/ont/odin/odin.owl#includesWholeObject_Descr
odin:includesWholeObject_Descr rdf:type owl:NamedIndividual .


###  http://www.ontologydesignpatterns.org/ont/odin/odin.owl#intensionextension.owl_Descr
odin:intensionextension.owl_Descr rdf:type owl:NamedIndividual ;
                                  isnet:activates <http://www.ontologydesignpatterns.org/ont/is/isaac_vanilla.owl#CONTAINMENT> ,
                                                  <http://www.ontologydesignpatterns.org/ont/is/isaac_vanilla.owl#PART_WHOLE> ,
                                                  <http://www.ontologydesignpatterns.org/ont/is/isaac_vanilla.owl#SOURCE_PATH_GOAL> ;
                                  isnet:hasActivator <https://w3id.org/framester/data/framestercore/Removing> ,
                                                     <https://w3id.org/framester/vn/vn31/data/Extract_10010000> ,
                                                     <https://w3id.org/framester/wn/wn30/instances/supersense-noun_group> ,
                                                     <https://w3id.org/framester/wn/wn30/instances/synset-partial-adjectivesatellite-1> ,
                                                     <https://w3id.org/framester/wn/wn30/instances/synset-reference-noun-6> .


###  http://www.ontologydesignpatterns.org/ont/odin/odin.owl#introduces_Descr
odin:introduces_Descr rdf:type owl:NamedIndividual .


###  http://www.ontologydesignpatterns.org/ont/odin/odin.owl#isAbout_Descr
odin:isAbout_Descr rdf:type owl:NamedIndividual ;
                   isnet:activates <http://www.ontologydesignpatterns.org/ont/is/isaac_vanilla.owl#PART_WHOLE> ;
                   isnet:hasActivator <https://w3id.org/framester/wn/wn30/instances/supersense-noun_group> ,
                                      <https://w3id.org/framester/wn/wn30/instances/synset-discourse-noun-1> ,
                                      <https://w3id.org/framester/wn/wn30/instances/synset-noun-noun-1> .


###  http://www.ontologydesignpatterns.org/ont/odin/odin.owl#isBasedOnSourceActivity_Descr
odin:isBasedOnSourceActivity_Descr rdf:type owl:NamedIndividual ;
                                   isnet:activates <http://www.ontologydesignpatterns.org/ont/is/isaac_vanilla.owl#CONTAINER> ,
                                                   <http://www.ontologydesignpatterns.org/ont/is/isaac_vanilla.owl#SOURCE_PATH_GOAL> ;
                                   isnet:hasActivator <https://w3id.org/framester/data/framestercore/Arriving> ,
                                                      <https://w3id.org/framester/data/framestercore/Origin> ,
                                                      <https://w3id.org/framester/wn/wn30/instances/supersense-noun_location> .


###  http://www.ontologydesignpatterns.org/ont/odin/odin.owl#isBasedOnSourceObject_Descr
odin:isBasedOnSourceObject_Descr rdf:type owl:NamedIndividual ;
                                 isnet:activates <http://www.ontologydesignpatterns.org/ont/is/isaac_vanilla.owl#CONTAINER> ,
                                                 <http://www.ontologydesignpatterns.org/ont/is/isaac_vanilla.owl#SOURCE_PATH_GOAL> ;
                                 isnet:hasActivator <https://w3id.org/framester/data/framestercore/Origin> ,
                                                    <https://w3id.org/framester/wn/wn30/instances/supersense-noun_location> .


###  http://www.ontologydesignpatterns.org/ont/odin/odin.owl#isBasedOn_Descr
odin:isBasedOn_Descr rdf:type owl:NamedIndividual ;
                     isnet:activates <http://www.ontologydesignpatterns.org/ont/is/isaac_vanilla.owl#PART_WHOLE> ;
                     isnet:hasActivator <https://w3id.org/framester/data/framestercore/ComeTogether> .


###  http://www.ontologydesignpatterns.org/ont/odin/odin.owl#isBathymetricRangeOf_Descr
odin:isBathymetricRangeOf_Descr rdf:type owl:NamedIndividual .


###  http://www.ontologydesignpatterns.org/ont/odin/odin.owl#isCatchRecordFor_Descr
odin:isCatchRecordFor_Descr rdf:type owl:NamedIndividual ;
                            isnet:activates <http://www.ontologydesignpatterns.org/ont/is/isaac_vanilla.owl#PART_WHOLE> ;
                            isnet:hasActivator <https://w3id.org/framester/wn/wn30/instances/supersense-noun_group> .


###  http://www.ontologydesignpatterns.org/ont/odin/odin.owl#isCaughtBy_Descr
odin:isCaughtBy_Descr rdf:type owl:NamedIndividual ;
                      isnet:activates <http://www.ontologydesignpatterns.org/ont/is/isaac_vanilla.owl#CONTAINMENT> ,
                                      <http://www.ontologydesignpatterns.org/ont/is/isaac_vanilla.owl#PART_WHOLE> ;
                      isnet:hasActivator <https://w3id.org/framester/data/framestercore/ComeTogether> ,
                                         <https://w3id.org/framester/data/framestercore/Ingestion> ,
                                         <https://w3id.org/framester/wn/wn30/instances/supersense-noun_group> .


###  http://www.ontologydesignpatterns.org/ont/odin/odin.owl#isClassifiedBy_Descr
odin:isClassifiedBy_Descr rdf:type owl:NamedIndividual ;
                          isnet:activates <http://www.ontologydesignpatterns.org/ont/is/isaac_vanilla.owl#GOAL> ,
                                          <http://www.ontologydesignpatterns.org/ont/is/isaac_vanilla.owl#SOURCE_PATH_GOAL> ;
                          isnet:hasActivator <https://w3id.org/framester/data/framestercore/Accomplishment> ,
                                             <https://w3id.org/framester/wn/wn30/instances/synset-accomplishment-noun-1> .


###  http://www.ontologydesignpatterns.org/ont/odin/odin.owl#isCompatibleWith_Descr
odin:isCompatibleWith_Descr rdf:type owl:NamedIndividual .


###  http://www.ontologydesignpatterns.org/ont/odin/odin.owl#isComponentOf_Descr
odin:isComponentOf_Descr rdf:type owl:NamedIndividual ;
                         isnet:activates <http://www.ontologydesignpatterns.org/ont/is/isaac_vanilla.owl#PART_WHOLE> ;
                         isnet:hasActivator <https://w3id.org/framester/wn/wn30/instances/synset-component-noun-1> .


###  http://www.ontologydesignpatterns.org/ont/odin/odin.owl#isConceptUsedIn_Descr
odin:isConceptUsedIn_Descr rdf:type owl:NamedIndividual .


###  http://www.ontologydesignpatterns.org/ont/odin/odin.owl#isConceptualizedBy_Descr
odin:isConceptualizedBy_Descr rdf:type owl:NamedIndividual ;
                              isnet:activates <http://www.ontologydesignpatterns.org/ont/is/isaac_vanilla.owl#GOAL> ,
                                              <http://www.ontologydesignpatterns.org/ont/is/isaac_vanilla.owl#SOURCE_PATH_GOAL> ;
                              isnet:hasActivator <https://w3id.org/framester/data/framestercore/Purpose> ,
                                                 <https://w3id.org/framester/wn/wn30/instances/synset-conspiracy-noun-2> ,
                                                 <https://w3id.org/framester/wn/wn30/instances/synset-plan-noun-1> .


###  http://www.ontologydesignpatterns.org/ont/odin/odin.owl#isConstituentOf_Descr
odin:isConstituentOf_Descr rdf:type owl:NamedIndividual ;
                           isnet:activates <http://www.ontologydesignpatterns.org/ont/is/isaac_vanilla.owl#PART_WHOLE> ;
                           isnet:hasActivator <https://w3id.org/framester/data/framestercore/Membership> ,
                                              <https://w3id.org/framester/wn/wn30/instances/synset-component-noun-3> ,
                                              <https://w3id.org/framester/wn/wn30/instances/synset-part-noun-1> ,
                                              <https://w3id.org/framester/wn/wn30/instances/synset-partition-noun-1> .


###  http://www.ontologydesignpatterns.org/ont/odin/odin.owl#isConsumedBy_Descr
odin:isConsumedBy_Descr rdf:type owl:NamedIndividual ;
                        isnet:activates <http://www.ontologydesignpatterns.org/ont/is/isaac_vanilla.owl#CONTAINMENT> ;
                        isnet:hasActivator <https://w3id.org/framester/data/framestercore/Ingestion> .


###  http://www.ontologydesignpatterns.org/ont/odin/odin.owl#isCoreConceptFor_Descr
odin:isCoreConceptFor_Descr rdf:type owl:NamedIndividual .


###  http://www.ontologydesignpatterns.org/ont/odin/odin.owl#isDefinedIn_Descr
odin:isDefinedIn_Descr rdf:type owl:NamedIndividual .


###  http://www.ontologydesignpatterns.org/ont/odin/odin.owl#isDescribedBy_Descr
odin:isDescribedBy_Descr rdf:type owl:NamedIndividual .


###  http://www.ontologydesignpatterns.org/ont/odin/odin.owl#isExecutedIn_Descr
odin:isExecutedIn_Descr rdf:type owl:NamedIndividual ;
                        isnet:activates <http://www.ontologydesignpatterns.org/ont/is/isaac_vanilla.owl#CENTER_PERIPHERY> ,
                                        <http://www.ontologydesignpatterns.org/ont/is/isaac_vanilla.owl#CONTAINMENT> ,
                                        <http://www.ontologydesignpatterns.org/ont/is/isaac_vanilla.owl#SOURCE_PATH_GOAL> ;
                        isnet:hasActivator <https://w3id.org/framester/data/framestercore/Containers> ,
                                           <https://w3id.org/framester/data/framestercore/Departing> ,
                                           <https://w3id.org/framester/data/framestercore/Placing> ,
                                           <https://w3id.org/framester/wn/wn30/instances/synset-pot-noun-1> .


###  http://www.ontologydesignpatterns.org/ont/odin/odin.owl#isFinalSituationIncludedIn_Descr
odin:isFinalSituationIncludedIn_Descr rdf:type owl:NamedIndividual .


###  http://www.ontologydesignpatterns.org/ont/odin/odin.owl#isFormallyRepresentedIn_Descr
odin:isFormallyRepresentedIn_Descr rdf:type owl:NamedIndividual ;
                                   isnet:activates <http://www.ontologydesignpatterns.org/ont/is/isaac_vanilla.owl#CONTAINMENT> ,
                                                   <http://www.ontologydesignpatterns.org/ont/is/isaac_vanilla.owl#PART_WHOLE> ;
                                   isnet:hasActivator <https://w3id.org/framester/data/framestercore/Ingestion> ,
                                                      <https://w3id.org/framester/wn/wn30/instances/supersense-noun_group> ,
                                                      <https://w3id.org/framester/wn/wn30/instances/synset-concept-noun-1> .


###  http://www.ontologydesignpatterns.org/ont/odin/odin.owl#isHeldBy_Descr
odin:isHeldBy_Descr rdf:type owl:NamedIndividual .


###  http://www.ontologydesignpatterns.org/ont/odin/odin.owl#isIntroducedBy_Descr
odin:isIntroducedBy_Descr rdf:type owl:NamedIndividual .


###  http://www.ontologydesignpatterns.org/ont/odin/odin.owl#isLocallyInconsistentWith_Descr
odin:isLocallyInconsistentWith_Descr rdf:type owl:NamedIndividual .


###  http://www.ontologydesignpatterns.org/ont/odin/odin.owl#isLocationOf_Descr
odin:isLocationOf_Descr rdf:type owl:NamedIndividual .


###  http://www.ontologydesignpatterns.org/ont/odin/odin.owl#isOutcomeOf_Descr
odin:isOutcomeOf_Descr rdf:type owl:NamedIndividual .


###  http://www.ontologydesignpatterns.org/ont/odin/odin.owl#isParameterFor_Descr
odin:isParameterFor_Descr rdf:type owl:NamedIndividual ;
                          isnet:activates <http://www.ontologydesignpatterns.org/ont/is/isaac_vanilla.owl#BLOCKAGE> ,
                                          <http://www.ontologydesignpatterns.org/ont/is/isaac_vanilla.owl#CONTAINMENT> ;
                          isnet:hasActivator <https://w3id.org/framester/data/framestercore/Hindering> ,
                                             <https://w3id.org/framester/data/framestercore/Ingestion> ,
                                             <https://w3id.org/framester/vn/vn31/data/Constrain_76000000> ,
                                             <https://w3id.org/framester/wn/wn30/instances/synset-concept-noun-1> .


###  http://www.ontologydesignpatterns.org/ont/odin/odin.owl#isParametrizedBy_Descr
odin:isParametrizedBy_Descr rdf:type owl:NamedIndividual .


###  http://www.ontologydesignpatterns.org/ont/odin/odin.owl#isPartObjectOf_Descr
odin:isPartObjectOf_Descr rdf:type owl:NamedIndividual ;
                          isnet:activates <http://www.ontologydesignpatterns.org/ont/is/isaac_vanilla.owl#PART_WHOLE> ;
                          isnet:hasActivator <https://w3id.org/framester/wn/wn30/instances/synset-part-noun-1> .


###  http://www.ontologydesignpatterns.org/ont/odin/odin.owl#isPartOf_Descr
odin:isPartOf_Descr rdf:type owl:NamedIndividual ;
                    isnet:activates <http://www.ontologydesignpatterns.org/ont/is/isaac_vanilla.owl#BLOCKAGE> ,
                                    <http://www.ontologydesignpatterns.org/ont/is/isaac_vanilla.owl#PART_WHOLE> ,
                                    <http://www.ontologydesignpatterns.org/ont/is/isaac_vanilla.owl#SOURCE_PATH_GOAL> ;
                    isnet:hasActivator <https://w3id.org/framester/data/framestercore/InhibitMovement> ,
                                       <https://w3id.org/framester/data/framestercore/Membership> ,
                                       <https://w3id.org/framester/data/framestercore/Removing> ,
                                       <https://w3id.org/framester/data/framestercore/Sending> ,
                                       <https://w3id.org/framester/vn/vn31/data/Restrict_76000000> ,
                                       <https://w3id.org/framester/vn/vn31/data/Take_10050000> ,
                                       <https://w3id.org/framester/wn/wn30/instances/synset-body-noun-1> ,
                                       <https://w3id.org/framester/wn/wn30/instances/synset-brain-noun-1> ,
                                       <https://w3id.org/framester/wn/wn30/instances/synset-part-noun-1> .


###  http://www.ontologydesignpatterns.org/ont/odin/odin.owl#isParticipantInAction_Descr
odin:isParticipantInAction_Descr rdf:type owl:NamedIndividual .


###  http://www.ontologydesignpatterns.org/ont/odin/odin.owl#isProcessIncludedIn_Descr
odin:isProcessIncludedIn_Descr rdf:type owl:NamedIndividual .


###  http://www.ontologydesignpatterns.org/ont/odin/odin.owl#isRangedByValue_Descr
odin:isRangedByValue_Descr rdf:type owl:NamedIndividual ;
                           isnet:activates <http://www.ontologydesignpatterns.org/ont/is/isaac_vanilla.owl#CONTAINMENT> ,
                                           <http://www.ontologydesignpatterns.org/ont/is/isaac_vanilla.owl#SOURCE_PATH_GOAL> ;
                           isnet:hasActivator <https://w3id.org/framester/data/framestercore/Arriving> ,
                                              <https://w3id.org/framester/wn/wn30/instances/synset-concept-noun-1> .


###  http://www.ontologydesignpatterns.org/ont/odin/odin.owl#isRealizedBy_Descr
odin:isRealizedBy_Descr rdf:type owl:NamedIndividual ;
                        isnet:activates <http://www.ontologydesignpatterns.org/ont/is/isaac_vanilla.owl#CONTAINMENT> ;
                        isnet:hasActivator <https://w3id.org/framester/data/framestercore/Filling> .


###  http://www.ontologydesignpatterns.org/ont/odin/odin.owl#isReferenceOf_Descr
odin:isReferenceOf_Descr rdf:type owl:NamedIndividual ;
                         isnet:activates <http://www.ontologydesignpatterns.org/ont/is/isaac_vanilla.owl#PART_WHOLE> ;
                         isnet:hasActivator <https://w3id.org/framester/wn/wn30/instances/supersense-noun_group> ,
                                            <https://w3id.org/framester/wn/wn30/instances/synset-discourse-noun-1> ,
                                            <https://w3id.org/framester/wn/wn30/instances/synset-noun-noun-1> .


###  http://www.ontologydesignpatterns.org/ont/odin/odin.owl#isRegionFor_Descr
odin:isRegionFor_Descr rdf:type owl:NamedIndividual ;
                       isnet:activates <http://www.ontologydesignpatterns.org/ont/is/isaac_vanilla.owl#CONTAINMENT> ;
                       isnet:hasActivator <https://w3id.org/framester/wn/wn30/instances/synset-car-noun-1> .


###  http://www.ontologydesignpatterns.org/ont/odin/odin.owl#isRoleOf_Descr
odin:isRoleOf_Descr rdf:type owl:NamedIndividual .


###  http://www.ontologydesignpatterns.org/ont/odin/odin.owl#isSatisfiedBy_Descr
odin:isSatisfiedBy_Descr rdf:type owl:NamedIndividual ;
                         isnet:activates <http://www.ontologydesignpatterns.org/ont/is/isaac_vanilla.owl#GOAL> ,
                                         <http://www.ontologydesignpatterns.org/ont/is/isaac_vanilla.owl#SOURCE_PATH_GOAL> ;
                         isnet:hasActivator <https://w3id.org/framester/data/framestercore/Purpose> ,
                                            <https://w3id.org/framester/wn/wn30/instances/synset-plan-noun-1> .


###  http://www.ontologydesignpatterns.org/ont/odin/odin.owl#isStateOf_Descr
odin:isStateOf_Descr rdf:type owl:NamedIndividual ;
                     isnet:activates <http://www.ontologydesignpatterns.org/ont/is/isaac_vanilla.owl#CONTAINER> ,
                                     <http://www.ontologydesignpatterns.org/ont/is/isaac_vanilla.owl#CONTAINMENT> ;
                     isnet:hasActivator <https://w3id.org/framester/data/framestercore/Ingestion> ,
                                        <https://w3id.org/framester/wn/wn30/instances/supersense-noun_location> .


###  http://www.ontologydesignpatterns.org/ont/odin/odin.owl#isSubTopicOf_Descr
odin:isSubTopicOf_Descr rdf:type owl:NamedIndividual .


###  http://www.ontologydesignpatterns.org/ont/odin/odin.owl#isSuitableForGearType_Descr
odin:isSuitableForGearType_Descr rdf:type owl:NamedIndividual ;
                                 isnet:activates <http://www.ontologydesignpatterns.org/ont/is/isaac_vanilla.owl#CONTAINMENT> ,
                                                 <http://www.ontologydesignpatterns.org/ont/is/isaac_vanilla.owl#PART_WHOLE> ;
                                 isnet:hasActivator <https://w3id.org/framester/data/framestercore/ComeTogether> ,
                                                    <https://w3id.org/framester/data/framestercore/Ingestion> ,
                                                    <https://w3id.org/framester/wn/wn30/instances/supersense-noun_group> .


###  http://www.ontologydesignpatterns.org/ont/odin/odin.owl#isTaskOf_Descr
odin:isTaskOf_Descr rdf:type owl:NamedIndividual ;
                    isnet:activates <http://www.ontologydesignpatterns.org/ont/is/isaac_vanilla.owl#CONTAINMENT> ;
                    isnet:hasActivator <https://w3id.org/framester/data/framestercore/Ingestion> .


###  http://www.ontologydesignpatterns.org/ont/odin/odin.owl#isTimePeriodBeforeNextEventOf_Descr
odin:isTimePeriodBeforeNextEventOf_Descr rdf:type owl:NamedIndividual .


###  http://www.ontologydesignpatterns.org/ont/odin/odin.owl#isTimePeriodMeasurementUnitOf_Descr
odin:isTimePeriodMeasurementUnitOf_Descr rdf:type owl:NamedIndividual .


###  http://www.ontologydesignpatterns.org/ont/odin/odin.owl#isTimePeriodOf_Descr
odin:isTimePeriodOf_Descr rdf:type owl:NamedIndividual ;
                          isnet:activates <http://www.ontologydesignpatterns.org/ont/is/isaac_vanilla.owl#CONTAINMENT> ,
                                          <http://www.ontologydesignpatterns.org/ont/is/isaac_vanilla.owl#PART_WHOLE> ;
                          isnet:hasActivator <https://w3id.org/framester/data/framestercore/Ingestion> ,
                                             <https://w3id.org/framester/wn/wn30/instances/supersense-noun_group> .


###  http://www.ontologydesignpatterns.org/ont/odin/odin.owl#isTopicOf_Descr
odin:isTopicOf_Descr rdf:type owl:NamedIndividual .


###  http://www.ontologydesignpatterns.org/ont/odin/odin.owl#isUnifyingFactorOf_Descr
odin:isUnifyingFactorOf_Descr rdf:type owl:NamedIndividual ;
                              isnet:activates <http://www.ontologydesignpatterns.org/ont/is/isaac_vanilla.owl#PART_WHOLE> ;
                              isnet:hasActivator <https://w3id.org/framester/wn/wn30/instances/supersense-noun_group> .


###  http://www.ontologydesignpatterns.org/ont/odin/odin.owl#isUsedInWaterArea_Descr
odin:isUsedInWaterArea_Descr rdf:type owl:NamedIndividual ;
                             isnet:activates <http://www.ontologydesignpatterns.org/ont/is/isaac_vanilla.owl#CONTAINMENT> ,
                                             <http://www.ontologydesignpatterns.org/ont/is/isaac_vanilla.owl#PART_WHOLE> ;
                             isnet:hasActivator <https://w3id.org/framester/data/framestercore/ComeTogether> ,
                                                <https://w3id.org/framester/data/framestercore/Ingestion> ,
                                                <https://w3id.org/framester/wn/wn30/instances/supersense-noun_group> .


###  http://www.ontologydesignpatterns.org/ont/odin/odin.owl#isWholeObjectOf_Descr
odin:isWholeObjectOf_Descr rdf:type owl:NamedIndividual ;
                           isnet:activates <http://www.ontologydesignpatterns.org/ont/is/isaac_vanilla.owl#WHOLE> ;
                           isnet:hasActivator <https://w3id.org/framester/wn/wn30/instances/synset-whole-adjective-1> .


###  http://www.ontologydesignpatterns.org/ont/odin/odin.owl#itemOf_Descr
odin:itemOf_Descr rdf:type owl:NamedIndividual ;
                  isnet:activates <http://www.ontologydesignpatterns.org/ont/is/isaac_vanilla.owl#CONTAINMENT> ;
                  isnet:hasActivator <https://w3id.org/framester/data/framestercore/Containing> ,
                                     <https://w3id.org/framester/data/framestercore/Placing> ,
                                     <https://w3id.org/framester/vn/vn31/data/Contain_54030000> .


###  http://www.ontologydesignpatterns.org/ont/odin/odin.owl#linksToAdministrativeRegion_Descr
odin:linksToAdministrativeRegion_Descr rdf:type owl:NamedIndividual .


###  http://www.ontologydesignpatterns.org/ont/odin/odin.owl#linksToCity_Descr
odin:linksToCity_Descr rdf:type owl:NamedIndividual .


###  http://www.ontologydesignpatterns.org/ont/odin/odin.owl#linksToContinent_Descr
odin:linksToContinent_Descr rdf:type owl:NamedIndividual .


###  http://www.ontologydesignpatterns.org/ont/odin/odin.owl#linksToCountry_Descr
odin:linksToCountry_Descr rdf:type owl:NamedIndividual ;
                          isnet:activates <http://www.ontologydesignpatterns.org/ont/is/isaac_vanilla.owl#PART_WHOLE> ;
                          isnet:hasActivator <https://w3id.org/framester/wn/wn30/instances/supersense-noun_group> .


###  http://www.ontologydesignpatterns.org/ont/odin/odin.owl#linksToEthnicGroup_Descr
odin:linksToEthnicGroup_Descr rdf:type owl:NamedIndividual .


###  http://www.ontologydesignpatterns.org/ont/odin/odin.owl#linksToIsland_Descr
odin:linksToIsland_Descr rdf:type owl:NamedIndividual .


###  http://www.ontologydesignpatterns.org/ont/odin/odin.owl#linksToLanguage_Descr
odin:linksToLanguage_Descr rdf:type owl:NamedIndividual .


###  http://www.ontologydesignpatterns.org/ont/odin/odin.owl#linksToMilitaryConflict_Descr
odin:linksToMilitaryConflict_Descr rdf:type owl:NamedIndividual .


###  http://www.ontologydesignpatterns.org/ont/odin/odin.owl#linksToMusicalArtist_Descr
odin:linksToMusicalArtist_Descr rdf:type owl:NamedIndividual .


###  http://www.ontologydesignpatterns.org/ont/odin/odin.owl#linksToOfficeHolder_Descr
odin:linksToOfficeHolder_Descr rdf:type owl:NamedIndividual .


###  http://www.ontologydesignpatterns.org/ont/odin/odin.owl#linksToPresident_Descr
odin:linksToPresident_Descr rdf:type owl:NamedIndividual .


###  http://www.ontologydesignpatterns.org/ont/odin/odin.owl#linksToRiver_Descr
odin:linksToRiver_Descr rdf:type owl:NamedIndividual .


###  http://www.ontologydesignpatterns.org/ont/odin/odin.owl#linksToTown_Descr
odin:linksToTown_Descr rdf:type owl:NamedIndividual .


###  http://www.ontologydesignpatterns.org/ont/odin/odin.owl#linksToWriter_Descr
odin:linksToWriter_Descr rdf:type owl:NamedIndividual .


###  http://www.ontologydesignpatterns.org/ont/odin/odin.owl#linnaeantaxonomy.owl_Descr
odin:linnaeantaxonomy.owl_Descr rdf:type owl:NamedIndividual ;
                                isnet:activates <http://www.ontologydesignpatterns.org/ont/is/isaac_vanilla.owl#PART_WHOLE> ;
                                isnet:hasActivator <https://w3id.org/framester/wn/wn30/instances/supersense-noun_group> .


###  http://www.ontologydesignpatterns.org/ont/odin/odin.owl#move.owl_Descr
odin:move.owl_Descr rdf:type owl:NamedIndividual .


###  http://www.ontologydesignpatterns.org/ont/odin/odin.owl#movedFrom_Descr
odin:movedFrom_Descr rdf:type owl:NamedIndividual .


###  http://www.ontologydesignpatterns.org/ont/odin/odin.owl#movedTo_Descr
odin:movedTo_Descr rdf:type owl:NamedIndividual ;
                   isnet:activates <http://www.ontologydesignpatterns.org/ont/is/isaac_vanilla.owl#CONTAINER> ,
                                   <http://www.ontologydesignpatterns.org/ont/is/isaac_vanilla.owl#PART_WHOLE> ,
                                   <http://www.ontologydesignpatterns.org/ont/is/isaac_vanilla.owl#SOURCE_PATH_GOAL> ;
                   isnet:hasActivator <https://w3id.org/framester/data/framestercore/Origin> ,
                                      <https://w3id.org/framester/wn/wn30/instances/supersense-noun_group> ,
                                      <https://w3id.org/framester/wn/wn30/instances/supersense-noun_location> .


###  http://www.ontologydesignpatterns.org/ont/odin/odin.owl#naryparticipation.owl_Descr
odin:naryparticipation.owl_Descr rdf:type owl:NamedIndividual ;
                                 isnet:activates <http://www.ontologydesignpatterns.org/ont/is/isaac_vanilla.owl#PART_WHOLE> ,
                                                 <http://www.ontologydesignpatterns.org/ont/is/isaac_vanilla.owl#SOURCE_PATH_GOAL> ;
                                 isnet:hasActivator <https://w3id.org/framester/data/framestercore/Removing> ,
                                                    <https://w3id.org/framester/vn/vn31/data/Extract_10010000> ,
                                                    <https://w3id.org/framester/wn/wn30/instances/supersense-noun_group> ,
                                                    <https://w3id.org/framester/wn/wn30/instances/synset-partial-adjectivesatellite-1> .


###  http://www.ontologydesignpatterns.org/ont/odin/odin.owl#nearTopicTo_Descr
odin:nearTopicTo_Descr rdf:type owl:NamedIndividual ;
                       isnet:activates <http://www.ontologydesignpatterns.org/ont/is/isaac_vanilla.owl#CONTAINER> ,
                                       <http://www.ontologydesignpatterns.org/ont/is/isaac_vanilla.owl#CONTAINMENT> ;
                       isnet:hasActivator <https://w3id.org/framester/data/framestercore/Placing> ,
                                          <https://w3id.org/framester/wn/wn30/instances/supersense-noun_location> .


###  http://www.ontologydesignpatterns.org/ont/odin/odin.owl#network.owl_Descr
odin:network.owl_Descr rdf:type owl:NamedIndividual .


###  http://www.ontologydesignpatterns.org/ont/odin/odin.owl#newsreportingevent.owl_Descr
odin:newsreportingevent.owl_Descr rdf:type owl:NamedIndividual .


###  http://www.ontologydesignpatterns.org/ont/odin/odin.owl#nextFix_Descr
odin:nextFix_Descr rdf:type owl:NamedIndividual .


###  http://www.ontologydesignpatterns.org/ont/odin/odin.owl#nextItem_Descr
odin:nextItem_Descr rdf:type owl:NamedIndividual .


###  http://www.ontologydesignpatterns.org/ont/odin/odin.owl#object.owl_Descr
odin:object.owl_Descr rdf:type owl:NamedIndividual ;
                      isnet:activates <http://www.ontologydesignpatterns.org/ont/is/isaac_vanilla.owl#PART_WHOLE> ;
                      isnet:hasActivator <https://w3id.org/framester/wn/wn30/instances/synset-context-noun-1> ,
                                         <https://w3id.org/framester/wn/wn30/instances/synset-sol-noun-3> .


###  http://www.ontologydesignpatterns.org/ont/odin/odin.owl#objectrole.owl_Descr
odin:objectrole.owl_Descr rdf:type owl:NamedIndividual ;
                          isnet:activates <http://www.ontologydesignpatterns.org/ont/is/isaac_vanilla.owl#CONTAINMENT> ,
                                          <http://www.ontologydesignpatterns.org/ont/is/isaac_vanilla.owl#SOURCE_PATH_GOAL> ;
                          isnet:hasActivator <https://w3id.org/framester/data/framestercore/Removing> ,
                                             <https://w3id.org/framester/vn/vn31/data/Extract_10010000> ,
                                             <https://w3id.org/framester/wn/wn30/instances/synset-concept-noun-1> .


###  http://www.ontologydesignpatterns.org/ont/odin/odin.owl#overlappingTopic_Descr
odin:overlappingTopic_Descr rdf:type owl:NamedIndividual ;
                            isnet:activates <http://www.ontologydesignpatterns.org/ont/is/isaac_vanilla.owl#CONTAINMENT> ,
                                            <http://www.ontologydesignpatterns.org/ont/is/isaac_vanilla.owl#PART_WHOLE> ;
                            isnet:hasActivator <https://w3id.org/framester/data/framestercore/Membership> ,
                                               <https://w3id.org/framester/data/framestercore/Placing> ,
                                               <https://w3id.org/framester/wn/wn30/instances/synset-overlap-noun-1> ,
                                               <https://w3id.org/framester/wn/wn30/instances/synset-part-noun-1> .


###  http://www.ontologydesignpatterns.org/ont/odin/odin.owl#owns_Descr
odin:owns_Descr rdf:type owl:NamedIndividual .


###  http://www.ontologydesignpatterns.org/ont/odin/odin.owl#parameter.owl_Descr
odin:parameter.owl_Descr rdf:type owl:NamedIndividual ;
                         isnet:activates <http://www.ontologydesignpatterns.org/ont/is/isaac_vanilla.owl#PART_WHOLE> ,
                                         <http://www.ontologydesignpatterns.org/ont/is/isaac_vanilla.owl#SOURCE_PATH_GOAL> ;
                         isnet:hasActivator <https://w3id.org/framester/data/framestercore/Removing> ,
                                            <https://w3id.org/framester/vn/vn31/data/Extract_10010000> ,
                                            <https://w3id.org/framester/wn/wn30/instances/supersense-noun_group> .


###  http://www.ontologydesignpatterns.org/ont/odin/odin.owl#parametrizes_Descr
odin:parametrizes_Descr rdf:type owl:NamedIndividual .


###  http://www.ontologydesignpatterns.org/ont/odin/odin.owl#participation.owl_Descr
odin:participation.owl_Descr rdf:type owl:NamedIndividual .


###  http://www.ontologydesignpatterns.org/ont/odin/odin.owl#precedes_Descr
odin:precedes_Descr rdf:type owl:NamedIndividual .


###  http://www.ontologydesignpatterns.org/ont/odin/odin.owl#presentedAt_Descr
odin:presentedAt_Descr rdf:type owl:NamedIndividual .


###  http://www.ontologydesignpatterns.org/ont/odin/odin.owl#previousItem_Descr
odin:previousItem_Descr rdf:type owl:NamedIndividual .


###  http://www.ontologydesignpatterns.org/ont/odin/odin.owl#processedBy_Descr
odin:processedBy_Descr rdf:type owl:NamedIndividual .


###  http://www.ontologydesignpatterns.org/ont/odin/odin.owl#providesParticipantRole_Descr
odin:providesParticipantRole_Descr rdf:type owl:NamedIndividual .


###  http://www.ontologydesignpatterns.org/ont/odin/odin.owl#reaction.owl_Descr
odin:reaction.owl_Descr rdf:type owl:NamedIndividual .


###  http://www.ontologydesignpatterns.org/ont/odin/odin.owl#realizes_Descr
odin:realizes_Descr rdf:type owl:NamedIndividual ;
                    isnet:activates <http://www.ontologydesignpatterns.org/ont/is/isaac_vanilla.owl#CONTAINMENT> ;
                    isnet:hasActivator <https://w3id.org/framester/data/framestercore/Filling> .


###  http://www.ontologydesignpatterns.org/ont/odin/odin.owl#receivedActuation_Descr
odin:receivedActuation_Descr rdf:type owl:NamedIndividual .


###  http://www.ontologydesignpatterns.org/ont/odin/odin.owl#referenceFrame_Descr
odin:referenceFrame_Descr rdf:type owl:NamedIndividual .


###  http://www.ontologydesignpatterns.org/ont/odin/odin.owl#referenceYear_Descr
odin:referenceYear_Descr rdf:type owl:NamedIndividual .


###  http://www.ontologydesignpatterns.org/ont/odin/odin.owl#refersToEventObjectComponent_Descr
odin:refersToEventObjectComponent_Descr rdf:type owl:NamedIndividual ;
                                        isnet:activates <http://www.ontologydesignpatterns.org/ont/is/isaac_vanilla.owl#PART_WHOLE> ;
                                        isnet:hasActivator <https://w3id.org/framester/wn/wn30/instances/supersense-noun_group> .


###  http://www.ontologydesignpatterns.org/ont/odin/odin.owl#refersToEventObjectConstituent_Descr
odin:refersToEventObjectConstituent_Descr rdf:type owl:NamedIndividual ;
                                          isnet:activates <http://www.ontologydesignpatterns.org/ont/is/isaac_vanilla.owl#CONTAINMENT> ,
                                                          <http://www.ontologydesignpatterns.org/ont/is/isaac_vanilla.owl#PART_WHOLE> ;
                                          isnet:hasActivator <https://w3id.org/framester/wn/wn30/instances/supersense-noun_group> ,
                                                             <https://w3id.org/framester/wn/wn30/instances/synset-abstraction-noun-1> .


###  http://www.ontologydesignpatterns.org/ont/odin/odin.owl#region.owl_Descr
odin:region.owl_Descr rdf:type owl:NamedIndividual ;
                      isnet:activates <http://www.ontologydesignpatterns.org/ont/is/isaac_vanilla.owl#CONTAINER> ,
                                      <http://www.ontologydesignpatterns.org/ont/is/isaac_vanilla.owl#PART_WHOLE> ,
                                      <http://www.ontologydesignpatterns.org/ont/is/isaac_vanilla.owl#SOURCE_PATH_GOAL> ;
                      isnet:hasActivator <https://w3id.org/framester/data/framestercore/Removing> ,
                                         <https://w3id.org/framester/vn/vn31/data/Extract_10010000> ,
                                         <https://w3id.org/framester/wn/wn30/instances/supersense-noun_group> ,
                                         <https://w3id.org/framester/wn/wn30/instances/supersense-noun_location> .


###  http://www.ontologydesignpatterns.org/ont/odin/odin.owl#reportingYear_Descr
odin:reportingYear_Descr rdf:type owl:NamedIndividual .


###  http://www.ontologydesignpatterns.org/ont/odin/odin.owl#reportingevent.owl_Descr
odin:reportingevent.owl_Descr rdf:type owl:NamedIndividual .


###  http://www.ontologydesignpatterns.org/ont/odin/odin.owl#reports_Descr
odin:reports_Descr rdf:type owl:NamedIndividual .


###  http://www.ontologydesignpatterns.org/ont/odin/odin.owl#requiresHardware_Descr
odin:requiresHardware_Descr rdf:type owl:NamedIndividual ;
                            isnet:activates <http://www.ontologydesignpatterns.org/ont/is/isaac_vanilla.owl#PART_WHOLE> ;
                            isnet:hasActivator <https://w3id.org/framester/wn/wn30/instances/synset-piece-noun-1> .


###  http://www.ontologydesignpatterns.org/ont/odin/odin.owl#requiresSoftware_Descr
odin:requiresSoftware_Descr rdf:type owl:NamedIndividual .


###  http://www.ontologydesignpatterns.org/ont/odin/odin.owl#satisfies_Descr
odin:satisfies_Descr rdf:type owl:NamedIndividual ;
                     isnet:activates <http://www.ontologydesignpatterns.org/ont/is/isaac_vanilla.owl#GOAL> ,
                                     <http://www.ontologydesignpatterns.org/ont/is/isaac_vanilla.owl#SOURCE_PATH_GOAL> ;
                     isnet:hasActivator <https://w3id.org/framester/data/framestercore/Purpose> ,
                                        <https://w3id.org/framester/wn/wn30/instances/synset-plan-noun-1> .


###  http://www.ontologydesignpatterns.org/ont/odin/odin.owl#set.owl_Descr
odin:set.owl_Descr rdf:type owl:NamedIndividual ;
                   isnet:activates <http://www.ontologydesignpatterns.org/ont/is/isaac_vanilla.owl#CONTAINMENT> ,
                                   <http://www.ontologydesignpatterns.org/ont/is/isaac_vanilla.owl#PART_WHOLE> ,
                                   <http://www.ontologydesignpatterns.org/ont/is/isaac_vanilla.owl#SOURCE_PATH_GOAL> ;
                   isnet:hasActivator <https://w3id.org/framester/data/framestercore/Containing> ,
                                      <https://w3id.org/framester/data/framestercore/Placing> ,
                                      <https://w3id.org/framester/data/framestercore/Removing> ,
                                      <https://w3id.org/framester/data/framestercore/Sending> ,
                                      <https://w3id.org/framester/vn/vn31/data/Contain_54030000> ,
                                      <https://w3id.org/framester/vn/vn31/data/Eliminate_10010000> ,
                                      <https://w3id.org/framester/wn/wn30/instances/supersense-noun_group> ,
                                      <https://w3id.org/framester/wn/wn30/instances/synset-incorporate-verb-2> .


###  http://www.ontologydesignpatterns.org/ont/odin/odin.owl#size_Descr
odin:size_Descr rdf:type owl:NamedIndividual ;
                isnet:activates <http://www.ontologydesignpatterns.org/ont/is/isaac_vanilla.owl#PART_WHOLE> ;
                isnet:hasActivator <https://w3id.org/framester/wn/wn30/instances/supersense-noun_group> .


###  http://www.ontologydesignpatterns.org/ont/odin/odin.owl#speciesbathymetry.owl_Descr
odin:speciesbathymetry.owl_Descr rdf:type owl:NamedIndividual ;
                                 isnet:activates <http://www.ontologydesignpatterns.org/ont/is/isaac_vanilla.owl#PART_WHOLE> ;
                                 isnet:hasActivator <https://w3id.org/framester/wn/wn30/instances/supersense-noun_group> .


###  http://www.ontologydesignpatterns.org/ont/odin/odin.owl#speciesconditions.owl_Descr
odin:speciesconditions.owl_Descr rdf:type owl:NamedIndividual ;
                                 isnet:activates <http://www.ontologydesignpatterns.org/ont/is/isaac_vanilla.owl#CONTAINER> ,
                                                 <http://www.ontologydesignpatterns.org/ont/is/isaac_vanilla.owl#PART_WHOLE> ,
                                                 <http://www.ontologydesignpatterns.org/ont/is/isaac_vanilla.owl#SOURCE_PATH_GOAL> ;
                                 isnet:hasActivator <https://w3id.org/framester/data/framestercore/Sending> ,
                                                    <https://w3id.org/framester/wn/wn30/instances/supersense-noun_group> ,
                                                    <https://w3id.org/framester/wn/wn30/instances/supersense-noun_location> .


###  http://www.ontologydesignpatterns.org/ont/odin/odin.owl#specieshabitat.owl_Descr
odin:specieshabitat.owl_Descr rdf:type owl:NamedIndividual ;
                              isnet:activates <http://www.ontologydesignpatterns.org/ont/is/isaac_vanilla.owl#CONTAINMENT> ,
                                              <http://www.ontologydesignpatterns.org/ont/is/isaac_vanilla.owl#GOAL> ,
                                              <http://www.ontologydesignpatterns.org/ont/is/isaac_vanilla.owl#PART_WHOLE> ,
                                              <http://www.ontologydesignpatterns.org/ont/is/isaac_vanilla.owl#SOURCE_PATH_GOAL> ;
                              isnet:hasActivator <https://w3id.org/framester/data/framestercore/Purpose> ,
                                                 <https://w3id.org/framester/wn/wn30/instances/supersense-noun_group> ,
                                                 <https://w3id.org/framester/wn/wn30/instances/synset-application-noun-1> ,
                                                 <https://w3id.org/framester/wn/wn30/instances/synset-representation-noun-1> ,
                                                 <https://w3id.org/framester/wn/wn30/instances/synset-schema-noun-1> ,
                                                 <https://w3id.org/framester/wn/wn30/instances/synset-suggestion-noun-1> .


###  http://www.ontologydesignpatterns.org/ont/odin/odin.owl#startsFrom_Descr
odin:startsFrom_Descr rdf:type owl:NamedIndividual ;
                      isnet:activates <http://www.ontologydesignpatterns.org/ont/is/isaac_vanilla.owl#BLOCKAGE> ,
                                      <http://www.ontologydesignpatterns.org/ont/is/isaac_vanilla.owl#CENTER_PERIPHERY> ,
                                      <http://www.ontologydesignpatterns.org/ont/is/isaac_vanilla.owl#PART_WHOLE> ,
                                      <http://www.ontologydesignpatterns.org/ont/is/isaac_vanilla.owl#SOURCE_PATH_GOAL> ;
                      isnet:hasActivator <https://w3id.org/framester/data/framestercore/Departing> ,
                                         <https://w3id.org/framester/data/framestercore/Predicament> ,
                                         <https://w3id.org/framester/wn/wn30/instances/synset-fix-noun-1> ,
                                         <https://w3id.org/framester/wn/wn30/instances/synset-section-noun-4> .


###  http://www.ontologydesignpatterns.org/ont/odin/odin.owl#subEventOf_Descr
odin:subEventOf_Descr rdf:type owl:NamedIndividual .


###  http://www.ontologydesignpatterns.org/ont/odin/odin.owl#subSpatioTemporalExtentOf_Descr
odin:subSpatioTemporalExtentOf_Descr rdf:type owl:NamedIndividual .


###  http://www.ontologydesignpatterns.org/ont/odin/odin.owl#tagging.owl_Descr
odin:tagging.owl_Descr rdf:type owl:NamedIndividual ;
                       isnet:activates <http://www.ontologydesignpatterns.org/ont/is/isaac_vanilla.owl#PART_WHOLE> ;
                       isnet:hasActivator <https://w3id.org/framester/wn/wn30/instances/synset-context-noun-1> .


###  http://www.ontologydesignpatterns.org/ont/odin/odin.owl#targetsEntity_Descr
odin:targetsEntity_Descr rdf:type owl:NamedIndividual ;
                         isnet:activates <http://www.ontologydesignpatterns.org/ont/is/isaac_vanilla.owl#GOAL> ;
                         isnet:hasActivator <https://w3id.org/framester/wn/wn30/instances/synset-policy-noun-1> .


###  http://www.ontologydesignpatterns.org/ont/odin/odin.owl#targetsUsers_Descr
odin:targetsUsers_Descr rdf:type owl:NamedIndividual ;
                        isnet:activates <http://www.ontologydesignpatterns.org/ont/is/isaac_vanilla.owl#GOAL> ,
                                        <http://www.ontologydesignpatterns.org/ont/is/isaac_vanilla.owl#PART_WHOLE> ;
                        isnet:hasActivator <https://w3id.org/framester/wn/wn30/instances/supersense-noun_group> ,
                                           <https://w3id.org/framester/wn/wn30/instances/synset-policy-noun-1> .


###  http://www.ontologydesignpatterns.org/ont/odin/odin.owl#taskrole.owl_Descr
odin:taskrole.owl_Descr rdf:type owl:NamedIndividual .


###  http://www.ontologydesignpatterns.org/ont/odin/odin.owl#timePeriodValue_Descr
odin:timePeriodValue_Descr rdf:type owl:NamedIndividual .


###  http://www.ontologydesignpatterns.org/ont/odin/odin.owl#timeindexedparticipation.owl_Descr
odin:timeindexedparticipation.owl_Descr rdf:type owl:NamedIndividual .


###  http://www.ontologydesignpatterns.org/ont/odin/odin.owl#timeindexedpartof.owl_Descr
odin:timeindexedpartof.owl_Descr rdf:type owl:NamedIndividual .


###  http://www.ontologydesignpatterns.org/ont/odin/odin.owl#timeindexedsituation.owl_Descr
odin:timeindexedsituation.owl_Descr rdf:type owl:NamedIndividual .


###  http://www.ontologydesignpatterns.org/ont/odin/odin.owl#timeinterval.owl_Descr
odin:timeinterval.owl_Descr rdf:type owl:NamedIndividual ;
                            isnet:activates <http://www.ontologydesignpatterns.org/ont/is/isaac_vanilla.owl#PART_WHOLE> ,
                                            <http://www.ontologydesignpatterns.org/ont/is/isaac_vanilla.owl#SOURCE_PATH_GOAL> ;
                            isnet:hasActivator <https://w3id.org/framester/data/framestercore/Removing> ,
                                               <https://w3id.org/framester/data/framestercore/Sending> ,
                                               <https://w3id.org/framester/vn/vn31/data/Extract_10010000> ,
                                               <https://w3id.org/framester/wn/wn30/instances/supersense-noun_group> ,
                                               <https://w3id.org/framester/wn/wn30/instances/synset-partial-adjectivesatellite-1> .


###  http://www.ontologydesignpatterns.org/ont/odin/odin.owl#timeperiod.owl_Descr
odin:timeperiod.owl_Descr rdf:type owl:NamedIndividual .


###  http://www.ontologydesignpatterns.org/ont/odin/odin.owl#tookPlaceAt_Descr
odin:tookPlaceAt_Descr rdf:type owl:NamedIndividual .


###  http://www.ontologydesignpatterns.org/ont/odin/odin.owl#topic.owl_Descr
odin:topic.owl_Descr rdf:type owl:NamedIndividual .


###  http://www.ontologydesignpatterns.org/ont/odin/odin.owl#transition.owl_Descr
odin:transition.owl_Descr rdf:type owl:NamedIndividual .


###  http://www.ontologydesignpatterns.org/ont/odin/odin.owl#traversedBy_Descr
odin:traversedBy_Descr rdf:type owl:NamedIndividual ;
                       isnet:activates <http://www.ontologydesignpatterns.org/ont/is/isaac_vanilla.owl#PART_WHOLE> ,
                                       <http://www.ontologydesignpatterns.org/ont/is/isaac_vanilla.owl#SOURCE_PATH_GOAL> ;
                       isnet:hasActivator <https://w3id.org/framester/data/framestercore/BodyMovement> ,
                                          <https://w3id.org/framester/data/framestercore/IntentionalTraversing> ,
                                          <https://w3id.org/framester/data/framestercore/Motion> ,
                                          <https://w3id.org/framester/data/framestercore/PathShape> ,
                                          <https://w3id.org/framester/data/framestercore/SelfMotion> ,
                                          <https://w3id.org/framester/data/framestercore/Travel> ,
                                          <https://w3id.org/framester/data/framestercore/Traversing> ,
                                          <https://w3id.org/framester/vn/vn31/data/Move_11020000> ,
                                          <https://w3id.org/framester/vn/vn31/data/Traverse_47080000> ,
                                          <https://w3id.org/framester/wn/wn30/instances/synset-section-noun-4> .


###  http://www.ontologydesignpatterns.org/ont/odin/odin.owl#triggersTransition_Descr
odin:triggersTransition_Descr rdf:type owl:NamedIndividual ;
                              isnet:activates <http://www.ontologydesignpatterns.org/ont/is/isaac_vanilla.owl#CONTAINER> ;
                              isnet:hasActivator <https://w3id.org/framester/wn/wn30/instances/supersense-noun_location> .


###  http://www.ontologydesignpatterns.org/ont/odin/odin.owl#unitUsedInRecord_Descr
odin:unitUsedInRecord_Descr rdf:type owl:NamedIndividual ;
                            isnet:activates <http://www.ontologydesignpatterns.org/ont/is/isaac_vanilla.owl#PART_WHOLE> ;
                            isnet:hasActivator <https://w3id.org/framester/wn/wn30/instances/supersense-noun_group> .


###  http://www.ontologydesignpatterns.org/ont/odin/odin.owl#usesConcept_Descr
odin:usesConcept_Descr rdf:type owl:NamedIndividual ;
                       isnet:activates <http://www.ontologydesignpatterns.org/ont/is/isaac_vanilla.owl#CONTAINMENT> ;
                       isnet:hasActivator <https://w3id.org/framester/wn/wn30/instances/synset-concept-noun-1> .


###  http://www.ontologydesignpatterns.org/ont/odin/odin.owl#usesDriver_Descr
odin:usesDriver_Descr rdf:type owl:NamedIndividual .


###  http://www.ontologydesignpatterns.org/ont/odin/odin.owl#usesHardware_Descr
odin:usesHardware_Descr rdf:type owl:NamedIndividual ;
                        isnet:activates <http://www.ontologydesignpatterns.org/ont/is/isaac_vanilla.owl#GOAL> ,
                                        <http://www.ontologydesignpatterns.org/ont/is/isaac_vanilla.owl#PART_WHOLE> ,
                                        <http://www.ontologydesignpatterns.org/ont/is/isaac_vanilla.owl#SOURCE_PATH_GOAL> ;
                        isnet:hasActivator <https://w3id.org/framester/data/framestercore/Purpose> ,
                                           <https://w3id.org/framester/wn/wn30/instances/synset-piece-noun-1> ,
                                           <https://w3id.org/framester/wn/wn30/instances/synset-use-noun-1> .


###  http://www.ontologydesignpatterns.org/ont/odin/odin.owl#usesOperatingSystem_Descr
odin:usesOperatingSystem_Descr rdf:type owl:NamedIndividual ;
                               isnet:activates <http://www.ontologydesignpatterns.org/ont/is/isaac_vanilla.owl#GOAL> ,
                                               <http://www.ontologydesignpatterns.org/ont/is/isaac_vanilla.owl#SOURCE_PATH_GOAL> ;
                               isnet:hasActivator <https://w3id.org/framester/data/framestercore/Purpose> ,
                                                  <https://w3id.org/framester/wn/wn30/instances/synset-use-noun-1> .


###  http://www.ontologydesignpatterns.org/ont/odin/odin.owl#usesSoftware_Descr
odin:usesSoftware_Descr rdf:type owl:NamedIndividual ;
                        isnet:activates <http://www.ontologydesignpatterns.org/ont/is/isaac_vanilla.owl#GOAL> ,
                                        <http://www.ontologydesignpatterns.org/ont/is/isaac_vanilla.owl#PART_WHOLE> ,
                                        <http://www.ontologydesignpatterns.org/ont/is/isaac_vanilla.owl#SOURCE_PATH_GOAL> ;
                        isnet:hasActivator <https://w3id.org/framester/data/framestercore/Purpose> ,
                                           <https://w3id.org/framester/wn/wn30/instances/synset-piece-noun-1> ,
                                           <https://w3id.org/framester/wn/wn30/instances/synset-use-noun-1> .


###  http://www.ontologydesignpatterns.org/ont/odin/odin.owl#vesselspecies.owl_Descr
odin:vesselspecies.owl_Descr rdf:type owl:NamedIndividual .


###  http://www.ontologydesignpatterns.org/ont/odin/odin.owl#vesselwaterarea.owl_Descr
odin:vesselwaterarea.owl_Descr rdf:type owl:NamedIndividual .


###  http://www.ontologydesignpatterns.org/ont/odin/odin.owl#wasActuationSent_Descr
odin:wasActuationSent_Descr rdf:type owl:NamedIndividual ;
                            isnet:activates <http://www.ontologydesignpatterns.org/ont/is/isaac_vanilla.owl#SOURCE_PATH_GOAL> ;
                            isnet:hasActivator <https://w3id.org/framester/data/framestercore/Sending> .


###  http://www.ontologydesignpatterns.org/ont/odin/odin.owl#withUnit_Descr
odin:withUnit_Descr rdf:type owl:NamedIndividual ;
                    isnet:activates <http://www.ontologydesignpatterns.org/ont/is/isaac_vanilla.owl#PART_WHOLE> ;
                    isnet:hasActivator <https://w3id.org/framester/wn/wn30/instances/supersense-noun_group> .


###  http://www.ontologydesignpatterns.org/ont/odin/odin.owl#wrappedBy_Descr
odin:wrappedBy_Descr rdf:type owl:NamedIndividual ;
                     isnet:activates <http://www.ontologydesignpatterns.org/ont/is/isaac_vanilla.owl#CONTAINMENT> ;
                     isnet:hasActivator <https://w3id.org/framester/data/framestercore/Containers> ,
                                        <https://w3id.org/framester/data/framestercore/Placing> ,
                                        <https://w3id.org/framester/wn/wn30/instances/synset-container-noun-1> ,
                                        <https://w3id.org/framester/wn/wn30/instances/synset-type-noun-1> .


###  http://www.ontologydesignpatterns.org/ont/odin/odin.owl#_:b0_Descr
odin:_:b0_Descr rdf:type owl:NamedIndividual .


###  http://www.ontologydesignpatterns.org/ont/odin/odin.owl#_:b1_Descr
odin:_:b1_Descr rdf:type owl:NamedIndividual .


###  http://www.ontologydesignpatterns.org/ont/odin/odin.owl#_:b2_Descr
odin:_:b2_Descr rdf:type owl:NamedIndividual .


###  http://www.ontologydesignpatterns.org/ont/odin/odin.owl#_:b3_Descr
odin:_:b3_Descr rdf:type owl:NamedIndividual .


###  http://www.ontologydesignpatterns.org/ont/odin/odin.owl#_:b4_Descr
odin:_:b4_Descr rdf:type owl:NamedIndividual ;
                isnet:activates <http://www.ontologydesignpatterns.org/ont/is/isaac_vanilla.owl#BLOCKAGE> ,
                                <http://www.ontologydesignpatterns.org/ont/is/isaac_vanilla.owl#SUPPORT> ;
                isnet:hasActivator <https://w3id.org/framester/data/framestercore/Assistance> ,
                                   <https://w3id.org/framester/data/framestercore/Supply> ,
                                   <https://w3id.org/framester/wn/wn30/instances/synset-restriction-noun-1> ,
                                   <https://w3id.org/framester/wn/wn30/instances/synset-supply-verb-1> .


###  http://www.ontologydesignpatterns.org/ont/odin/odin.owl#owl/EthnicGroup.owl_Descr
<http://www.ontologydesignpatterns.org/ont/odin/odin.owl#owl/EthnicGroup.owl_Descr> rdf:type owl:NamedIndividual .


###  https://w3id.org/food/ontology/dir
<https://w3id.org/food/ontology/dir> rdf:type owl:NamedIndividual ,
                                              odin:ODP ;
                                     odin:describedIn <http://w3id.org/food/ontology/dir_Descr> ;
                                     odin:hasODPComponent <https://w3id.org/food/ontology/dir/DescriptionInRange> ,
                                                          <https://w3id.org/food/ontology/dir/Entity> ,
                                                          <https://w3id.org/food/ontology/dir/hasInclusiveLowerBoundValue> ,
                                                          <https://w3id.org/food/ontology/dir/hasInclusiveUpperBoundValue> ,
                                                          <https://w3id.org/food/ontology/dir/hasNonInclusiveLowerBoundValue> ,
                                                          <https://w3id.org/food/ontology/dir/hasNonInclusiveUpperBoundValue> ,
                                                          <https://w3id.org/food/ontology/dir/isRangedByValue> ;
                                     odin:odpType odin:Foundational ;
                                     rdfs:comment "The Description In Range (DIR) ontology design patterns is a specialization of the Description ODP, that allows one to range the conceptualization of a descriptive context within specific borders defined by means of literal values." .


###  https://w3id.org/food/ontology/dir/DescriptionInRange
<https://w3id.org/food/ontology/dir/DescriptionInRange> rdf:type owl:NamedIndividual ,
                                                                 odin:ODPElement ;
                                                        odin:describedIn odin:DescriptionInRange_Descr ;
                                                        rdfs:comment "This class allows one to identify descriptions involving a specific concept (i.e. description:usesConcept) relating to a literal value that can be defined within a particular a range. For instance:     * 100% of sheep milk;  * at least 25cm of diameter (circular shape).     Individuals of this class cannot exist without the entity they (partially or fully) describe - see the class [Entity](#https://w3id.org/food/ontology/dir/Entity)." .


###  https://w3id.org/food/ontology/dir/Entity
<https://w3id.org/food/ontology/dir/Entity> rdf:type owl:NamedIndividual ,
                                                     odin:ODPElement ;
                                            odin:describedIn odin:Entity_Descr ;
                                            odin:odpType odin:Foundational ;
                                            rdfs:comment "This class allows the specification of entities that that are (partially or fully) described by means of descriptions." .


###  https://w3id.org/food/ontology/dir/hasInclusiveLowerBoundValue
<https://w3id.org/food/ontology/dir/hasInclusiveLowerBoundValue> rdf:type owl:NamedIndividual ,
                                                                          odin:ODPElement ;
                                                                 odin:describedIn odin:hasInclusiveLowerBoundValue_Descr ;
                                                                 odin:odpType odin:Foundational ;
                                                                 rdfs:comment "Any value that specifies an inclusive lower bound for a certain amount of a concept as conceived in a particular description (e.g. at least 25cm)." .


###  https://w3id.org/food/ontology/dir/hasInclusiveUpperBoundValue
<https://w3id.org/food/ontology/dir/hasInclusiveUpperBoundValue> rdf:type owl:NamedIndividual ,
                                                                          odin:ODPElement ;
                                                                 odin:describedIn odin:hasInclusiveUpperBoundValue_Descr ;
                                                                 odin:odpType odin:Foundational ;
                                                                 rdfs:comment "Any value that specifies an inclusive upper bound for a certain amount of a concept as conceived in a particular description (e.g. at most 25cm)." .


###  https://w3id.org/food/ontology/dir/hasNonInclusiveLowerBoundValue
<https://w3id.org/food/ontology/dir/hasNonInclusiveLowerBoundValue> rdf:type owl:NamedIndividual ,
                                                                             odin:ODPElement ;
                                                                    odin:describedIn odin:hasNonInclusiveLowerBoundValue_Descr ;
                                                                    odin:odpType odin:Foundational ;
                                                                    rdfs:comment "Any value that specifies a non-inclusive lower bound for a certain amount of a concept as conceived in a particular description (e.g. greater than 25cm)." .


###  https://w3id.org/food/ontology/dir/hasNonInclusiveUpperBoundValue
<https://w3id.org/food/ontology/dir/hasNonInclusiveUpperBoundValue> rdf:type owl:NamedIndividual ,
                                                                             odin:ODPElement ;
                                                                    odin:describedIn odin:hasNonInclusiveUpperBoundValue_Descr ;
                                                                    odin:odpType odin:Foundational ;
                                                                    rdfs:comment "Any value that specifies a non-inclusive upper bound for a certain amount of a concept as conceived in a particular description (e.g. less than 25cm)." .


###  https://w3id.org/food/ontology/dir/isRangedByValue
<https://w3id.org/food/ontology/dir/isRangedByValue> rdf:type owl:NamedIndividual ,
                                                              odin:ODPElement ;
                                                     odin:describedIn odin:isRangedByValue_Descr ;
                                                     rdfs:comment "Any value that specifies a certain amount of a concept as conceived in a particular description (e.g. 100% and 25cm).      The value is defined as a free-text literal, instead of specifying more complex structure, so as to be easily populated with data of different natures, such as those coming from heterogeneous (and even multilingual) documents." .


###  https://w3id.org/framester/data/framestercore/Accomplishment
<https://w3id.org/framester/data/framestercore/Accomplishment> rdf:type owl:NamedIndividual .


###  https://w3id.org/framester/data/framestercore/Adorning
<https://w3id.org/framester/data/framestercore/Adorning> rdf:type owl:NamedIndividual .


###  https://w3id.org/framester/data/framestercore/Aiming
<https://w3id.org/framester/data/framestercore/Aiming> rdf:type owl:NamedIndividual .


###  https://w3id.org/framester/data/framestercore/Arriving
<https://w3id.org/framester/data/framestercore/Arriving> rdf:type owl:NamedIndividual .


###  https://w3id.org/framester/data/framestercore/Assistance
<https://w3id.org/framester/data/framestercore/Assistance> rdf:type owl:NamedIndividual .


###  https://w3id.org/framester/data/framestercore/BodyMovement
<https://w3id.org/framester/data/framestercore/BodyMovement> rdf:type owl:NamedIndividual .


###  https://w3id.org/framester/data/framestercore/Closure
<https://w3id.org/framester/data/framestercore/Closure> rdf:type owl:NamedIndividual .


###  https://w3id.org/framester/data/framestercore/ComeTogether
<https://w3id.org/framester/data/framestercore/ComeTogether> rdf:type owl:NamedIndividual .


###  https://w3id.org/framester/data/framestercore/Conduct
<https://w3id.org/framester/data/framestercore/Conduct> rdf:type owl:NamedIndividual .


###  https://w3id.org/framester/data/framestercore/Containers
<https://w3id.org/framester/data/framestercore/Containers> rdf:type owl:NamedIndividual .


###  https://w3id.org/framester/data/framestercore/Containing
<https://w3id.org/framester/data/framestercore/Containing> rdf:type owl:NamedIndividual .


###  https://w3id.org/framester/data/framestercore/Departing
<https://w3id.org/framester/data/framestercore/Departing> rdf:type owl:NamedIndividual .


###  https://w3id.org/framester/data/framestercore/Eclipse
<https://w3id.org/framester/data/framestercore/Eclipse> rdf:type owl:NamedIndividual .


###  https://w3id.org/framester/data/framestercore/Filling
<https://w3id.org/framester/data/framestercore/Filling> rdf:type owl:NamedIndividual .


###  https://w3id.org/framester/data/framestercore/Fullness
<https://w3id.org/framester/data/framestercore/Fullness> rdf:type owl:NamedIndividual .


###  https://w3id.org/framester/data/framestercore/Goal
<https://w3id.org/framester/data/framestercore/Goal> rdf:type owl:NamedIndividual .


###  https://w3id.org/framester/data/framestercore/Grasp
<https://w3id.org/framester/data/framestercore/Grasp> rdf:type owl:NamedIndividual .


###  https://w3id.org/framester/data/framestercore/Hindering
<https://w3id.org/framester/data/framestercore/Hindering> rdf:type owl:NamedIndividual .


###  https://w3id.org/framester/data/framestercore/Ingestion
<https://w3id.org/framester/data/framestercore/Ingestion> rdf:type owl:NamedIndividual .


###  https://w3id.org/framester/data/framestercore/InhibitMovement
<https://w3id.org/framester/data/framestercore/InhibitMovement> rdf:type owl:NamedIndividual .


###  https://w3id.org/framester/data/framestercore/IntentionalTraversing
<https://w3id.org/framester/data/framestercore/IntentionalTraversing> rdf:type owl:NamedIndividual .


###  https://w3id.org/framester/data/framestercore/LocativeRelation
<https://w3id.org/framester/data/framestercore/LocativeRelation> rdf:type owl:NamedIndividual .


###  https://w3id.org/framester/data/framestercore/Membership
<https://w3id.org/framester/data/framestercore/Membership> rdf:type owl:NamedIndividual .


###  https://w3id.org/framester/data/framestercore/Motion
<https://w3id.org/framester/data/framestercore/Motion> rdf:type owl:NamedIndividual .


###  https://w3id.org/framester/data/framestercore/Needing
<https://w3id.org/framester/data/framestercore/Needing> rdf:type owl:NamedIndividual .


###  https://w3id.org/framester/data/framestercore/Origin
<https://w3id.org/framester/data/framestercore/Origin> rdf:type owl:NamedIndividual .


###  https://w3id.org/framester/data/framestercore/PartInnerOuter
<https://w3id.org/framester/data/framestercore/PartInnerOuter> rdf:type owl:NamedIndividual .


###  https://w3id.org/framester/data/framestercore/PathShape
<https://w3id.org/framester/data/framestercore/PathShape> rdf:type owl:NamedIndividual .


###  https://w3id.org/framester/data/framestercore/Placing
<https://w3id.org/framester/data/framestercore/Placing> rdf:type owl:NamedIndividual .


###  https://w3id.org/framester/data/framestercore/Predicament
<https://w3id.org/framester/data/framestercore/Predicament> rdf:type owl:NamedIndividual .


###  https://w3id.org/framester/data/framestercore/ProcessEnd
<https://w3id.org/framester/data/framestercore/ProcessEnd> rdf:type owl:NamedIndividual .


###  https://w3id.org/framester/data/framestercore/Purpose
<https://w3id.org/framester/data/framestercore/Purpose> rdf:type owl:NamedIndividual .


###  https://w3id.org/framester/data/framestercore/Range
<https://w3id.org/framester/data/framestercore/Range> rdf:type owl:NamedIndividual .


###  https://w3id.org/framester/data/framestercore/Removing
<https://w3id.org/framester/data/framestercore/Removing> rdf:type owl:NamedIndividual .


###  https://w3id.org/framester/data/framestercore/Replacing
<https://w3id.org/framester/data/framestercore/Replacing> rdf:type owl:NamedIndividual .


###  https://w3id.org/framester/data/framestercore/Roadways
<https://w3id.org/framester/data/framestercore/Roadways> rdf:type owl:NamedIndividual .


###  https://w3id.org/framester/data/framestercore/SelfMotion
<https://w3id.org/framester/data/framestercore/SelfMotion> rdf:type owl:NamedIndividual .


###  https://w3id.org/framester/data/framestercore/Sending
<https://w3id.org/framester/data/framestercore/Sending> rdf:type owl:NamedIndividual .


###  https://w3id.org/framester/data/framestercore/Supply
<https://w3id.org/framester/data/framestercore/Supply> rdf:type owl:NamedIndividual .


###  https://w3id.org/framester/data/framestercore/Travel
<https://w3id.org/framester/data/framestercore/Travel> rdf:type owl:NamedIndividual .


###  https://w3id.org/framester/data/framestercore/Traversing
<https://w3id.org/framester/data/framestercore/Traversing> rdf:type owl:NamedIndividual .


###  https://w3id.org/framester/vn/vn31/data/Achieve_55020000
<https://w3id.org/framester/vn/vn31/data/Achieve_55020000> rdf:type owl:NamedIndividual .


###  https://w3id.org/framester/vn/vn31/data/Aim_62000000
<https://w3id.org/framester/vn/vn31/data/Aim_62000000> rdf:type owl:NamedIndividual .


###  https://w3id.org/framester/vn/vn31/data/Arrange_26010000
<https://w3id.org/framester/vn/vn31/data/Arrange_26010000> rdf:type owl:NamedIndividual .


###  https://w3id.org/framester/vn/vn31/data/Carry_11040000
<https://w3id.org/framester/vn/vn31/data/Carry_11040000> rdf:type owl:NamedIndividual .


###  https://w3id.org/framester/vn/vn31/data/Constrain_76000000
<https://w3id.org/framester/vn/vn31/data/Constrain_76000000> rdf:type owl:NamedIndividual .


###  https://w3id.org/framester/vn/vn31/data/Consume_66000000
<https://w3id.org/framester/vn/vn31/data/Consume_66000000> rdf:type owl:NamedIndividual .


###  https://w3id.org/framester/vn/vn31/data/Contain_54030000
<https://w3id.org/framester/vn/vn31/data/Contain_54030000> rdf:type owl:NamedIndividual .


###  https://w3id.org/framester/vn/vn31/data/Eliminate_10010000
<https://w3id.org/framester/vn/vn31/data/Eliminate_10010000> rdf:type owl:NamedIndividual .


###  https://w3id.org/framester/vn/vn31/data/Extract_10010000
<https://w3id.org/framester/vn/vn31/data/Extract_10010000> rdf:type owl:NamedIndividual .


###  https://w3id.org/framester/vn/vn31/data/Happen_48030000
<https://w3id.org/framester/vn/vn31/data/Happen_48030000> rdf:type owl:NamedIndividual .


###  https://w3id.org/framester/vn/vn31/data/Hold_54030000
<https://w3id.org/framester/vn/vn31/data/Hold_54030000> rdf:type owl:NamedIndividual .


###  https://w3id.org/framester/vn/vn31/data/Intend_61000000
<https://w3id.org/framester/vn/vn31/data/Intend_61000000> rdf:type owl:NamedIndividual .


###  https://w3id.org/framester/vn/vn31/data/Move_11020000
<https://w3id.org/framester/vn/vn31/data/Move_11020000> rdf:type owl:NamedIndividual .


###  https://w3id.org/framester/vn/vn31/data/Plan_62000000
<https://w3id.org/framester/vn/vn31/data/Plan_62000000> rdf:type owl:NamedIndividual .


###  https://w3id.org/framester/vn/vn31/data/Restrict_76000000
<https://w3id.org/framester/vn/vn31/data/Restrict_76000000> rdf:type owl:NamedIndividual .


###  https://w3id.org/framester/vn/vn31/data/Sit_50000000
<https://w3id.org/framester/vn/vn31/data/Sit_50000000> rdf:type owl:NamedIndividual .


###  https://w3id.org/framester/vn/vn31/data/Take_10050000
<https://w3id.org/framester/vn/vn31/data/Take_10050000> rdf:type owl:NamedIndividual .


###  https://w3id.org/framester/vn/vn31/data/Traverse_47080000
<https://w3id.org/framester/vn/vn31/data/Traverse_47080000> rdf:type owl:NamedIndividual .


###  https://w3id.org/framester/vn/vn31/data/Underlie_47080000
<https://w3id.org/framester/vn/vn31/data/Underlie_47080000> rdf:type owl:NamedIndividual .


###  https://w3id.org/framester/vn/vn31/data/Undertake_98000000
<https://w3id.org/framester/vn/vn31/data/Undertake_98000000> rdf:type owl:NamedIndividual .


###  https://w3id.org/framester/wn/wn30/instances/supersense-noun_group
<https://w3id.org/framester/wn/wn30/instances/supersense-noun_group> rdf:type owl:NamedIndividual .


###  https://w3id.org/framester/wn/wn30/instances/supersense-noun_location
<https://w3id.org/framester/wn/wn30/instances/supersense-noun_location> rdf:type owl:NamedIndividual .


###  https://w3id.org/framester/wn/wn30/instances/synset-abstraction-noun-1
<https://w3id.org/framester/wn/wn30/instances/synset-abstraction-noun-1> rdf:type owl:NamedIndividual .


###  https://w3id.org/framester/wn/wn30/instances/synset-accomplishment-noun-1
<https://w3id.org/framester/wn/wn30/instances/synset-accomplishment-noun-1> rdf:type owl:NamedIndividual .


###  https://w3id.org/framester/wn/wn30/instances/synset-achieve-verb-1
<https://w3id.org/framester/wn/wn30/instances/synset-achieve-verb-1> rdf:type owl:NamedIndividual .


###  https://w3id.org/framester/wn/wn30/instances/synset-application-noun-1
<https://w3id.org/framester/wn/wn30/instances/synset-application-noun-1> rdf:type owl:NamedIndividual .


###  https://w3id.org/framester/wn/wn30/instances/synset-automation-noun-1
<https://w3id.org/framester/wn/wn30/instances/synset-automation-noun-1> rdf:type owl:NamedIndividual .


###  https://w3id.org/framester/wn/wn30/instances/synset-bag-noun-1
<https://w3id.org/framester/wn/wn30/instances/synset-bag-noun-1> rdf:type owl:NamedIndividual .


###  https://w3id.org/framester/wn/wn30/instances/synset-body-noun-1
<https://w3id.org/framester/wn/wn30/instances/synset-body-noun-1> rdf:type owl:NamedIndividual .


###  https://w3id.org/framester/wn/wn30/instances/synset-brain-noun-1
<https://w3id.org/framester/wn/wn30/instances/synset-brain-noun-1> rdf:type owl:NamedIndividual .


###  https://w3id.org/framester/wn/wn30/instances/synset-bulb-noun-1
<https://w3id.org/framester/wn/wn30/instances/synset-bulb-noun-1> rdf:type owl:NamedIndividual .


###  https://w3id.org/framester/wn/wn30/instances/synset-car-noun-1
<https://w3id.org/framester/wn/wn30/instances/synset-car-noun-1> rdf:type owl:NamedIndividual .


###  https://w3id.org/framester/wn/wn30/instances/synset-colony-noun-1
<https://w3id.org/framester/wn/wn30/instances/synset-colony-noun-1> rdf:type owl:NamedIndividual .


###  https://w3id.org/framester/wn/wn30/instances/synset-complete-adjective-1
<https://w3id.org/framester/wn/wn30/instances/synset-complete-adjective-1> rdf:type owl:NamedIndividual .


###  https://w3id.org/framester/wn/wn30/instances/synset-component-noun-1
<https://w3id.org/framester/wn/wn30/instances/synset-component-noun-1> rdf:type owl:NamedIndividual .


###  https://w3id.org/framester/wn/wn30/instances/synset-component-noun-3
<https://w3id.org/framester/wn/wn30/instances/synset-component-noun-3> rdf:type owl:NamedIndividual .


###  https://w3id.org/framester/wn/wn30/instances/synset-concept-noun-1
<https://w3id.org/framester/wn/wn30/instances/synset-concept-noun-1> rdf:type owl:NamedIndividual .


###  https://w3id.org/framester/wn/wn30/instances/synset-conspiracy-noun-2
<https://w3id.org/framester/wn/wn30/instances/synset-conspiracy-noun-2> rdf:type owl:NamedIndividual .


###  https://w3id.org/framester/wn/wn30/instances/synset-container-noun-1
<https://w3id.org/framester/wn/wn30/instances/synset-container-noun-1> rdf:type owl:NamedIndividual .


###  https://w3id.org/framester/wn/wn30/instances/synset-context-noun-1
<https://w3id.org/framester/wn/wn30/instances/synset-context-noun-1> rdf:type owl:NamedIndividual .


###  https://w3id.org/framester/wn/wn30/instances/synset-core-noun-1
<https://w3id.org/framester/wn/wn30/instances/synset-core-noun-1> rdf:type owl:NamedIndividual .


###  https://w3id.org/framester/wn/wn30/instances/synset-course-noun-1
<https://w3id.org/framester/wn/wn30/instances/synset-course-noun-1> rdf:type owl:NamedIndividual .


###  https://w3id.org/framester/wn/wn30/instances/synset-cover-verb-1
<https://w3id.org/framester/wn/wn30/instances/synset-cover-verb-1> rdf:type owl:NamedIndividual .


###  https://w3id.org/framester/wn/wn30/instances/synset-discourse-noun-1
<https://w3id.org/framester/wn/wn30/instances/synset-discourse-noun-1> rdf:type owl:NamedIndividual .


###  https://w3id.org/framester/wn/wn30/instances/synset-dish-noun-1
<https://w3id.org/framester/wn/wn30/instances/synset-dish-noun-1> rdf:type owl:NamedIndividual .


###  https://w3id.org/framester/wn/wn30/instances/synset-distance-noun-1
<https://w3id.org/framester/wn/wn30/instances/synset-distance-noun-1> rdf:type owl:NamedIndividual .


###  https://w3id.org/framester/wn/wn30/instances/synset-door-noun-1
<https://w3id.org/framester/wn/wn30/instances/synset-door-noun-1> rdf:type owl:NamedIndividual .


###  https://w3id.org/framester/wn/wn30/instances/synset-end-noun-1
<https://w3id.org/framester/wn/wn30/instances/synset-end-noun-1> rdf:type owl:NamedIndividual .


###  https://w3id.org/framester/wn/wn30/instances/synset-fix-noun-1
<https://w3id.org/framester/wn/wn30/instances/synset-fix-noun-1> rdf:type owl:NamedIndividual .


###  https://w3id.org/framester/wn/wn30/instances/synset-form-noun-1
<https://w3id.org/framester/wn/wn30/instances/synset-form-noun-1> rdf:type owl:NamedIndividual .


###  https://w3id.org/framester/wn/wn30/instances/synset-full-adjective-1
<https://w3id.org/framester/wn/wn30/instances/synset-full-adjective-1> rdf:type owl:NamedIndividual .


###  https://w3id.org/framester/wn/wn30/instances/synset-genus-noun-1
<https://w3id.org/framester/wn/wn30/instances/synset-genus-noun-1> rdf:type owl:NamedIndividual .


###  https://w3id.org/framester/wn/wn30/instances/synset-hand-noun-1
<https://w3id.org/framester/wn/wn30/instances/synset-hand-noun-1> rdf:type owl:NamedIndividual .


###  https://w3id.org/framester/wn/wn30/instances/synset-idea-noun-1
<https://w3id.org/framester/wn/wn30/instances/synset-idea-noun-1> rdf:type owl:NamedIndividual .


###  https://w3id.org/framester/wn/wn30/instances/synset-image-noun-1
<https://w3id.org/framester/wn/wn30/instances/synset-image-noun-1> rdf:type owl:NamedIndividual .


###  https://w3id.org/framester/wn/wn30/instances/synset-incorporate-verb-2
<https://w3id.org/framester/wn/wn30/instances/synset-incorporate-verb-2> rdf:type owl:NamedIndividual .


###  https://w3id.org/framester/wn/wn30/instances/synset-interpretation-noun-1
<https://w3id.org/framester/wn/wn30/instances/synset-interpretation-noun-1> rdf:type owl:NamedIndividual .


###  https://w3id.org/framester/wn/wn30/instances/synset-intersection-noun-1
<https://w3id.org/framester/wn/wn30/instances/synset-intersection-noun-1> rdf:type owl:NamedIndividual .


###  https://w3id.org/framester/wn/wn30/instances/synset-kind-noun-1
<https://w3id.org/framester/wn/wn30/instances/synset-kind-noun-1> rdf:type owl:NamedIndividual .


###  https://w3id.org/framester/wn/wn30/instances/synset-light-adjective-1
<https://w3id.org/framester/wn/wn30/instances/synset-light-adjective-1> rdf:type owl:NamedIndividual .


###  https://w3id.org/framester/wn/wn30/instances/synset-lodge-verb-2
<https://w3id.org/framester/wn/wn30/instances/synset-lodge-verb-2> rdf:type owl:NamedIndividual .


###  https://w3id.org/framester/wn/wn30/instances/synset-member-noun-1
<https://w3id.org/framester/wn/wn30/instances/synset-member-noun-1> rdf:type owl:NamedIndividual .


###  https://w3id.org/framester/wn/wn30/instances/synset-module-noun-4
<https://w3id.org/framester/wn/wn30/instances/synset-module-noun-4> rdf:type owl:NamedIndividual .


###  https://w3id.org/framester/wn/wn30/instances/synset-name-noun-1
<https://w3id.org/framester/wn/wn30/instances/synset-name-noun-1> rdf:type owl:NamedIndividual .


###  https://w3id.org/framester/wn/wn30/instances/synset-notion-noun-2
<https://w3id.org/framester/wn/wn30/instances/synset-notion-noun-2> rdf:type owl:NamedIndividual .


###  https://w3id.org/framester/wn/wn30/instances/synset-noun-noun-1
<https://w3id.org/framester/wn/wn30/instances/synset-noun-noun-1> rdf:type owl:NamedIndividual .


###  https://w3id.org/framester/wn/wn30/instances/synset-out-noun-1
<https://w3id.org/framester/wn/wn30/instances/synset-out-noun-1> rdf:type owl:NamedIndividual .


###  https://w3id.org/framester/wn/wn30/instances/synset-overlap-noun-1
<https://w3id.org/framester/wn/wn30/instances/synset-overlap-noun-1> rdf:type owl:NamedIndividual .


###  https://w3id.org/framester/wn/wn30/instances/synset-part-noun-1
<https://w3id.org/framester/wn/wn30/instances/synset-part-noun-1> rdf:type owl:NamedIndividual .


###  https://w3id.org/framester/wn/wn30/instances/synset-partial-adjectivesatellite-1
<https://w3id.org/framester/wn/wn30/instances/synset-partial-adjectivesatellite-1> rdf:type owl:NamedIndividual .


###  https://w3id.org/framester/wn/wn30/instances/synset-partition-noun-1
<https://w3id.org/framester/wn/wn30/instances/synset-partition-noun-1> rdf:type owl:NamedIndividual .


###  https://w3id.org/framester/wn/wn30/instances/synset-piece-noun-1
<https://w3id.org/framester/wn/wn30/instances/synset-piece-noun-1> rdf:type owl:NamedIndividual .


###  https://w3id.org/framester/wn/wn30/instances/synset-plan-noun-1
<https://w3id.org/framester/wn/wn30/instances/synset-plan-noun-1> rdf:type owl:NamedIndividual .


###  https://w3id.org/framester/wn/wn30/instances/synset-plan-verb-1
<https://w3id.org/framester/wn/wn30/instances/synset-plan-verb-1> rdf:type owl:NamedIndividual .


###  https://w3id.org/framester/wn/wn30/instances/synset-platform-noun-1
<https://w3id.org/framester/wn/wn30/instances/synset-platform-noun-1> rdf:type owl:NamedIndividual .


###  https://w3id.org/framester/wn/wn30/instances/synset-point-noun-1
<https://w3id.org/framester/wn/wn30/instances/synset-point-noun-1> rdf:type owl:NamedIndividual .


###  https://w3id.org/framester/wn/wn30/instances/synset-policy-noun-1
<https://w3id.org/framester/wn/wn30/instances/synset-policy-noun-1> rdf:type owl:NamedIndividual .


###  https://w3id.org/framester/wn/wn30/instances/synset-position-noun-3
<https://w3id.org/framester/wn/wn30/instances/synset-position-noun-3> rdf:type owl:NamedIndividual .


###  https://w3id.org/framester/wn/wn30/instances/synset-pot-noun-1
<https://w3id.org/framester/wn/wn30/instances/synset-pot-noun-1> rdf:type owl:NamedIndividual .


###  https://w3id.org/framester/wn/wn30/instances/synset-principle-noun-1
<https://w3id.org/framester/wn/wn30/instances/synset-principle-noun-1> rdf:type owl:NamedIndividual .


###  https://w3id.org/framester/wn/wn30/instances/synset-purpose-noun-1
<https://w3id.org/framester/wn/wn30/instances/synset-purpose-noun-1> rdf:type owl:NamedIndividual .


###  https://w3id.org/framester/wn/wn30/instances/synset-put-verb-1
<https://w3id.org/framester/wn/wn30/instances/synset-put-verb-1> rdf:type owl:NamedIndividual .


###  https://w3id.org/framester/wn/wn30/instances/synset-range-verb-1
<https://w3id.org/framester/wn/wn30/instances/synset-range-verb-1> rdf:type owl:NamedIndividual .


###  https://w3id.org/framester/wn/wn30/instances/synset-reference-noun-6
<https://w3id.org/framester/wn/wn30/instances/synset-reference-noun-6> rdf:type owl:NamedIndividual .


###  https://w3id.org/framester/wn/wn30/instances/synset-representation-noun-1
<https://w3id.org/framester/wn/wn30/instances/synset-representation-noun-1> rdf:type owl:NamedIndividual .


###  https://w3id.org/framester/wn/wn30/instances/synset-restriction-noun-1
<https://w3id.org/framester/wn/wn30/instances/synset-restriction-noun-1> rdf:type owl:NamedIndividual .


###  https://w3id.org/framester/wn/wn30/instances/synset-schema-noun-1
<https://w3id.org/framester/wn/wn30/instances/synset-schema-noun-1> rdf:type owl:NamedIndividual .


###  https://w3id.org/framester/wn/wn30/instances/synset-section-noun-4
<https://w3id.org/framester/wn/wn30/instances/synset-section-noun-4> rdf:type owl:NamedIndividual .


###  https://w3id.org/framester/wn/wn30/instances/synset-separate-verb-1
<https://w3id.org/framester/wn/wn30/instances/synset-separate-verb-1> rdf:type owl:NamedIndividual .


###  https://w3id.org/framester/wn/wn30/instances/synset-several-adjectivesatellite-1
<https://w3id.org/framester/wn/wn30/instances/synset-several-adjectivesatellite-1> rdf:type owl:NamedIndividual .


###  https://w3id.org/framester/wn/wn30/instances/synset-sol-noun-3
<https://w3id.org/framester/wn/wn30/instances/synset-sol-noun-3> rdf:type owl:NamedIndividual .


###  https://w3id.org/framester/wn/wn30/instances/synset-suggestion-noun-1
<https://w3id.org/framester/wn/wn30/instances/synset-suggestion-noun-1> rdf:type owl:NamedIndividual .


###  https://w3id.org/framester/wn/wn30/instances/synset-supply-verb-1
<https://w3id.org/framester/wn/wn30/instances/synset-supply-verb-1> rdf:type owl:NamedIndividual .


###  https://w3id.org/framester/wn/wn30/instances/synset-surface-noun-1
<https://w3id.org/framester/wn/wn30/instances/synset-surface-noun-1> rdf:type owl:NamedIndividual .


###  https://w3id.org/framester/wn/wn30/instances/synset-technology-noun-1
<https://w3id.org/framester/wn/wn30/instances/synset-technology-noun-1> rdf:type owl:NamedIndividual .


###  https://w3id.org/framester/wn/wn30/instances/synset-term-noun-1
<https://w3id.org/framester/wn/wn30/instances/synset-term-noun-1> rdf:type owl:NamedIndividual .


###  https://w3id.org/framester/wn/wn30/instances/synset-there-noun-1
<https://w3id.org/framester/wn/wn30/instances/synset-there-noun-1> rdf:type owl:NamedIndividual .


###  https://w3id.org/framester/wn/wn30/instances/synset-travel-verb-1
<https://w3id.org/framester/wn/wn30/instances/synset-travel-verb-1> rdf:type owl:NamedIndividual .


###  https://w3id.org/framester/wn/wn30/instances/synset-trip-noun-1
<https://w3id.org/framester/wn/wn30/instances/synset-trip-noun-1> rdf:type owl:NamedIndividual .


###  https://w3id.org/framester/wn/wn30/instances/synset-truck-noun-1
<https://w3id.org/framester/wn/wn30/instances/synset-truck-noun-1> rdf:type owl:NamedIndividual .


###  https://w3id.org/framester/wn/wn30/instances/synset-type-noun-1
<https://w3id.org/framester/wn/wn30/instances/synset-type-noun-1> rdf:type owl:NamedIndividual .


###  https://w3id.org/framester/wn/wn30/instances/synset-use-noun-1
<https://w3id.org/framester/wn/wn30/instances/synset-use-noun-1> rdf:type owl:NamedIndividual .


###  https://w3id.org/framester/wn/wn30/instances/synset-whole-adjective-1
<https://w3id.org/framester/wn/wn30/instances/synset-whole-adjective-1> rdf:type owl:NamedIndividual .


###  https://w3id.org/framester/wn/wn30/instances/synset-whole-noun-1
<https://w3id.org/framester/wn/wn30/instances/synset-whole-noun-1> rdf:type owl:NamedIndividual .


###  https://w3id.org/smartenvironment/patterns/event.owl
<https://w3id.org/smartenvironment/patterns/event.owl> rdf:type owl:NamedIndividual ,
                                                                odin:ODP ;
                                                       odin:describedIn odin:event.owl_Descr ;
                                                       odin:hasODPComponent <https://w3id.org/smartenvironment/patterns/event.owl#EventCondition> ,
                                                                            <https://w3id.org/smartenvironment/patterns/event.owl#Manifestation> ;
                                                       rdfs:comment "This pattern is used to represent events in the context of smart environments. An event in this pattern is represented in the form of either a Manifestation or a Complex Event, where a manifestation represents the occurance of a specific situation of an object which can be directly captured from sensor data (the tv is switched on), whereas a complex event is defined based on its precoditions that can involve different events (e.g., watching tv happens when the tv is switched on and someone is sitting on the couch).      The precondition of a complex event is represented in the form of a situation (DUL:Situation) which indicates proper temporal distances between a complex event and, the events involved in its definition." .


###  https://w3id.org/smartenvironment/patterns/network.owl
<https://w3id.org/smartenvironment/patterns/network.owl> rdf:type owl:NamedIndividual ,
                                                                  odin:ODP ;
                                                         odin:describedIn odin:network.owl_Descr ;
                                                         odin:hasODPComponent <https://w3id.org/smartenvironment/patterns/network.owl#DataReceiverNode> ,
                                                                              <https://w3id.org/smartenvironment/patterns/network.owl#DataSenderNode> ,
                                                                              <https://w3id.org/smartenvironment/patterns/network.owl#Network> ,
                                                                              <https://w3id.org/smartenvironment/patterns/network.owl#NetworkModule> ,
                                                                              <https://w3id.org/smartenvironment/patterns/network.owl#Node> ,
                                                                              <https://w3id.org/smartenvironment/patterns/network.owl#NodeStation> ,
                                                                              <https://w3id.org/smartenvironment/patterns/network.owl#ReceiverNodeStation> ,
                                                                              <https://w3id.org/smartenvironment/patterns/network.owl#SenderNodeStation> ;
                                                         rdfs:comment "This pattern relies on the SSN ontology and represents sensors and the other modules needed to deploy a network in a smart environment." .


###  https://w3id.org/smartenvironment/patterns/object.owl
<https://w3id.org/smartenvironment/patterns/object.owl> rdf:type owl:NamedIndividual ,
                                                                 odin:ODP ;
                                                        odin:describedIn odin:object.owl_Descr ;
                                                        odin:hasODPComponent <https://w3id.org/smartenvironment/patterns/object.owl#MobileObject> ,
                                                                             <https://w3id.org/smartenvironment/patterns/object.owl#NodeHolder> ,
                                                                             <https://w3id.org/smartenvironment/patterns/object.owl#SmartObject> ;
                                                        rdfs:comment "This pattern relies on both the SSN ontology and DUL in order to represent an object in the context of a smart environment. Using this model we categorize the objects in to two groups of Smart Object and NodeHolder.     Due to usual difficulties to install sensors in a smart environment it is common that some other objects (i.e. NodeHolder) are used to hosts sensors so as to observe the situation of other objects (i.e. SmartObject). Using this pattern we are able to diffrentiate between these two types of objects." .


###  https://w3id.org/smartenvironment/patterns/event.owl#EventCondition
<https://w3id.org/smartenvironment/patterns/event.owl#EventCondition> rdf:type owl:NamedIndividual ,
                                                                               odin:ODPElement ;
                                                                      odin:describedIn odin:EventCondition_Descr ;
                                                                      odin:odpType odin:Foundational ;
                                                                      rdfs:comment "Describes a precondition for a complex event needed to be recognized within specific temporal distance from the timestamp at which the complex event is recognized." .


###  https://w3id.org/smartenvironment/patterns/event.owl#Manifestation
<https://w3id.org/smartenvironment/patterns/event.owl#Manifestation> rdf:type owl:NamedIndividual ,
                                                                              odin:ODPElement ;
                                                                     odin:describedIn odin:Manifestation_Descr ;
                                                                     odin:odpType odin:Foundational ;
                                                                     rdfs:comment "Describes the occurance/realization of a specific situation of a feature of interest (for its specific property) which can be directly captured from sensor data (the tv is switched on)," .


###  https://w3id.org/smartenvironment/patterns/geometry.owl#SpatialObject
<https://w3id.org/smartenvironment/patterns/geometry.owl#SpatialObject> rdf:type owl:NamedIndividual ,
                                                                                 odin:ODPElement ;
                                                                        odin:describedIn odin:SpatialObject_Descr ;
                                                                        odin:odpType odin:Foundational ;
                                                                        rdfs:comment "Describes any physcical object in a smart environment that has a geometry." .


###  https://w3id.org/smartenvironment/patterns/geometry.owl#hasDescriptiveSpatialRelation
<https://w3id.org/smartenvironment/patterns/geometry.owl#hasDescriptiveSpatialRelation> rdf:type owl:NamedIndividual ,
                                                                                                 odin:ODPElement ;
                                                                                        odin:describedIn odin:hasDescriptiveSpatialRelation_Descr ;
                                                                                        odin:odpType odin:Foundational ;
                                                                                        rdfs:comment "This object property, as an spacialization of the object property hasSpatialRelation, generalizes spatial relations defined in the Open Time and Space Core Vocabulary, which are more declarative than those defined in GeoSPARQL." .


###  https://w3id.org/smartenvironment/patterns/geometry.owl#hasSpatialRelation
<https://w3id.org/smartenvironment/patterns/geometry.owl#hasSpatialRelation> rdf:type owl:NamedIndividual ,
                                                                                      odin:ODPElement ;
                                                                             odin:describedIn odin:hasSpatialRelation_Descr ;
                                                                             rdfs:comment "Describes any possible spatial relations between any two given spatial objects. This object properties is used to generalize all the spatial relations defined in GeoSPARQL ontology." .


###  https://w3id.org/smartenvironment/patterns/network.owl#DataReceiverNode
<https://w3id.org/smartenvironment/patterns/network.owl#DataReceiverNode> rdf:type owl:NamedIndividual ,
                                                                                   odin:ODPElement ;
                                                                          odin:describedIn odin:DataReceiverNode_Descr ;
                                                                          rdfs:comment "Decsribes a node in a network that receives data from sensors," .


###  https://w3id.org/smartenvironment/patterns/network.owl#DataSenderNode
<https://w3id.org/smartenvironment/patterns/network.owl#DataSenderNode> rdf:type owl:NamedIndividual ,
                                                                                 odin:ODPElement ;
                                                                        odin:describedIn odin:DataSenderNode_Descr ;
                                                                        rdfs:comment "Decsribes a node as part of a nore station that contributes sending the data read by sensors." .


###  https://w3id.org/smartenvironment/patterns/network.owl#Network
<https://w3id.org/smartenvironment/patterns/network.owl#Network> rdf:type owl:NamedIndividual ,
                                                                          odin:ODPElement ;
                                                                 odin:describedIn odin:Network_Descr ;
                                                                 rdfs:comment "A network which is a collection of Nodes" .


###  https://w3id.org/smartenvironment/patterns/network.owl#NetworkModule
<https://w3id.org/smartenvironment/patterns/network.owl#NetworkModule> rdf:type owl:NamedIndividual ,
                                                                                odin:ODPElement ;
                                                                       odin:describedIn odin:NetworkModule_Descr ;
                                                                       rdfs:comment "Describes the network modules in the form of node stations and nodes contributing in sending and receiving data within a sensor network in the context of a smart environment." .


###  https://w3id.org/smartenvironment/patterns/network.owl#Node
<https://w3id.org/smartenvironment/patterns/network.owl#Node> rdf:type owl:NamedIndividual ,
                                                                       odin:ODPElement ;
                                                              odin:describedIn odin:Node_Descr ;
                                                              rdfs:comment "Decsribes a node in a network that either sends or receives the data read by a sensor." .


###  https://w3id.org/smartenvironment/patterns/network.owl#NodeStation
<https://w3id.org/smartenvironment/patterns/network.owl#NodeStation> rdf:type owl:NamedIndividual ,
                                                                              odin:ODPElement ;
                                                                     odin:describedIn odin:NodeStation_Descr ;
                                                                     rdfs:comment "Decsribes a module in a network that contains nodes, batteries, etc." .


###  https://w3id.org/smartenvironment/patterns/network.owl#ReceiverNodeStation
<https://w3id.org/smartenvironment/patterns/network.owl#ReceiverNodeStation> rdf:type owl:NamedIndividual ,
                                                                                      odin:ODPElement ;
                                                                             odin:describedIn odin:ReceiverNodeStation_Descr ;
                                                                             rdfs:comment "Describes a node station which holds a data receiver node as its part (sub-system)" .


###  https://w3id.org/smartenvironment/patterns/network.owl#SenderNodeStation
<https://w3id.org/smartenvironment/patterns/network.owl#SenderNodeStation> rdf:type owl:NamedIndividual ,
                                                                                    odin:ODPElement ;
                                                                           odin:describedIn odin:SenderNodeStation_Descr ;
                                                                           rdfs:comment "Describes a node station which is assumed to contain both a data sender node and also sensing devices (sensors)" .


###  https://w3id.org/smartenvironment/patterns/object.owl#MobileObject
<https://w3id.org/smartenvironment/patterns/object.owl#MobileObject> rdf:type owl:NamedIndividual ,
                                                                              odin:ODPElement ;
                                                                     odin:describedIn odin:MobileObject_Descr ;
                                                                     rdfs:comment "Describes any type of physical object that has the possibility to move in a smart environment." .


###  https://w3id.org/smartenvironment/patterns/object.owl#NodeHolder
<https://w3id.org/smartenvironment/patterns/object.owl#NodeHolder> rdf:type owl:NamedIndividual ,
                                                                            odin:ODPElement ;
                                                                   odin:describedIn odin:NodeHolder_Descr ;
                                                                   odin:odpType odin:Core ;
                                                                   rdfs:comment "Describes any object in a smart environment, which is used to host network modules such as nodes or node stations." .


###  https://w3id.org/smartenvironment/patterns/object.owl#SmartObject
<https://w3id.org/smartenvironment/patterns/object.owl#SmartObject> rdf:type owl:NamedIndividual ,
                                                                             odin:ODPElement ;
                                                                    odin:describedIn odin:SmartObject_Descr ;
                                                                    rdfs:comment "Describes any physical object in a smart environment which is a feature of interest for an observation process." .


###  https://w3id.org/smartenvironment/patterns/place.owl#Section
<https://w3id.org/smartenvironment/patterns/place.owl#Section> rdf:type owl:NamedIndividual ,
                                                                        odin:ODPElement ;
                                                               odin:describedIn odin:Section_Descr ;
                                                               rdfs:comment "Sections belonging to a smart environment (e.g., kitchen, livingroom, etc., in case of a smart home)" .


###  https://w3id.org/smartenvironment/patterns/place.owl#SmartEnvironment
<https://w3id.org/smartenvironment/patterns/place.owl#SmartEnvironment> rdf:type owl:NamedIndividual ,
                                                                                 odin:ODPElement ;
                                                                        odin:describedIn odin:SmartEnvironment_Descr ;
                                                                        rdfs:comment "Represent a smart environment as a physical place which is also supposed to be a platform for a sensor network deployment." .


###  https://w3id.org/smartenvironment/patterns/sensing.owl#ConfigurationProcedure
<https://w3id.org/smartenvironment/patterns/sensing.owl#ConfigurationProcedure> rdf:type owl:NamedIndividual ,
                                                                                         odin:ODPElement ;
                                                                                odin:describedIn odin:ConfigurationProcedure_Descr ;
                                                                                rdfs:comment "Descibes a procedure required to configure a sensor to be used for an observation process in a smart environment context. This configuration can include both hardware ans software setup related to sensors such as the sampling rate, etc." .


###  https://w3id.org/smartenvironment/patterns/sensing.owl#Observation
<https://w3id.org/smartenvironment/patterns/sensing.owl#Observation> rdf:type owl:NamedIndividual ,
                                                                              odin:ODPElement ;
                                                                     odin:describedIn odin:Observation_Descr ;
                                                                     rdfs:comment "Using a Sensor it describes the process of observing a property of a feature of interest." .


###  https://w3id.org/smartenvironment/patterns/sensing.owl#Sensor
<https://w3id.org/smartenvironment/patterns/sensing.owl#Sensor> rdf:type owl:NamedIndividual ,
                                                                         odin:ODPElement ;
                                                                odin:describedIn odin:Sensor_Descr ;
                                                                odin:odpType odin:Core ;
                                                                rdfs:comment "Descibes a device that with a specific set of configuration is able to implements an observation process in order to monitor a property of a feature of interest in a smart environment." .


###  https://w3id.org/smartenvironment/patterns/situation.owl#Situation
<https://w3id.org/smartenvironment/patterns/situation.owl#Situation> rdf:type owl:NamedIndividual ,
                                                                              odin:ODPElement ;
                                                                     odin:describedIn odin:Situation_Descr ;
                                                                     rdfs:comment "Describes a specific situation in the context of smart environments in the form of a feature of interest, its property and a specific state that express it." .


###  https://w3id.org/smartenvironment/patterns/situation.owl#State
<https://w3id.org/smartenvironment/patterns/situation.owl#State> rdf:type owl:NamedIndividual ,
                                                                          odin:ODPElement ;
                                                                 odin:describedIn odin:State_Descr ;
                                                                 odin:odpType odin:Foundational ;
                                                                 rdfs:comment "Describes a specific state of a feature of interest regardless of how it has been realized." .


###  https://w3id.org/smartenvironment/patterns/time.owl#Instant
<https://w3id.org/smartenvironment/patterns/time.owl#Instant> rdf:type owl:NamedIndividual ;
                                                              odin:describedIn odin:Instant_Descr ;
                                                              odin:odpType odin:Foundational ;
                                                              rdfs:comment "Describes a temporal instant specifiying a specific datetimestamp" .


###  https://w3id.org/smartenvironment/patterns/time.owl#Interval
<https://w3id.org/smartenvironment/patterns/time.owl#Interval> rdf:type owl:NamedIndividual ;
                                                               odin:describedIn odin:Interval_Descr ;
                                                               odin:odpType odin:Foundational ;
                                                               rdfs:comment "Describes a temporal entity with an extent or duration with a known starting time." .


###  https://w3id.org/smartenvironment/patterns/time.owl#TemporalDistance
<https://w3id.org/smartenvironment/patterns/time.owl#TemporalDistance> rdf:type owl:NamedIndividual ;
                                                                       odin:describedIn odin:TemporalDistance_Descr ;
                                                                       odin:odpType odin:Foundational ;
                                                                       rdfs:comment "Describes a temporal distance relatively set to a given time instant. The distance is specified using two separate temporal durations both ending with the given time instant. The object property 'before' indicates that the distance is temporaly behind the time instant as the target time." .


###  https://w3id.org/smartenvironment/patterns/time.owl#TemporalEntity
<https://w3id.org/smartenvironment/patterns/time.owl#TemporalEntity> rdf:type owl:NamedIndividual ;
                                                                     odin:describedIn odin:TemporalEntity_Descr ;
                                                                     rdfs:comment "Describes a temporal entity that can represent a single time instant, a time interval, or a temporal distance." .


###  https://w3id.org/smartenvironment/patterns/time.owl#TimeDuration
<https://w3id.org/smartenvironment/patterns/time.owl#TimeDuration> rdf:type owl:NamedIndividual ;
                                                                   odin:describedIn odin:TimeDuration_Descr ;
                                                                   rdfs:comment "Describes time duration in the form of a numeric value indicating its length, and a temporal unit type." .


[ odin:describedIn odin:_:b4_Descr
] .

[ odin:describedIn odin:_:b1_Descr
 ] .

[ odin:describedIn odin:_:b2_Descr
 ] .

[ odin:describedIn odin:_:b0_Descr
 ] .

[ odin:describedIn odin:_:b3_Descr
 ] .

[ rdfs:comment "This is necessarly to preserve the coherence of the ontology.  if Action1->hasOutcome->Event1 and Event1->raise->Reaction2 is not possible that Reaction2->hasNextAction->Action1"
 ] .

[ rdfs:comment "This is necessarly to preserve the coherence of the ontology.  if Action1->hasOutcome->Event1 and Event1->raise->Reaction2 is not possible that Reaction2->hasNextAction->Action1"
 ] .

[ rdfs:comment "This is a guarded domain restriction for providesAgentRole with ChessGame as the domain. Note that the corresponding guarded range restriction is not asserted since ChessGame may provide roles of types other than WhitePlayerRole and BlackPlayerRole"
 ] .

[ rdfs:comment "This is the guarded domain restriction for providesAgentRole with ChessGameManifestation as the domain. The corresponding guarded range restriction for the property is not asserted since ChessGameManifestation may provide roles of types other than AuthorRole"
 ] .

[ rdfs:comment "This is a guarded domain restriction for providesAgentRole with HalfMove as the domain. The corresponding guarded range restriction since HalfMove may provide roles of types other than ActingPlayerRole"
 ] .

###  Generated by the OWL API (version 4.5.9.2019-02-01T07:24:44Z) https://github.com/owlcs/owlapi
